<rdf:RDF
    xmlns:rdf="http://www.w3.org/1999/02/22-rdf-syntax-ns#"
    xmlns:xsd="http://www.w3.org/2001/XMLSchema#"
    xmlns:rdfs="http://www.w3.org/2000/01/rdf-schema#"
    xmlns:owl="http://www.w3.org/2002/07/owl#"
    xmlns="http://www.tc184-sc4.org/iso15926/part2/2003-12#"
    xml:base="http://www.tc184-sc4.org/iso15926/part2/2003-12">

    <owl:Ontology rdf:about="">
        <rdfs:comment>EXPRESS model of ISO 15926-2 mapped to OWL</rdfs:comment>
        <rdfs:label>DataModel</rdfs:label>
        <versionInfo>August 2005</versionInfo>
    </owl:Ontology>
    <owl:DatatypeProperty rdf:ID="LogicalValue">
        #<rdfs:range>
            #<owl:DataRange>
                #<owl:oneof>
                    ##<rdf:List>
                        ##<rdf:first rdf:datatype="http://www.w3.org/2001/XMLSchema#string">0</rdf:first>
                        ##<rdf:rest>
                            ##<rdf:List>
                                ##<rdf:first rdf:datatype="http://www.w3.org/2001/XMLSchema#string">1</rdf:first>
                                ##<rdf:rest>
                                    ##<rdf:List>
                                        ##<rdf:first rdf:datatype="http://www.w3.org/2001/XMLSchema#string">-</rdf:first>
                                        ##<rdf:rest rdf:resource="http://www.w3.org/1999/02/22-rdf-syntax-ns#nil"/>
                                    ##</rdf:List>
                                ##</rdf:rest>
                            ##</rdf:List>
                        ##</rdf:rest>
                    ##</rdf:List>
                #</owl:oneof>
            #</owl:DataRange>
        #</rdfs:range>
    </owl:DatatypeProperty>
    <owl:ObjectProperty rdf:ID="approved"/>
    <owl:ObjectProperty rdf:ID="approver"/>
    <owl:ObjectProperty rdf:ID="bounded"/>
    <owl:ObjectProperty rdf:ID="bounding"/>
    <owl:ObjectProperty rdf:ID="cardinalities"/>
    <owl:ObjectProperty rdf:ID="caused"/>
    <owl:ObjectProperty rdf:ID="causer"/>
    <owl:ObjectProperty rdf:ID="classOfApproved"/>
    <owl:ObjectProperty rdf:ID="classOfApprover"/>
    <owl:ObjectProperty rdf:ID="classOfBegun"/>
    <owl:ObjectProperty rdf:ID="classOfCauser"/>
    <owl:ObjectProperty rdf:ID="classOfClassOfControlled"/>
    <owl:ObjectProperty rdf:ID="classOfClassOfPart"/>
    <owl:ObjectProperty rdf:ID="classOfClassOfUsed"/>
    <owl:ObjectProperty rdf:ID="classOfClassOfWhole"/>
    <owl:ObjectProperty rdf:ID="classOfClassified"/>
    <owl:ObjectProperty rdf:ID="classOfClassifier"/>
    <owl:ObjectProperty rdf:ID="classOfConnection"/>
    <owl:ObjectProperty rdf:ID="classOfControlled"/>
    <owl:ObjectProperty rdf:ID="classOfDimension"/>
    <owl:ObjectProperty rdf:ID="classOfEnd1"/>
    <owl:ObjectProperty rdf:ID="classOfEnd2"/>
    <owl:ObjectProperty rdf:ID="classOfEnded"/>
    <owl:ObjectProperty rdf:ID="classOfFirst"/>
    <owl:ObjectProperty rdf:ID="classOfInvolved"/>
    <owl:ObjectProperty rdf:ID="classOfInvolver"/>
    <owl:ObjectProperty rdf:ID="classOfLocated"/>
    <owl:ObjectProperty rdf:ID="classOfLocator"/>
    <owl:ObjectProperty rdf:ID="classOfPart"/>
    <owl:ObjectProperty rdf:ID="classOfPattern"/>
    <owl:ObjectProperty rdf:ID="classOfPlayer"/>
    <owl:ObjectProperty rdf:ID="classOfPossessor"/>
    <owl:ObjectProperty rdf:ID="classOfPredecessor"/>
    <owl:ObjectProperty rdf:ID="classOfRecognized"/>
    <owl:ObjectProperty rdf:ID="classOfRecognizing"/>
    <owl:ObjectProperty rdf:ID="classOfRepresented"/>
    <owl:ObjectProperty rdf:ID="classOfSecond"/>
    <owl:ObjectProperty rdf:ID="classOfShape"/>
    <owl:ObjectProperty rdf:ID="classOfShapeDimension"/>
    <owl:ObjectProperty rdf:ID="classOfSide1"/>
    <owl:ObjectProperty rdf:ID="classOfSide2"/>
    <owl:ObjectProperty rdf:ID="classOfSubclass"/>
    <owl:ObjectProperty rdf:ID="classOfSuccessor"/>
    <owl:ObjectProperty rdf:ID="classOfSuperclass"/>
    <owl:ObjectProperty rdf:ID="classOfUsage"/>
    <owl:ObjectProperty rdf:ID="classOfUsed"/>
    <owl:ObjectProperty rdf:ID="classOfWhole"/>
    <owl:ObjectProperty rdf:ID="codomain"/>
    <owl:ObjectProperty rdf:ID="connection"/>
    <owl:ObjectProperty rdf:ID="content"/>
    <owl:ObjectProperty rdf:ID="controlled"/>
    <owl:ObjectProperty rdf:ID="controller"/>
    <owl:ObjectProperty rdf:ID="day"/>
    <owl:ObjectProperty rdf:ID="dimension"/>
    <owl:ObjectProperty rdf:ID="domain"/>
    <owl:ObjectProperty rdf:ID="elements"/>
    <owl:ObjectProperty rdf:ID="end1"/>
    <owl:ObjectProperty rdf:ID="end1Cardinality"/>
    <owl:ObjectProperty rdf:ID="end2"/>
    <owl:ObjectProperty rdf:ID="end2Cardinality"/>
    <owl:ObjectProperty rdf:ID="greaterElement"/>
    <owl:ObjectProperty rdf:ID="highestNumber"/>
    <owl:ObjectProperty rdf:ID="highestProperty"/>
    <owl:ObjectProperty rdf:ID="hour"/>
    <owl:ObjectProperty rdf:ID="individual"/>
    <owl:ObjectProperty rdf:ID="individualDimension"/>
    <owl:ObjectProperty rdf:ID="input"/>
    <owl:ObjectProperty rdf:ID="interest"/>
    <owl:ObjectProperty rdf:ID="interested"/>
    <owl:ObjectProperty rdf:ID="involved"/>
    <owl:ObjectProperty rdf:ID="involver"/>
    <owl:ObjectProperty rdf:ID="lesserElement"/>
    <owl:ObjectProperty rdf:ID="located"/>
    <owl:ObjectProperty rdf:ID="locator"/>
    <owl:ObjectProperty rdf:ID="lowestNumber"/>
    <owl:ObjectProperty rdf:ID="lowestProperty"/>
    <owl:ObjectProperty rdf:ID="maximumCardinality"/>
    <owl:ObjectProperty rdf:ID="minimumCardinality"/>
    <owl:ObjectProperty rdf:ID="minute"/>
    <owl:ObjectProperty rdf:ID="month"/>
    <owl:ObjectProperty rdf:ID="optionalElement"/>
    <owl:ObjectProperty rdf:ID="parameterPosition"/>
    <owl:ObjectProperty rdf:ID="parameters"/>
    <owl:ObjectProperty rdf:ID="part"/>
    <owl:ObjectProperty rdf:ID="pattern"/>
    <owl:ObjectProperty rdf:ID="played"/>
    <owl:ObjectProperty rdf:ID="player"/>
    <owl:ObjectProperty rdf:ID="position"/>
    <owl:ObjectProperty rdf:ID="possessor"/>
    <owl:ObjectProperty rdf:ID="predecessor"/>
    <owl:ObjectProperty rdf:ID="property"/>
    <owl:ObjectProperty rdf:ID="propertySpace"/>
    <owl:ObjectProperty rdf:ID="range"/>
    <owl:ObjectProperty rdf:ID="recognized"/>
    <owl:ObjectProperty rdf:ID="recognizing"/>
    <owl:ObjectProperty rdf:ID="recordCopyCreated"/>
    <owl:ObjectProperty rdf:ID="recordCreated"/>
    <owl:ObjectProperty rdf:ID="recordCreator"/>
    <owl:ObjectProperty rdf:ID="recordLogicallyDeleted"/>
    <owl:ObjectProperty rdf:ID="related"/>
    <owl:ObjectProperty rdf:ID="represented"/>
    <owl:ObjectProperty rdf:ID="result"/>
    <owl:ObjectProperty rdf:ID="roles"/>
    <owl:ObjectProperty rdf:ID="second"/>
    <owl:ObjectProperty rdf:ID="shape"/>
    <owl:ObjectProperty rdf:ID="shapeDimension"/>
    <owl:ObjectProperty rdf:ID="side1"/>
    <owl:ObjectProperty rdf:ID="side2"/>
    <owl:ObjectProperty rdf:ID="sign"/>
    <owl:ObjectProperty rdf:ID="successor"/>
    <owl:ObjectProperty rdf:ID="usage"/>
    <owl:ObjectProperty rdf:ID="used"/>
    <owl:ObjectProperty rdf:ID="user"/>
    <owl:ObjectProperty rdf:ID="whole"/>
    <owl:ObjectProperty rdf:ID="whyDeleted"/>
    <owl:ObjectProperty rdf:ID="year"/>

    <owl:Class rdf:ID="AbstractObject">
        <rdf:type rdf:resource="#ClassOfAbstractObject"/>
        <rdfs:subClassOf rdf:resource="#Thing"/>
        <owl:intersectionOf rdf:parseType="Collection">  
            <owl:Class rdf:about="#Class"/>  
            <owl:Class rdf:about="#Relationship"/>  
            <owl:Class rdf:about="#MultidimensionalObject"/>  
        </owl:intersectionOf>
        <owl:disjointWith rdf:resource="#PossibleIndividual"/>
        <rdfs:comment>
        	DEFINITION An AbstractObject is a Thing that does not exist in space-time
        </rdfs:comment>
    </owl:Class>

    <owl:Class rdf:ID="Activity">
        <rdf:type rdf:resource="#ClassOfActivity"/>
        <rdfs:subClassOf rdf:resource="#PossibleIndividual"/>
        <rdfs:comment>
        	DEFINITION An Activity is a PossibleIndividual that brings about 
        	change by causing the Event that marks the Beginning, or the Event that marks 
        	the Ending of a PossibleIndividual .
            An Activity consists of the temporal parts of those members of
            PossibleIndividual that participate in the Activity. The participating
            temporal parts will be classified by the ParticipatingRoleAndDomain
            that indicates the role of the temporal part in the Activity
        </rdfs:comment>
        <rdfs:comment>
        	EXAMPLE Pumping a fluid with a mechanical pump can be represented 
        	by an instance of Activity
        </rdfs:comment>
    </owl:Class>

    <owl:Class rdf:ID="ActualIndividual">
        <rdfs:subClassOf rdf:resource="#PossibleIndividual"/>
        <rdfs:comment>
            DEFINITION An ActualIndividual is a PossibleIndividual that is a part of
            the space-time continuum that we inhabit. It exists in the present, past,
            or future of our universe, as opposed to some imagined universe.
        </rdfs:comment>
        <rdfs:comment>
            NOTE The things we plan can usually only be assumed to be part of some
            imagined universe, until they come about.
        </rdfs:comment>
        <rdfs:comment>
            EXAMPLE The Eiffel Tower is an ActualIndividual .
        </rdfs:comment>
        <rdfs:comment>
            EXAMPLE The fictional character, Sherlock Holmes, is a PossibleIndividual
            who is not an ActualIndividual .
        </rdfs:comment>
        <rdfs:comment>
            EXAMPLE The Earth in the year 2300 (assuming it still exists) is an
            ActualIndividual .
        </rdfs:comment>
    </owl:Class>

#####    <owl:Class rdf:ID="Approval">
#####        <rdf:type rdf:resource="#ClassOfApproval"/>
#####        <rdf:type rdf:resource="#ClassOfApprovalByStatus"/>
#####        <rdfs:subClassOf rdf:resource="#Relationship"/>
#####        <owl:disjointWith rdf:resource="#CauseOfEvent"/>
#####        <owl:disjointWith rdf:resource="#ClassOfRelationshipWithSignature"/>
#####        <owl:disjointWith rdf:resource="#ComparisonOfProperty"/>
#####        <owl:disjointWith rdf:resource="#CompositionOfIndividual"/>
#####        <owl:disjointWith rdf:resource="#ConnectionOfIndividual"/>
#####        <owl:disjointWith rdf:resource="#FunctionalMapping"/>
#####        <owl:disjointWith rdf:resource="#IndirectProperty"/>
#####        <owl:disjointWith rdf:resource="#IndividualUsedInConnection"/>
#####        <owl:disjointWith rdf:resource="#IntendedRoleAndDomain"/>
#####        <owl:disjointWith rdf:resource="#InvolvementByReference"/>
#####        <owl:disjointWith rdf:resource="#LifecycleStage"/>
#####        <owl:disjointWith rdf:resource="#OtherRelationship"/>
#####        <owl:disjointWith rdf:resource="#PossibleRoleAndDomain"/>
#####        <owl:disjointWith rdf:resource="#Recognition"/>
#####        <owl:disjointWith rdf:resource="#RelativeLocation"/>
#####        <owl:disjointWith rdf:resource="#RepresentationOfThing"/>
#####        <owl:disjointWith rdf:resource="#ResponsibilityForRepresentation"/>
#####        <owl:disjointWith rdf:resource="#TemporalSequence"/>
#####        <owl:disjointWith rdf:resource="#UsageOfRepresentation"/>
#####        <rdfs:subClassOf>
#####            <owl:Restriction>
#####                <owl:onProperty rdf:resource="#approved"/>
#####                <owl:allValuesFrom rdf:resource="#Relationship"/>
#####            </owl:Restriction>
#####        </rdfs:subClassOf>
#####        <rdfs:subClassOf>
#####            <owl:Restriction>
#####                <owl:onProperty rdf:resource="#approver"/>
#####                <owl:allValuesFrom rdf:resource="#PossibleIndividual"/>
#####            </owl:Restriction>
#####        </rdfs:subClassOf>
#####        <rdfs:comment>
#####            DEFINITION An Approval is a Relationship that indicates that a Relationship
#####            has been approved by a PossibleIndividual that is an approver.
#####        </rdfs:comment>
#####        <rdfs:comment>
#####            NOTE Care should be taken as to what is approved. Sometimes it will not be
#####            say a pump that is approved, but the participation of the pump in a
#####            particular Activity, or member of some ClassOfActivity .
#####        </rdfs:comment>
#####        <rdfs:comment>
#####            EXAMPLE The InvolvementByReference of a plant design with a construction
#####            activity, being approved by the site manager, is an example of an Approval.
#####        </rdfs:comment>
#####    </owl:Class>

    <owl:Class rdf:ID="ArithmeticNumber">
        <rdf:type rdf:resource="#ClassOfNumber"/>
        <rdfs:subClassOf rdf:resource="#ClassOfClass"/>
        <owl:unionOf rdf:parseType="Collection">  
            <owl:Class rdf:about="#IntegerNumber"/>  
            <owl:Class rdf:about="#MultidimensionalNumber"/>  
            <owl:Class rdf:about="#RealNumber"/>  
        </owl:unionOf>
        <owl:disjointWith rdf:resource="#ClassOfClassOfIndividual"/>
        <owl:disjointWith rdf:resource="#ClassOfClassOfRelationship"/>
        <owl:disjointWith rdf:resource="#ClassOfNumber"/>
        <owl:disjointWith rdf:resource="#ClassOfPropertySpace"/>
        <owl:disjointWith rdf:resource="#ClassOfShapeDimension"/>
        <rdfs:comment>
            DEFINITION An ArithmeticNumber is a ClassOfClass whose member classes have
            the same sign and count or magnitude. An ArithmeticNumber is the number
            itself, not any representation of the number.
        </rdfs:comment>
        <rdfs:comment>
            EXAMPLE The number 2 and the number 2.0 can be represented by instances of
            ArithmeticNumber .
        </rdfs:comment>
        <rdfs:comment>
            EXAMPLE Fifteen, the number itself not the English word "fifteen", is an
            ArithmeticNumber. It could be represented by an ExpressInteger or an
            ExpressReal but could also be represented by "XV", or a binary, or a
            hexadecimal representation.
        </rdfs:comment>
    </owl:Class>

    <owl:Class rdf:ID="ArrangedIndividual">
        <rdf:type rdf:resource="#ClassOfArrangedIndividual"/>
        <rdfs:subClassOf rdf:resource="#PossibleIndividual"/>
        <rdfs:comment>
            DEFINITION An ArrangedIndividual is a PossibleIndividual that has parts
            that play distinct roles with respect to the whole. The qualities of an
            ArrangedIndividual are distinct from the qualities of its parts.
        </rdfs:comment>
        <rdfs:comment>
            EXAMPLE The vessel with serial number V-1234 is an ArrangedIndividual .
        </rdfs:comment>
        <rdfs:comment>
            EXAMPLE The company Bloggs  Co. is an ArrangedIndividual .
        </rdfs:comment>
        <rdfs:comment>
            EXAMPLE John Doe is an ArrangedIndividual .
        </rdfs:comment>
    </owl:Class>

    <owl:Class rdf:ID="ArrangementOfIndividual">
        <rdf:type rdf:resource="#ClassOfArrangementOfIndividual"/>
        <rdfs:subClassOf rdf:resource="#CompositionOfIndividual"/>
        <owl:unionOf rdf:parseType="Collection">  
            <owl:Class rdf:about="#AssemblyOfIndividual"/>  
            <owl:Class rdf:about="#FeatureWholePart"/>  
        </owl:unionOf>
        <owl:disjointWith rdf:resource="#Participation"/>
        <owl:disjointWith rdf:resource="#TemporalBounding"/>
        <owl:disjointWith rdf:resource="#TemporalWholePart"/>
        <rdfs:subClassOf>
            <owl:Restriction>
                <owl:onProperty rdf:resource="#whole"/>
                <owl:allValuesFrom rdf:resource="#ArrangedIndividual"/>
            </owl:Restriction>
        </rdfs:subClassOf>
        <rdfs:comment>
            DEFINITION An ArrangementOfIndividual is a CompositionOfIndividual that
            indicates that the part is a part of an ArrangedIndividual.
            The temporal extent of the part is that of the whole.
            An ArrangementOfIndividual may be an AssemblyOfIndividual .
        </rdfs:comment>
        <rdfs:comment>
            NOTE The term "arranged" implies that parts have particular roles with
            respect to the whole.
        </rdfs:comment>
        <rdfs:comment>
            NOTE The natures of the relations to other parts of the whole are not
            specified by the arrangement relation. Relationships like
            ConnectionOfIndividual and RelativeLocation would indicate this.
        </rdfs:comment>
        <rdfs:comment>
            EXAMPLE The relationship that indicates that a particular aircraft is
            flying as part of a formation can be represented by an instance of
            ArrangementOfIndividual .
        </rdfs:comment>
        <rdfs:comment>
            EXAMPLE The relationship that indicates that a particular bin in a warehouse
            is part of the warehouse layout can be represented by an instance of
            ArrangementOfIndividual .
        </rdfs:comment>
    </owl:Class>

    <owl:Class rdf:ID="AssemblyOfIndividual">
        <rdf:type rdf:resource="#ClassOfAssemblyOfIndividual"/>
        <rdfs:subClassOf rdf:resource="#ArrangementOfIndividual"/>
        <owl:disjointWith rdf:resource="#FeatureWholePart"/>
        <rdfs:comment>
            DEFINITION An AssemblyOfIndividual is an ArrangementOfIndividual that
            indicates that the part is connected directly or indirectly to other parts
            of the whole. The parts and wholes are super-molecular objects.
        </rdfs:comment>
        <rdfs:comment>
            NOTE Composition of molecules and smaller is represented through instances
            of ClassOfArrangementOfIndividual .
        </rdfs:comment>
        <rdfs:comment>
            EXAMPLE The relation that indicates that a temporal part of an impeller is a
            part of an assembled pump can be represented by an instance of
            AssemblyOfIndividual .
        </rdfs:comment>
    </owl:Class>

    <owl:Class rdf:ID="Beginning">
        <rdfs:subClassOf rdf:resource="#TemporalBounding"/>
        <owl:disjointWith rdf:resource="#Ending"/>
        <rdfs:comment>
            DEFINITION A Beginning is a TemporalBounding that marks the temporal start
            of a PossibleIndividual .
        </rdfs:comment>
        <rdfs:comment>
            EXAMPLE The relation that indicates that the PointInTime known as 0000hrs
            1st July 1999 UTC is the beginning of the PeriodInTime known as July 1999
            00:00UTC can be represented by an instance of Beginning .
        </rdfs:comment>
        <rdfs:comment>
            EXAMPLE The relation that indicates that the Event 'loading complete' marks
            the start of the PossibleIndividual 'loading plant idle' can be represented
            by an instance of Beginning .
        </rdfs:comment>
    </owl:Class>

    <owl:Class rdf:ID="BoundaryOfNumberSpace">
        <rdfs:subClassOf rdf:resource="#Relationship"/>
        <rdfs:subClassOf>
            <owl:Restriction>
                <owl:onProperty rdf:resource="#bounding"/>
                <owl:allValuesFrom rdf:resource="#NumberSpace"/>
            </owl:Restriction>
        </rdfs:subClassOf>
        <rdfs:subClassOf>
            <owl:Restriction>
                <owl:onProperty rdf:resource="#bounded"/>
                <owl:allValuesFrom rdf:resource="#NumberSpace"/>
            </owl:Restriction>
        </rdfs:subClassOf>
        <rdfs:comment>
            DEFINITION A BoundaryOfNumberSpace is a Specialization that indicates that a
            NumberSpace is a boundary to another NumberSpace .
        </rdfs:comment>
        <rdfs:comment>
            EXAMPLE The side of a cube in R3 is a NumberSpace that is a plane in R3 and
            that is a boundary to the NumberSpace that is a cube in R3.
        </rdfs:comment>
    </owl:Class>

    <owl:Class rdf:ID="BoundaryOfPropertySpace">
        <rdfs:subClassOf rdf:resource="#Relationship"/>
        <rdfs:subClassOf>
            <owl:Restriction>
                <owl:onProperty rdf:resource="#bounding"/>
                <owl:allValuesFrom rdf:resource="#PropertySpace"/>
            </owl:Restriction>
        </rdfs:subClassOf>
        <rdfs:subClassOf>
            <owl:Restriction>
                <owl:onProperty rdf:resource="#bounded"/>
                <owl:allValuesFrom rdf:resource="#PropertySpace"/>
            </owl:Restriction>
        </rdfs:subClassOf>
        <rdfs:comment>
            DEFINITION A BoundaryOfPropertySpace is a Specialization that indicates the
            members of the subclass form a boundary of the superclass.
        </rdfs:comment>
        <rdfs:comment>
            NOTE For reasons of mapping to OWL where specialization is represented by
            rdfs:subClassOf, the expressivity of this relationship would be lost; for
            that reason we have mapped it to the supertype of spepcialization, i.e.
            Relationship.
        </rdfs:comment>
        <rdfs:comment>
            EXAMPLE The PropertySpace that corresponds to the maximum speed head flow
            curve is a boundary of the PropertySpace that corresponds to the pump
            operating envelope.
        </rdfs:comment>
    </owl:Class>

    <owl:Class rdf:ID="Cardinality">
        <rdfs:subClassOf rdf:resource="#Class"/>
        <rdfs:subClassOf>
            <owl:Restriction>
                <owl:onProperty rdf:resource="#maximumCardinality"/>
                <owl:maxCardinality rdf:datatype="http://www.w3.org/2001/XMLSchema#nonNegativeInteger"/>
            </owl:Restriction>
        </rdfs:subClassOf>
        <rdfs:subClassOf>
            <owl:Restriction>
                <owl:onProperty rdf:resource="#minimumCardinality"/>
                <owl:minCardinality rdf:datatype="http://www.w3.org/2001/XMLSchema#nonNegativeInteger"/>
            </owl:Restriction>
        </rdfs:subClassOf>
        <rdfs:comment>
            DEFINITION A Cardinality is a Class that is the maximum and/or minimum number
            of times a thing can play a particular role in a ClassOfRelationship or
            ClassOfMultidimensionalObject .
        </rdfs:comment>
        <rdfs:comment>
            EXAMPLE A minimum of 1 and a maximum of 1 means that there is exactly one
            Relationship MultidimensionalObject of this type for each object.
        </rdfs:comment>
    </owl:Class>

    <owl:Class rdf:ID="CauseOfEvent">
        <rdfs:subClassOf rdf:resource="#Relationship"/>
        <owl:disjointWith rdf:resource="#ClassOfRelationshipWithSignature"/>
        <owl:disjointWith rdf:resource="#ComparisonOfProperty"/>
        <owl:disjointWith rdf:resource="#CompositionOfIndividual"/>
        <owl:disjointWith rdf:resource="#ConnectionOfIndividual"/>
        <owl:disjointWith rdf:resource="#FunctionalMapping"/>
        <owl:disjointWith rdf:resource="#IndirectProperty"/>
        <owl:disjointWith rdf:resource="#IndividualUsedInConnection"/>
        <owl:disjointWith rdf:resource="#IntendedRoleAndDomain"/>
        <owl:disjointWith rdf:resource="#InvolvementByReference"/>
        <owl:disjointWith rdf:resource="#LifecycleStage"/>
        <owl:disjointWith rdf:resource="#OtherRelationship"/>
        <owl:disjointWith rdf:resource="#PossibleRoleAndDomain"/>
        <owl:disjointWith rdf:resource="#Recognition"/>
        <owl:disjointWith rdf:resource="#RelativeLocation"/>
        <owl:disjointWith rdf:resource="#RepresentationOfThing"/>
        <owl:disjointWith rdf:resource="#ResponsibilityForRepresentation"/>
        <owl:disjointWith rdf:resource="#TemporalSequence"/>
        <owl:disjointWith rdf:resource="#UsageOfRepresentation"/>
        <rdfs:subClassOf>
            <owl:Restriction>
                <owl:onProperty rdf:resource="#caused"/>
                <owl:allValuesFrom rdf:resource="#Event"/>
            </owl:Restriction>
        </rdfs:subClassOf>
        <rdfs:subClassOf>
            <owl:Restriction>
                <owl:onProperty rdf:resource="#causer"/>
                <owl:allValuesFrom rdf:resource="#Activity"/>
            </owl:Restriction>
        </rdfs:subClassOf>
        <rdfs:comment>
            DEFINITION A CauseOfEvent is a Relationship that indicates that the caused
            Event is caused by the causer Activity .
        </rdfs:comment>
        <rdfs:comment>
            EXAMPLE The relation that indicates that the tanker loading activity caused
            the Event described as 'tank liquid level full' can be represented by an
            instance of CauseOfEvent .
        </rdfs:comment>
    </owl:Class>

#####    <owl:Class rdf:ID="Class">
#####        <rdf:type rdf:resource="#ClassOfClass"/>
#####        <rdfs:subClassOf rdf:resource="#AbstractObject"/>
#####        <owl:intersectionOf rdf:parseType="Collection">  
#####            <owl:Class rdf:about="#Cardinality"/>  
#####            <owl:Class rdf:about="#RoleAndDomain"/>  
#####            <owl:Class>
#####                <owl:unionOf rdf:parseType="Collection">  
#####                    <owl:Class rdf:about="#ClassOfAbstractObject"/>  
#####                    <owl:Class rdf:about="#ClassOfIndividual"/>  
#####                </owl:unionOf>
#####            </owl:Class>
#####        </owl:intersectionOf>
#####        <rdfs:comment>
#####            DEFINITION A Class is a Thing that is an understanding of the nature of
#####            things and that divides things into those which are members of the class and
#####            those which are not according to one or more criteria.
#####            The identity of a Class is ultimately defined by its members. No two classes
#####            have the same membership. However, a distinction must be made between a Class
#####            having members, and those members being known, so within an information
#####            system the members recorded may change over time, even though the true
#####            membership does not change.
#####        </rdfs:comment>
#####        <rdfs:comment>
#####            NOTE The membership of a Class is unchanging as a result of the
#####            spatio-temporal paradigm upon which this schema is based. In another paradigm
#####            it might be stated that a car is red at one time, and green at another time,
#####            indicating that the class of red things and class of green things changed
#####            members. However, using a spatio-temporal paradigm, a temporal part, state 1,
#####            of the car is red, and another temporal part of the car, state 2, is green.
#####            In this way the members of the classes red and green are unchanging. The same
#####            principle applies to future temporal parts as to past temporal parts, it is
#####            just more likely that the membership of these is not known.
#####        </rdfs:comment>
#####        <rdfs:comment>
#####            NOTE A class may be a member of another class or itself.
#####        </rdfs:comment>
#####        <rdfs:comment>
#####            NOTE The set theory that applies to classes in this model is non-wellfounded
#####            set theory (see: ACZEL, Peter. Non-Well-Founded Sets, Center for the Study of
#####            Language and Information, Stanford, California, 1988, ISBN 0937073229).
#####            This permits statements like "class is a member of class", unlike traditional
#####            set theories such as Zermelo-Fraenkel set theory found in standard texts
#####            (see: ITÒ¬ K. (editor). Encyclopedic Dictionary of Mathematics, Mathematical
#####            Society of Japan, Edition 2, Cambridge, Massachusetts, MIT Press, 1993,
#####            ISBN 0262590204)
#####        </rdfs:comment>
#####        <rdfs:comment>
#####            NOTE There is a null Class that has no members. Although there is only one
#####            Class that has no members, there can be a Class that has no members in the
#####            actual world, but which does have members in other possible worlds.
#####        </rdfs:comment>
#####        <rdfs:comment>
#####            NOTE The known members of a Class are identified by Classification .
#####        </rdfs:comment>
#####        <rdfs:comment>
#####            EXAMPLE Centrifugal pump is a Class .
#####        </rdfs:comment>
#####        <rdfs:comment>
#####            EXAMPLE Mechanical equipment type is a Class .
#####        </rdfs:comment>
#####        <rdfs:comment>
#####            EXAMPLE Temperature is a Class .
#####        </rdfs:comment>
#####        <rdfs:comment>
#####            EXAMPLE Commercial fusion reactor is a Class, with no members at present.
#####        </rdfs:comment>
#####        <rdfs:comment>
#####            EXAMPLE The Centigrade scale is a Class .
#####        </rdfs:comment>
#####    </owl:Class>

    <owl:Class rdf:ID="ClassOfAbstractObject">
        <rdfs:subClassOf rdf:resource="#Class"/>
        <owl:intersectionOf rdf:parseType="Collection">  
            <owl:Class rdf:about="#ClassOfClass"/>  
            <owl:Class rdf:about="#ClassOfRelationship"/>  
            <owl:Class rdf:about="#ClassOfMultidimensionalObject"/>  
        </owl:intersectionOf>
        <owl:disjointWith rdf:resource="#ClassOfIndividual"/>
        <rdfs:comment>
            DEFINITION A ClassOfAbstractObject is a Class whose members classify members
            of AbstractObject .
        </rdfs:comment>
    </owl:Class>

    <owl:Class rdf:ID="ClassOfActivity">
        <rdfs:subClassOf rdf:resource="#ClassOfArrangedIndividual"/>
        <rdfs:comment>
            DEFINITION A ClassOfActivity is a ClassOfArrangedIndividual whose members are
            instances of Activity .
        </rdfs:comment>
        <rdfs:comment>
            NOTE Behaviour is a term used to describe a ClassOfActivity either where
            there are preconditions and the ClassOfActivity is a response to those
            preconditions, e.g. reaction to touching a hot surface, or where the way an
            activity occurs is described by some property or function, e.g. fluid flow
            being described by the viscosity of the fluid.
        </rdfs:comment>
        <rdfs:comment>
            EXAMPLE Drilling, distilling, and approving can be represented by instances
            of ClassOfActivity .
        </rdfs:comment>
    </owl:Class>

    <owl:Class rdf:ID="ClassOfApproval">
        <rdfs:subClassOf rdf:resource="#ClassOfRelationship"/>
        <owl:disjointWith rdf:resource="#ClassOfApprovalByStatus"/>
        <owl:disjointWith rdf:resource="#ClassOfAssertion"/>
        <owl:disjointWith rdf:resource="#ClassOfCauseOfBeginningOfClassOfIndividual"/>
        <owl:disjointWith rdf:resource="#ClassOfCauseOfEndingOfClassOfIndividual"/>
        <owl:disjointWith rdf:resource="#ClassOfClassification"/>
        <owl:disjointWith rdf:resource="#ClassOfCompositionOfIndividual"/>
        <owl:disjointWith rdf:resource="#ClassOfConnectionOfIndividual"/>
        <owl:disjointWith rdf:resource="#ClassOfFunctionalMapping"/>
        <owl:disjointWith rdf:resource="#ClassOfIndirectProperty"/>
        <owl:disjointWith rdf:resource="#ClassOfIndividualUsedInConnection"/>
        <owl:disjointWith rdf:resource="#ClassOfIntendedRoleAndDomain"/>
        <owl:disjointWith rdf:resource="#ClassOfInvolvementByReference"/>
        <owl:disjointWith rdf:resource="#ClassOfLifecycleStage"/>
        <owl:disjointWith rdf:resource="#ClassOfPossibleRoleAndDomain"/>
        <owl:disjointWith rdf:resource="#ClassOfRecognition"/>
        <owl:disjointWith rdf:resource="#ClassOfRelationshipWithSignature"/>
        <owl:disjointWith rdf:resource="#ClassOfRelativeLocation"/>
        <owl:disjointWith rdf:resource="#ClassOfRepresentationOfThing"/>
        <owl:disjointWith rdf:resource="#ClassOfRepresentationTranslation"/>
        <owl:disjointWith rdf:resource="#ClassOfResponsibilityForRepresentation"/>
        <owl:disjointWith rdf:resource="#ClassOfSpecialization"/>
        <owl:disjointWith rdf:resource="#ClassOfTemporalSequence"/>
        <owl:disjointWith rdf:resource="#ClassOfUsageOfRepresentation"/>
        <owl:disjointWith rdf:resource="#DimensionOfIndividual"/>
        <owl:disjointWith rdf:resource="#PropertyForShapeDimension"/>
        <rdfs:subClassOf>
            <owl:Restriction>
                <owl:onProperty rdf:resource="#classOfApproved"/>
                <owl:allValuesFrom rdf:resource="#ClassOfRelationship"/>
            </owl:Restriction>
        </rdfs:subClassOf>
        <rdfs:subClassOf>
            <owl:Restriction>
                <owl:onProperty rdf:resource="#classOfApprover"/>
                <owl:allValuesFrom rdf:resource="#ClassOfIndividual"/>
            </owl:Restriction>
        </rdfs:subClassOf>
        <rdfs:comment>
            DEFINITION A ClassOfApproval is a ClassOfRelationship whose members are
            members of Approval that indicates that members of the ClassOfIndividual are
            approvers in an Approval for the members of the Class that are approved.
        </rdfs:comment>
        <rdfs:comment>
            EXAMPLE That site managers approve designs for construction
            (a ClassOfInvolvementByReference ) is an example of ClassOfApproval .
        </rdfs:comment>
    </owl:Class>

    <owl:Class rdf:ID="ClassOfApprovalByStatus">
        <rdfs:subClassOf rdf:resource="#ClassOfRelationship"/>
        <owl:disjointWith rdf:resource="#ClassOfAssertion"/>
        <owl:disjointWith rdf:resource="#ClassOfCauseOfBeginningOfClassOfIndividual"/>
        <owl:disjointWith rdf:resource="#ClassOfCauseOfEndingOfClassOfIndividual"/>
        <owl:disjointWith rdf:resource="#ClassOfClassification"/>
        <owl:disjointWith rdf:resource="#ClassOfCompositionOfIndividual"/>
        <owl:disjointWith rdf:resource="#ClassOfConnectionOfIndividual"/>
        <owl:disjointWith rdf:resource="#ClassOfFunctionalMapping"/>
        <owl:disjointWith rdf:resource="#ClassOfIndirectProperty"/>
        <owl:disjointWith rdf:resource="#ClassOfIndividualUsedInConnection"/>
        <owl:disjointWith rdf:resource="#ClassOfIntendedRoleAndDomain"/>
        <owl:disjointWith rdf:resource="#ClassOfInvolvementByReference"/>
        <owl:disjointWith rdf:resource="#ClassOfLifecycleStage"/>
        <owl:disjointWith rdf:resource="#ClassOfPossibleRoleAndDomain"/>
        <owl:disjointWith rdf:resource="#ClassOfRecognition"/>
        <owl:disjointWith rdf:resource="#ClassOfRelationshipWithSignature"/>
        <owl:disjointWith rdf:resource="#ClassOfRelativeLocation"/>
        <owl:disjointWith rdf:resource="#ClassOfRepresentationOfThing"/>
        <owl:disjointWith rdf:resource="#ClassOfRepresentationTranslation"/>
        <owl:disjointWith rdf:resource="#ClassOfResponsibilityForRepresentation"/>
        <owl:disjointWith rdf:resource="#ClassOfSpecialization"/>
        <owl:disjointWith rdf:resource="#ClassOfTemporalSequence"/>
        <owl:disjointWith rdf:resource="#ClassOfUsageOfRepresentation"/>
        <owl:disjointWith rdf:resource="#DimensionOfIndividual"/>
        <owl:disjointWith rdf:resource="#PropertyForShapeDimension"/>
        <rdfs:comment>
            DEFINITION A ClassOfApprovalByStatus is a ClassOfRelationship that indicates
            a status of the approval that is independent of what is being approved by
            whom.
        </rdfs:comment>
        <rdfs:comment>
            EXAMPLE approved, approved with comments, disapproved with comments are
            examples of ClassOfApprovalByStatus .
        </rdfs:comment>
    </owl:Class>

    <owl:Class rdf:ID="ClassOfArrangedIndividual">
        <rdfs:subClassOf rdf:resource="#ClassOfIndividual"/>
        <owl:intersectionOf rdf:parseType="Collection">  
            <owl:Class rdf:about="#ClassOfActivity"/>  
            <owl:Class rdf:about="#ClassOfFeature"/>  
            <owl:Class rdf:about="#ClassOfInformationObject"/>  
            <owl:Class rdf:about="#ClassOfOrganization"/> 
            <owl:Class>
                <owl:unionOf rdf:parseType="Collection">  
                    <owl:Class rdf:about="#ClassOfInanimatePhysicalObject"/>  
                    <owl:Class rdf:about="#ClassOfOrganism"/>  
                </owl:unionOf>
            </owl:Class>
            <owl:Class>
                <owl:unionOf rdf:parseType="Collection">  
                    <owl:Class rdf:about="#ClassOfAtom"/>  
                    <owl:Class rdf:about="#ClassOfBiologicalMatter"/>  
                    <owl:Class rdf:about="#ClassOfCompound"/>  
                    <owl:Class rdf:about="#ClassOfCompositeMaterial"/>  
                    <owl:Class rdf:about="#ClassOfFunctionalObject"/>  
                    <owl:Class rdf:about="#ClassOfInformationPresentation"/>  
                    <owl:Class rdf:about="#ClassOfInformationRepresentation"/>  
                    <owl:Class rdf:about="#ClassOfMolecule"/>  
                    <owl:Class rdf:about="#ClassOfParticulateMaterial"/>  
                    <owl:Class rdf:about="#ClassOfSubAtomicParticle"/>  
                    <owl:Class rdf:about="#CrystallineStructure"/>  
                    <owl:Class rdf:about="#Phase"/>  
                </owl:unionOf>
            </owl:Class>
        </owl:intersectionOf>
        <owl:disjointWith rdf:resource="#ClassOfEvent"/>
        <owl:disjointWith rdf:resource="#ClassOfPeriodInTime"/>
        <owl:disjointWith rdf:resource="#IndividualDimension"/>
        <owl:disjointWith rdf:resource="#Property"/>
        <owl:disjointWith rdf:resource="#Status"/>
        <rdfs:comment>
            DEFINITION A ClassOfArrangedIndividual is a ClassOfIndividual whose members
            are an arrangement of components.
        </rdfs:comment>
        <rdfs:comment>
            NOTE The ONEOF constraint on some of the subtypes does not prevent a
            particular PossibleIndividual from being, say, classified by
            ClassOfBiologicalMatter and a member of a particular
            ClassOfCompositeMaterial . It is only the classes themselves that are not
            members of more than one of the entity types.
        </rdfs:comment>
        <rdfs:comment>
            NOTE Specifications or descriptions of useful objects are often intersections
            of several arrangement classes, allowing both shape and material aspects to
            be constrained. In this part of ISO 15926, such intersections are members of
            ClassOfArrangedIndividual , ClassOfFeature , ClassOfInanimatePhysicalObject ,
            ClassOfOrganization , ClassOfActivity , ClassOfOrganism , or
            ClassOfInformationObject .
        </rdfs:comment>
        <rdfs:comment>
            EXAMPLE Robocop is a ClassOfArrangedIndividual that has some parts that are
            members of some ClassOfInanimatePhysicalObject and parts that are members of
            some ClassOfOrganism .
        </rdfs:comment>
    </owl:Class>

    <owl:Class rdf:ID="ClassOfArrangementOfIndividual">
        <rdfs:subClassOf rdf:resource="#ClassOfCompositionOfIndividual"/>
        <owl:unionOf rdf:parseType="Collection">  
            <owl:Class rdf:about="#ClassOfAssemblyOfIndividual"/>  
            <owl:Class rdf:about="#ClassOfFeatureWholePart"/>  
            <owl:Class rdf:about="#Namespace"/>  
        </owl:unionOf>
        <owl:disjointWith rdf:resource="#ClassOfParticipation"/>
        <owl:disjointWith rdf:resource="#ClassOfTemporalWholePart"/>
        <rdfs:subClassOf>
            <owl:Restriction>
                <owl:onProperty rdf:resource="#classOfWhole"/>
                <owl:allValuesFrom rdf:resource="#ClassOfArrangedIndividual"/>
            </owl:Restriction>
        </rdfs:subClassOf>
        <rdfs:comment>
            DEFINITION A ClassOfArrangementOfIndividual is a
            ClassOfCompositionOfIndividual whose members are instances of
            ArrangementOfIndividual .
        </rdfs:comment>
        <rdfs:comment>
            EXAMPLE The fact that water is made up of H2O molecules is an instance of
            ClassOfArrangementOfIndividual .
        </rdfs:comment>
    </owl:Class>

    <owl:Class rdf:ID="ClassOfAssemblyOfIndividual">
        <rdfs:subClassOf rdf:resource="#ClassOfArrangementOfIndividual"/>
        <owl:disjointWith rdf:resource="#ClassOfFeatureWholePart"/>
        <owl:disjointWith rdf:resource="#Namespace"/>
        <rdfs:comment>
            DEFINITION A ClassOfAssemblyOfIndividual is a ClassOfArrangementOfIndividual
            whose members are instances of AssemblyOfIndividual .
        </rdfs:comment>
        <rdfs:comment>
            EXAMPLE That impellers are parts of centrifugal pumps is a
            ClassOfAssemblyOfIndividual .
        </rdfs:comment>
    </owl:Class>

    <owl:Class rdf:ID="ClassOfAssertion">
        <rdfs:subClassOf rdf:resource="#ClassOfRelationship"/>
        <owl:disjointWith rdf:resource="#ClassOfCauseOfBeginningOfClassOfIndividual"/>
        <owl:disjointWith rdf:resource="#ClassOfCauseOfEndingOfClassOfIndividual"/>
        <owl:disjointWith rdf:resource="#ClassOfClassification"/>
        <owl:disjointWith rdf:resource="#ClassOfCompositionOfIndividual"/>
        <owl:disjointWith rdf:resource="#ClassOfConnectionOfIndividual"/>
        <owl:disjointWith rdf:resource="#ClassOfFunctionalMapping"/>
        <owl:disjointWith rdf:resource="#ClassOfIndirectProperty"/>
        <owl:disjointWith rdf:resource="#ClassOfIndividualUsedInConnection"/>
        <owl:disjointWith rdf:resource="#ClassOfIntendedRoleAndDomain"/>
        <owl:disjointWith rdf:resource="#ClassOfInvolvementByReference"/>
        <owl:disjointWith rdf:resource="#ClassOfLifecycleStage"/>
        <owl:disjointWith rdf:resource="#ClassOfPossibleRoleAndDomain"/>
        <owl:disjointWith rdf:resource="#ClassOfRecognition"/>
        <owl:disjointWith rdf:resource="#ClassOfRelationshipWithSignature"/>
        <owl:disjointWith rdf:resource="#ClassOfRelativeLocation"/>
        <owl:disjointWith rdf:resource="#ClassOfRepresentationOfThing"/>
        <owl:disjointWith rdf:resource="#ClassOfRepresentationTranslation"/>
        <owl:disjointWith rdf:resource="#ClassOfResponsibilityForRepresentation"/>
        <owl:disjointWith rdf:resource="#ClassOfSpecialization"/>
        <owl:disjointWith rdf:resource="#ClassOfTemporalSequence"/>
        <owl:disjointWith rdf:resource="#ClassOfUsageOfRepresentation"/>
        <owl:disjointWith rdf:resource="#DimensionOfIndividual"/>
        <owl:disjointWith rdf:resource="#PropertyForShapeDimension"/>
        <rdfs:comment>
            DEFINITION A ClassOfAssertion is a ClassOfRelationship that describes the
            assertive nature of the member relations.
        </rdfs:comment>
        <rdfs:comment>
            EXAMPLE Asserting, denying, and probabilistic can be represented by instances
            of ClassOfAssertion .
        </rdfs:comment>
    </owl:Class>

    <owl:Class rdf:ID="ClassOfAtom">
        <rdfs:subClassOf rdf:resource="#ClassOfArrangedIndividual"/>
        <owl:disjointWith rdf:resource="#ClassOfBiologicalMatter"/>
        <owl:disjointWith rdf:resource="#ClassOfCompositeMaterial"/>
        <owl:disjointWith rdf:resource="#ClassOfCompound"/>
        <owl:disjointWith rdf:resource="#ClassOfFunctionalObject"/>
        <owl:disjointWith rdf:resource="#ClassOfInformationPresentation"/>
        <owl:disjointWith rdf:resource="#ClassOfInformationRepresentation"/>
        <owl:disjointWith rdf:resource="#ClassOfMolecule"/>
        <owl:disjointWith rdf:resource="#ClassOfParticulateMaterial"/>
        <owl:disjointWith rdf:resource="#ClassOfSubAtomicParticle"/>
        <owl:disjointWith rdf:resource="#CrystallineStructure"/>
        <owl:disjointWith rdf:resource="#Phase"/>
        <rdfs:comment>
            DEFINITION A ClassOfAtom is a ClassOfArrangedIndividual whose members are
            atoms.
        </rdfs:comment>
        <rdfs:comment>
            EXAMPLE All entries in the periodic table of elements can be represented by
            instances of ClassOfAtom .
        </rdfs:comment>
    </owl:Class>

    <owl:Class rdf:ID="ClassOfBiologicalMatter">
        <rdfs:subClassOf rdf:resource="#ClassOfArrangedIndividual"/>
        <owl:disjointWith rdf:resource="#ClassOfCompositeMaterial"/>
        <owl:disjointWith rdf:resource="#ClassOfCompound"/>
        <owl:disjointWith rdf:resource="#ClassOfFunctionalObject"/>
        <owl:disjointWith rdf:resource="#ClassOfInformationPresentation"/>
        <owl:disjointWith rdf:resource="#ClassOfInformationRepresentation"/>
        <owl:disjointWith rdf:resource="#ClassOfMolecule"/>
        <owl:disjointWith rdf:resource="#ClassOfParticulateMaterial"/>
        <owl:disjointWith rdf:resource="#ClassOfSubAtomicParticle"/>
        <owl:disjointWith rdf:resource="#CrystallineStructure"/>
        <owl:disjointWith rdf:resource="#Phase"/>
        <rdfs:comment>
            DEFINITION A ClassOfBiologicalMatter is a ClassOfArrangedIndividual whose
            members are particular types of cell or aggregations of cells.
        </rdfs:comment>
        <rdfs:comment>
            EXAMPLE The classes known as 'blood', 'enzyme', and 'plasma' can be
            represented by instances of ClassOfBiologicalMatter .
        </rdfs:comment>
    </owl:Class>

    <owl:Class rdf:ID="ClassOfCauseOfBeginningOfClassOfIndividual">
        <rdfs:subClassOf rdf:resource="#ClassOfRelationship"/>
        <owl:disjointWith rdf:resource="#ClassOfCauseOfEndingOfClassOfIndividual"/>
        <owl:disjointWith rdf:resource="#ClassOfClassification"/>
        <owl:disjointWith rdf:resource="#ClassOfCompositionOfIndividual"/>
        <owl:disjointWith rdf:resource="#ClassOfConnectionOfIndividual"/>
        <owl:disjointWith rdf:resource="#ClassOfFunctionalMapping"/>
        <owl:disjointWith rdf:resource="#ClassOfIndirectProperty"/>
        <owl:disjointWith rdf:resource="#ClassOfIndividualUsedInConnection"/>
        <owl:disjointWith rdf:resource="#ClassOfIntendedRoleAndDomain"/>
        <owl:disjointWith rdf:resource="#ClassOfInvolvementByReference"/>
        <owl:disjointWith rdf:resource="#ClassOfLifecycleStage"/>
        <owl:disjointWith rdf:resource="#ClassOfPossibleRoleAndDomain"/>
        <owl:disjointWith rdf:resource="#ClassOfRecognition"/>
        <owl:disjointWith rdf:resource="#ClassOfRelationshipWithSignature"/>
        <owl:disjointWith rdf:resource="#ClassOfRelativeLocation"/>
        <owl:disjointWith rdf:resource="#ClassOfRepresentationOfThing"/>
        <owl:disjointWith rdf:resource="#ClassOfRepresentationTranslation"/>
        <owl:disjointWith rdf:resource="#ClassOfResponsibilityForRepresentation"/>
        <owl:disjointWith rdf:resource="#ClassOfSpecialization"/>
        <owl:disjointWith rdf:resource="#ClassOfTemporalSequence"/>
        <owl:disjointWith rdf:resource="#ClassOfUsageOfRepresentation"/>
        <owl:disjointWith rdf:resource="#DimensionOfIndividual"/>
        <owl:disjointWith rdf:resource="#PropertyForShapeDimension"/>
        <rdfs:subClassOf>
            <owl:Restriction>
                <owl:onProperty rdf:resource="#classOfBegun"/>
                <owl:allValuesFrom rdf:resource="#ClassOfIndividual"/>
            </owl:Restriction>
        </rdfs:subClassOf>
        <rdfs:subClassOf>
            <owl:Restriction>
                <owl:onProperty rdf:resource="#classOfCauser"/>
                <owl:allValuesFrom rdf:resource="#ClassOfActivity"/>
            </owl:Restriction>
        </rdfs:subClassOf>
        <rdfs:comment>
            DEFINITION A ClassOfCauseOfBeginningOfClassOfIndividual is a
            ClassOfRelationship that indicates that a member of a ClassOfActivity causes
            the beginning of a member of a ClassOfIndividual .
        </rdfs:comment>
        <rdfs:comment>
            EXAMPLE A car manufacturing activity causes the beginning of a car.
        </rdfs:comment>
    </owl:Class>

    <owl:Class rdf:ID="ClassOfCauseOfEndingOfClassOfIndividual">
        <rdfs:subClassOf rdf:resource="#ClassOfRelationship"/>
        <owl:disjointWith rdf:resource="#ClassOfClassification"/>
        <owl:disjointWith rdf:resource="#ClassOfCompositionOfIndividual"/>
        <owl:disjointWith rdf:resource="#ClassOfConnectionOfIndividual"/>
        <owl:disjointWith rdf:resource="#ClassOfFunctionalMapping"/>
        <owl:disjointWith rdf:resource="#ClassOfIndirectProperty"/>
        <owl:disjointWith rdf:resource="#ClassOfIndividualUsedInConnection"/>
        <owl:disjointWith rdf:resource="#ClassOfIntendedRoleAndDomain"/>
        <owl:disjointWith rdf:resource="#ClassOfInvolvementByReference"/>
        <owl:disjointWith rdf:resource="#ClassOfLifecycleStage"/>
        <owl:disjointWith rdf:resource="#ClassOfPossibleRoleAndDomain"/>
        <owl:disjointWith rdf:resource="#ClassOfRecognition"/>
        <owl:disjointWith rdf:resource="#ClassOfRelationshipWithSignature"/>
        <owl:disjointWith rdf:resource="#ClassOfRelativeLocation"/>
        <owl:disjointWith rdf:resource="#ClassOfRepresentationOfThing"/>
        <owl:disjointWith rdf:resource="#ClassOfRepresentationTranslation"/>
        <owl:disjointWith rdf:resource="#ClassOfResponsibilityForRepresentation"/>
        <owl:disjointWith rdf:resource="#ClassOfSpecialization"/>
        <owl:disjointWith rdf:resource="#ClassOfTemporalSequence"/>
        <owl:disjointWith rdf:resource="#ClassOfUsageOfRepresentation"/>
        <owl:disjointWith rdf:resource="#DimensionOfIndividual"/>
        <owl:disjointWith rdf:resource="#PropertyForShapeDimension"/>
        <rdfs:subClassOf>
            <owl:Restriction>
                <owl:onProperty rdf:resource="#classOfCauser"/>
                <owl:allValuesFrom rdf:resource="#ClassOfActivity"/>
            </owl:Restriction>
        </rdfs:subClassOf>
        <rdfs:subClassOf>
            <owl:Restriction>
                <owl:onProperty rdf:resource="#classOfEnded"/>
                <owl:allValuesFrom rdf:resource="#ClassOfIndividual"/>
            </owl:Restriction>
        </rdfs:subClassOf>
        <rdfs:comment>
            DEFINITION A ClassOfCauseOfEndingOfClassOfIndividual is a ClassOfRelationship
            that indicates that a member of the ClassOfActivity causes the ending of
            a member of the ClassOfIndividual .
        </rdfs:comment>
        <rdfs:comment>
            EXAMPLE A car crushing activity causes the end of the life of a car.
        </rdfs:comment>
    </owl:Class>

    <owl:Class rdf:ID="ClassOfClass">
        <rdfs:subClassOf rdf:resource="#ClassOfAbstractObject"/>
        <owl:intersectionOf rdf:parseType="Collection">  
            <owl:Class rdf:about="#EnumeratedSetOfClass"/>  
            <owl:Class>
                <owl:unionOf rdf:parseType="Collection">  
                    <owl:Class rdf:about="#ArithmeticNumber"/>  
                    <owl:Class rdf:about="#ClassOfClassOfIndividual"/>  
                    <owl:Class rdf:about="#ClassOfClassOfRelationship"/>  
                    <owl:Class rdf:about="#ClassOfNumber"/>  
                    <owl:Class rdf:about="#ClassOfPropertySpace"/>  
                    <owl:Class rdf:about="#ClassOfShapeDimension"/>  
                </owl:unionOf>
            </owl:Class>
        </owl:intersectionOf>
        <rdfs:comment>
            DEFINITION A ClassOfClass is a Class whose members are instances of Class .
        </rdfs:comment>
        <rdfs:comment>
            NOTE When it is necessary to classify a ClassOfClass, another ClassOfClass
            can be used. This is because a ClassOfClass is a Class .
        </rdfs:comment>
    </owl:Class>

    <owl:Class rdf:ID="ClassOfClassOfComposition">
        <rdfs:subClassOf rdf:resource="#ClassOfClassOfRelationship"/>
        <owl:disjointWith rdf:resource="#ClassOfClassOfRelationshipWithSignature"/>
        <owl:disjointWith rdf:resource="#ClassOfClassOfRepresentation"/>
        <owl:disjointWith rdf:resource="#ClassOfClassOfRepresentationTranslation"/>
        <owl:disjointWith rdf:resource="#ClassOfClassOfResponsibilityForRepresentation"/>
        <owl:disjointWith rdf:resource="#ClassOfClassOfUsageOfRepresentation"/>
        <owl:disjointWith rdf:resource="#ClassOfDimensionForShape"/>
        <owl:disjointWith rdf:resource="#ClassOfNamespace"/>
        <owl:disjointWith rdf:resource="#ClassOfScale"/>
        <owl:disjointWith rdf:resource="#DimensionOfShape"/>
        <owl:disjointWith rdf:resource="#PropertySpaceForClassOfShapeDimension"/>
        <rdfs:subClassOf>
            <owl:Restriction>
                <owl:onProperty rdf:resource="#classOfClassOfPart"/>
                <owl:allValuesFrom rdf:resource="#ClassOfClassOfIndividual"/>
            </owl:Restriction>
        </rdfs:subClassOf>
        <rdfs:subClassOf>
            <owl:Restriction>
                <owl:onProperty rdf:resource="#classOfClassOfWhole"/>
                <owl:allValuesFrom rdf:resource="#ClassOfClassOfIndividual"/>
            </owl:Restriction>
        </rdfs:subClassOf>
        <rdfs:comment>
            DEFINITION A ClassOfClassOfComposition is a ClassOfClassOfRelationship whose
            members are instances of ClassOfComposition . It indicates that a member of a
            member of the classOfClassOfPart is a part of a member of an instance of the
            classOfClassOfWhole.
        </rdfs:comment>
        <rdfs:comment>
            EXAMPLE Toxicity description is a classOfClassOfPart of a material data
            sheet, where the description "has carcinogenic components" is a classOfPart
            on the Mogas Material Safety Data Sheet, and copy #5 of the Mogas Material
            Safety Data Sheet has "has carcinogenic components" as a part.
        </rdfs:comment>
    </owl:Class>

    <owl:Class rdf:ID="ClassOfClassOfDefinition">
        <rdfs:subClassOf rdf:resource="#ClassOfClassOfRepresentation"/>
        <rdfs:comment>
            DEFINITION A ClassOfClassOfDefinition is a ClassOfClassOfRepresentation whose
            members are members of ClassOfDefinition .
        </rdfs:comment>
        <rdfs:comment>
            EXAMPLE 'Normative' is a ClassOfClassOfDefinition.
        </rdfs:comment>
    </owl:Class>

    <owl:Class rdf:ID="ClassOfClassOfDescription">
        <rdfs:subClassOf rdf:resource="#ClassOfClassOfRepresentation"/>
        <rdfs:comment>
            DEFINITION A ClassOfClassOfDescription is a ClassOfClassOfRepresentation
            whose members are members of ClassOfDescription .
        </rdfs:comment>
        <rdfs:comment>
            EXAMPLE 'Service description' is a ClassOfClassOfDescription .
        </rdfs:comment>
    </owl:Class>

    <owl:Class rdf:ID="ClassOfClassOfIdentification">
        <rdfs:subClassOf rdf:resource="#ClassOfClassOfRepresentation"/>
        <rdfs:comment>
            DEFINITION A ClassOfClassOfIdentification is a ClassOfClassOfRepresentation
            whose members are members of ClassOfIdentification .
        </rdfs:comment>
        <rdfs:comment>
            EXAMPLE The link between the Class 'family of manufactured parts' and the
            RepresentationForm 'ISO 13584 Basic Semantic Unit', that indicates that part
            families can be identified using ISO 13584, can be represented by an instance
            of ClassOfClassOfIdentification.
        </rdfs:comment>
    </owl:Class>

    <owl:Class rdf:ID="ClassOfClassOfIndividual">
        <rdfs:subClassOf rdf:resource="#ClassOfClass"/>
        <owl:unionOf rdf:parseType="Collection">  
            <owl:Class rdf:about="#ClassOfClassOfInformationRepresentation"/>  
            <owl:Class rdf:about="#ClassOfProperty"/>  
            <owl:Class rdf:about="#ClassOfStatus"/>  
            <owl:Class rdf:about="#ShapeDimension"/>  
        </owl:unionOf>
       <owl:disjointWith rdf:resource="#ClassOfClassOfRelationship"/>
        <owl:disjointWith rdf:resource="#ClassOfNumber"/>
        <owl:disjointWith rdf:resource="#ClassOfPropertySpace"/>
        <owl:disjointWith rdf:resource="#ClassOfShapeDimension"/>
        <rdfs:comment>
            DEFINITION A ClassOfClassOfIndividual is a ClassOfClass whose members are
            instances of ClassOfIndividual .
        </rdfs:comment>
        <rdfs:comment>
            EXAMPLE "Premium Product" is a ClassOfClassOfIndividual that has
            ClassOfIndividual "mogas" as a member.
        </rdfs:comment>
    </owl:Class>

    <owl:Class rdf:ID="ClassOfClassOfInformationRepresentation">
        <rdfs:subClassOf rdf:resource="#ClassOfClassOfIndividual"/>
        <owl:unionOf rdf:parseType="Collection">  
            <owl:Class rdf:about="#DocumentDefinition"/>  
            <owl:Class rdf:about="#Language"/>  
            <owl:Class rdf:about="#RepresentationForm"/>  
        </owl:unionOf>
        <owl:disjointWith rdf:resource="#ClassOfProperty"/>
        <owl:disjointWith rdf:resource="#ClassOfStatus"/>
        <owl:disjointWith rdf:resource="#ShapeDimension"/>
        <rdfs:comment>
            DEFINITION A ClassOfClassOfInformationRepresentation is a
            ClassOfClassOfIndividual that classifies information representation classes.
        </rdfs:comment>
        <rdfs:comment>
            EXAMPLE Integer Octal is a ClassOfClassOfInformationRepresentation whose
            members are all the information representation classes that correspond to
            Octal formatted integers.
        </rdfs:comment>
    </owl:Class>

    <owl:Class rdf:ID="ClassOfClassOfRelationship">
        <rdfs:subClassOf rdf:resource="#ClassOfClass"/>
        <owl:unionOf rdf:parseType="Collection">  
            <owl:Class rdf:about="#ClassOfClassOfComposition"/>  
            <owl:Class rdf:about="#ClassOfClassOfRelationshipWithSignature"/>  
            <owl:Class rdf:about="#ClassOfClassOfRepresentation"/>  
            <owl:Class rdf:about="#ClassOfClassOfRepresentationTranslation"/>  
            <owl:Class rdf:about="#ClassOfClassOfResponsibilityForRepresentation"/>  
            <owl:Class rdf:about="#ClassOfClassOfUsageOfRepresentation"/>  
            <owl:Class rdf:about="#ClassOfDimensionForShape"/>  
            <owl:Class rdf:about="#ClassOfNamespace"/>  
            <owl:Class rdf:about="#ClassOfScale"/>  
            <owl:Class rdf:about="#DimensionOfShape"/>  
            <owl:Class rdf:about="#PropertySpaceForClassOfShapeDimension"/>  
        </owl:unionOf>
        <owl:disjointWith rdf:resource="#ClassOfNumber"/>
        <owl:disjointWith rdf:resource="#ClassOfPropertySpace"/>
        <owl:disjointWith rdf:resource="#ClassOfShapeDimension"/>
        <rdfs:comment>
            DEFINITION A ClassOfClassOfRelationship is a ClassOfClass whose members are
            instances of ClassOfRelationship.
        </rdfs:comment>
        <rdfs:comment>
            EXAMPLE Reflexive is an example of ClassOfClassOfRelationship . A reflexive
            ClassOfRelationship is one that may have the same Thing playing both roles,
            such as connection, where something may be connected to itself.
        </rdfs:comment>
    </owl:Class>

    <owl:Class rdf:ID="ClassOfClassOfRelationshipWithSignature">
        <rdfs:subClassOf rdf:resource="#ClassOfClassOfRelationship"/>
        <rdfs:subClassOf rdf:resource="#ClassOfRelationshipWithSignature"/>
        <owl:disjointWith rdf:resource="#ClassOfClassOfRepresentation"/>
        <owl:disjointWith rdf:resource="#ClassOfClassOfRepresentationTranslation"/>
        <owl:disjointWith rdf:resource="#ClassOfClassOfResponsibilityForRepresentation"/>
        <owl:disjointWith rdf:resource="#ClassOfClassOfUsageOfRepresentation"/>
        <owl:disjointWith rdf:resource="#ClassOfDimensionForShape"/>
        <owl:disjointWith rdf:resource="#ClassOfNamespace"/>
        <owl:disjointWith rdf:resource="#ClassOfScale"/>
        <owl:disjointWith rdf:resource="#DimensionOfShape"/>
        <owl:disjointWith rdf:resource="#PropertySpaceForClassOfShapeDimension"/>
        <rdfs:comment>
            DEFINITION An ClassOfClassOfRelationshipWithSignature is a
            ClassOfClassOfRelationship and ClassOfRelationshipWithSignature.
        </rdfs:comment>
        <rdfs:comment>
            NOTE The purpose of ClassOfClassOfRelationshipWithSignature is to allow other
            types of classes of relationship, not explicitly defined as entity data types
            in this part of ISO 15926, to be defined as reference data.
        </rdfs:comment>
        <rdfs:comment>
            EXAMPLE 'Transitive', with the roles from and to indicating the direction of
            transitivity, is a ClassOfClassOfRelationshipWithSignature.
            (A ClassOfRelationship is transitive if when A relates to B and B relates to C
            then A relates to C, all in the same way).
        </rdfs:comment>
    </owl:Class>

    <owl:Class rdf:ID="ClassOfClassOfRepresentation">
        <rdfs:subClassOf rdf:resource="#ClassOfClassOfRelationship"/>
        <owl:intersectionOf rdf:parseType="Collection">  
            <owl:Class rdf:about="#ClassOfClassOfDefinition"/>  
            <owl:Class rdf:about="#ClassOfClassOfDescription"/>  
            <owl:Class rdf:about="#ClassOfClassOfIdentification"/>  
        </owl:intersectionOf>
        <owl:disjointWith rdf:resource="#ClassOfClassOfRepresentationTranslation"/>
        <owl:disjointWith rdf:resource="#ClassOfClassOfResponsibilityForRepresentation"/>
        <owl:disjointWith rdf:resource="#ClassOfClassOfUsageOfRepresentation"/>
        <owl:disjointWith rdf:resource="#ClassOfDimensionForShape"/>
        <owl:disjointWith rdf:resource="#ClassOfNamespace"/>
        <owl:disjointWith rdf:resource="#ClassOfScale"/>
        <owl:disjointWith rdf:resource="#DimensionOfShape"/>
        <owl:disjointWith rdf:resource="#PropertySpaceForClassOfShapeDimension"/>
        <rdfs:subClassOf>
            <owl:Restriction>
                <owl:onProperty rdf:resource="#classOfPattern"/>
                <owl:allValuesFrom rdf:resource="#ClassOfClassOfInformationRepresentation"/>
            </owl:Restriction>
        </rdfs:subClassOf>
        <rdfs:subClassOf>
            <owl:Restriction>
                <owl:onProperty rdf:resource="#classOfRepresented"/>
                <owl:allValuesFrom rdf:resource="#Class"/>
            </owl:Restriction>
        </rdfs:subClassOf>
        <rdfs:comment>
            DEFINITION A ClassOfClassOfRepresentation is a ClassOfClassOfRelationship
            whose members are instances of ClassOfRepresentationOfThing .
        </rdfs:comment>
        <rdfs:comment>
            EXAMPLE The link that indicates that members of the class 'document' can be
            represented by patterns of the class 'XML' is a ClassOfClassOfRepresentation .
        </rdfs:comment>
    </owl:Class>

    <owl:Class rdf:ID="ClassOfClassOfRepresentationTranslation">
        <rdfs:subClassOf rdf:resource="#ClassOfClassOfRelationship"/>
        <owl:disjointWith rdf:resource="#ClassOfClassOfResponsibilityForRepresentation"/>
        <owl:disjointWith rdf:resource="#ClassOfClassOfUsageOfRepresentation"/>
        <owl:disjointWith rdf:resource="#ClassOfDimensionForShape"/>
        <owl:disjointWith rdf:resource="#ClassOfNamespace"/>
        <owl:disjointWith rdf:resource="#ClassOfScale"/>
        <owl:disjointWith rdf:resource="#DimensionOfShape"/>
        <owl:disjointWith rdf:resource="#PropertySpaceForClassOfShapeDimension"/>
        <rdfs:subClassOf>
            <owl:Restriction>
                <owl:onProperty rdf:resource="#classOfFirst"/>
                <owl:allValuesFrom rdf:resource="#ClassOfClassOfInformationRepresentation"/>
            </owl:Restriction>
        </rdfs:subClassOf>
        <rdfs:subClassOf>
            <owl:Restriction>
                <owl:onProperty rdf:resource="#classOfSecond"/>
                <owl:allValuesFrom rdf:resource="#ClassOfClassOfInformationRepresentation"/>
            </owl:Restriction>
        </rdfs:subClassOf>
        <rdfs:comment>
            DEFINITION A ClassOfClassOfRepresentationTranslation is a
            ClassOfClassOfRelationship whose members are members of
            ClassOfRepresentationTranslation .
        </rdfs:comment>
        <rdfs:comment>
            EXAMPLE The class ASCII whose members include all translation classes between
            members of the ASCII Binary and ASCII Text representation classes is a
            ClassOfClassOfRepresentationTranslation .
        </rdfs:comment>
    </owl:Class>

    <owl:Class rdf:ID="ClassOfClassOfResponsibilityForRepresentation">
        <rdfs:subClassOf rdf:resource="#ClassOfClassOfRelationship"/>
        <owl:disjointWith rdf:resource="#ClassOfClassOfUsageOfRepresentation"/>
        <owl:disjointWith rdf:resource="#ClassOfDimensionForShape"/>
        <owl:disjointWith rdf:resource="#ClassOfNamespace"/>
        <owl:disjointWith rdf:resource="#ClassOfScale"/>
        <owl:disjointWith rdf:resource="#DimensionOfShape"/>
        <owl:disjointWith rdf:resource="#PropertySpaceForClassOfShapeDimension"/>
        <rdfs:subClassOf>
            <owl:Restriction>
                <owl:onProperty rdf:resource="#classOfClassOfControlled"/>
                <owl:allValuesFrom rdf:resource="#ClassOfClassOfRepresentation"/>
            </owl:Restriction>
        </rdfs:subClassOf>
        <rdfs:subClassOf>
            <owl:Restriction>
                <owl:onProperty rdf:resource="#controller"/>
                <owl:allValuesFrom rdf:resource="#PossibleIndividual"/>
            </owl:Restriction>
        </rdfs:subClassOf>
        <rdfs:comment>
            DEFINITION A ClassOfClassOfResponsibilityForRepresentation is a
            ClassOfClassOfRelationship whose members are members of
            ClassOfResponsibilityForRepresentation linking the controller to a set of
            representations.
        </rdfs:comment>
        <rdfs:comment>
            EXAMPLE The link between Weir and the identification set between Weir pumps
            and Weir serial numbers indicating that the identifications are defined by
            Weir can be represented by an instance of
            ClassOfClassOfResponsibilityForRepresentation .
        </rdfs:comment>
    </owl:Class>

    <owl:Class rdf:ID="ClassOfClassOfUsageOfRepresentation">
        <rdfs:subClassOf rdf:resource="#ClassOfClassOfRelationship"/>
        <owl:disjointWith rdf:resource="#ClassOfDimensionForShape"/>
        <owl:disjointWith rdf:resource="#ClassOfNamespace"/>
        <owl:disjointWith rdf:resource="#ClassOfScale"/>
        <owl:disjointWith rdf:resource="#DimensionOfShape"/>
        <owl:disjointWith rdf:resource="#PropertySpaceForClassOfShapeDimension"/>
        <rdfs:subClassOf>
            <owl:Restriction>
                <owl:onProperty rdf:resource="#classOfClassOfUsed"/>
                <owl:allValuesFrom rdf:resource="#ClassOfClassOfRepresentation"/>
            </owl:Restriction>
        </rdfs:subClassOf>
        <rdfs:subClassOf>
            <owl:Restriction>
                <owl:onProperty rdf:resource="#user"/>
                <owl:allValuesFrom rdf:resource="#PossibleIndividual"/>
            </owl:Restriction>
        </rdfs:subClassOf>
        <rdfs:comment>
            DEFINITION A ClassOfClassOfUsageOfRepresentation is a
            ClassOfClassOfRelationship whose members are members of
            ClassOfUsageOfRepresentation linking the user to a set of representations.
        </rdfs:comment>
        <rdfs:comment>
            EXAMPLE The link between a user company and the identification set between
            Weir pumps and Weir serial numbers indicating that the user company uses the
            Weir identifiers can be represented by an instance of
            ClassOfClassOfUsageOfRepresentation.
        </rdfs:comment>
    </owl:Class>

    <owl:Class rdf:ID="ClassOfClassification">
        <rdfs:subClassOf rdf:resource="#ClassOfRelationship"/>
        <owl:disjointWith rdf:resource="#ClassOfCompositionOfIndividual"/>
        <owl:disjointWith rdf:resource="#ClassOfConnectionOfIndividual"/>
        <owl:disjointWith rdf:resource="#ClassOfFunctionalMapping"/>
        <owl:disjointWith rdf:resource="#ClassOfIndirectProperty"/>
        <owl:disjointWith rdf:resource="#ClassOfIndividualUsedInConnection"/>
        <owl:disjointWith rdf:resource="#ClassOfIntendedRoleAndDomain"/>
        <owl:disjointWith rdf:resource="#ClassOfInvolvementByReference"/>
        <owl:disjointWith rdf:resource="#ClassOfLifecycleStage"/>
        <owl:disjointWith rdf:resource="#ClassOfPossibleRoleAndDomain"/>
        <owl:disjointWith rdf:resource="#ClassOfRecognition"/>
        <owl:disjointWith rdf:resource="#ClassOfRelationshipWithSignature"/>
        <owl:disjointWith rdf:resource="#ClassOfRelativeLocation"/>
        <owl:disjointWith rdf:resource="#ClassOfRepresentationOfThing"/>
        <owl:disjointWith rdf:resource="#ClassOfRepresentationTranslation"/>
        <owl:disjointWith rdf:resource="#ClassOfResponsibilityForRepresentation"/>
        <owl:disjointWith rdf:resource="#ClassOfSpecialization"/>
        <owl:disjointWith rdf:resource="#ClassOfTemporalSequence"/>
        <owl:disjointWith rdf:resource="#ClassOfUsageOfRepresentation"/>
        <owl:disjointWith rdf:resource="#DimensionOfIndividual"/>
        <owl:disjointWith rdf:resource="#PropertyForShapeDimension"/>
        <rdfs:subClassOf>
            <owl:Restriction>
                <owl:onProperty rdf:resource="#classOfClassified"/>
                <owl:allValuesFrom rdf:resource="#Class"/>
            </owl:Restriction>
        </rdfs:subClassOf>
        <rdfs:subClassOf>
            <owl:Restriction>
                <owl:onProperty rdf:resource="#classOfClassifier"/>
                <owl:allValuesFrom rdf:resource="#ClassOfClass"/>
            </owl:Restriction>
        </rdfs:subClassOf>
        <rdfs:comment>
            DEFINITION A ClassOfClassification is a ClassOfRelationship whose members
            are members of Classification . A ClassOfClassification indicates that a
            member of the classOfClassified Class is classified by one or more members
            of the classOfClassifier ClassOfClass .
        </rdfs:comment>
        <rdfs:comment>
            EXAMPLE The link between Class centrifugal pump and the ClassOfProperty 'RPM',
            indicating that a centrifugal pump is a member of at least one RPM class,
            can be represented by an instance of ClassOfClassification .
        </rdfs:comment>
        <rdfs:comment>
            NOTE Since in OWL there is no Classification possible because of the use of
            the standard rdf:type construct, this ClassOfClassification cannot be used
            as such.
        </rdfs:comment>
    </owl:Class>

    <owl:Class rdf:ID="ClassOfCompositeMaterial">
        <rdfs:subClassOf rdf:resource="#ClassOfArrangedIndividual"/>
        <owl:disjointWith rdf:resource="#ClassOfCompound"/>
        <owl:disjointWith rdf:resource="#ClassOfFunctionalObject"/>
        <owl:disjointWith rdf:resource="#ClassOfInformationPresentation"/>
        <owl:disjointWith rdf:resource="#ClassOfInformationRepresentation"/>
        <owl:disjointWith rdf:resource="#ClassOfMolecule"/>
        <owl:disjointWith rdf:resource="#ClassOfParticulateMaterial"/>
        <owl:disjointWith rdf:resource="#ClassOfSubAtomicParticle"/>
        <owl:disjointWith rdf:resource="#CrystallineStructure"/>
        <owl:disjointWith rdf:resource="#Phase"/>
        <rdfs:comment>
            DEFINITION A ClassOfCompositeMaterial is a ClassOfArrangedIndividual whose
            members have a common arrangement of separable compounds.
        </rdfs:comment>
        <rdfs:comment>
            EXAMPLE Laminates such as plywood, fibreglass, and carbon fibre can be
            represented by instances of ClassOfCompositeMaterial.
        </rdfs:comment>
        <rdfs:comment>
            EXAMPLE Wood, muscle, and skin can be represented by instances of
            ClassOfCompositeMaterial.
        </rdfs:comment>
    </owl:Class>

    <owl:Class rdf:ID="ClassOfCompositionOfIndividual">
        <rdf:type rdf:resource="#ClassOfClassOfComposition"/>
        <rdfs:subClassOf rdf:resource="#ClassOfRelationship"/>
        <owl:unionOf rdf:parseType="Collection">  
            <owl:Class rdf:about="#ClassOfArrangementOfIndividual"/>  
            <owl:Class rdf:about="#ClassOfParticipation"/>  
            <owl:Class rdf:about="#ClassOfTemporalWholePart"/>  
        </owl:unionOf>
        <owl:disjointWith rdf:resource="#ClassOfConnectionOfIndividual"/>
        <owl:disjointWith rdf:resource="#ClassOfFunctionalMapping"/>
        <owl:disjointWith rdf:resource="#ClassOfIndirectProperty"/>
        <owl:disjointWith rdf:resource="#ClassOfIndividualUsedInConnection"/>
        <owl:disjointWith rdf:resource="#ClassOfIntendedRoleAndDomain"/>
        <owl:disjointWith rdf:resource="#ClassOfInvolvementByReference"/>
        <owl:disjointWith rdf:resource="#ClassOfLifecycleStage"/>
        <owl:disjointWith rdf:resource="#ClassOfPossibleRoleAndDomain"/>
        <owl:disjointWith rdf:resource="#ClassOfRecognition"/>
        <owl:disjointWith rdf:resource="#ClassOfRelationshipWithSignature"/>
        <owl:disjointWith rdf:resource="#ClassOfRelativeLocation"/>
        <owl:disjointWith rdf:resource="#ClassOfRepresentationOfThing"/>
        <owl:disjointWith rdf:resource="#ClassOfRepresentationTranslation"/>
        <owl:disjointWith rdf:resource="#ClassOfResponsibilityForRepresentation"/>
        <owl:disjointWith rdf:resource="#ClassOfSpecialization"/>
        <owl:disjointWith rdf:resource="#ClassOfTemporalSequence"/>
        <owl:disjointWith rdf:resource="#ClassOfUsageOfRepresentation"/>
        <owl:disjointWith rdf:resource="#DimensionOfIndividual"/>
        <owl:disjointWith rdf:resource="#PropertyForShapeDimension"/>
        <rdfs:subClassOf>
            <owl:Restriction>
                <owl:onProperty rdf:resource="#classOfPart"/>
                <owl:allValuesFrom rdf:resource="#ClassOfIndividual"/>
            </owl:Restriction>
        </rdfs:subClassOf>
        <rdfs:subClassOf>
            <owl:Restriction>
                <owl:onProperty rdf:resource="#classOfWhole"/>
                <owl:allValuesFrom rdf:resource="#ClassOfIndividual"/>
            </owl:Restriction>
        </rdfs:subClassOf>
        <rdfs:comment>
            DEFINITION A ClassOfCompositionOfIndividual is a ClassOfRelationship whose
            members are members of CompositionOfIndividual .
        </rdfs:comment>
        <rdfs:comment>
            EXAMPLE That piles of sand may have grains of sand as parts is an example of
            ClassOfCompositionOfIndividual .
        </rdfs:comment>
    </owl:Class>

    <owl:Class rdf:ID="ClassOfCompound">
        <rdfs:subClassOf rdf:resource="#ClassOfArrangedIndividual"/>
        <owl:disjointWith rdf:resource="#ClassOfFunctionalObject"/>
        <owl:disjointWith rdf:resource="#ClassOfInformationPresentation"/>
        <owl:disjointWith rdf:resource="#ClassOfInformationRepresentation"/>
        <owl:disjointWith rdf:resource="#ClassOfMolecule"/>
        <owl:disjointWith rdf:resource="#ClassOfParticulateMaterial"/>
        <owl:disjointWith rdf:resource="#ClassOfSubAtomicParticle"/>
        <owl:disjointWith rdf:resource="#CrystallineStructure"/>
        <owl:disjointWith rdf:resource="#Phase"/>
        <rdfs:comment>
            DEFINITION A ClassOfCompound is a ClassOfArrangedIndividual whose members
            consist of arrangements of molecules of the same or different types, bound
            together by intermolecular forces. This includes both mixtures and alloys.
        </rdfs:comment>
        <rdfs:comment>
            EXAMPLE Water, sulphuric acid, sand, limestone, and steel can be represented
            by instances of ClassOfCompound .
        </rdfs:comment>
    </owl:Class>

    <owl:Class rdf:ID="ClassOfConnectionOfIndividual">
        <rdfs:subClassOf rdf:resource="#ClassOfRelationship"/>
        <owl:unionOf rdf:parseType="Collection">  
            <owl:Class rdf:about="#ClassOfDirectConnection"/>  
            <owl:Class rdf:about="#ClassOfIndirectConnection"/>  
        </owl:unionOf>
        <owl:disjointWith rdf:resource="#ClassOfFunctionalMapping"/>
        <owl:disjointWith rdf:resource="#ClassOfIndirectProperty"/>
        <owl:disjointWith rdf:resource="#ClassOfIndividualUsedInConnection"/>
        <owl:disjointWith rdf:resource="#ClassOfIntendedRoleAndDomain"/>
        <owl:disjointWith rdf:resource="#ClassOfInvolvementByReference"/>
        <owl:disjointWith rdf:resource="#ClassOfLifecycleStage"/>
        <owl:disjointWith rdf:resource="#ClassOfPossibleRoleAndDomain"/>
        <owl:disjointWith rdf:resource="#ClassOfRecognition"/>
        <owl:disjointWith rdf:resource="#ClassOfRelationshipWithSignature"/>
        <owl:disjointWith rdf:resource="#ClassOfRelativeLocation"/>
        <owl:disjointWith rdf:resource="#ClassOfRepresentationOfThing"/>
        <owl:disjointWith rdf:resource="#ClassOfRepresentationTranslation"/>
        <owl:disjointWith rdf:resource="#ClassOfResponsibilityForRepresentation"/>
        <owl:disjointWith rdf:resource="#ClassOfSpecialization"/>
        <owl:disjointWith rdf:resource="#ClassOfTemporalSequence"/>
        <owl:disjointWith rdf:resource="#ClassOfUsageOfRepresentation"/>
        <owl:disjointWith rdf:resource="#DimensionOfIndividual"/>
        <owl:disjointWith rdf:resource="#PropertyForShapeDimension"/>
        <rdfs:subClassOf>
            <owl:Restriction>
                <owl:onProperty rdf:resource="#classOfSide1"/>
                <owl:allValuesFrom rdf:resource="#ClassOfIndividual"/>
            </owl:Restriction>
        </rdfs:subClassOf>
        <rdfs:subClassOf>
            <owl:Restriction>
                <owl:onProperty rdf:resource="#classOfSide2"/>
                <owl:allValuesFrom rdf:resource="#ClassOfIndividual"/>
            </owl:Restriction>
        </rdfs:subClassOf>
        <rdfs:comment>
            DEFINITION A ClassOfConnectionOfIndividual is a ClassOfRelationship whose
            members are members of ConnectionOfIndividual. It indicates that a member
            of the classOfSide1 ClassOfIndividual can be connected to a member of the
            classOfSide2 ClassOfIndividual .
        </rdfs:comment>
        <rdfs:comment>
            NOTE 1 The classOfSide1 and classOfSide2 indicate the ClassOfIndividual that
            is the side1 and side2 respectively in a ConnectionOfIndividual that is a
            member of this ClassOfConnectionOfIndividual .
        </rdfs:comment>
        <rdfs:comment>
            NOTE 2 Flexible, rigid, and welded cannot be represented as instances of
            ClassOfConnectionOfIndividual , these are classes of the materials connected
            or used in the connection.
        </rdfs:comment>
        <rdfs:comment>
            EXAMPLE Electrical connection between wires is a
            ClassOfConnectionOfIndividual .
        </rdfs:comment>
    </owl:Class>

    <owl:Class rdf:ID="ClassOfContainmentOfIndividual">
        <rdfs:subClassOf rdf:resource="#ClassOfRelativeLocation"/>
        <rdfs:comment>
            DEFINITION A ClassOfContainmentOfIndividual is a ClassOfRelativeLocation
            whose members are instances of ContainmentOfIndividual . It indicates that
            a member of the classOfLocator ClassOfIndividual can contain a member of the
            classOfLocated ClassOfIndividual .
        </rdfs:comment>
        <rdfs:comment>
            EXAMPLE That 'de-icing fluid' can be contained by a '1500ml screw-top plastic
            bottle' is a ClassOfContainmentOfIndividual .
        </rdfs:comment>
    </owl:Class>

    <owl:Class rdf:ID="ClassOfDefinition">
        <rdf:type rdf:resource="#ClassOfClassOfDefinition"/>
        <rdfs:subClassOf rdf:resource="#ClassOfRepresentationOfThing"/>
        <rdfs:subClassOf>
            <owl:Restriction>
                <owl:onProperty rdf:resource="#represented"/>
                <owl:allValuesFrom rdf:resource="#Class"/>
            </owl:Restriction>
        </rdfs:subClassOf>
        <rdfs:comment>
            DEFINITION A ClassOfDefinition is a ClassOfRepresentationOfThing that
            indicates the pattern is a definition of the represented Class .
        </rdfs:comment>
        <rdfs:comment>
            EXAMPLE The link between the pattern 'pump' and the Class that goes by that
            name in English can be represented by an instance of ClassOfDefinition .
        </rdfs:comment>
    </owl:Class>

    <owl:Class rdf:ID="ClassOfDescription">
        <rdf:type rdf:resource="#ClassOfClassOfDescription"/>
        <rdfs:subClassOf rdf:resource="#ClassOfRepresentationOfThing"/>
        <rdfs:comment>
            DEFINITION A ClassOfDescription is a ClassOfRepresentationOfThing that
            indicates the pattern is a description of the represented Thing.
        </rdfs:comment>
        <rdfs:comment>
            EXAMPLE The link between the pattern 'this is an old bilge pump' and a
            particular pump can be represented by an instance of ClassOfDescription .
        </rdfs:comment>
    </owl:Class>

    <owl:Class rdf:ID="ClassOfDimensionForShape">
        <rdfs:subClassOf rdf:resource="#ClassOfClassOfRelationship"/>
        <owl:disjointWith rdf:resource="#ClassOfNamespace"/>
        <owl:disjointWith rdf:resource="#ClassOfScale"/>
        <owl:disjointWith rdf:resource="#DimensionOfShape"/>
        <owl:disjointWith rdf:resource="#PropertySpaceForClassOfShapeDimension"/>
        <rdfs:subClassOf>
            <owl:Restriction>
                <owl:onProperty rdf:resource="#classOfDimension"/>
                <owl:allValuesFrom rdf:resource="#ClassOfShapeDimension"/>
            </owl:Restriction>
        </rdfs:subClassOf>
        <rdfs:subClassOf>
            <owl:Restriction>
                <owl:onProperty rdf:resource="#classOfShape"/>
                <owl:allValuesFrom rdf:resource="#ClassOfShape"/>
            </owl:Restriction>
        </rdfs:subClassOf>
        <rdfs:comment>
            DEFINITION A ClassOfDimensionForShape is a ClassOfClassOfRelationship that
            indicates that members of the classOfShape have a dimension that is a
            member of the classOfDimension .
        </rdfs:comment>
        <rdfs:comment>
            EXAMPLE Specifying that members of the "class of circle" have members of
            "class of diameter" is an instance of ClassOfDimensionForShape .
        </rdfs:comment>
    </owl:Class>

    <owl:Class rdf:ID="ClassOfDirectConnection">
        <rdfs:subClassOf rdf:resource="#ClassOfConnectionOfIndividual"/>
        <owl:disjointWith rdf:resource="#ClassOfIndirectConnection"/>
        <rdfs:comment>
            DEFINITION A ClassOfDirectConnection is a ClassOfConnectionOfIndividual whose
            members are members of DirectConnection .
        </rdfs:comment>
        <rdfs:comment>
            EXAMPLE Three-pin electrical plug into three-pin socket is an example of
            ClassOfDirectConnection .
        </rdfs:comment>
    </owl:Class>

    <owl:Class rdf:ID="ClassOfEvent">
        <rdfs:subClassOf rdf:resource="#ClassOfIndividual"/>
        <owl:disjointWith rdf:resource="#ClassOfPeriodInTime"/>
        <owl:disjointWith rdf:resource="#IndividualDimension"/>
        <owl:disjointWith rdf:resource="#Property"/>
        <owl:disjointWith rdf:resource="#Status"/>
        <rdfs:comment>
            DEFINITION A ClassOfEvent is a ClassOfIndividual whose members are members
            of Event .
        </rdfs:comment>
        <rdfs:comment>
            EXAMPLE Continuous and instantaneous are instances of ClassOfEvent. A
            continuous event is one such as a stream boundary flowing through a pipe.
        </rdfs:comment>
    </owl:Class>

    <owl:Class rdf:ID="ClassOfExpressInformationRepresentation">
        <rdfs:subClassOf rdf:resource="#ClassOfInformationRepresentation"/>
        <owl:unionOf rdf:parseType="Collection">  
            <owl:Class rdf:about="#ExpressBinary"/>  
            <owl:Class rdf:about="#ExpressBoolean"/>  
            <owl:Class rdf:about="#ExpressInteger"/>  
            <owl:Class rdf:about="#ExpressLogical"/>  
            <owl:Class rdf:about="#ExpressReal"/>  
            <owl:Class rdf:about="#ExpressString"/>  
        </owl:unionOf>
        <owl:disjointWith rdf:resource="#RepresentationOfGregorianDateAndUtcTime"/>
        <rdfs:comment>
            DEFINITION A ClassOfExpressInformationRepresentation is a
            ClassOfInformationRepresentation that is defined by ISO 10303-11.
        </rdfs:comment>
    </owl:Class>

    <owl:Class rdf:ID="ClassOfFeature">
        <rdfs:subClassOf rdf:resource="#ClassOfArrangedIndividual"/>
        <rdfs:comment>
            DEFINITION A ClassOfFeature is a ClassOfArrangedIndividual whose members are
            contiguous, non-separable parts of some PossibleIndividual and have an
            incompletely defined boundary.
        </rdfs:comment>
        <rdfs:comment>
            EXAMPLE The classes known as 'mountain', 'groove', 'rim', 'nozzle', 'nose',
            and 'raised face' can all be represented as instances of ClassOfFeature .
        </rdfs:comment>
    </owl:Class>

    <owl:Class rdf:ID="ClassOfFeatureWholePart">
        <rdfs:subClassOf rdf:resource="#ClassOfArrangementOfIndividual"/>
        <owl:disjointWith rdf:resource="#Namespace"/>
        <rdfs:comment>
            DEFINITION A ClassOfFeatureWholePart is a ClassOfArrangementOfIndividual
            whose members are instances of FeatureWholePart .
        </rdfs:comment>
        <rdfs:comment>
            EXAMPLE Thermowells have stems, and tables have tops are examples of
            ClassOfFeatureWholePart .
        </rdfs:comment>
    </owl:Class>

    <owl:Class rdf:ID="ClassOfFunctionalMapping">
        <rdfs:subClassOf rdf:resource="#ClassOfRelationship"/>
        <owl:disjointWith rdf:resource="#ClassOfIndirectProperty"/>
        <owl:disjointWith rdf:resource="#ClassOfIndividualUsedInConnection"/>
        <owl:disjointWith rdf:resource="#ClassOfIntendedRoleAndDomain"/>
        <owl:disjointWith rdf:resource="#ClassOfInvolvementByReference"/>
        <owl:disjointWith rdf:resource="#ClassOfLifecycleStage"/>
        <owl:disjointWith rdf:resource="#ClassOfPossibleRoleAndDomain"/>
        <owl:disjointWith rdf:resource="#ClassOfRecognition"/>
        <owl:disjointWith rdf:resource="#ClassOfRelationshipWithSignature"/>
        <owl:disjointWith rdf:resource="#ClassOfRelativeLocation"/>
        <owl:disjointWith rdf:resource="#ClassOfRepresentationOfThing"/>
        <owl:disjointWith rdf:resource="#ClassOfRepresentationTranslation"/>
        <owl:disjointWith rdf:resource="#ClassOfResponsibilityForRepresentation"/>
        <owl:disjointWith rdf:resource="#ClassOfSpecialization"/>
        <owl:disjointWith rdf:resource="#ClassOfTemporalSequence"/>
        <owl:disjointWith rdf:resource="#ClassOfUsageOfRepresentation"/>
        <owl:disjointWith rdf:resource="#DimensionOfIndividual"/>
        <owl:disjointWith rdf:resource="#PropertyForShapeDimension"/>
        <rdfs:subClassOf>
            <owl:Restriction>
                <owl:onProperty rdf:resource="#codomain"/>
                <owl:allValuesFrom rdf:resource="#Class"/>
            </owl:Restriction>
        </rdfs:subClassOf>
        <rdfs:subClassOf>
            <owl:Restriction>
                <owl:onProperty rdf:resource="#domain"/>
                <owl:allValuesFrom rdf:resource="#Class"/>
            </owl:Restriction>
        </rdfs:subClassOf>
        <rdfs:comment>
            DEFINITION A ClassOfFunctionalMapping is a ClassOfRelationship that is a many
            to one mapping. A ClassOfRelationship is a function.
        </rdfs:comment>
        <rdfs:comment>
            NOTE This entity type would naturally have the name of function, but this is
            an EXPRESS reserved word (note that the data model was expressed in EXPRESS).
        </rdfs:comment>
        <rdfs:comment>
            NOTE 2 The significance of a function being a many to one mapping is that the
            same answer is always obtained. So, for example, 5 - 3 always gives 2. Note
            that the minus function on two other arguments can also give 2.
        </rdfs:comment>
        <rdfs:comment>
            NOTE 3 When there are several arguments to a function, then these are
            presented in a MultidimensionalObject .
        </rdfs:comment>
        <rdfs:comment>
            EXAMPLE Minus is an example of ClassOfFunctionalMapping .
        </rdfs:comment>
    </owl:Class>

    <owl:Class rdf:ID="ClassOfFunctionalObject">
        <rdfs:subClassOf rdf:resource="#ClassOfArrangedIndividual"/>
        <owl:disjointWith rdf:resource="#ClassOfInformationPresentation"/>
        <owl:disjointWith rdf:resource="#ClassOfInformationRepresentation"/>
        <owl:disjointWith rdf:resource="#ClassOfMolecule"/>
        <owl:disjointWith rdf:resource="#ClassOfParticulateMaterial"/>
        <owl:disjointWith rdf:resource="#ClassOfSubAtomicParticle"/>
        <owl:disjointWith rdf:resource="#CrystallineStructure"/>
        <owl:disjointWith rdf:resource="#Phase"/>
        <rdfs:comment>
            DEFINITION A ClassOfFunctionalObject is a ClassOfArrangedIndividual that
            indicates the function or purpose of an object.
        </rdfs:comment>
        <rdfs:comment>
            EXAMPLE Pump, valve, and car are examples of ClassOfFunctionalObject .
            Particular models of pump, valve, car, etc are instances of
            ClassOfInanimatePhysicalObject that are specializations of these instances
            of ClassOfFunctionalObject .
        </rdfs:comment>
    </owl:Class>

    <owl:Class rdf:ID="ClassOfIdentification">
        <rdf:type rdf:resource="#ClassOfClassOfIdentification"/>
        <rdfs:subClassOf rdf:resource="#ClassOfRepresentationOfThing"/>
        <rdfs:comment>
            DEFINITION A ClassOfIdentification is a ClassOfRepresentationOfThing that
            indicates that the pattern is used to refer to the represented Thing.
        </rdfs:comment>
        <rdfs:comment>
            EXAMPLE The link between the pattern 'AC-1234' and a particular pump,
            indicating that members of 'AC-1234' are used to refer to the pump, can be
            represented by an instance of ClassOfIdentification .
        </rdfs:comment>
    </owl:Class>

    <owl:Class rdf:ID="ClassOfInanimatePhysicalObject">
        <rdfs:subClassOf rdf:resource="#ClassOfArrangedIndividual"/>
        <owl:disjointWith rdf:resource="#Organism"/>
        <rdfs:comment>
            DEFINITION A ClassOfInanimatePhysicalObject is a ClassOfArrangedIndividual
            whose members are not living.
        </rdfs:comment>
        <rdfs:comment>
            EXAMPLE The classes known as 'oil' and 'oilwell' can be represented by
            instances of ClassOfInanimatePhysicalObject .
        </rdfs:comment>
    </owl:Class>

    <owl:Class rdf:ID="ClassOfIndirectConnection">
        <rdfs:subClassOf rdf:resource="#ClassOfConnectionOfIndividual"/>
        <rdfs:comment>
            DEFINITION A ClassOfIndirectConnection is a ClassOfConnectionOfIndividual
            whose members are members of IndirectConnection .
        </rdfs:comment>
        <rdfs:comment>
            EXAMPLE Drip pipe indirectly connected to drain funnel is an example of
            ClassOfIndirectConnection .
        </rdfs:comment>
    </owl:Class>

    <owl:Class rdf:ID="ClassOfIndirectProperty">
        <rdfs:subClassOf rdf:resource="#ClassOfRelationship"/>
        <owl:disjointWith rdf:resource="#ClassOfIndividualUsedInConnection"/>
        <owl:disjointWith rdf:resource="#ClassOfIntendedRoleAndDomain"/>
        <owl:disjointWith rdf:resource="#ClassOfInvolvementByReference"/>
        <owl:disjointWith rdf:resource="#ClassOfLifecycleStage"/>
        <owl:disjointWith rdf:resource="#ClassOfPossibleRoleAndDomain"/>
        <owl:disjointWith rdf:resource="#ClassOfRecognition"/>
        <owl:disjointWith rdf:resource="#ClassOfRelationshipWithSignature"/>
        <owl:disjointWith rdf:resource="#ClassOfRelativeLocation"/>
        <owl:disjointWith rdf:resource="#ClassOfRepresentationOfThing"/>
        <owl:disjointWith rdf:resource="#ClassOfRepresentationTranslation"/>
        <owl:disjointWith rdf:resource="#ClassOfResponsibilityForRepresentation"/>
        <owl:disjointWith rdf:resource="#ClassOfSpecialization"/>
        <owl:disjointWith rdf:resource="#ClassOfTemporalSequence"/>
        <owl:disjointWith rdf:resource="#ClassOfUsageOfRepresentation"/>
        <owl:disjointWith rdf:resource="#DimensionOfIndividual"/>
        <owl:disjointWith rdf:resource="#PropertyForShapeDimension"/>
        <rdfs:subClassOf>
            <owl:Restriction>
                <owl:onProperty rdf:resource="#classOfPossessor"/>
                <owl:allValuesFrom rdf:resource="#ClassOfIndividual"/>
            </owl:Restriction>
        </rdfs:subClassOf>
        <rdfs:subClassOf>
            <owl:Restriction>
                <owl:onProperty rdf:resource="#propertySpace"/>
                <owl:allValuesFrom rdf:resource="#PropertySpace"/>
            </owl:Restriction>
        </rdfs:subClassOf>
        <rdfs:comment>
            DEFINITION A ClassOfIndirectProperty is a ClassOfRelationship that indicates
            that a member of the ClassOfIndividual can possess a member of the
            ClassOfProperty as an IndirectProperty of this type.
        </rdfs:comment>
        <rdfs:comment>
            EXAMPLE Maximum Allowable Working Pressure is a ClassOfIndirectProperty that
            is indicated by a pressure, and can be possessed by a pressure vessel.
        </rdfs:comment>
    </owl:Class>

    <owl:Class rdf:ID="ClassOfIndividual">
        <rdf:type rdf:resource="#ClassOfClassOfIndividual"/>
        <rdfs:subClassOf rdf:resource="#Class"/>
        <owl:intersectionOf rdf:parseType="Collection">  
            <owl:Class rdf:about="#ParticipatingRoleAndDomain"/>  
            <owl:Class>
                <owl:unionOf rdf:parseType="Collection">  
                    <owl:Class rdf:about="#ClassOfArrangedIndividual"/>  
                    <owl:Class rdf:about="#ClassOfEvent"/>  
                    <owl:Class rdf:about="#ClassOfPeriodInTime"/>  
                    <owl:Class rdf:about="#IndividualDimension"/>  
                    <owl:Class rdf:about="#Property"/>  
                    <owl:Class rdf:about="#Status"/>  
                </owl:unionOf>
            </owl:Class>
        </owl:intersectionOf>
        <rdfs:comment>
            DEFINITION A ClassOfIndividual is a Class whose members are instances of
            PossibleIndividual .
        </rdfs:comment>
        <rdfs:comment>
            EXAMPLE The class known as 'engineer', whose members are people qualified or
            skilled in engineering principles and practices can be represented by an
            instance of ClassOfIndividual .
        </rdfs:comment>
    </owl:Class>

    <owl:Class rdf:ID="ClassOfIndividualUsedInConnection">
        <rdfs:subClassOf rdf:resource="#ClassOfRelationship"/>
        <owl:disjointWith rdf:resource="#ClassOfIntendedRoleAndDomain"/>
        <owl:disjointWith rdf:resource="#ClassOfInvolvementByReference"/>
        <owl:disjointWith rdf:resource="#ClassOfLifecycleStage"/>
        <owl:disjointWith rdf:resource="#ClassOfPossibleRoleAndDomain"/>
        <owl:disjointWith rdf:resource="#ClassOfRecognition"/>
        <owl:disjointWith rdf:resource="#ClassOfRelationshipWithSignature"/>
        <owl:disjointWith rdf:resource="#ClassOfRelativeLocation"/>
        <owl:disjointWith rdf:resource="#ClassOfRepresentationOfThing"/>
        <owl:disjointWith rdf:resource="#ClassOfRepresentationTranslation"/>
        <owl:disjointWith rdf:resource="#ClassOfResponsibilityForRepresentation"/>
        <owl:disjointWith rdf:resource="#ClassOfSpecialization"/>
        <owl:disjointWith rdf:resource="#ClassOfTemporalSequence"/>
        <owl:disjointWith rdf:resource="#ClassOfUsageOfRepresentation"/>
        <owl:disjointWith rdf:resource="#DimensionOfIndividual"/>
        <owl:disjointWith rdf:resource="#PropertyForShapeDimension"/>
        <rdfs:subClassOf>
            <owl:Restriction>
                <owl:onProperty rdf:resource="#classOfConnection"/>
                <owl:allValuesFrom rdf:resource="#ClassOfConnectionOfIndividual"/>
            </owl:Restriction>
        </rdfs:subClassOf>
        <rdfs:subClassOf>
            <owl:Restriction>
                <owl:onProperty rdf:resource="#classOfInvolved"/>
                <owl:allValuesFrom rdf:resource="#ClassOfIndividual"/>
            </owl:Restriction>
        </rdfs:subClassOf>
        <rdfs:comment>
            DEFINITION A ClassOfIndividualUsedInConnection is a ClassOfRelationship whose
            members are members of IndividualUsedInConnection. It indicates that a member
            of the ClassOfIndividual is used in a ClassOfConnectionOfIndividual .
        </rdfs:comment>
        <rdfs:comment>
            EXAMPLE The link between the ClassOfIndividualUsedInConnection that indicates
            that B12 type beams are connected to pipe hangers, and the ClassOfIndividual
            "20mm Diameter bolt", that indicates that four 20mm diameter bolts are used
            in the connection of a pipe hanger to a type B12 beam can be represented by
            an instance of ClassOfIndividualUsedInConnection .
        </rdfs:comment>
    </owl:Class>

    <owl:Class rdf:ID="ClassOfInformationObject">
        <rdfs:subClassOf rdf:resource="#ClassOfArrangedIndividual"/>
        <rdfs:comment>
            DEFINITION A ClassOfInformationObject is a ClassOfArrangedIndividual whose
            members are members of zero or more ClassOfInformationRepresentation and of
            zero or more ClassOfInformationPresentation .
        </rdfs:comment>
        <rdfs:comment>
            NOTE Usually, it is a physical_object (like a paper document) that is
            classified as a ClassOfInformationObject.
        </rdfs:comment>
        <rdfs:comment>
            EXAMPLE 'Newspaper' is a ClassOfInformationObject.
        </rdfs:comment>
    </owl:Class>

    <owl:Class rdf:ID="ClassOfInformationPresentation">
        <rdfs:subClassOf rdf:resource="#ClassOfArrangedIndividual"/>
        <owl:disjointWith rdf:resource="#ClassOfInformationRepresentation"/>
        <owl:disjointWith rdf:resource="#ClassOfMolecule"/>
        <owl:disjointWith rdf:resource="#ClassOfParticulateMaterial"/>
        <owl:disjointWith rdf:resource="#ClassOfSubAtomicParticle"/>
        <owl:disjointWith rdf:resource="#CrystallineStructure"/>
        <owl:disjointWith rdf:resource="#Phase"/>
        <rdfs:comment>
            DEFINITION A ClassOfInformationPresentation is a ClassOfArrangedIndividual
            that distinguishes styles for presenting information.
        </rdfs:comment>
        <rdfs:comment>
            EXAMPLE The character styles bold, italic, Times New Roman, and 16pt can be
            represented as instances of ClassOfInformationPresentation .
        </rdfs:comment>
    </owl:Class>

    <owl:Class rdf:ID="ClassOfInformationRepresentation">
        <rdf:type rdf:resource="#ClassOfClassOfInformationRepresentation"/>
        <rdfs:subClassOf rdf:resource="#ClassOfArrangedIndividual"/>
        <owl:unionOf rdf:parseType="Collection">  
            <owl:Class rdf:about="#ClassOfExpressInformationRepresentation"/>  
            <owl:Class rdf:about="#RepresentationOfGregorianDateAndUtcTime"/>  
        </owl:unionOf>
        <owl:disjointWith rdf:resource="#ClassOfMolecule"/>
        <owl:disjointWith rdf:resource="#ClassOfParticulateMaterial"/>
        <owl:disjointWith rdf:resource="#ClassOfSubAtomicParticle"/>
        <owl:disjointWith rdf:resource="#CrystallineStructure"/>
        <owl:disjointWith rdf:resource="#Phase"/>
        <rdfs:comment>
            DEFINITION A ClassOfInformationRepresentation is a ClassOfArrangedIndividual
            that defines a pattern that represents information.
        </rdfs:comment>
        <rdfs:comment>
            EXAMPLE The texts formed with the pattern of characters 's' concatenated
            with 'u' concatenated with 'n' are members of the 'sun'
            ClassOfInformationRepresentation .
        </rdfs:comment>
    </owl:Class>

    <owl:Class rdf:ID="ClassOfIntendedRoleAndDomain">
        <rdfs:subClassOf rdf:resource="#ClassOfRelationship"/>
        <owl:disjointWith rdf:resource="#ClassOfInvolvementByReference"/>
        <owl:disjointWith rdf:resource="#ClassOfLifecycleStage"/>
        <owl:disjointWith rdf:resource="#ClassOfPossibleRoleAndDomain"/>
        <owl:disjointWith rdf:resource="#ClassOfRecognition"/>
        <owl:disjointWith rdf:resource="#ClassOfRelationshipWithSignature"/>
        <owl:disjointWith rdf:resource="#ClassOfRelativeLocation"/>
        <owl:disjointWith rdf:resource="#ClassOfRepresentationOfThing"/>
        <owl:disjointWith rdf:resource="#ClassOfRepresentationTranslation"/>
        <owl:disjointWith rdf:resource="#ClassOfResponsibilityForRepresentation"/>
        <owl:disjointWith rdf:resource="#ClassOfSpecialization"/>
        <owl:disjointWith rdf:resource="#ClassOfTemporalSequence"/>
        <owl:disjointWith rdf:resource="#ClassOfUsageOfRepresentation"/>
        <owl:disjointWith rdf:resource="#DimensionOfIndividual"/>
        <owl:disjointWith rdf:resource="#PropertyForShapeDimension"/>
        <rdfs:subClassOf>
            <owl:Restriction>
                <owl:onProperty rdf:resource="#classOfPlayer"/>
                <owl:allValuesFrom rdf:resource="#ClassOfIndividual"/>
            </owl:Restriction>
        </rdfs:subClassOf>
        <rdfs:subClassOf>
            <owl:Restriction>
                <owl:onProperty rdf:resource="#played"/>
                <owl:allValuesFrom rdf:resource="#RoleAndDomain"/>
            </owl:Restriction>
        </rdfs:subClassOf>
        <rdfs:comment>
            DEFINITION A ClassOfIntendedRoleAndDomain is a ClassOfRelationship that
            indicates that a member of the ClassOfIndividual is intended to act as a
            member of the RoleAndDomain .
        </rdfs:comment>
        <rdfs:comment>
            EXAMPLE Pumps are intended to play the RoleAndDomain of performer in some
            pumping activity.
        </rdfs:comment>
    </owl:Class>

    <owl:Class rdf:ID="ClassOfInvolvementByReference">
        <rdfs:subClassOf rdf:resource="#ClassOfRelationship"/>
        <owl:disjointWith rdf:resource="#ClassOfLifecycleStage"/>
        <owl:disjointWith rdf:resource="#ClassOfPossibleRoleAndDomain"/>
        <owl:disjointWith rdf:resource="#ClassOfRecognition"/>
        <owl:disjointWith rdf:resource="#ClassOfRelationshipWithSignature"/>
        <owl:disjointWith rdf:resource="#ClassOfRelativeLocation"/>
        <owl:disjointWith rdf:resource="#ClassOfRepresentationOfThing"/>
        <owl:disjointWith rdf:resource="#ClassOfRepresentationTranslation"/>
        <owl:disjointWith rdf:resource="#ClassOfResponsibilityForRepresentation"/>
        <owl:disjointWith rdf:resource="#ClassOfSpecialization"/>
        <owl:disjointWith rdf:resource="#ClassOfTemporalSequence"/>
        <owl:disjointWith rdf:resource="#ClassOfUsageOfRepresentation"/>
        <owl:disjointWith rdf:resource="#DimensionOfIndividual"/>
        <owl:disjointWith rdf:resource="#PropertyForShapeDimension"/>
        <rdfs:subClassOf>
            <owl:Restriction>
                <owl:onProperty rdf:resource="#classOfInvolved"/>
                <owl:allValuesFrom rdf:resource="#ClassOfIndividual"/>
            </owl:Restriction>
        </rdfs:subClassOf>
        <rdfs:subClassOf>
            <owl:Restriction>
                <owl:onProperty rdf:resource="#classOfInvolver"/>
                <owl:allValuesFrom rdf:resource="#ClassOfActivity"/>
            </owl:Restriction>
        </rdfs:subClassOf>
        <rdfs:comment>
            DEFINITION A ClassOfInvolvementByReference is a ClassOfRelationship whose
            members are instances of InvolvementByReference .
        </rdfs:comment>
        <rdfs:comment>
            EXAMPLE Discussion of historical activities is an example of
            ClassOfInvolvementByReference .
        </rdfs:comment>
        <rdfs:comment>
            EXAMPLE The relation between API 610 and the ClassOfActivity 'design of
            centrifugal pumps' is represented by an instance of
            ClassOfInvolvementByReference .
        </rdfs:comment>
    </owl:Class>

    <owl:Class rdf:ID="ClassOfIsomorphicFunctionalMapping">
        <rdfs:subClassOf rdf:resource="#ClassOfFunctionalMapping"/>
        <owl:unionOf rdf:parseType="Collection">  
            <owl:Class rdf:about="#ClassOfScaleConversion"/>  
            <owl:Class rdf:about="#Scale"/>  
        </owl:unionOf>
        <rdfs:comment>
            DEFINITION A ClassOfIsomorphicFunctionalMapping is a ClassOfFunctionalMapping
            that is isomorphic.
        </rdfs:comment>
        <rdfs:comment>
            EXAMPLE The natural logarithm function is a
            ClassOfIsomorphicFunctionalMapping .
        </rdfs:comment>
    </owl:Class>

    <owl:Class rdf:ID="ClassOfLeftNamespace">
        <rdfs:subClassOf rdf:resource="#ClassOfNamespace"/>
        <owl:disjointWith rdf:resource="#ClassOfRightNamespace"/>
        <rdfs:comment>
            DEFINITION A ClassOfLeftNamespace is a ClassOfNamespace that indicates that
            the classOfPart is the left namespace for the members of the
            classOfClassOfWhole .
        </rdfs:comment>
        <rdfs:comment>
            EXAMPLE WC1: is the left namespace for customer site identifiers for Water
            Company 1.
        </rdfs:comment>
    </owl:Class>

    <owl:Class rdf:ID="ClassOfLifecycleStage">
        <rdfs:subClassOf rdf:resource="#ClassOfRelationship"/>
        <owl:disjointWith rdf:resource="#ClassOfPossibleRoleAndDomain"/>
        <owl:disjointWith rdf:resource="#ClassOfRecognition"/>
        <owl:disjointWith rdf:resource="#ClassOfRelationshipWithSignature"/>
        <owl:disjointWith rdf:resource="#ClassOfRelativeLocation"/>
        <owl:disjointWith rdf:resource="#ClassOfRepresentationOfThing"/>
        <owl:disjointWith rdf:resource="#ClassOfRepresentationTranslation"/>
        <owl:disjointWith rdf:resource="#ClassOfResponsibilityForRepresentation"/>
        <owl:disjointWith rdf:resource="#ClassOfSpecialization"/>
        <owl:disjointWith rdf:resource="#ClassOfTemporalSequence"/>
        <owl:disjointWith rdf:resource="#ClassOfUsageOfRepresentation"/>
        <owl:disjointWith rdf:resource="#DimensionOfIndividual"/>
        <owl:disjointWith rdf:resource="#PropertyForShapeDimension"/>
        <rdfs:comment>
            DEFINITION A ClassOfLifecycleStage is a ClassOfRelationship whose members are
            members of LifecycleStage .
        </rdfs:comment>
        <rdfs:comment>
            EXAMPLE 'Planned', 'required', 'expected', and 'proposed' can be represented
            by instances of ClassOfLifecycleStage .
        </rdfs:comment>
    </owl:Class>

    <owl:Class rdf:ID="ClassOfMolecule">
        <rdfs:subClassOf rdf:resource="#ClassOfArrangedIndividual"/>
        <owl:disjointWith rdf:resource="#ClassOfParticulateMaterial"/>
        <owl:disjointWith rdf:resource="#ClassOfSubAtomicParticle"/>
        <owl:disjointWith rdf:resource="#CrystallineStructure"/>
        <owl:disjointWith rdf:resource="#Phase"/>
        <rdfs:comment>
            DEFINITION A ClassOfMolecule is a ClassOfArrangedIndividual whose members
            are molecules.
        </rdfs:comment>
        <rdfs:comment>
            EXAMPLE H2O, H2SO4, and DNA can be represented by instances of
            ClassOfMolecule .
        </rdfs:comment>
    </owl:Class>

    <owl:Class rdf:ID="ClassOfMultidimensionalObject">
        <rdfs:subClassOf rdf:resource="#ClassOfAbstractObject"/>
        <rdfs:subClassOf>
            <owl:Restriction>
                <owl:onProperty rdf:resource="#cardinalities"/>
                <owl:allValuesFrom rdf:resource="#Cardinality"/>
            </owl:Restriction>
        </rdfs:subClassOf>
        <rdfs:subClassOf>
            <owl:Restriction>
                <owl:onProperty rdf:resource="#optionalElement"/>
                <owl:allValuesFrom rdf:datatype="http://www.w3.org/2001/XMLSchema#boolean"/>
            </owl:Restriction>
        </rdfs:subClassOf>
        <rdfs:subClassOf>
            <owl:Restriction>
                <owl:onProperty rdf:resource="#parameters"/>
                <owl:allValuesFrom rdf:resource="#Thing"/>
            </owl:Restriction>
        </rdfs:subClassOf>
        <rdfs:subClassOf>
            <owl:Restriction>
                <owl:onProperty rdf:resource="#parameterPosition"/>
                <owl:allValuesFrom rdf:datatype="http://www.w3.org/2001/XMLSchema#nonNegativeInteger"/>
            </owl:Restriction>
        </rdfs:subClassOf>
        <rdfs:subClassOf>
            <owl:Restriction>
                <owl:onProperty rdf:resource="#roles"/>
                <owl:allValuesFrom rdf:resource="#RoleAndDomain"/>
            </owl:Restriction>
        </rdfs:subClassOf>
        <rdfs:comment>
            DEFINITION A ClassOfMultidimensionalObject is a ClassOfAbstractObject whose
            members are instances of MultidimensionalObject . The role played by each
            position in the classified MultidimensionalObject is specified at the same
            position in the roles attribute. Constant values that apply to any position
            in the roles attribute are specified in the same position in the parameters
            attribute. The cardinalities for the roles attribute are specified by the
            same position in the cardinalities attribute.
        </rdfs:comment>
        <rdfs:comment>
            EXAMPLE The definition of the input to a function y = a + bx to convert
            Celsius to Fahrenheit with roles [a, b, x] defining the input
            MultidimensionalObject , and parameter list [32,1.8,] is an example of a
            ClassOfMultidimensionalObject .
        </rdfs:comment>
    </owl:Class>

    <owl:Class rdf:ID="ClassOfNamespace">
        <rdfs:subClassOf rdf:resource="#ClassOfClassOfRelationship"/>
        <owl:unionOf rdf:parseType="Collection">  
            <owl:Class rdf:about="#ClassOfLeftNamespace"/>  
            <owl:Class rdf:about="#ClassOfRightNamespace"/>  
        </owl:unionOf>
        <owl:disjointWith rdf:resource="#ClassOfScale"/>
        <owl:disjointWith rdf:resource="#DimensionOfShape"/>
        <owl:disjointWith rdf:resource="#PropertySpaceForClassOfShapeDimension"/>
        <rdfs:subClassOf>
            <owl:Restriction>
                <owl:onProperty rdf:resource="#classOfClassOfWhole"/>
                <owl:allValuesFrom rdf:resource="#ClassOfClassOfInformationRepresentation"/>
            </owl:Restriction>
        </rdfs:subClassOf>
        <rdfs:subClassOf>
            <owl:Restriction>
                <owl:onProperty rdf:resource="#classOfPart"/>
                <owl:allValuesFrom rdf:resource="#ClassOfInformationRepresentation"/>
            </owl:Restriction>
        </rdfs:subClassOf>
        <rdfs:comment>
            DEFINITION A ClassOfNamespace is a ClassOfClassOfRelationship that indicates
            that a ClassOfInformationRepresentation is the classOfPart used as a
            namespace for each member of a ClassOfClassOfInformationRepresentation that
            is the classOfClassOfWhole .
        </rdfs:comment>
        <rdfs:comment>
            EXAMPLE WC1: is used as the name space for a set of water company identifiers.
        </rdfs:comment>
    </owl:Class>

    <owl:Class rdf:ID="ClassOfNumber">
        <rdfs:subClassOf rdf:resource="#ClassOfClass"/>
        <owl:unionOf rdf:parseType="Collection">  
            <owl:Class rdf:about="#EnumeratedNumberSet"/>  
            <owl:Class rdf:about="#NumberSpace"/>  
        </owl:unionOf>
       <owl:disjointWith rdf:resource="#ClassOfPropertySpace"/>
        <owl:disjointWith rdf:resource="#ClassOfShapeDimension"/>
        <rdfs:comment>
            DEFINITION A ClassOfNumber is a ClassOfClass whose members are members of
            ArithmeticNumber .
        </rdfs:comment>
        <rdfs:comment>
            EXAMPLE The class of prime numbers can be represented by an instance
            ClassOfNumber .
        </rdfs:comment>
    </owl:Class>

    <owl:Class rdf:ID="ClassOfOrganism">
        <rdfs:subClassOf rdf:resource="#ClassOfArrangedIndividual"/>
        <rdfs:comment>
            DEFINITION A ClassOfOrganism is a ClassOfArrangedIndividual whose members are
            living organisms.
        </rdfs:comment>
        <rdfs:comment>
            EXAMPLE Human being, sheep, earthworm, oak tree, and bacteria are instances
            of ClassOfOrganism .
        </rdfs:comment>
    </owl:Class>

    <owl:Class rdf:ID="ClassOfOrganization">
        <rdfs:subClassOf rdf:resource="#ClassOfArrangedIndividual"/>
        <rdfs:comment>
            DEFINITION A ClassOfOrganization is a ClassOfArrangedIndividual whose members
            are instances of PhysicalObject that are composed of temporal parts of people
            and other assets, and are organised with a particular purpose.
        </rdfs:comment>
        <rdfs:comment>
            EXAMPLE Company, government, and project team can be represented by instances
            of ClassOfOrganization .
        </rdfs:comment>
    </owl:Class>

    <owl:Class rdf:ID="ClassOfParticipation">
        <rdfs:subClassOf rdf:resource="#ClassOfCompositionOfIndividual"/>
        <owl:disjointWith rdf:resource="#ClassOfTemporalWholePart"/>
        <rdfs:subClassOf>
            <owl:Restriction>
                <owl:onProperty rdf:resource="#classOfPart"/>
                <owl:allValuesFrom rdf:resource="#ParticipatingRoleAndDomain"/>
            </owl:Restriction>
        </rdfs:subClassOf>
        <rdfs:subClassOf>
            <owl:Restriction>
                <owl:onProperty rdf:resource="#classOfWhole"/>
                <owl:allValuesFrom rdf:resource="#ClassOfActivity"/>
            </owl:Restriction>
        </rdfs:subClassOf>
        <rdfs:comment>
            DEFINITION A ClassOfParticipation is a ClassOfCompositionOfIndividual that
            indicates a member of an instance of ParticipatingRoleAndDomain participates
            in a member of an instance of ClassOfActivity .
        </rdfs:comment>
        <rdfs:comment>
            EXAMPLE 'Conductor of a musical performance' is an example of
            ClassOfParticipation .
        </rdfs:comment>
    </owl:Class>

    <owl:Class rdf:ID="ClassOfParticulateMaterial">
        <rdfs:subClassOf rdf:resource="#ClassOfArrangedIndividual"/>
        <owl:disjointWith rdf:resource="#ClassOfSubAtomicParticle"/>
        <owl:disjointWith rdf:resource="#CrystallineStructure"/>
        <owl:disjointWith rdf:resource="#Phase"/>
        <rdfs:comment>
            DEFINITION A ClassOfParticulateMaterial is a ClassOfArrangedIndividual whose
            members are arranged amounts of super-molecular sized objects of the same or
            different types.
        </rdfs:comment>
        <rdfs:comment>
            EXAMPLE Pile of sand, sand and cement mix, bag of bolts, catalyst fill for a
            reactor are examples of ClassOfParticulateMaterial .
        </rdfs:comment>
    </owl:Class>

    <owl:Class rdf:ID="ClassOfPeriodInTime">
        <rdfs:subClassOf rdf:resource="#ClassOfIndividual"/>
        <owl:disjointWith rdf:resource="#IndividualDimension"/>
        <owl:disjointWith rdf:resource="#Property"/>
        <owl:disjointWith rdf:resource="#Status"/>
        <rdfs:comment>
            DEFINITION A ClassOfPeriodInTime is a ClassOfIndividual whose members are
            instances of PeriodInTime .
        </rdfs:comment>
        <rdfs:comment>
            EXAMPLE Monday and June are examples of ClassOfPeriodInTime .
        </rdfs:comment>
    </owl:Class>

    <owl:Class rdf:ID="ClassOfPerson">
        <rdfs:subClassOf rdf:resource="#ClassOfOrganism"/>
        <rdfs:comment>
            DEFINITION A ClassOfPerson is a ClassOfOrganism whose members are people.
        </rdfs:comment>
        <rdfs:comment>
            EXAMPLE 'Engineer', 'plant manager', 'student', 'male', 'female',
            'senior citizen', 'adult', 'girl', and 'boy' can be represented by instances
            of ClassOfPerson. Engineer, plant manager, and student are also instances of
            ClassOfFunctionalObject .
        </rdfs:comment>
    </owl:Class>

    <owl:Class rdf:ID="ClassOfPointInTime">
        <rdfs:subClassOf rdf:resource="#ClassOfEvent"/>
        <rdfs:comment>
            DEFINITION A ClassOfPointInTime is a ClassOfEvent whose members are members
            of PointInTime .
        </rdfs:comment>
        <rdfs:comment>
            EXAMPLE Midnight is a ClassOfPointInTime .
        </rdfs:comment>
    </owl:Class>

    <owl:Class rdf:ID="ClassOfPossibleRoleAndDomain">
        <rdfs:subClassOf rdf:resource="#ClassOfRelationship"/>
        <owl:disjointWith rdf:resource="#ClassOfRecognition"/>
        <owl:disjointWith rdf:resource="#ClassOfRelationshipWithSignature"/>
        <owl:disjointWith rdf:resource="#ClassOfRelativeLocation"/>
        <owl:disjointWith rdf:resource="#ClassOfRepresentationOfThing"/>
        <owl:disjointWith rdf:resource="#ClassOfRepresentationTranslation"/>
        <owl:disjointWith rdf:resource="#ClassOfResponsibilityForRepresentation"/>
        <owl:disjointWith rdf:resource="#ClassOfSpecialization"/>
        <owl:disjointWith rdf:resource="#ClassOfTemporalSequence"/>
        <owl:disjointWith rdf:resource="#ClassOfUsageOfRepresentation"/>
        <owl:disjointWith rdf:resource="#DimensionOfIndividual"/>
        <owl:disjointWith rdf:resource="#PropertyForShapeDimension"/>
        <rdfs:subClassOf>
            <owl:Restriction>
                <owl:onProperty rdf:resource="#classOfPlayer"/>
                <owl:allValuesFrom rdf:resource="#ClassOfIndividual"/>
            </owl:Restriction>
        </rdfs:subClassOf>
        <rdfs:subClassOf>
            <owl:Restriction>
                <owl:onProperty rdf:resource="#played"/>
                <owl:allValuesFrom rdf:resource="#RoleAndDomain"/>
            </owl:Restriction>
        </rdfs:subClassOf>
        <rdfs:comment>
            DEFINITION A ClassOfPossibleRoleAndDomain is a ClassOfRelationship that
            indicates the RoleAndDomain that can be played by a member of the
            ClassOfIndividual , in some Activity .
        </rdfs:comment>
        <rdfs:comment>
            EXAMPLE Pumps can play the role of anchor (although they are not intended
            to do so).
        </rdfs:comment>
    </owl:Class>

    <owl:Class rdf:ID="ClassOfProperty">
        <rdfs:subClassOf rdf:resource="#ClassOfClassOfIndividual"/>
        <owl:unionOf rdf:parseType="Collection">  
            <owl:Class rdf:about="#EnumeratedPropertySet"/>  
            <owl:Class rdf:about="#PropertySpace"/>  
        </owl:unionOf>
        <owl:disjointWith rdf:resource="#ClassOfStatus"/>
        <owl:disjointWith rdf:resource="#ShapeDimension"/>
        <rdfs:comment>
            DEFINITION A ClassOfProperty is a ClassOfClassOfIndividual whose members are
            instances of Property .
        </rdfs:comment>
        <rdfs:comment>
            EXAMPLE 'Temperature' is an example of ClassOfProperty .
        </rdfs:comment>
    </owl:Class>

    <owl:Class rdf:ID="ClassOfPropertySpace">
        <rdfs:subClassOf rdf:resource="#ClassOfClass"/>
       <owl:disjointWith rdf:resource="#ClassOfShapeDimension"/>
        <rdfs:comment>
            DEFINITION A ClassOfPropertySpace is a ClassOfClass whose members are members
            of PropertySpace .
        </rdfs:comment>
        <rdfs:comment>
            EXAMPLE Property curves, property areas, and property volumes of various
            dimensionality and degrees of freedom are members of ClassOfPropertySpace .
        </rdfs:comment>
        <rdfs:comment>
            EXAMPLE Pump performance curve is an example of ClassOfPropertySpace .
        </rdfs:comment>
    </owl:Class>

    <owl:Class rdf:ID="ClassOfRecognition">
        <rdfs:subClassOf rdf:resource="#ClassOfRelationship"/>
        <owl:disjointWith rdf:resource="#ClassOfRelationshipWithSignature"/>
        <owl:disjointWith rdf:resource="#ClassOfRelativeLocation"/>
        <owl:disjointWith rdf:resource="#ClassOfRepresentationOfThing"/>
        <owl:disjointWith rdf:resource="#ClassOfRepresentationTranslation"/>
        <owl:disjointWith rdf:resource="#ClassOfResponsibilityForRepresentation"/>
        <owl:disjointWith rdf:resource="#ClassOfSpecialization"/>
        <owl:disjointWith rdf:resource="#ClassOfTemporalSequence"/>
        <owl:disjointWith rdf:resource="#ClassOfUsageOfRepresentation"/>
        <owl:disjointWith rdf:resource="#DimensionOfIndividual"/>
        <owl:disjointWith rdf:resource="#PropertyForShapeDimension"/>
        <rdfs:subClassOf>
            <owl:Restriction>
                <owl:onProperty rdf:resource="#classOfRecognized"/>
                <owl:allValuesFrom rdf:resource="#Class"/>
            </owl:Restriction>
        </rdfs:subClassOf>
        <rdfs:subClassOf>
            <owl:Restriction>
                <owl:onProperty rdf:resource="#classOfRecognizing"/>
                <owl:allValuesFrom rdf:resource="#ClassOfActivity"/>
            </owl:Restriction>
        </rdfs:subClassOf>
        <rdfs:comment>
            DEFINITION A ClassOfRecognition is a ClassOfRelationship that indicates that
            a member of a ClassOfActivity may result in the recognition of a member of a
            Class .
        </rdfs:comment>
        <rdfs:comment>
            EXAMPLE A measurement activity may result in the recognition of the
            Classification of a PossibleIndividual by a Property .
        </rdfs:comment>
    </owl:Class>

    <owl:Class rdf:ID="ClassOfRelationship">
        <rdf:type rdf:resource="#ClassOfClassOfRelationship"/>
        <rdfs:subClassOf rdf:resource="#ClassOfAbstractObject"/>
        <owl:intersectionOf rdf:parseType="Collection">  
            <owl:Class>
                <owl:unionOf rdf:parseType="Collection">  
                    <owl:Class rdf:about="#ClassOfApproval"/>  
                    <owl:Class rdf:about="#ClassOfApprovalByStatus"/>  
                    <owl:Class rdf:about="#ClassOfAssertion"/>  
                    <owl:Class rdf:about="#ClassOfCauseOfBeginningOfClassOfIndividual"/>  
                    <owl:Class rdf:about="#ClassOfCauseOfEndingOfClassOfIndividual"/>  
                    <owl:Class rdf:about="#ClassOfClassification"/>  
                    <owl:Class rdf:about="#ClassOfCompositionOfIndividual"/>  
                    <owl:Class rdf:about="#ClassOfConnectionOfIndividual"/>  
                    <owl:Class rdf:about="#ClassOfFunctionalMapping"/>  
                    <owl:Class rdf:about="#ClassOfIndirectProperty"/>  
                    <owl:Class rdf:about="#ClassOfIndividualUsedInConnection"/>  
                    <owl:Class rdf:about="#ClassOfIntendedRoleAndDomain"/>  
                    <owl:Class rdf:about="#ClassOfInvolvementByReference"/>  
                    <owl:Class rdf:about="#ClassOfLifecycleStage"/>  
                    <owl:Class rdf:about="#ClassOfPossibleRoleAndDomain"/>  
                    <owl:Class rdf:about="#ClassOfRecognition"/>  
                    <owl:Class rdf:about="#ClassOfRelationshipWithSignature"/>  
                    <owl:Class rdf:about="#ClassOfRelativeLocation"/>  
                    <owl:Class rdf:about="#ClassOfRepresentationOfThing"/>  
                    <owl:Class rdf:about="#ClassOfRepresentationTranslation"/>  
                    <owl:Class rdf:about="#ClassOfResponsibilityForRepresentation"/>  
                    <owl:Class rdf:about="#ClassOfSpecialization"/>  
                    <owl:Class rdf:about="#ClassOfTemporalSequence"/>  
                    <owl:Class rdf:about="#ClassOfUsageOfRepresentation"/>  
                    <owl:Class rdf:about="#DimensionOfIndividual"/>  
                    <owl:Class rdf:about="#PropertyForShapeDimension"/>  
                </owl:unionOf>
            </owl:Class>
            <owl:Class>
                <owl:unionOf rdf:parseType="Collection">  
                    <owl:Class rdf:about="#ClassOfRelationshipWithRelatedEnd1"/>  
                    <owl:Class rdf:about="#ClassOfRelationshipWithRelatedEnd2"/>  
                </owl:unionOf>
            </owl:Class>
        </owl:intersectionOf>
        <rdfs:comment>
            DEFINITION A ClassOfRelationship is a ClassOfAbstractObject whose members are
            members of Relationship .
        </rdfs:comment>
    </owl:Class>

    <owl:Class rdf:ID="ClassOfRelationshipWithRelatedEnd1">
        <rdfs:subClassOf rdf:resource="#ClassOfRelationship"/>
        <owl:disjointWith rdf:resource="#ClassOfRelationshipWithRelatedEnd2"/>
        <rdfs:subClassOf>
            <owl:Restriction>
                <owl:onProperty rdf:resource="#related"/>
                <owl:allValuesFrom rdf:resource="#Thing"/>
            </owl:Restriction>
        </rdfs:subClassOf>
        <rdfs:comment>
            DEFINITION A ClassOfRelationshipWithRelatedEnd1 is a ClassOfRelationship
            where a particular Thing is related in the ClassOfRelationship , rather than
            the members of a Class . The related Thing plays the RoleAndDomain indicated
            by the classOfEnd1 attribute.
        </rdfs:comment>
        <rdfs:comment>
            EXAMPLE Products manufactured by Bloggs and Co is a
            ClassOfRelationshipWithRelatedEnd1 that points to Bloggs and Co as the related
            Thing .
        </rdfs:comment>
    </owl:Class>

    <owl:Class rdf:ID="ClassOfRelationshipWithRelatedEnd2">
        <rdfs:subClassOf rdf:resource="#ClassOfRelationship"/>
        <rdfs:subClassOf>
            <owl:Restriction>
                <owl:onProperty rdf:resource="#related"/>
                <owl:allValuesFrom rdf:resource="#Thing"/>
            </owl:Restriction>
        </rdfs:subClassOf>
        <rdfs:comment>
            DEFINITION A ClassOfRelationshipWithRelatedEnd2 is a ClassOfRelationship
            where a particular Thing is related in the ClassOfRelationship , rather than
            the members of a Class . The related Thing plays the RoleAndDomain indicated
            by the classOfEnd2 attribute.
        </rdfs:comment>
        <rdfs:comment>
            EXAMPLE Possession of welding skills by John Doe is an example of
            ClassOfRelationshipWithRelatedEnd2 , where John Doe is the related
            Thing .
        </rdfs:comment>
    </owl:Class>

    <owl:Class rdf:ID="ClassOfRelationshipWithSignature">
        <rdfs:subClassOf rdf:resource="#ClassOfRelationship"/>
        <rdfs:subClassOf rdf:resource="#Relationship"/>
        <owl:disjointWith rdf:resource="#ClassOfRelativeLocation"/>
        <owl:disjointWith rdf:resource="#ClassOfRepresentationOfThing"/>
        <owl:disjointWith rdf:resource="#ClassOfRepresentationTranslation"/>
        <owl:disjointWith rdf:resource="#ClassOfResponsibilityForRepresentation"/>
        <owl:disjointWith rdf:resource="#ClassOfSpecialization"/>
        <owl:disjointWith rdf:resource="#ClassOfTemporalSequence"/>
        <owl:disjointWith rdf:resource="#ClassOfUsageOfRepresentation"/>
        <owl:disjointWith rdf:resource="#DimensionOfIndividual"/>
        <owl:disjointWith rdf:resource="#PropertyForShapeDimension"/>
        <owl:disjointWith rdf:resource="#ComparisonOfProperty"/>
        <owl:disjointWith rdf:resource="#CompositionOfIndividual"/>
        <owl:disjointWith rdf:resource="#ConnectionOfIndividual"/>
        <owl:disjointWith rdf:resource="#FunctionalMapping"/>
        <owl:disjointWith rdf:resource="#IndirectProperty"/>
        <owl:disjointWith rdf:resource="#IndividualUsedInConnection"/>
        <owl:disjointWith rdf:resource="#IntendedRoleAndDomain"/>
        <owl:disjointWith rdf:resource="#InvolvementByReference"/>
        <owl:disjointWith rdf:resource="#LifecycleStage"/>
        <owl:disjointWith rdf:resource="#OtherRelationship"/>
        <owl:disjointWith rdf:resource="#PossibleRoleAndDomain"/>
        <owl:disjointWith rdf:resource="#Recognition"/>
        <owl:disjointWith rdf:resource="#RelativeLocation"/>
        <owl:disjointWith rdf:resource="#RepresentationOfThing"/>
        <owl:disjointWith rdf:resource="#ResponsibilityForRepresentation"/>
        <owl:disjointWith rdf:resource="#TemporalSequence"/>
        <owl:disjointWith rdf:resource="#UsageOfRepresentation"/>
        <rdfs:subClassOf>
            <owl:Restriction>
                <owl:onProperty rdf:resource="#classOfEnd1"/>
                <owl:allValuesFrom rdf:resource="#RoleAndDomain"/>
            </owl:Restriction>
        </rdfs:subClassOf>
        <rdfs:subClassOf>
            <owl:Restriction>
                <owl:onProperty rdf:resource="#classOfEnd2"/>
                <owl:allValuesFrom rdf:resource="#RoleAndDomain"/>
            </owl:Restriction>
        </rdfs:subClassOf>
        <rdfs:comment>
            DEFINITION A ClassOfRelationshipWithSignature is a ClassOfRelationship that
            may have a RoleAndDomain specified for each end.
        </rdfs:comment>
        <rdfs:comment>
            NOTE A ClassOfRelationshipWithSignature is analogous to a simple EXPRESS
            attribute and its inverse. More complex objects can be modelled with
            MultidimensionalObject and ClassOfMultidimensionalObject .
        </rdfs:comment>
        <rdfs:comment>
            EXAMPLE Married is a ClassOfRelationship where classOfEnd1 is the
            RoleAndDomain husband, and classOfEnd2 the RoleAndDomain wife.
        </rdfs:comment>
    </owl:Class>

    <owl:Class rdf:ID="ClassOfRelativeLocation">
        <rdfs:subClassOf rdf:resource="#ClassOfRelationship"/>
        <owl:disjointWith rdf:resource="#ClassOfRepresentationOfThing"/>
        <owl:disjointWith rdf:resource="#ClassOfRepresentationTranslation"/>
        <owl:disjointWith rdf:resource="#ClassOfResponsibilityForRepresentation"/>
        <owl:disjointWith rdf:resource="#ClassOfSpecialization"/>
        <owl:disjointWith rdf:resource="#ClassOfTemporalSequence"/>
        <owl:disjointWith rdf:resource="#ClassOfUsageOfRepresentation"/>
        <owl:disjointWith rdf:resource="#DimensionOfIndividual"/>
        <owl:disjointWith rdf:resource="#PropertyForShapeDimension"/>
        <rdfs:subClassOf>
            <owl:Restriction>
                <owl:onProperty rdf:resource="#classOfLocated"/>
                <owl:allValuesFrom rdf:resource="#ClassOfIndividual"/>
            </owl:Restriction>
        </rdfs:subClassOf>
        <rdfs:subClassOf>
            <owl:Restriction>
                <owl:onProperty rdf:resource="#classOfLocator"/>
                <owl:allValuesFrom rdf:resource="#ClassOfIndividual"/>
            </owl:Restriction>
        </rdfs:subClassOf>
        <rdfs:comment>
            DEFINITION A ClassOfRelativeLocation is a ClassOfRelationship whose members
            are instances of RelativeLocation .
        </rdfs:comment>
        <rdfs:comment>
            EXAMPLE Beside, above, and below are examples of ClassOfRelativeLocation.
        </rdfs:comment>
    </owl:Class>

    <owl:Class rdf:ID="ClassOfRepresentationOfThing">
        <rdf:type rdf:resource="#ClassOfClassOfRepresentation"/>
        <rdfs:subClassOf rdf:resource="#ClassOfRelationship"/>
        <owl:intersectionOf rdf:parseType="Collection">  
            <owl:Class rdf:about="#ClassOfDefinition"/>  
            <owl:Class rdf:about="#ClassOfDescription"/>  
            <owl:Class rdf:about="#ClassOfIdentification"/>  
        </owl:intersectionOf>
        <owl:disjointWith rdf:resource="#ClassOfRepresentationTranslation"/>
        <owl:disjointWith rdf:resource="#ClassOfResponsibilityForRepresentation"/>
        <owl:disjointWith rdf:resource="#ClassOfSpecialization"/>
        <owl:disjointWith rdf:resource="#ClassOfTemporalSequence"/>
        <owl:disjointWith rdf:resource="#ClassOfUsageOfRepresentation"/>
        <owl:disjointWith rdf:resource="#DimensionOfIndividual"/>
        <owl:disjointWith rdf:resource="#PropertyForShapeDimension"/>
        <rdfs:subClassOf>
            <owl:Restriction>
                <owl:onProperty rdf:resource="#pattern"/>
                <owl:allValuesFrom rdf:resource="#ClassOfInformationRepresentation"/>
            </owl:Restriction>
        </rdfs:subClassOf>
        <rdfs:subClassOf>
            <owl:Restriction>
                <owl:onProperty rdf:resource="#represented"/>
                <owl:allValuesFrom rdf:resource="#Thing"/>
            </owl:Restriction>
        </rdfs:subClassOf>
        <rdfs:comment>
            DEFINITION A ClassOfRepresentationOfThing is a ClassOfRelationship that
            indicates that all members of the pattern ClassOfInformationRepresentation
            represent the Thing .
        </rdfs:comment>
        <rdfs:comment>
            EXAMPLE The ClassOfRelationship that indicates that occurrences of the
            pattern denoted by 'London' represent the concept of the capital of the
            United Kingdom can be represented by an instance of
            ClassOfRepresentationOfThing .
        </rdfs:comment>
    </owl:Class>

    <owl:Class rdf:ID="ClassOfRepresentationTranslation">
        <rdf:type rdf:resource="#ClassOfClassOfRepresentationTranslation"/>
        <rdfs:subClassOf rdf:resource="#ClassOfRelationship"/>
        <owl:disjointWith rdf:resource="#ClassOfResponsibilityForRepresentation"/>
        <owl:disjointWith rdf:resource="#ClassOfSpecialization"/>
        <owl:disjointWith rdf:resource="#ClassOfTemporalSequence"/>
        <owl:disjointWith rdf:resource="#ClassOfUsageOfRepresentation"/>
        <owl:disjointWith rdf:resource="#DimensionOfIndividual"/>
        <owl:disjointWith rdf:resource="#PropertyForShapeDimension"/>
        <rdfs:subClassOf>
            <owl:Restriction>
                <owl:onProperty rdf:resource="#classOfFirst"/>
                <owl:allValuesFrom rdf:resource="#ClassOfInformationRepresentation"/>
            </owl:Restriction>
        </rdfs:subClassOf>
        <rdfs:subClassOf>
            <owl:Restriction>
                <owl:onProperty rdf:resource="#classOfSecond"/>
                <owl:allValuesFrom rdf:resource="#ClassOfInformationRepresentation"/>
            </owl:Restriction>
        </rdfs:subClassOf>
        <rdfs:comment>
            DEFINITION A ClassOfRepresentationTranslation is a ClassOfRelationship that
            indicates the translation of two instances of
            ClassOfInformationRepresentation .
        </rdfs:comment>
        <rdfs:comment>
            EXAMPLE The link that indicates that the representations 'F' and '15' are
            equivalent (concept of fifteen in hexadecimal and octal respectively) can be
            represented by an instance of ClassOfRepresentationTranslation.
        </rdfs:comment>
    </owl:Class>

    <owl:Class rdf:ID="ClassOfResposibilityForRepresentation">
        <rdf:type rdf:resource="#ClassOfClassOfResponsibilityForRepresentation"/>
        <rdfs:subClassOf rdf:resource="#ClassOfRelationship"/>
        <owl:disjointWith rdf:resource="#ClassOfSpecialization"/>
        <owl:disjointWith rdf:resource="#ClassOfTemporalSequence"/>
        <owl:disjointWith rdf:resource="#ClassOfUsageOfRepresentation"/>
        <owl:disjointWith rdf:resource="#DimensionOfIndividual"/>
        <owl:disjointWith rdf:resource="#PropertyForShapeDimension"/>
        <rdfs:subClassOf>
            <owl:Restriction>
                <owl:onProperty rdf:resource="#classOfControlled"/>
                <owl:allValuesFrom rdf:resource="#ClassOfRepresentationOfThing"/>
            </owl:Restriction>
        </rdfs:subClassOf>
        <rdfs:subClassOf>
            <owl:Restriction>
                <owl:onProperty rdf:resource="#controller"/>
                <owl:allValuesFrom rdf:resource="#PossibleIndividual"/>
            </owl:Restriction>
        </rdfs:subClassOf>
        <rdfs:comment>
            DEFINITION A ClassOfResposibilityForRepresentation is a ClassOfRelationship
            whose members indicate that a PossibleIndividual (usually an organization)
            deems that members of the pattern can be used as representations of the
            represented Thing .
        </rdfs:comment>
        <rdfs:comment>
            EXAMPLE The link between the identification of pump #1234 and the XYZ
            Corporation, that indicates that the XYZ Corporation controls this
            identification, can be represented by an instance of
            ClassOfResposibilityForRepresentation .
        </rdfs:comment>
    </owl:Class>

    <owl:Class rdf:ID="ClassOfRightNamespace">
        <rdfs:subClassOf rdf:resource="#ClassOfNamespace"/>
        <rdfs:comment>
            DEFINITION A ClassOfRightNamespace is a ClassOfNamespace where the
            classOfPart is the namespace for the members of the classOfClassOfWhole .
        </rdfs:comment>
    </owl:Class>

    <owl:Class rdf:ID="ClassOfScale">
        <rdfs:subClassOf rdf:resource="#ClassOfClassOfRelationship"/>
        <owl:disjointWith rdf:resource="#DimensionOfShape"/>
        <owl:disjointWith rdf:resource="#PropertySpaceForClassOfShapeDimension"/>
        <rdfs:comment>
            DEFINITION A ClassOfScale is a ClassOfClassOfRelationship whose members are
            instances of Scale .
        </rdfs:comment>
        <rdfs:comment>
            EXAMPLE 'SI Unit' is an instance of ClassOfScale .
        </rdfs:comment>
    </owl:Class>

    <owl:Class rdf:ID="ClassOfScaleConversion">
        <rdfs:subClassOf rdf:resource="#ClassOfIsomorphicFunctionalMapping"/>
        <owl:disjointWith rdf:resource="#Scale"/>
        <rdfs:subClassOf>
            <owl:Restriction>
                <owl:onProperty rdf:resource="#codomain"/>
                <owl:allValuesFrom rdf:resource="#Scale"/>
            </owl:Restriction>
        </rdfs:subClassOf>
        <rdfs:subClassOf>
            <owl:Restriction>
                <owl:onProperty rdf:resource="#domain"/>
                <owl:allValuesFrom rdf:resource="#Scale"/>
            </owl:Restriction>
        </rdfs:subClassOf>
        <rdfs:comment>
            DEFINITION A ClassOfScaleConversion is a ClassOfIsomorphicFunctionalMapping
            that defines a conversion between two different scales of units used for the
            quantification of properties.
        </rdfs:comment>
        <rdfs:comment>
            EXAMPLE The Fahrenheit scale for temperature and the Celsius scale for
            temperature can each be represented by instances of Scale . The conversion
            between these scales can be represented by an instance of
            ClassOfScaleConversion.
        </rdfs:comment>
    </owl:Class>

    <owl:Class rdf:ID="ClassOfShape">
        <rdfs:subClassOf rdf:resource="#PropertySpace"/>
        <rdfs:comment>
            DEFINITION A ClassOfShape is a PropertySpace that has instances of Shape as
            its members.
        </rdfs:comment>
        <rdfs:comment>
            EXAMPLE Regular geometric forms such as 'line', 'circle', 'square',
            'cylinder', 'sphere', and 'cone' can be represented by instances of
            ClassOfShape .
        </rdfs:comment>
    </owl:Class>

    <owl:Class rdf:ID="ClassOfShapeDimension">
        <rdfs:subClassOf rdf:resource="#ClassOfClass"/>
        <rdfs:comment>
            DEFINITION A ClassOfShapeDimension is a ClassOfClass that is a dimension of a
            ClassOfShape .
        </rdfs:comment>
        <rdfs:comment>
            EXAMPLE 'Diameter', 'height', and 'width' (in general rather than a
            particular one) are examples of ClassOfShapeDimension .
        </rdfs:comment>
    </owl:Class>

    <owl:Class rdf:ID="ClassOfSpecialization">
        <rdfs:subClassOf rdf:resource="#ClassOfRelationship"/>
        <owl:disjointWith rdf:resource="#ClassOfTemporalSequence"/>
        <owl:disjointWith rdf:resource="#ClassOfUsageOfRepresentation"/>
        <owl:disjointWith rdf:resource="#DimensionOfIndividual"/>
        <owl:disjointWith rdf:resource="#PropertyForShapeDimension"/>
        <rdfs:subClassOf>
            <owl:Restriction>
                <owl:onProperty rdf:resource="#classOfSubclass"/>
                <owl:allValuesFrom rdf:resource="#ClassOfClass"/>
            </owl:Restriction>
        </rdfs:subClassOf>
        <rdfs:subClassOf>
            <owl:Restriction>
                <owl:onProperty rdf:resource="#classOfSuperclass"/>
                <owl:allValuesFrom rdf:resource="#ClassOfClass"/>
            </owl:Restriction>
        </rdfs:subClassOf>
        <rdfs:comment>
            DEFINITION A ClassOfSpecialization is a ClassOfRelationship whose members are
            instances of Specialization . It indicates that a member of the
            classOfSubclass is a subclass of a member of the classOfSuperclass.
        </rdfs:comment>
        <rdfs:comment>
            EXAMPLE The ClassOfSpecialization that indicates that members of the class
            "family of ASME bolts", e.g. '3 inch bolts', '2 inch bolts', are
            specializations of members of the EnumeratedPropertySet "set of bolt
            lengths", e.g. '3 inch', '2 inch'.
        </rdfs:comment>
        <rdfs:comment>
            NOTE Since in OWL there is no Specialization possible because of the use of
            the standard rdfs:subClassOf construct, this ClassOfClassification cannot be 
            used as such.
        </rdfs:comment>
    </owl:Class>

    <owl:Class rdf:ID="ClassOfStatus">
        <rdfs:subClassOf rdf:resource="#ClassOfClassOfIndividual"/>
        <owl:disjointWith rdf:resource="#ShapeDimension"/>
        <rdfs:comment>
            DEFINITION A ClassOfStatus is a ClassOfClassOfIndividual whose members are a
            Status .
        </rdfs:comment>
        <rdfs:comment>
            EXAMPLE An example of ClassOfStatus is 'approval', with members:
            'not assessed', 'approved', 'rejected'.
        </rdfs:comment>
    </owl:Class>

    <owl:Class rdf:ID="ClassOfSubAtomicParticle">
        <rdfs:subClassOf rdf:resource="#ClassOfArrangedIndividual"/>
        <owl:disjointWith rdf:resource="#CrystallineStructure"/>
        <owl:disjointWith rdf:resource="#Phase"/>
        <rdfs:comment>
            DEFINITION A ClassOfSubAtomicParticle is a ClassOfArrangedIndividual whose
            members are constituent particles of atoms.
        </rdfs:comment>
        <rdfs:comment>
            EXAMPLE 'Proton', 'electron', 'meson', 'neutron', 'positron', 'muon',
            'quark', and 'neutrino' can be represented by instances of
            ClassOfSubAtomicParticle .
        </rdfs:comment>
    </owl:Class>

    <owl:Class rdf:ID="ClassOfTemporalSequence">
        <rdfs:subClassOf rdf:resource="#ClassOfRelationship"/>
        <owl:disjointWith rdf:resource="#ClassOfUsageOfRepresentation"/>
        <owl:disjointWith rdf:resource="#DimensionOfIndividual"/>
        <owl:disjointWith rdf:resource="#PropertyForShapeDimension"/>
        <rdfs:subClassOf>
            <owl:Restriction>
                <owl:onProperty rdf:resource="#classOfPredecessor"/>
                <owl:allValuesFrom rdf:resource="#ClassOfIndividual"/>
            </owl:Restriction>
        </rdfs:subClassOf>
        <rdfs:subClassOf>
            <owl:Restriction>
                <owl:onProperty rdf:resource="#classOfSuccessor"/>
                <owl:allValuesFrom rdf:resource="#ClassOfIndividual"/>
            </owl:Restriction>
        </rdfs:subClassOf>
        <rdfs:comment>
            DEFINITION A ClassOfTemporalSequence is a ClassOfRelationship where the
            sequence is of a temporal nature.
        </rdfs:comment>
        <rdfs:comment>
            EXAMPLE 1 The link that indicates that members of July follow members of June
            can be represented by an instance of ClassOfTemporalSequence .
        </rdfs:comment>
        <rdfs:comment>
            EXAMPLE 2 The link that indicates that emptying activities for a tank precede
            cleaning activities can be represented by an instance of
            ClassOfTemporalSequence .
        </rdfs:comment>
    </owl:Class>

    <owl:Class rdf:ID="ClassOfTemporalWholePart">
        <rdfs:subClassOf rdf:resource="#ClassOfCompositionOfIndividual"/>
        <rdfs:comment>
            DEFINITION A ClassOfTemporalWholePart is a ClassOfCompositionOfIndividual
            whose members are members of TemporalWholePart .
        </rdfs:comment>
        <rdfs:comment>
            EXAMPLE The class that indicates that Crude Distillation Units may have a
            maximum naphtha mode can be represented by an instance of
            ClassOfTemporalWholePart .
        </rdfs:comment>
    </owl:Class>

    <owl:Class rdf:ID="ClassOfUsageOfRepresentation">
        <rdf:type rdf:resource="#ClassOfClassOfUsageOfRepresentation"/>
        <rdfs:subClassOf rdf:resource="#ClassOfRelationship"/>
        <owl:disjointWith rdf:resource="#DimensionOfIndividual"/>
        <owl:disjointWith rdf:resource="#PropertyForShapeDimension"/>
        <rdfs:subClassOf>
            <owl:Restriction>
                <owl:onProperty rdf:resource="#classOfUsed"/>
                <owl:allValuesFrom rdf:resource="#ClassOfRepresentationOfThing"/>
            </owl:Restriction>
        </rdfs:subClassOf>
        <rdfs:subClassOf>
            <owl:Restriction>
                <owl:onProperty rdf:resource="#user"/>
                <owl:allValuesFrom rdf:resource="#PossibleIndividual"/>
            </owl:Restriction>
        </rdfs:subClassOf>
        <rdfs:comment>
            DEFINITION A ClassOfUsageOfRepresentation is a ClassOfRelationship whose
            members indicate that a PossibleIndividual (usually an organization) reads or
            otherwise uses members of the pattern as a representation of the represented
            Thing .
        </rdfs:comment>
        <rdfs:comment>
            EXAMPLE The link between the identification of pump #1234 and contractor
            ABC Ltd, that indicates that ABC Ltd uses this identification can be
            represented by a class of ClassOfUsageOfRepresentation.
        </rdfs:comment>
    </owl:Class>

    <owl:Class rdf:ID="ComparisonOfProperty">
        <rdfs:subClassOf rdf:resource="#Relationship"/>
        <owl:disjointWith rdf:resource="#CompositionOfIndividual"/>
        <owl:disjointWith rdf:resource="#ConnectionOfIndividual"/>
        <owl:disjointWith rdf:resource="#FunctionalMapping"/>
        <owl:disjointWith rdf:resource="#IndirectProperty"/>
        <owl:disjointWith rdf:resource="#IndividualUsedInConnection"/>
        <owl:disjointWith rdf:resource="#IntendedRoleAndDomain"/>
        <owl:disjointWith rdf:resource="#InvolvementByReference"/>
        <owl:disjointWith rdf:resource="#LifecycleStage"/>
        <owl:disjointWith rdf:resource="#OtherRelationship"/>
        <owl:disjointWith rdf:resource="#PossibleRoleAndDomain"/>
        <owl:disjointWith rdf:resource="#Recognition"/>
        <owl:disjointWith rdf:resource="#RelativeLocation"/>
        <owl:disjointWith rdf:resource="#RepresentationOfThing"/>
        <owl:disjointWith rdf:resource="#ResponsibilityForRepresentation"/>
        <owl:disjointWith rdf:resource="#TemporalSequence"/>
        <owl:disjointWith rdf:resource="#UsageOfRepresentation"/>
        <rdfs:subClassOf>
            <owl:Restriction>
                <owl:onProperty rdf:resource="#greaterElement"/>
                <owl:allValuesFrom rdf:resource="#Property"/>
            </owl:Restriction>
        </rdfs:subClassOf>
        <rdfs:subClassOf>
            <owl:Restriction>
                <owl:onProperty rdf:resource="#lesserElement"/>
                <owl:allValuesFrom rdf:resource="#Property"/>
            </owl:Restriction>
        </rdfs:subClassOf>
        <rdfs:comment>
            DEFINITION A ComparisonOfProperty is a Relationship that indicates the
            magnitude of one Property is greater than that of another.
        </rdfs:comment>
        <rdfs:comment>
            EXAMPLE That the temperature in a room is less than that in a furnace can be
            indicated by an instance of ComparisonOfProperty .
        </rdfs:comment>
    </owl:Class>

    <owl:Class rdf:ID="CompositionOfIndividual">
        <rdf:type rdf:resource="#ClassOfCompositionOfIndividual"/>
        <rdfs:subClassOf rdf:resource="#Relationship"/>
        <owl:unionOf rdf:parseType="Collection">  
            <owl:Class rdf:about="#ArrangementOfIndividual"/>  
            <owl:Class rdf:about="#Participation"/>  
            <owl:Class rdf:about="#TemporalBounding"/>  
            <owl:Class rdf:about="#TemporalWholePart"/>  
        </owl:unionOf>
        <owl:disjointWith rdf:resource="#ConnectionOfIndividual"/>
        <owl:disjointWith rdf:resource="#FunctionalMapping"/>
        <owl:disjointWith rdf:resource="#IndirectProperty"/>
        <owl:disjointWith rdf:resource="#IndividualUsedInConnection"/>
        <owl:disjointWith rdf:resource="#IntendedRoleAndDomain"/>
        <owl:disjointWith rdf:resource="#InvolvementByReference"/>
        <owl:disjointWith rdf:resource="#LifecycleStage"/>
        <owl:disjointWith rdf:resource="#OtherRelationship"/>
        <owl:disjointWith rdf:resource="#PossibleRoleAndDomain"/>
        <owl:disjointWith rdf:resource="#Recognition"/>
        <owl:disjointWith rdf:resource="#RelativeLocation"/>
        <owl:disjointWith rdf:resource="#RepresentationOfThing"/>
        <owl:disjointWith rdf:resource="#ResponsibilityForRepresentation"/>
        <owl:disjointWith rdf:resource="#TemporalSequence"/>
        <owl:disjointWith rdf:resource="#UsageOfRepresentation"/>
        <rdfs:subClassOf>
            <owl:Restriction>
                <owl:onProperty rdf:resource="#part"/>
                <owl:allValuesFrom rdf:resource="#PossibleIndividual"/>
            </owl:Restriction>
        </rdfs:subClassOf>
        <rdfs:subClassOf>
            <owl:Restriction>
                <owl:onProperty rdf:resource="#whole"/>
                <owl:allValuesFrom rdf:resource="#PossibleIndividual"/>
            </owl:Restriction>
        </rdfs:subClassOf>
        <rdfs:comment>
            DEFINITION A CompositionOfIndividual is a Relationship that indicates that
            the part PossibleIndividual is a part of the whole PossibleIndividual .
            A simple composition is indicated, unless a subtype is instantiated too.
        </rdfs:comment>
        <rdfs:comment>
            CompositionOfIndividual is transitive.
        </rdfs:comment>
        <rdfs:comment>
            NOTE Simple composition means that for example no arrangement of parts is
            necessarily implied or of concern. Where there is an arrangement of parts,
            this is indicated by an ArrangementOfIndividual , which, by being a subtype,
            implies also a simple composition.
        </rdfs:comment>
        <rdfs:comment>
            EXAMPLE A grain of sand being part of a pile of sand is an example of
            CompositionOfIndividual.
        </rdfs:comment>
    </owl:Class>

    <owl:Class rdf:ID="ConnectionOfIndividual">
        <rdf:type rdf:resource="#ClassOfConnectionOfIndividual"/>
        <rdfs:subClassOf rdf:resource="#Relationship"/>
        <owl:unionOf rdf:parseType="Collection">  
            <owl:Class rdf:about="#DirectConnection"/>  
            <owl:Class rdf:about="#IndirectConnection"/>  
        </owl:unionOf>
        <owl:disjointWith rdf:resource="#FunctionalMapping"/>
        <owl:disjointWith rdf:resource="#IndirectProperty"/>
        <owl:disjointWith rdf:resource="#IndividualUsedInConnection"/>
        <owl:disjointWith rdf:resource="#IntendedRoleAndDomain"/>
        <owl:disjointWith rdf:resource="#InvolvementByReference"/>
        <owl:disjointWith rdf:resource="#LifecycleStage"/>
        <owl:disjointWith rdf:resource="#OtherRelationship"/>
        <owl:disjointWith rdf:resource="#PossibleRoleAndDomain"/>
        <owl:disjointWith rdf:resource="#Recognition"/>
        <owl:disjointWith rdf:resource="#RelativeLocation"/>
        <owl:disjointWith rdf:resource="#RepresentationOfThing"/>
        <owl:disjointWith rdf:resource="#ResponsibilityForRepresentation"/>
        <owl:disjointWith rdf:resource="#TemporalSequence"/>
        <owl:disjointWith rdf:resource="#UsageOfRepresentation"/>
        <rdfs:subClassOf>
            <owl:Restriction>
                <owl:onProperty rdf:resource="#side1"/>
                <owl:allValuesFrom rdf:resource="#PossibleIndividual"/>
            </owl:Restriction>
        </rdfs:subClassOf>
        <rdfs:subClassOf>
            <owl:Restriction>
                <owl:onProperty rdf:resource="#side2"/>
                <owl:allValuesFrom rdf:resource="#PossibleIndividual"/>
            </owl:Restriction>
        </rdfs:subClassOf>
        <rdfs:comment>
            DEFINITION A ConnectionOfIndividual is a Relationship that indicates that
            matter, energy, or both can be transferred between the members of
            PossibleIndividual that are connected, either directly or indirectly.
        </rdfs:comment>
        <rdfs:comment>
            NOTE There is no significance to the ordering of the two related instances of
            PossibleIndividual . The names side1 and side2 serve only to distinguish the
            attributes.
        </rdfs:comment>
    </owl:Class>

    <owl:Class rdf:ID="ContainmentOfIndividual">
        <rdf:type rdf:resource="#ClassOfContainmentOfIndividual"/>
        <rdfs:subClassOf rdf:resource="#RelativeLocation"/>
        <rdfs:comment>
            DEFINITION A ContainmentOfIndividual is a RelativeLocation where the located
            PossibleIndividual is contained by the locator PossibleIndividual but is not
            part of it.
        </rdfs:comment>
        <rdfs:comment>
            NOTE Containment is distinct from composition; in composition the whole
            consists of all of its part, with containment, what is contained is not a
            part of the container.
        </rdfs:comment>
        <rdfs:comment>
            EXAMPLE The contents of a vessel being inside the vessel can be represented
            by an instance of ContainmentOfIndividual .
        </rdfs:comment>
    </owl:Class>

    <owl:Class rdf:ID="CoordinateSystem">
        <rdfs:subClassOf rdf:resource="#MultidimensionalScale"/>
        <rdfs:comment>
            DEFINITION A CoordinateSystem is a MultidimensionalScale for locating and
            relating a PossibleIndividual in an n-dimensional space in which arbitrary
            geometric transformations are valid.
        </rdfs:comment>
        <rdfs:comment>
            EXAMPLE The XYZ site coordinate system, is an example of a CoordinateSystem .
        </rdfs:comment>
    </owl:Class>

    <owl:Class rdf:ID="CrystallineStructure">
        <rdfs:subClassOf rdf:resource="#ClassOfArrangedIndividual"/>
        <owl:disjointWith rdf:resource="#Phase"/>
        <rdfs:comment>
            DEFINITION A CrystallineStructure is a ClassOfArrangedIndividual that is a
            form in which many simple elements and their natural compounds regularly
            aggregate by the operation of natural affinity: it has a definite internal
            structure, with the external form of a solid enclosed by a number of
            symmetrically arranged plane faces, and varying in simplicity from the cube
            to much more complicated geometric bodies.
        </rdfs:comment>
        <rdfs:comment>
            EXAMPLE Ferritic, martensitic, and austenitic are examples of
            CrystallineStructure .
        </rdfs:comment>
    </owl:Class>

    <owl:Class rdf:ID="Definition">
        <rdf:type rdf:resource="#ClassOfDefinition"/>
        <rdfs:subClassOf rdf:resource="#RepresentationOfThing"/>
        <rdfs:subClassOf>
            <owl:Restriction>
                <owl:onProperty rdf:resource="#represented"/>
                <owl:allValuesFrom rdf:resource="#Class"/>
            </owl:Restriction>
        </rdfs:subClassOf>
        <rdfs:comment>
            DEFINITION A Definition is a RepresentationOfThing that indicates that the
            Class is defined by the sign PossibleIndividual .
        </rdfs:comment>
        <rdfs:comment>
            NOTE In semiotics, a sign is generally defined as "something that stands for
            something else, to someone in some capacity". It may be understood as a
            discrete unit of meaning. Signs are not limited to words but also include
            images, gestures, scents, tastes, textures, sounds - essentially all of the
            ways in which information can be processed and communicated by any sentient,
            reasoning mind.
        </rdfs:comment>
        <rdfs:comment>
            EXAMPLE The Relationship between the ClassOfInanimatePhysicalObject
            'condensate' and the PhysicalObject that is the ink-on-paper
            (or pixels-on-screeen): "An aggregate which is in condensed form which means
            in liquid state, resulting from a substance in vapour state." is an instance
            of Definition .
        </rdfs:comment>
    </owl:Class>

    <owl:Class rdf:ID="Description">
        <rdf:type rdf:resource="#ClassOfDescription"/>
        <rdfs:subClassOf rdf:resource="#RepresentationOfThing"/>
        <rdfs:comment>
            DEFINITION A Description is a RepresentationOfThing that indicates that the
            PossibleIndividual describes the Thing .
        </rdfs:comment>
        <rdfs:comment>
            EXAMPLE A paper copy of the Piping and Instrumentation Diagram for Crude
            Distillation Unit 1 at refinery X has a Description relationship with the
            plant.
        </rdfs:comment>
    </owl:Class>

    <owl:Class rdf:ID="DifferenceOfSetOfClass">
        <rdfs:subClassOf rdf:resource="#FunctionalMapping"/>
        <owl:disjointWith rdf:resource="#IntersectionOfSetOfClass"/>
        <owl:disjointWith rdf:resource="#UnionOfSetOfClass"/>
        <owl:disjointWith rdf:resource="#PropertyQuantification"/>
        <rdfs:subClassOf>
            <owl:Restriction>
                <owl:onProperty rdf:resource="#input"/>
                <owl:allValuesFrom rdf:resource="#EnumeratedSetOfClass"/>
            </owl:Restriction>
        </rdfs:subClassOf>
        <rdfs:subClassOf>
            <owl:Restriction>
                <owl:onProperty rdf:resource="#result"/>
                <owl:allValuesFrom rdf:resource="#Class"/>
            </owl:Restriction>
        </rdfs:subClassOf>
        <rdfs:comment>
            DEFINITION A DifferenceOfSetOfClass is a FunctionalMapping that indicates
            that the membership of the result Class is the difference between the
            membership of the union of the classes that are members of the
            EnumeratedSetOfClass and their intersection.
        </rdfs:comment>
        <rdfs:comment>
            NOTE When the EnumeratedSetOfClass consists of a Class and another Class that
            is a subclass of the first class, then the difference is the complement of
            the subclass.
        </rdfs:comment>
        <rdfs:comment>
            EXAMPLE The difference of the EnumeratedSetOfClass {{A,B,C},{B,C,D},{C,D,E}}
            is {A,B,D,E}.
        </rdfs:comment>
    </owl:Class>

    <owl:Class rdf:ID="DimensionOfIndividual">
        <rdf:type rdf:resource="#DimensionOfShape"/>
        <rdfs:subClassOf rdf:resource="#ClassOfRelationship"/>
        <owl:disjointWith rdf:resource="#PropertyForShapeDimension"/>
        <rdfs:subClassOf>
            <owl:Restriction>
                <owl:onProperty rdf:resource="#individual"/>
                <owl:allValuesFrom rdf:resource="#PossibleIndividual"/>
            </owl:Restriction>
        </rdfs:subClassOf>
        <rdfs:subClassOf>
            <owl:Restriction>
                <owl:onProperty rdf:resource="#individualDimension"/>
                <owl:allValuesFrom rdf:resource="#IndividualDimension"/>
            </owl:Restriction>
        </rdfs:subClassOf>
        <rdfs:comment>
            DEFINITION A DimensionOfIndividual is a ClassOfRelationship that indicates
            that each member of the set of lines that are the IndividualDimension are a
            dimension of the PossibleIndividual .
        </rdfs:comment>
        <rdfs:comment>
            EXAMPLE The set of all lines that pass through the centre of a particular
            circle and end at the circumference of that circle, are a dimension
            (diameter) of that circle. The particular dimension is indicated by the
            DimensionOfShape that classifies the DimensionOfIndividual .
        </rdfs:comment>
    </owl:Class>

    <owl:Class rdf:ID="DimensionOfShape">
        <rdfs:subClassOf rdf:resource="#ClassOfClassOfRelationship"/>
        <owl:disjointWith rdf:resource="#PropertySpaceForClassOfShapeDimension"/>
        <rdfs:subClassOf>
            <owl:Restriction>
                <owl:onProperty rdf:resource="#dimension"/>
                <owl:allValuesFrom rdf:resource="#ShapeDimension"/>
            </owl:Restriction>
        </rdfs:subClassOf>
        <rdfs:subClassOf>
            <owl:Restriction>
                <owl:onProperty rdf:resource="#shape"/>
                <owl:allValuesFrom rdf:resource="#Shape"/>
            </owl:Restriction>
        </rdfs:subClassOf>
        <rdfs:comment>
            DEFINITION A DimensionOfShape is a ClassOfClassOfRelationship that indicates
            that members of the ShapeDimension are dimensions of the Shape members.
        </rdfs:comment>
        <rdfs:comment>
            EXAMPLE The sets of 10m lines that are diameters of 10m circles is an example
            of DimensionOfShape .
        </rdfs:comment>
    </owl:Class>

    <owl:Class rdf:ID="DirectConnection">
        <rdf:type rdf:resource="#ClassOfDirectConnection"/>
        <rdfs:subClassOf rdf:resource="#ConnectionOfIndividual"/>
        <owl:disjointWith rdf:resource="#IndirectConnection"/>
        <rdfs:comment>
            DEFINITION A DirectConnection is a ConnectionOfIndividual that indicates that
            the side1 and side2 are directly connected via a common spatial boundary.
        </rdfs:comment>
        <rdfs:comment>
            EXAMPLE The relation that indicates that the plug terminating a serial
            communications cable is connected to the socket on a piece of computer
            equipment can be represented by an instance of DirectConnection.
        </rdfs:comment>
    </owl:Class>

    <owl:Class rdf:ID="DocumentDefinition">
        <rdfs:subClassOf rdf:resource="#ClassOfClassOfInformationRepresentation"/>
        <owl:disjointWith rdf:resource="#Language"/>
        <owl:disjointWith rdf:resource="#RepresentationForm"/>
        <rdfs:comment>
            DEFINITION A DocumentDefinition is a ClassOfClassOfInformationRepresentation
            that defines the content and/or structure of documents.
        </rdfs:comment>
        <rdfs:comment>
            EXAMPLE XYZ Corp. Material Safety Data Sheet is a DocumentDefinition.
        </rdfs:comment>
        <rdfs:comment>
            EXAMPLE In ISO 15926-7 a Template Specification defines and describes a
            template; the latter is a DocumentDefinition .
        </rdfs:comment>
    </owl:Class>

    <owl:Class rdf:ID="Ending">
        <rdfs:subClassOf rdf:resource="#TemporalBounding"/>
        <rdfs:comment>
            DEFINITION An Ending is a TemporalBounding that marks the end of a PossibleIndividual .
        </rdfs:comment>
        <rdfs:comment>
            EXAMPLE 1 The relation that indicates that the PointInTime known as 0000hrs
            1st July 1999 GMT is the end of the PeriodInTime known as June 1999 00.00 GMT
            can be represented by an instance of Ending .
        </rdfs:comment>
        <rdfs:comment>
            EXAMPLE 2 The relation that indicates that the Event 'loading complete'
            marks the end of the PossibleIndividual 'loading plant operating period 1'
            (a temporal part of the loading plant) is an instance of Ending .
        </rdfs:comment>
    </owl:Class>

    <owl:Class rdf:ID="EnumeratedNumberSet">
        <rdfs:subClassOf rdf:resource="#ClassOfNumber"/>
        <rdfs:subClassOf rdf:resource="#EnumeratedSetOfClass"/>
        <owl:disjointWith rdf:resource="#NumberSpace"/>
        <rdfs:comment>
            DEFINITION An EnumeratedNumberSet is a ClassOfNumber and an
            EnumeratedSetOfClass .
        </rdfs:comment>
        <rdfs:comment>
            EXAMPLE The set of integer numbers {3,4,5} can be represented by an instance
            of EnumeratedNumberSet .
        </rdfs:comment>
    </owl:Class>

    <owl:Class rdf:ID="EnumeratedPropertySet">
        <rdfs:subClassOf rdf:resource="#ClassOfProperty"/>
        <rdfs:subClassOf rdf:resource="#EnumeratedSetOfClass"/>
        <owl:disjointWith rdf:resource="#PropertySpace"/>
        <rdfs:comment>
            DEFINITION An EnumeratedPropertySet is a ClassOfProperty and an
            EnumeratedSetOfClass whose members are an enumerated set of properties of the
            same SinglePropertyDimension or MultidimensionalPropertySpace .
        </rdfs:comment>
        <rdfs:comment>
            EXAMPLE {115 Volt, 240 Volt} is an example of an EnumeratedPropertySet .
        </rdfs:comment>
    </owl:Class>

    <owl:Class rdf:ID="EnumeratedSetOfClass">
        <rdfs:subClassOf rdf:resource="#ClassOfClass"/>
        <owl:intersectionOf rdf:parseType="Collection">  
            <owl:Class rdf:about="#EnumeratedNumberSet"/>  
            <owl:Class rdf:about="#EnumeratedPropertySet"/>  
        </owl:intersectionOf>
        <rdfs:comment>
            DEFINITION An EnumeratedSetOfClass is a ClassOfClass that is an enumerated
            set of the instances of Class . Enumerated means that the full set of
            members is specified.
        </rdfs:comment>
        <rdfs:comment>
            EXAMPLE {Plastic, 1.2kg, frame} is an EnumeratedSetOfClass.
            More generally {{A,B,C},{B,C,D},{C,D,E}} is an EnumeratedSetOfClass. Also
            "electrical engineering classes for ERDL V1.1" is an EnumeratedSetOfClass.
        </rdfs:comment>
    </owl:Class>

    <owl:Class rdf:ID="Event">
        <rdf:type rdf:resource="#ClassOfEvent"/>
        <rdfs:subClassOf rdf:resource="#PossibleIndividual"/>
        <rdfs:comment>
            DEFINITION An Event is a PossibleIndividual with zero extent in time.
            An Event is the temporal boundary of one or more instances of
            PossibleIndividual, although there may be no knowledge of these instances.
        </rdfs:comment>
        <rdfs:comment>
            EXAMPLE The connection of power to a pump is an Event that marks the
            beginning of a temporal part of that pump.
        </rdfs:comment>
    </owl:Class>

    <owl:Class rdf:ID="ExpressBinary">
        <rdfs:subClassOf rdf:resource="#ClassOfExpressInformationRepresentation"/>
        <owl:disjointWith rdf:resource="#ExpressBoolean"/>
        <owl:disjointWith rdf:resource="#ExpressInteger"/>
        <owl:disjointWith rdf:resource="#ExpressLogical"/>
        <owl:disjointWith rdf:resource="#ExpressReal"/>
        <owl:disjointWith rdf:resource="#ExpressString"/>
        <rdfs:subClassOf>
            <owl:Restriction>
                <owl:onProperty rdf:resource="#content"/>
                <owl:allValuesFrom rdf:datatype="http://www.w3.org/2001/XMLSchema#base64Binary"/>
            </owl:Restriction>
        </rdfs:subClassOf>
        <rdfs:comment>
            DEFINITION An ExpressBinary is a ClassOfExpressInformationRepresentation that
            represents a binary value as defined in ISO 10303-11:1994, 8.1.7 .
        </rdfs:comment>
    </owl:Class>

    <owl:Class rdf:ID="ExpressBoolean">
        <rdfs:subClassOf rdf:resource="#ClassOfExpressInformationRepresentation"/>
        <owl:disjointWith rdf:resource="#ExpressInteger"/>
        <owl:disjointWith rdf:resource="#ExpressLogical"/>
        <owl:disjointWith rdf:resource="#ExpressReal"/>
        <owl:disjointWith rdf:resource="#ExpressString"/>
        <rdfs:subClassOf>
            <owl:Restriction>
                <owl:onProperty rdf:resource="#content"/>
                <owl:allValuesFrom rdf:datatype="http://www.w3.org/2001/XMLSchema#boolean"/>
            </owl:Restriction>
        </rdfs:subClassOf>
        <rdfs:comment>
            DEFINITION An ExpressBoolean is a ClassOfExpressInformationRepresentation
            that represents a Boolean value as defined in ISO 10303-11:1994, 8.1.5 .
        </rdfs:comment>
    </owl:Class>

    <owl:Class rdf:ID="ExpressInteger">
        <rdfs:subClassOf rdf:resource="#ClassOfExpressInformationRepresentation"/>
        <owl:disjointWith rdf:resource="#ExpressLogical"/>
        <owl:disjointWith rdf:resource="#ExpressReal"/>
        <owl:disjointWith rdf:resource="#ExpressString"/>
        <rdfs:subClassOf>
            <owl:Restriction>
                <owl:onProperty rdf:resource="#content"/>
                <owl:allValuesFrom rdf:datatype="http://www.w3.org/2001/XMLSchema#integer"/>
            </owl:Restriction>
        </rdfs:subClassOf>
        <rdfs:comment>
            DEFINITION An ExpressInteger is a ClassOfExpressInformationRepresentation
            that represents an integer number as defined in ISO 10303-11:1994, 8.1.3 .
        </rdfs:comment>
    </owl:Class>

    <owl:Class rdf:ID="ExpressLogical">
        <rdfs:subClassOf rdf:resource="#ClassOfExpressInformationRepresentation"/>
        <owl:disjointWith rdf:resource="#ExpressReal"/>
        <owl:disjointWith rdf:resource="#ExpressString"/>
        <rdfs:subClassOf>
            <owl:Restriction>
                <owl:onProperty rdf:resource="#content"/>
                <owl:allValuesFrom rdf:resource="#LogicalValue"/>
            </owl:Restriction>
        </rdfs:subClassOf>
        <rdfs:comment>
            DEFINITION An ExpressLogical is a ClassOfExpressInformationRepresentation
            that represents a logical value as defined in ISO 10303-11:1994, 8.1.4 .
        </rdfs:comment>
    </owl:Class>

    <owl:Class rdf:ID="ExpressReal">
        <rdfs:subClassOf rdf:resource="#ClassOfExpressInformationRepresentation"/>
        <owl:disjointWith rdf:resource="#ExpressString"/>
        <rdfs:subClassOf>
            <owl:Restriction>
                <owl:onProperty rdf:resource="#content"/>
                <owl:allValuesFrom rdf:datatype="http://www.w3.org/2001/XMLSchema#long"/>
            </owl:Restriction>
        </rdfs:subClassOf>
        <rdfs:comment>
            DEFINITION An ExpressReal is a ClassOfExpressInformationRepresentation
            that represents a real number as defined in ISO 10303-11:1994, 8.1.2 .
        </rdfs:comment>
    </owl:Class>

    <owl:Class rdf:ID="ExpressString">
        <rdfs:subClassOf rdf:resource="#ClassOfExpressInformationRepresentation"/>
        <rdfs:subClassOf>
            <owl:Restriction>
                <owl:onProperty rdf:resource="#content"/>
                <owl:allValuesFrom rdf:datatype="http://www.w3.org/2001/XMLSchema#string"/>
            </owl:Restriction>
        </rdfs:subClassOf>
        <rdfs:comment>
            DEFINITION An ExpressString is a ClassOfExpressInformationRepresentation
            that represents a string as defined in ISO 10303-11:1994, 8.1.6 .
        </rdfs:comment>
    </owl:Class>

    <owl:Class rdf:ID="FeatureWholePart">
        <rdf:type rdf:resource="#ClassOfFeatureWholePart"/>
        <rdfs:subClassOf rdf:resource="#ArrangementOfIndividual"/>
        <rdfs:comment>
            DEFINITION A FeatureWholePart is an ArrangementOfIndividual that indicates
            that the part is a non-separable, contiguous part of the whole.
        </rdfs:comment>
        <rdfs:comment>
            NOTE This includes wholes that cannot be non-destructively disassembled and
            reassembled such as the inlet flange of a pump.
        </rdfs:comment>
        <rdfs:comment>
            EXAMPLE The relation that indicates that a flange face is part of a flange
            can be represented by an instance of FeatureWholePart .
        </rdfs:comment>
    </owl:Class>

    <owl:Class rdf:ID="FunctionalMapping">
        <rdfs:subClassOf rdf:resource="#Relationship"/>
        <owl:unionOf rdf:parseType="Collection">  
            <owl:Class rdf:about="#DifferenceOfSetOfClass"/>  
            <owl:Class rdf:about="#IntersectionOfSetOfClass"/>  
            <owl:Class rdf:about="#UnionOfSetOfClass"/>  
            <owl:Class rdf:about="#PropertyQuantification"/>  
        </owl:unionOf>
        <owl:disjointWith rdf:resource="#IndirectProperty"/>
        <owl:disjointWith rdf:resource="#IndividualUsedInConnection"/>
        <owl:disjointWith rdf:resource="#IntendedRoleAndDomain"/>
        <owl:disjointWith rdf:resource="#InvolvementByReference"/>
        <owl:disjointWith rdf:resource="#LifecycleStage"/>
        <owl:disjointWith rdf:resource="#OtherRelationship"/>
        <owl:disjointWith rdf:resource="#PossibleRoleAndDomain"/>
        <owl:disjointWith rdf:resource="#Recognition"/>
        <owl:disjointWith rdf:resource="#RelativeLocation"/>
        <owl:disjointWith rdf:resource="#RepresentationOfThing"/>
        <owl:disjointWith rdf:resource="#ResponsibilityForRepresentation"/>
        <owl:disjointWith rdf:resource="#TemporalSequence"/>
        <owl:disjointWith rdf:resource="#UsageOfRepresentation"/>
        <rdfs:subClassOf>
            <owl:Restriction>
                <owl:onProperty rdf:resource="#input"/>
                <owl:allValuesFrom rdf:resource="#Thing"/>
            </owl:Restriction>
        </rdfs:subClassOf>
        <rdfs:subClassOf>
            <owl:Restriction>
                <owl:onProperty rdf:resource="#result"/>
                <owl:allValuesFrom rdf:resource="#Thing"/>
            </owl:Restriction>
        </rdfs:subClassOf>
        <rdfs:comment>
            DEFINITION A FunctionalMapping is a Relationship that indicates that the
            input gave the result for the classifying ClassOfFunctionalMapping .
        </rdfs:comment>
        <rdfs:comment>
            EXAMPLE The mapping of [5, 3] to 2, classified by the minus function is an
            example of FunctionalMapping .
        </rdfs:comment>
    </owl:Class>

    <owl:Class rdf:ID="FunctionalPhysicalObject">
        <rdfs:subClassOf rdf:resource="#PhysicalObject"/>
        <rdfs:comment>
            DEFINITION A FunctionalPhysicalObject is a PhysicalObject that has
            functional, rather than material, continuity as its basis for identity.
            Adjacent temporal parts of a FunctionalPhysicalObject need not have common
            matter or energy, provided the matter or energy of each temporal part fulfils
            the same function.
        </rdfs:comment>
        <rdfs:comment>
            EXAMPLE The heat exchanger system known as tag E-4507, which is part of a
            distillate transfer system, can be represented by an instance of
            FunctionalPhysicalObject. Note that this is distinct from the "shell and tube
            heat exchanger manufacture number ES/1234" that was installed as E-4507 when
            the plant was first built and later removed when worn out, to be replaced by
            a new heat exchanger with different serial number. "Shell and tube heat
            exchanger manufacture number ES/1234" and its differently numbered
            replacement can be represented by instances of MaterializedPhysicalObject .
            When ES/1234 is installed as E-4507 there is a temporal part of ES/1234 that
            is also a temporal part of E-4507.
        </rdfs:comment>
    </owl:Class>

    <owl:Class rdf:ID="Identification">
        <rdf:type rdf:resource="#ClassOfIdentification"/>
        <rdfs:subClassOf rdf:resource="#RepresentationOfThing"/>
        <rdfs:comment>
            DEFINITION An Identification is a RepresentationOfThing that indicates that
            the PossibleIndividual is an identifier for the Thing identified.
        </rdfs:comment>
        <rdfs:comment>
            EXAMPLE The relationship between the text "P101" on a printed copy of a pump
            data sheet and the applicable FunctionalPhysicalObject is an example of
            Identification .
        </rdfs:comment>
        <rdfs:comment>
            EXAMPLE The relationship between a name tag and an employee wearing it is an
            example of Identification .
        </rdfs:comment>
    </owl:Class>

    <owl:Class rdf:ID="IndirectConnection">
        <rdf:type rdf:resource="#ClassOfIndirectConnection"/>
        <rdfs:subClassOf rdf:resource="#ConnectionOfIndividual"/>
        <rdfs:comment>
            DEFINITION An IndirectConnection is a ConnectionOfIndividual that indicates
            that side1 and side2 are connected via other individuals.
        </rdfs:comment>
        <rdfs:comment>
            EXAMPLE The relation that indicates that there is a railway connection
            between the cities of London and Paris can be represented by an instance of
            IndirectConnection .
        </rdfs:comment>
    </owl:Class>

    <owl:Class rdf:ID="IndirectProperty">
        <rdf:type rdf:resource="#ClassOfIndirectProperty"/>
        <rdfs:subClassOf rdf:resource="#Relationship"/>
        <owl:disjointWith rdf:resource="#IndividualUsedInConnection"/>
        <owl:disjointWith rdf:resource="#IntendedRoleAndDomain"/>
        <owl:disjointWith rdf:resource="#InvolvementByReference"/>
        <owl:disjointWith rdf:resource="#LifecycleStage"/>
        <owl:disjointWith rdf:resource="#OtherRelationship"/>
        <owl:disjointWith rdf:resource="#PossibleRoleAndDomain"/>
        <owl:disjointWith rdf:resource="#Recognition"/>
        <owl:disjointWith rdf:resource="#RelativeLocation"/>
        <owl:disjointWith rdf:resource="#RepresentationOfThing"/>
        <owl:disjointWith rdf:resource="#ResponsibilityForRepresentation"/>
        <owl:disjointWith rdf:resource="#TemporalSequence"/>
        <owl:disjointWith rdf:resource="#UsageOfRepresentation"/>
        <rdfs:subClassOf>
            <owl:Restriction>
                <owl:onProperty rdf:resource="#possessor"/>
                <owl:allValuesFrom rdf:resource="#PossibleIndividual"/>
            </owl:Restriction>
        </rdfs:subClassOf>
        <rdfs:subClassOf>
            <owl:Restriction>
                <owl:onProperty rdf:resource="#property"/>
                <owl:allValuesFrom rdf:resource="#Property"/>
            </owl:Restriction>
        </rdfs:subClassOf>
        <rdfs:comment>
            DEFINITION An IndirectProperty is a Relationship between a Property and a
            PossibleIndividual . The nature of the IndirectProperty is defined by its
            Classification by a ClassOfIndirectProperty . A Property is indirect when it
            does not directly apply to the PossibleIndividual it applies to, but is
            derived from some process.
        </rdfs:comment>
        <rdfs:comment>
            NOTE A property is indirect because it does not directly apply. There can
            only be one temperature that a thing has (at a time), so a Maximum Allowable
            Working Temperature is not its temperature, but an indirect property derived
            from doing some tests or calculations to determine its value (as opposed to
            it being a current measurement). This is what makes it indirect.
        </rdfs:comment>
        <rdfs:comment>
            EXAMPLE A Maximum Allowable Working Pressure of 50 BarA for V101 is specified
            by an IndirectProperty between the pressure of 50 BarA and V101, classified
            by the ClassOfIndirectProperty Maximum Allowable Working Pressure.
        </rdfs:comment>
    </owl:Class>

    <owl:Class rdf:ID="IndividualDimension">
        <rdf:type rdf:resource="#ShapeDimension"/>
        <rdfs:subClassOf rdf:resource="#ClassOfIndividual"/>
        <owl:disjointWith rdf:resource="#Property"/>
        <owl:disjointWith rdf:resource="#Status"/>
        <rdfs:comment>
            DEFINITION An IndividualDimension is a ClassOfIndividual whose members
            characterize a particular PossibleIndividual .
        </rdfs:comment>
        <rdfs:comment>
            EXAMPLE The set of lines that are each a diameter of a particular circle are
            instances of IndividualDimension .
        </rdfs:comment>
    </owl:Class>

    <owl:Class rdf:ID="IndividualUsedInConnection">
        <rdf:type rdf:resource="#ClassOfIndividualUsedInConnection"/>
        <rdfs:subClassOf rdf:resource="#Relationship"/>
        <owl:disjointWith rdf:resource="#IntendedRoleAndDomain"/>
        <owl:disjointWith rdf:resource="#InvolvementByReference"/>
        <owl:disjointWith rdf:resource="#LifecycleStage"/>
        <owl:disjointWith rdf:resource="#OtherRelationship"/>
        <owl:disjointWith rdf:resource="#PossibleRoleAndDomain"/>
        <owl:disjointWith rdf:resource="#Recognition"/>
        <owl:disjointWith rdf:resource="#RelativeLocation"/>
        <owl:disjointWith rdf:resource="#RepresentationOfThing"/>
        <owl:disjointWith rdf:resource="#ResponsibilityForRepresentation"/>
        <owl:disjointWith rdf:resource="#TemporalSequence"/>
        <owl:disjointWith rdf:resource="#UsageOfRepresentation"/>
        <rdfs:subClassOf>
            <owl:Restriction>
                <owl:onProperty rdf:resource="#connection"/>
                <owl:allValuesFrom rdf:resource="#ConnectionOfIndividual"/>
            </owl:Restriction>
        </rdfs:subClassOf>
        <rdfs:subClassOf>
            <owl:Restriction>
                <owl:onProperty rdf:resource="#usage"/>
                <owl:allValuesFrom rdf:resource="#PossibleIndividual"/>
            </owl:Restriction>
        </rdfs:subClassOf>
        <rdfs:comment>
            DEFINITION An IndividualUsedInConnection is a Relationship that indicates
            that a PossibleIndividual is used in a ConnectionOfIndividual .
        </rdfs:comment>
        <rdfs:comment>
            EXAMPLE The Relationship between the connection of the flanged ends of two
            pipes and a temporal part of the bolts, nuts, washers and gasket set that
            indicates that the bolt and gasket set participates in the connection can be
            represented by an instance of IndividualUsedInConnection .
        </rdfs:comment>
    </owl:Class>

    <owl:Class rdf:ID="IntegerNumber">
        <rdfs:subClassOf rdf:resource="#ArithmeticNumber"/>
       <owl:disjointWith rdf:resource="#MultidimensionalNumber"/>
        <owl:disjointWith rdf:resource="#RealNumber"/>
        <rdfs:comment>
            DEFINITION An IntegerNumber is an ArithmeticNumber that is an integer number.
        </rdfs:comment>
        <rdfs:comment>
            NOTE IntegerNumber is not a subtype of RealNumber. The members of
            IntegerNumber are part of a different continuum from the members of
            RealNumber, but are isomorphic to a subset of it.
        </rdfs:comment>
        <rdfs:comment>
            EXAMPLE '1', '2', and '10' are instances of IntegerNumber .
        </rdfs:comment>
    </owl:Class>

    <owl:Class rdf:ID="IntendedRoleAndDomain">
        <rdf:type rdf:resource="#ClassOfIntendedRoleAndDomain"/>
        <rdfs:subClassOf rdf:resource="#Relationship"/>
        <owl:disjointWith rdf:resource="#InvolvementByReference"/>
        <owl:disjointWith rdf:resource="#LifecycleStage"/>
        <owl:disjointWith rdf:resource="#OtherRelationship"/>
        <owl:disjointWith rdf:resource="#PossibleRoleAndDomain"/>
        <owl:disjointWith rdf:resource="#Recognition"/>
        <owl:disjointWith rdf:resource="#RelativeLocation"/>
        <owl:disjointWith rdf:resource="#RepresentationOfThing"/>
        <owl:disjointWith rdf:resource="#ResponsibilityForRepresentation"/>
        <owl:disjointWith rdf:resource="#TemporalSequence"/>
        <owl:disjointWith rdf:resource="#UsageOfRepresentation"/>
        <rdfs:subClassOf>
            <owl:Restriction>
                <owl:onProperty rdf:resource="#played"/>
                <owl:allValuesFrom rdf:resource="#RoleAndDomain"/>
            </owl:Restriction>
        </rdfs:subClassOf>
        <rdfs:subClassOf>
            <owl:Restriction>
                <owl:onProperty rdf:resource="#player"/>
                <owl:allValuesFrom rdf:resource="#PossibleIndividual"/>
            </owl:Restriction>
        </rdfs:subClassOf>
        <rdfs:comment>
            DEFINITION An IntendedRoleAndDomain is a Relationship that indicates the
            RoleAndDomain some temporal part of the PossibleIndividual is intended to
            take with respect to some Activity .
        </rdfs:comment>
        <rdfs:comment>
            EXAMPLE The Relationship between a PossibleIndividual, that is classified as
            'pump', and the RoleAndDomain of 'performer and pumping' that it is intended
            to play is an instance of IntendedRoleAndDomain .
        </rdfs:comment>
    </owl:Class>

    <owl:Class rdf:ID="IntersectionOfSetOfClass">
        <rdfs:subClassOf rdf:resource="#FunctionalMapping"/>
        <owl:disjointWith rdf:resource="#UnionOfSetOfClass"/>
        <owl:disjointWith rdf:resource="#PropertyQuantification"/>
        <rdfs:subClassOf>
            <owl:Restriction>
                <owl:onProperty rdf:resource="#input"/>
                <owl:allValuesFrom rdf:resource="#EnumeratedSetOfClass"/>
            </owl:Restriction>
        </rdfs:subClassOf>
        <rdfs:subClassOf>
            <owl:Restriction>
                <owl:onProperty rdf:resource="#result"/>
                <owl:allValuesFrom rdf:resource="#Class"/>
            </owl:Restriction>
        </rdfs:subClassOf>
        <rdfs:comment>
            DEFINITION An IntersectionOfSetOfClass is a FunctionalMapping that indicates
            that the result Class consists of those members of the members of the classes
            EnumeratedSetOfClass that are common to each Class .
        </rdfs:comment>
        <rdfs:comment>
            EXAMPLE The intersection of the EnumeratedSetOfClass
            {{A,B,C},{B,C,D},{C,D,E}} is {C}.
        </rdfs:comment>
    </owl:Class>

    <owl:Class rdf:ID="InvolvementByReference">
        <rdf:type rdf:resource="#ClassOfInvolvementByReference"/>
        <rdfs:subClassOf rdf:resource="#Relationship"/>
        <owl:disjointWith rdf:resource="#LifecycleStage"/>
        <owl:disjointWith rdf:resource="#OtherRelationship"/>
        <owl:disjointWith rdf:resource="#PossibleRoleAndDomain"/>
        <owl:disjointWith rdf:resource="#Recognition"/>
        <owl:disjointWith rdf:resource="#RelativeLocation"/>
        <owl:disjointWith rdf:resource="#RepresentationOfThing"/>
        <owl:disjointWith rdf:resource="#ResponsibilityForRepresentation"/>
        <owl:disjointWith rdf:resource="#TemporalSequence"/>
        <owl:disjointWith rdf:resource="#UsageOfRepresentation"/>
        <rdfs:subClassOf>
            <owl:Restriction>
                <owl:onProperty rdf:resource="#involved"/>
                <owl:allValuesFrom rdf:resource="#Thing"/>
            </owl:Restriction>
        </rdfs:subClassOf>
        <rdfs:subClassOf>
            <owl:Restriction>
                <owl:onProperty rdf:resource="#involver"/>
                <owl:allValuesFrom rdf:resource="#Activity"/>
            </owl:Restriction>
        </rdfs:subClassOf>
        <rdfs:comment>
            DEFINITION An InvolvementByReference is a Relationship that indicates that a
            Thing is referred to in an Activity .
        </rdfs:comment>
        <rdfs:comment>
            NOTE This entity type is for involvements that are not direct Participation
            of a Thing , such as involvement of a Class, or of a historical or future
            temporal part of a PossibleIndividual .
        </rdfs:comment>
        <rdfs:comment>
            EXAMPLE A conversation that refers to the Roman Empire is an Activity that
            relates to the Roman Empire by an InvolvementByReference .
        </rdfs:comment>
        <rdfs:comment>
            EXAMPLE The use of the ASME Boiler and Pressure Vessel Code for the Activity
            'design Boiler E-106' is represented by an instance of InvolvementByReference
            between that ClassOfInformationRepresentation and that Activity .
        </rdfs:comment>
    </owl:Class>

    <owl:Class rdf:ID="Language">
        <rdfs:subClassOf rdf:resource="#ClassOfClassOfInformationRepresentation"/>
        <owl:disjointWith rdf:resource="#RepresentationForm"/>
        <rdfs:comment>
            DEFINITION A Language is a ClassOfClassOfInformationRepresentation whose
            members are all the information representations made in the language.
        </rdfs:comment>
        <rdfs:comment>
            EXAMPLE English, French, C++ and Java can be represented by instances of
            Language .
        </rdfs:comment>
    </owl:Class>

    <owl:Class rdf:ID="LeftNamespace">
        <rdf:type rdf:resource="#ClassOfLeftNamespace"/>
        <rdfs:subClassOf rdf:resource="#Namespace"/>
        <owl:disjointWith rdf:resource="#RightNamespace"/>
        <rdfs:comment>
            DEFINITION A LeftNamespace is a Namespace where the classOfPart is the left
            part of the classOfWhole .
        </rdfs:comment>
        <rdfs:comment>
            EXAMPLE Where WC1: is the Namespace in WC1:1234, it is a LeftNamespace .
        </rdfs:comment>
    </owl:Class>

    <owl:Class rdf:ID="LifecycleStage">
        <rdf:type rdf:resource="#ClassOfLifecycleStage"/>
        <rdfs:subClassOf rdf:resource="#Relationship"/>
        <owl:disjointWith rdf:resource="#OtherRelationship"/>
        <owl:disjointWith rdf:resource="#PossibleRoleAndDomain"/>
        <owl:disjointWith rdf:resource="#Recognition"/>
        <owl:disjointWith rdf:resource="#RelativeLocation"/>
        <owl:disjointWith rdf:resource="#RepresentationOfThing"/>
        <owl:disjointWith rdf:resource="#ResponsibilityForRepresentation"/>
        <owl:disjointWith rdf:resource="#TemporalSequence"/>
        <owl:disjointWith rdf:resource="#UsageOfRepresentation"/>
        <rdfs:subClassOf>
            <owl:Restriction>
                <owl:onProperty rdf:resource="#interest"/>
                <owl:allValuesFrom rdf:resource="#PossibleIndividual"/>
            </owl:Restriction>
        </rdfs:subClassOf>
        <rdfs:subClassOf>
            <owl:Restriction>
                <owl:onProperty rdf:resource="#interested"/>
                <owl:allValuesFrom rdf:resource="#PossibleIndividual"/>
            </owl:Restriction>
        </rdfs:subClassOf>
        <rdfs:comment>
            DEFINITION A LifecycleStage is a Relationship that indicates the interest
            that a PossibleIndividual has in some PossibleIndividual .
        </rdfs:comment>
        <rdfs:comment>
            EXAMPLE The relation that links a possible building to a temporal part of the
            XYZ Corp. can be represented by an instance of LifecycleStage. The nature of
            that LifecycleStage (e.g. 'planned') can be expressed by classifying with the
            applicable ClassOfLifecycleStage .
        </rdfs:comment>
    </owl:Class>

    <owl:Class rdf:ID="LowerBoundOfNumberRange">
        <rdfs:subClassOf rdf:resource="#Relationship"/>
        <rdfs:subClassOf>
            <owl:Restriction>
                <owl:onProperty rdf:resource="#lowestNumber"/>
                <owl:allValuesFrom rdf:resource="#ArithmeticNumber"/>
            </owl:Restriction>
        </rdfs:subClassOf>
        <rdfs:subClassOf>
            <owl:Restriction>
                <owl:onProperty rdf:resource="#range"/>
                <owl:allValuesFrom rdf:resource="#NumberRange"/>
            </owl:Restriction>
        </rdfs:subClassOf>
        <rdfs:comment>
            DEFINITION A LowerBoundOfNumberRange is a Classification that indicates an
            ArithmeticNumber is the lowest value in a NumberRange .
        </rdfs:comment>
        <rdfs:comment>
            EXAMPLE The instance of RealNumber that is represented by the instance of
            ExpressReal '3.1' has a LowerBoundOfNumberRange relationship with the
            instance of NumberRange'[3.1 to 5.3]'.
        </rdfs:comment>
    </owl:Class>

    <owl:Class rdf:ID="LowerBoundOfPropertyRange">
        <rdfs:subClassOf rdf:resource="#Relationship"/>
        <rdfs:subClassOf>
            <owl:Restriction>
                <owl:onProperty rdf:resource="#lowestProperty"/>
                <owl:allValuesFrom rdf:resource="#Property"/>
            </owl:Restriction>
        </rdfs:subClassOf>
        <rdfs:subClassOf>
            <owl:Restriction>
                <owl:onProperty rdf:resource="#range"/>
                <owl:allValuesFrom rdf:resource="#PropertyRange"/>
            </owl:Restriction>
        </rdfs:subClassOf>
        <rdfs:comment>
            DEFINITION A LowerBoundOfPropertyRange is a Classification that indicates
            that a Property is the lower bound of a PropertyRange .
        </rdfs:comment>
        <rdfs:comment>
            EXAMPLE The instance of Property that is represented by the instance of
            ExpressReal '-10' has a LowerBoundOfPropertyRange relationship with the
            instance of PropertyRange'[-10 to +20 degrees Celsius]'.
        </rdfs:comment>
    </owl:Class>

    <owl:Class rdf:ID="MaterializedPhysicalObject">
        <rdfs:subClassOf rdf:resource="#PhysicalObject"/>
        <rdfs:comment>
            DEFINITION A MaterializedPhysicalObject is a PhysicalObject that has matter
            and/or energy continuity as its basis for identity. Matter or energy
            continuity requires some matter or energy to be common to adjacent temporal
            parts of the MaterializedPhysicalObject . Replacement of some components from
            time to time does not create a new identity.
        </rdfs:comment>
        <rdfs:comment>
            EXAMPLE The shell and tube heat exchanger with manufacture's number ES/1234
            can be represented by an instance of MaterializedPhysicalObject .
        </rdfs:comment>
    </owl:Class>

    <owl:Class rdf:ID="MultidimensionalNumber">
        <rdfs:subClassOf rdf:resource="#ArithmeticNumber"/>
        <rdfs:subClassOf rdf:resource="#MultidimensionalObject"/>
        <owl:disjointWith rdf:resource="#MultidimensionalNumberSpace"/>
        <owl:disjointWith rdf:resource="#MultidimensionalProperty"/>
        <owl:disjointWith rdf:resource="#MultidimensionalPropertySpace"/>
        <owl:disjointWith rdf:resource="#MultidimensionalScale"/>
        <owl:disjointWith rdf:resource="#RealNumber"/>
        <rdfs:comment>
            DEFINITION A MultidimensionalNumber is an ArithmeticNumber that is also a
            MultidimensionalObject .
        </rdfs:comment>
        <rdfs:comment>
            EXAMPLE '[3.2, 5.4, 55.6]' is a MultidimensionalNumber.
        </rdfs:comment>
    </owl:Class>

    <owl:Class rdf:ID="MultidimensionalNumberSpace">
        <rdfs:subClassOf rdf:resource="#NumberSpace"/>
        <rdfs:subClassOf rdf:resource="#MultidimensionalObject"/>
        <owl:disjointWith rdf:resource="#MultidimensionalProperty"/>
        <owl:disjointWith rdf:resource="#MultidimensionalPropertySpace"/>
        <owl:disjointWith rdf:resource="#MultidimensionalScale"/>
        <owl:disjointWith rdf:resource="#NumberRange"/>
        <rdfs:comment>
            DEFINITION A MultidimensionalNumberSpace is a NumberSpace and a
            MultidimensionalObject .
        </rdfs:comment>
        <rdfs:comment>
            EXAMPLE R3, the space defined as being all the triples of real numbers
            (e.g. '[1.0, 2.1, 5.4]'), is a MultidimensionalNumberSpace .
        </rdfs:comment>
    </owl:Class>

    <owl:Class rdf:ID="MultidimensionalObject">
        <rdf:type rdf:resource="#ClassOfMultidimensionalObject"/>
        <rdfs:subClassOf rdf:resource="#AbstractObject"/>
        <owl:unionOf rdf:parseType="Collection">  
            <owl:Class rdf:about="#MultidimensionalNumber"/>  
            <owl:Class rdf:about="#MultidimensionalNumberSpace"/>  
            <owl:Class rdf:about="#MultidimensionalProperty"/>  
            <owl:Class rdf:about="#MultidimensionalPropertySpace"/>  
            <owl:Class rdf:about="#MultidimensionalScale"/>  
        </owl:unionOf>
        <rdfs:subClassOf>
            <owl:Restriction>
                <owl:onProperty rdf:resource="#elements"/>
                <owl:allValuesFrom rdf:resource="#Thing"/>
            </owl:Restriction>
        </rdfs:subClassOf>
        <rdfs:subClassOf>
            <owl:Restriction>
                <owl:onProperty rdf:resource="#position"/>
                <owl:allValuesFrom rdf:datatype="http://www.w3.org/2001/XMLSchema#nonNegativeInteger"/>
            </owl:Restriction>
        </rdfs:subClassOf>
        <rdfs:comment>
            DEFINITION A MultidimensionalObject is an AbstractObject that is an
            ordered list of Thing . The significance of the MultidimensionalObject is
            determined by being a member of a ClassOfMultidimensionalObject that
            indicates the role played by each of its elements.
        </rdfs:comment>
        <rdfs:comment>
            NOTE The MultidimensionalObject [A,B,C] is different from [B,C,A].
        </rdfs:comment>
        <rdfs:comment>
            EXAMPLE '[32, 1.8, 20]' is a MultidimensionalObject that may be specified to
            be the input parameters for the function y=a+bx to convert 20 Celsius to
            Fahrenheit.
        </rdfs:comment>
    </owl:Class>

    <owl:Class rdf:ID="MultidimensionalProperty">
        <rdfs:subClassOf rdf:resource="#Property"/>
        <rdfs:subClassOf rdf:resource="#MultidimensionalObject"/>
        <owl:disjointWith rdf:resource="#MultidimensionalPropertySpace"/>
        <owl:disjointWith rdf:resource="#MultidimensionalScale"/>
        <rdfs:comment>
            DEFINITION A MultidimensionalProperty is a Property that is also a
            MultidimensionalObject .
        </rdfs:comment>
        <rdfs:comment>
            EXAMPLE A pump flow head characteristic is a MultidimensionalProperty. It
            consists of a continuum of Q, H property pairs, where Q is the flow rate and
            H is the flowing head difference. Each pair of properties Qa and Ha, where Qa
            is a particular flow rate and Ha a particular head, is a multidimensional
            property [Qa, Ha].
        </rdfs:comment>
    </owl:Class>

    <owl:Class rdf:ID="MultidimensionalPropertySpace">
        <rdfs:subClassOf rdf:resource="#PropertySpace"/>
        <rdfs:subClassOf rdf:resource="#MultidimensionalObject"/>
        <owl:disjointWith rdf:resource="#MultidimensionalScale"/>
        <rdfs:comment>
            DEFINITION A MultidimensionalPropertySpace is a PropertySpace and a
            MultidimensionalObject whose members are instances of Property each of which
            maps to more than one number. Each Property will consist of elements of the
            same property dimensions.
        </rdfs:comment>
        <rdfs:comment>
            EXAMPLE A pump performance curve of flowrate and differential head is a
            MultidimensionalPropertySpace .
        </rdfs:comment>
    </owl:Class>

    <owl:Class rdf:ID="MultidimensionalScale">
        <rdfs:subClassOf rdf:resource="#Scale"/>
        <rdfs:subClassOf rdf:resource="#MultidimensionalObject"/>
        <rdfs:subClassOf>
            <owl:Restriction>
                <owl:onProperty rdf:resource="#codomain"/>
                <owl:allValuesFrom rdf:resource="#NumberSpace"/>
            </owl:Restriction>
        </rdfs:subClassOf>
        <rdfs:subClassOf>
            <owl:Restriction>
                <owl:onProperty rdf:resource="#domain"/>
                <owl:allValuesFrom rdf:resource="#PropertySpace"/>
            </owl:Restriction>
        </rdfs:subClassOf>
        <rdfs:comment>
            DEFINITION A MultidimensionalScale is a Scale that is also a
            MultidimensionalObject .
        </rdfs:comment>
        <rdfs:comment>
            EXAMPLE A '[Celsius, seconds]' scale is a MultidimensionalScale on which
            temperature variation over time can be plotted.
        </rdfs:comment>
    </owl:Class>

    <owl:Class rdf:ID="Namespace">
        <rdf:type rdf:resource="#ClassOfNamespace"/>
        <rdfs:subClassOf rdf:resource="#ClassOfArrangementOfIndividual"/>
        <owl:unionOf rdf:parseType="Collection">  
            <owl:Class rdf:about="#LeftNamespace"/>  
            <owl:Class rdf:about="#RightNamespace"/>  
        </owl:unionOf>
        <rdfs:subClassOf>
            <owl:Restriction>
                <owl:onProperty rdf:resource="#classOfPart"/>
                <owl:allValuesFrom rdf:resource="#ClassOfInformationRepresentation"/>
            </owl:Restriction>
        </rdfs:subClassOf>
        <rdfs:subClassOf>
            <owl:Restriction>
                <owl:onProperty rdf:resource="#classOfWhole"/>
                <owl:allValuesFrom rdf:resource="#ClassOfInformationRepresentation"/>
            </owl:Restriction>
        </rdfs:subClassOf>
        <rdfs:comment>
            DEFINITION A Namespace is a ClassOfArrangementOfIndividual where the
            classOfWhole and classOfPart are members of ClassOfInformationRepresentation
            and the part is the most significant part of the whole that is the namespace.
        </rdfs:comment>
        <rdfs:comment>
            EXAMPLE The string 'owl:' is the (left_)namespace in the name owl:Class .
        </rdfs:comment>
    </owl:Class>

    <owl:Class rdf:ID="NumberRange">
        <rdfs:subClassOf rdf:resource="#NumberSpace"/>
        <rdfs:comment>
            DEFINITION A NumberRange is a one-dimensional NumberSpace .
        </rdfs:comment>
        <rdfs:comment>
            EXAMPLE The NumberSpace -273.1 to +infinity is a NumberRange.
        </rdfs:comment>
    </owl:Class>

    <owl:Class rdf:ID="NumberSpace">
        <rdfs:subClassOf rdf:resource="#ClassOfNumber"/>
        <owl:unionOf rdf:parseType="Collection">  
            <owl:Class rdf:about="#MultidimensionalNumberSpace"/>  
            <owl:Class rdf:about="#NumberRange"/>  
        </owl:unionOf>
        <rdfs:comment>
            DEFINITION A NumberSpace is a ClassOfNumber that is a continuum.
        </rdfs:comment>
        <rdfs:comment>
            EXAMPLE The integers from 1 to 5 and the reals from 0.000 to 1.000 are
            examples of NumberSpace.
        </rdfs:comment>
    </owl:Class>

    <owl:Class rdf:ID="OtherRelationship">
        <rdf:type rdf:resource="#ClassOfClassOfRelationshipWithSignature"/>
        <rdfs:subClassOf rdf:resource="#Relationship"/>
        <owl:disjointWith rdf:resource="#PossibleRoleAndDomain"/>
        <owl:disjointWith rdf:resource="#Recognition"/>
        <owl:disjointWith rdf:resource="#RelativeLocation"/>
        <owl:disjointWith rdf:resource="#RepresentationOfThing"/>
        <owl:disjointWith rdf:resource="#ResponsibilityForRepresentation"/>
        <owl:disjointWith rdf:resource="#TemporalSequence"/>
        <owl:disjointWith rdf:resource="#UsageOfRepresentation"/>
        <rdfs:subClassOf>
            <owl:Restriction>
                <owl:onProperty rdf:resource="#end1"/>
                <owl:allValuesFrom rdf:resource="#Thing"/>
            </owl:Restriction>
        </rdfs:subClassOf>
        <rdfs:subClassOf>
            <owl:Restriction>
                <owl:onProperty rdf:resource="#end2"/>
                <owl:allValuesFrom rdf:resource="#Thing"/>
            </owl:Restriction>
        </rdfs:subClassOf>
        <rdfs:comment>
            DEFINITION An OtherRelationship is a Relationship that is not a member of any
            of the other explicit subtypes of Relationship . The meaning of an
            OtherRelationship is specified by a Classification by an instance of
            ClassOfRelationshipWithSignature .
        </rdfs:comment>
        <rdfs:comment>
            NOTE The RoleAndDomain for the end1 and end2 is given by the classOfEnd1 and
            classOfEnd2 respectively for the ClassOfRelationshipWithSignature that
            classifies the OtherRelationship .
            Where the ClassOfRelationshipWithSignature is also a
            ClassOfRelationshipWithRelatedEnd1 or a ClassOfRelationshipWithRelatedEnd2
            then the end1 or end2 respectively of the OtherRelationship shall take the
            value specified by the related instance of rdf:Property.
        </rdfs:comment>
        <rdfs:comment>
            EXAMPLE The Relationship that indicates that a particular car is manufactured
            by Ford can be represented by an instance of OtherRelationship.
        </rdfs:comment>
    </owl:Class>

    <owl:Class rdf:ID="ParticipatingRoleAndDomain">
        <rdfs:subClassOf rdf:resource="#RoleAndDomain"/>
        <rdfs:subClassOf rdf:resource="#ClassOfIndividual"/>
        <rdfs:comment>
            DEFINITION A ParticipatingRoleAndDomain is a RoleAndDomain that is also a
            ClassOfIndividual that indicates a participating role in an Activity .
        </rdfs:comment>
        <rdfs:comment>
            EXAMPLE Performer and pumper are examples of ParticipatingRoleAndDomain .
        </rdfs:comment>
    </owl:Class>

    <owl:Class rdf:ID="Participation">
        <rdf:type rdf:resource="#ClassOfParticipation"/>
        <rdfs:subClassOf rdf:resource="#CompositionOfIndividual"/>
        <owl:disjointWith rdf:resource="#TemporalBounding"/>
        <owl:disjointWith rdf:resource="#TemporalWholePart"/>
        <rdfs:subClassOf>
            <owl:Restriction>
                <owl:onProperty rdf:resource="#whole"/>
                <owl:allValuesFrom rdf:resource="#Activity"/>
            </owl:Restriction>
        </rdfs:subClassOf>
        <rdfs:comment>
            DEFINITION A Participation is a CompositionOfIndividual that indicates that
            a PossibleIndividual is a participant in an Activity .
        </rdfs:comment>
        <rdfs:comment>
            NOTE The PossibleIndividual that is the part in the Participation is may be a
            temporal part of a WholeLifeIndividual that is classified by the
            RoleAndDomain that indicates the role it plays in the Activity .
        </rdfs:comment>
        <rdfs:comment>
            EXAMPLE The relationship between the temporal part of P1234 that performs the
            discharge of the Motor Vessel Murex on 2nd December 2002, and the activity
            that is that discharge of that vessel is a Participation.
        </rdfs:comment>
    </owl:Class>

    <owl:Class rdf:ID="PeriodInTime">
        <rdf:type rdf:resource="#ClassOfPeriodInTime"/>
        <rdfs:subClassOf rdf:resource="#PossibleIndividual"/>
        <rdfs:comment>
            DEFINITION A PeriodInTime is a PossibleIndividual that is all space for
            part of time - a temporal part of the universe.
        </rdfs:comment>
        <rdfs:comment>
            EXAMPLE July 2000 is an instance of PeriodInTime.
        </rdfs:comment>
        <rdfs:comment>
            EXAMPLE The period described by UTC 2000-11-21T06:00 to
            UTC 2000-11-21T11:53 is an instance of PeriodInTime compliant with ISO8601.
        </rdfs:comment>
    </owl:Class>

    <owl:Class rdf:ID="Phase">
        <rdfs:subClassOf rdf:resource="#ClassOfArrangedIndividual"/>
        <rdfs:comment>
            DEFINITION A Phase is a ClassOfArrangedIndividual based on the nature of the
            boundary behaviour of material resulting from its atomic and molecular
            bonding.
        </rdfs:comment>
        <rdfs:comment>
            NOTE Phase excludes types of internal structure such as crystalline.
        </rdfs:comment>
        <rdfs:comment>
            EXAMPLE The classes known as 'liquid' and 'solid' can be represented by
            instances of Phase .
        </rdfs:comment>
    </owl:Class>

    <owl:Class rdf:ID="PhysicalObject">
        <rdfs:subClassOf rdf:resource="#PossibleIndividual"/>
        <owl:intersectionOf rdf:parseType="Collection">  
            <owl:Class rdf:about="#FunctionalPhysicalObject"/>  
            <owl:Class rdf:about="#MaterializedPhysicalObject"/>  
            <owl:Class rdf:about="#SpatialLocation"/>  
            <owl:Class rdf:about="#Stream"/>  
        </owl:intersectionOf>
        <rdfs:comment>
            DEFINITION A PhysicalObject is a PossibleIndividual that is a distribution
            of matter, energy, or both.
        </rdfs:comment>
        <rdfs:comment>
            EXAMPLE A piece of metal is a PhysicalObject .
        </rdfs:comment>
        <rdfs:comment>
            EXAMPLE A tree is a PhysicalObject .
        </rdfs:comment>
        <rdfs:comment>
            EXAMPLE The thing identified by tag P101 is a PhysicalObject .
        </rdfs:comment>
        <rdfs:comment>
            EXAMPLE A light beam is a PhysicalObject .
        </rdfs:comment>
        <rdfs:comment>
            EXAMPLE A tank that is built and dismantled on site is both a
            MaterializedPhysicalObject and a FunctionalPhysicalObject .
        </rdfs:comment>
        <rdfs:comment>
            EXAMPLE John Doe is a PhysicalObject .
        </rdfs:comment>
        <rdfs:comment>
            EXAMPLE The XYZ Corporation is a PhysicalObject .
        </rdfs:comment>
    </owl:Class>

    <owl:Class rdf:ID="PointInTime">
        <rdf:type rdf:resource="#ClassOfPointInTime"/>
        <rdfs:subClassOf rdf:resource="#Event"/>
        <rdfs:comment>
            DEFINITION A PointInTime is an Event that is the whole space extension with
            zero extent in time.
        </rdfs:comment>
        <rdfs:comment>
            NOTE In using this part of ISO15926, a PointInTime should be represented by a
            RepresentationOfGregorianDateAndUtcTime .
        </rdfs:comment>
        <rdfs:comment>
            EXAMPLE The time known as UTC 1999-05-13T16:31:23.56 is a PointInTime .
        </rdfs:comment>
    </owl:Class>

    <owl:Class rdf:ID="PossibleIndividual">
        <rdf:type rdf:resource="#ClassOfIndividual"/>
        <rdfs:subClassOf rdf:resource="#Thing"/>
        <owl:intersectionOf rdf:parseType="Collection">  
            <owl:Class rdf:about="#Activity"/>  
            <owl:Class rdf:about="#ActualIndividual"/>  
            <owl:Class rdf:about="#ArrangedIndividual"/>  
            <owl:Class rdf:about="#Event"/>  
            <owl:Class rdf:about="#PeriodInTime"/>  
            <owl:Class rdf:about="#PhysicalObject"/>  
            <owl:Class rdf:about="#WholeLifeIndividual"/>  
        </owl:intersectionOf>
        <rdfs:comment>
            DEFINITION A PossibleIndividual is a Thing that exists in space and time.
            This includes:
            - things where any of the space time dimensions are vanishingly small;
            - those that are either all space for any time, or all time and any space;
            - the entirety of all space time;
            - things that actually exist, or have existed;
            - things that are fictional or conjectured and possibly exist in the past,
              present or future;
            - temporal parts (states) of other individuals;
            - things that have a specific position, but zero extent in one or more
              dimensions, such as points, lines, and surfaces.
            In this context existence is based upon being imaginable within some
            consistent logic, including actual, hypothetical, planned, expected, or
            required individuals.
        </rdfs:comment>
        <rdfs:comment>
            EXAMPLE The pump with serial number ABC123, Battersea Power Station, Sir
            Joseph Whitworth, Shakespeare, and the starship "Enterprise" can be
            represented by instances of PossibleIndividual .
        </rdfs:comment>
    </owl:Class>

    <owl:Class rdf:ID="PossibleRoleAndDomain">
        <rdf:type rdf:resource="#ClassOfPossibleRoleAndDomain"/>
        <rdfs:subClassOf rdf:resource="#Relationship"/>
        <owl:disjointWith rdf:resource="#Recognition"/>
        <owl:disjointWith rdf:resource="#RelativeLocation"/>
        <owl:disjointWith rdf:resource="#RepresentationOfThing"/>
        <owl:disjointWith rdf:resource="#ResponsibilityForRepresentation"/>
        <owl:disjointWith rdf:resource="#TemporalSequence"/>
        <owl:disjointWith rdf:resource="#UsageOfRepresentation"/>
        <rdfs:subClassOf>
            <owl:Restriction>
                <owl:onProperty rdf:resource="#played"/>
                <owl:allValuesFrom rdf:resource="#RoleAndDomain"/>
            </owl:Restriction>
        </rdfs:subClassOf>
        <rdfs:subClassOf>
            <owl:Restriction>
                <owl:onProperty rdf:resource="#player"/>
                <owl:allValuesFrom rdf:resource="#PossibleIndividual"/>
            </owl:Restriction>
        </rdfs:subClassOf>
        <rdfs:comment>
            DEFINITION A PossibleRoleAndDomain is a Relationship that indicates that a
            player PossibleIndividual can possibly play the played RoleAndDomain .
        </rdfs:comment>
        <rdfs:comment>
            EXAMPLE 'Acting as an anchor' is a PossibleRoleAndDomain for pump 1234.
        </rdfs:comment>
    </owl:Class>

    <owl:Class rdf:ID="Property">
        <rdf:type rdf:resource="#ClassOfProperty"/>
        <rdfs:subClassOf rdf:resource="#ClassOfIndividual"/>
        <owl:intersectionOf rdf:parseType="Collection">  
            <owl:Class rdf:about="#MultidimensionalProperty"/>  
            <owl:Class rdf:about="#Shape"/>  
        </owl:intersectionOf>
        <owl:disjointWith rdf:resource="#Status"/>
        <rdfs:comment>
            DEFINITION A Property is a ClassOfIndividual that is a member of a continuum
            of a ClassOfProperty . The Property may be quantified by mapping to a number
            on a scale.
        </rdfs:comment>
        <rdfs:comment>
            NOTE A member of a Property is a PossibleIndividual that has the same degree
            or magnitude of the quality or characteristic represented by the Property as
            other members.
        </rdfs:comment>
        <rdfs:comment>
            NOTE The types of characteristic or quality, such as temperature or density,
            are instances of ClassOfProperty .
        </rdfs:comment>
        <rdfs:comment>
            NOTE Duplicate properties (e.g. that map to the same number on the same
            scale) should not be created within the same data store.
        </rdfs:comment>
        <rdfs:comment>
            NOTE The owl:Class rdf:ID="Property" defined here is different from
            rdf:Property
        </rdfs:comment>
        <rdfs:comment>
            EXAMPLE A particular degree of hotness can be represented as an instance of
            Property .
        </rdfs:comment>
    </owl:Class>

    <owl:Class rdf:ID="PropertyForShapeDimension">
        <rdfs:subClassOf rdf:resource="#ClassOfRelationship"/>
        <rdfs:subClassOf>
            <owl:Restriction>
                <owl:onProperty rdf:resource="#property"/>
                <owl:allValuesFrom rdf:resource="#Property"/>
            </owl:Restriction>
        </rdfs:subClassOf>
        <rdfs:subClassOf>
            <owl:Restriction>
                <owl:onProperty rdf:resource="#shapeDimension"/>
                <owl:allValuesFrom rdf:resource="#ShapeDimension"/>
            </owl:Restriction>
        </rdfs:subClassOf>
        <rdfs:comment>
            DEFINITION A PropertyForShapeDimension is a ClassOfRelationship that
            indicates that the members of the ShapeDimension are of the Property .
        </rdfs:comment>
        <rdfs:comment>
            EXAMPLE The ShapeDimension '10m diameter' is related to the Property
            '10m length' by means of an instance of PropertyForShapeDimension .
        </rdfs:comment>
    </owl:Class>

    <owl:Class rdf:ID="PropertyQuantification">
        <rdf:type rdf:resource="#Scale"/>
        <rdfs:subClassOf rdf:resource="#FunctionalMapping"/>
        <rdfs:comment>
            DEFINITION A PropertyQuantification is a FunctionalMapping whose members map
            a Property to an ArithmeticNumber .
        </rdfs:comment>
        <rdfs:comment>
            NOTE The actual representation of the number is done by linking the
            ArithmeticNumber to a  ClassOfExpressInformationRepresentation via a
            ClassOfRepresentationOfThing .
        </rdfs:comment>
        <rdfs:comment>
            NOTE The unit or scale of the quantification is given by classifying the
            PropertyQuantification by a Scale .
        </rdfs:comment>
        <rdfs:comment>
            EXAMPLE The link that maps a particular mass to the RealNumber '4.2' can be
            represented by an instance of PropertyQuantification .
        </rdfs:comment>
    </owl:Class>

    <owl:Class rdf:ID="PropertyRange">
        <rdfs:subClassOf rdf:resource="#PropertySpace"/>
        <rdfs:comment>
            DEFINITION A PropertyRange is a PropertySpace that is a continuous subset of
            a SinglePropertyDimension .
        </rdfs:comment>
        <rdfs:comment>
            EXAMPLE '[-10C to +20C]' is a PropertyRange of temperature.
        </rdfs:comment>
    </owl:Class>

    <owl:Class rdf:ID="PropertySpace">
        <rdf:type rdf:resource="#ClassOfPropertySpace"/>
        <rdfs:subClassOf rdf:resource="#ClassOfProperty"/>
        <owl:intersectionOf rdf:parseType="Collection">  
            <owl:Class rdf:about="#ClassOfShape"/>  
            <owl:Class rdf:about="#MultidimensionalPropertySpace"/>  
            <owl:Class rdf:about="#PropertyRange"/>  
            <owl:Class rdf:about="#SinglePropertyDimension"/>  
        </owl:intersectionOf>
        <rdfs:comment>
            DEFINITION A PropertySpace is a ClassOfProperty whose members are a coherent
            continuum of Property .
        </rdfs:comment>
        <rdfs:comment>
            EXAMPLE The set of temperature properties, known as temperature, is a
            PropertySpace.
        </rdfs:comment>
        <rdfs:comment>
            EXAMPLE The members of the 'pressure' and 'flow rate' ClassOfProperty that
            fall on a particular pump curve is a PropertySpace .
        </rdfs:comment>
    </owl:Class>

    <owl:Class rdf:ID="PropertySpaceForClassOfShapeDimension">
        <rdfs:subClassOf rdf:resource="#ClassOfClassOfRelationship"/>
        <rdfs:subClassOf>
            <owl:Restriction>
                <owl:onProperty rdf:resource="#classOfShapeDimension"/>
                <owl:allValuesFrom rdf:resource="#ClassOfShapeDimension"/>
            </owl:Restriction>
        </rdfs:subClassOf>
        <rdfs:subClassOf>
            <owl:Restriction>
                <owl:onProperty rdf:resource="#propertySpace"/>
                <owl:allValuesFrom rdf:resource="#PropertySpace"/>
            </owl:Restriction>
        </rdfs:subClassOf>
        <rdfs:comment>
            DEFINITION A PropertySpaceForClassOfShapeDimension is a
            ClassOfClassOfRelationship that indicates the PropertySpace that a
            ClassOfShapeDimension is from.
        </rdfs:comment>
        <rdfs:comment>
            EXAMPLE The ClassOfShapeDimension 'diameter' is linked to the PropertySpace
            'length' by an instance of PropertySpaceForClassOfShapeDimension .
        </rdfs:comment>
    </owl:Class>

    <owl:Class rdf:ID="RealNumber">
        <rdfs:subClassOf rdf:resource="#ArithmeticNumber"/>
        <rdfs:comment>
            DEFINITION A RealNumber is an ArithmeticNumber that is a real number.
        </rdfs:comment>
        <rdfs:comment>
            EXAMPLE '3.2146' is a representation of a RealNumber .
        </rdfs:comment>
    </owl:Class>

    <owl:Class rdf:ID="Recognition">
        <rdf:type rdf:resource="#ClassOfRecognition"/>
        <rdfs:subClassOf rdf:resource="#Relationship"/>
        <owl:disjointWith rdf:resource="#RelativeLocation"/>
        <owl:disjointWith rdf:resource="#RepresentationOfThing"/>
        <owl:disjointWith rdf:resource="#ResponsibilityForRepresentation"/>
        <owl:disjointWith rdf:resource="#TemporalSequence"/>
        <owl:disjointWith rdf:resource="#UsageOfRepresentation"/>
        <rdfs:subClassOf>
            <owl:Restriction>
                <owl:onProperty rdf:resource="#recognized"/>
                <owl:allValuesFrom rdf:resource="#Thing"/>
            </owl:Restriction>
        </rdfs:subClassOf>
        <rdfs:subClassOf>
            <owl:Restriction>
                <owl:onProperty rdf:resource="#recognizing"/>
                <owl:allValuesFrom rdf:resource="#Activity"/>
            </owl:Restriction>
        </rdfs:subClassOf>
        <rdfs:comment>
            DEFINITION A Recognition is a Relationship that indicates that a Thing is
            recognized through an Activity .
        </rdfs:comment>
        <rdfs:comment>
            EXAMPLE Measurement activity #358 recognized that the room was a member of
            the 20 Celsius Property .
        </rdfs:comment>
    </owl:Class>

    <owl:Class rdf:ID="Relationship">
        <rdf:type rdf:resource="#ClassOfAssertion"/>
        <rdf:type rdf:resource="#ClassOfRelationship"/>
        <rdfs:subClassOf rdf:resource="#AbstractObject"/>
        <owl:unionOf rdf:parseType="Collection">  
            <owl:Class rdf:about="#Approval"/>  
            <owl:Class rdf:about="#CauseOfEvent"/>  
            <owl:Class rdf:about="#ClassOfRelationshipWithSignature"/>  
            <owl:Class rdf:about="#ComparisonOfProperty"/>  
            <owl:Class rdf:about="#CompositionOfIndividual"/>  
            <owl:Class rdf:about="#ConnectionOfIndividual"/>  
            <owl:Class rdf:about="#FunctionalMapping"/>  
            <owl:Class rdf:about="#IndirectProperty"/>  
            <owl:Class rdf:about="#IndividualUsedInConnection"/>  
            <owl:Class rdf:about="#IntendedRoleAndDomain"/>  
            <owl:Class rdf:about="#InvolvementByReference"/>  
            <owl:Class rdf:about="#LifecycleStage"/>  
            <owl:Class rdf:about="#OtherRelationship"/>  
            <owl:Class rdf:about="#PossibleRoleAndDomain"/>  
            <owl:Class rdf:about="#Recognition"/>  
            <owl:Class rdf:about="#RelativeLocation"/>  
            <owl:Class rdf:about="#RepresentationOfThing"/>  
            <owl:Class rdf:about="#ResponsibilityForRepresentation"/>  
            <owl:Class rdf:about="#TemporalSequence"/>  
            <owl:Class rdf:about="#UsageOfRepresentation"/>  
        </owl:unionOf>
        <rdfs:comment>
            DEFINITION A Relationship is an AbstractObject that indicates something that
            one Thing has to do with another.
        </rdfs:comment>
        <rdfs:comment>
            NOTE Only classes of binary relationship are supported. More complex objects
            can be supported using MultidimensionalObject and
            ClassOfMultidimensionalObject . Instances of ISO 15926-7 Templates are such
            complex objects.
        </rdfs:comment>
        <rdfs:comment>
            NOTE An rdf:Property comes close, but has one direction. The two attributes
            of a relationship are mapped to rdf:Property, with the subclass of
            Relationship as rdf:domain, and the rdg:range defined using the built-in
            OWL properties owl:onProperty and owl:allValuesFrom.
        </rdfs:comment>
    </owl:Class>

    <owl:Class rdf:ID="RelativeLocation">
        <rdf:type rdf:resource="#ClassOfRelativeLocation"/>
        <rdfs:subClassOf rdf:resource="#Relationship"/>
        <owl:disjointWith rdf:resource="#RepresentationOfThing"/>
        <owl:disjointWith rdf:resource="#ResponsibilityForRepresentation"/>
        <owl:disjointWith rdf:resource="#TemporalSequence"/>
        <owl:disjointWith rdf:resource="#UsageOfRepresentation"/>
        <rdfs:subClassOf>
            <owl:Restriction>
                <owl:onProperty rdf:resource="#located"/>
                <owl:allValuesFrom rdf:resource="#PossibleIndividual"/>
            </owl:Restriction>
        </rdfs:subClassOf>
        <rdfs:subClassOf>
            <owl:Restriction>
                <owl:onProperty rdf:resource="#locator"/>
                <owl:allValuesFrom rdf:resource="#PossibleIndividual"/>
            </owl:Restriction>
        </rdfs:subClassOf>
        <rdfs:comment>
            DEFINITION A RelativeLocation is a Relationship that indicates that the
            position of one PossibleIndividual is relative to another.
        </rdfs:comment>
        <rdfs:comment>
            NOTE The Classification of the RelativeLocation indicates the nature of the
            RelativeLocation , e.g. 'above', 'below', 'beside'.
        </rdfs:comment>
        <rdfs:comment>
            EXAMPLE A being the located relative to B being the locator in a
            RelativeLocation that is classified by the ClassOfRelativeLocation 'above'
            indicates that A is above B.
        </rdfs:comment>
    </owl:Class>

    <owl:Class rdf:ID="RepresentationForm">
        <rdfs:subClassOf rdf:resource="#ClassOfClassOfInformationRepresentation"/>
        <rdfs:comment>
            DEFINITION A RepresentationForm is a ClassOfClassOfInformationRepresentation
            that distinguishes the form of representation.
        </rdfs:comment>
        <rdfs:comment>
            EXAMPLE 'Hexadecimal', 'text', 'script', 'symbol', 'picture', 'diagram',
            'semaphore', 'Morse code', 'music score', 'MIDI', 'XML', and 'OWL' are
            instances of RepresentationForm.
        </rdfs:comment>
    </owl:Class>

    <owl:Class rdf:ID="RepresentationOfGregorianDateAndUtcTime">
        <rdfs:subClassOf rdf:resource="#ClassOfInformationRepresentation"/>
        <rdfs:subClassOf>
            <owl:Restriction>
                <owl:onProperty rdf:resource="#year"/>
                <owl:allValuesFrom rdf:datatype="http://www.w3.org/2001/XMLSchema#nonNegativeInteger"/>
            </owl:Restriction>
        </rdfs:subClassOf>
        <rdfs:subClassOf>
            <owl:Restriction>
                <owl:onProperty rdf:resource="#month"/>
                <owl:allValuesFrom rdf:datatype="http://www.w3.org/2001/XMLSchema#nonNegativeInteger"/>
            </owl:Restriction>
        </rdfs:subClassOf>
        <rdfs:subClassOf>
            <owl:Restriction>
                <owl:onProperty rdf:resource="#day"/>
                <owl:allValuesFrom rdf:datatype="http://www.w3.org/2001/XMLSchema#nonNegativeInteger"/>
            </owl:Restriction>
        </rdfs:subClassOf>
        <rdfs:subClassOf>
            <owl:Restriction>
                <owl:onProperty rdf:resource="#hour"/>
                <owl:allValuesFrom rdf:datatype="http://www.w3.org/2001/XMLSchema#nonNegativeInteger"/>
            </owl:Restriction>
        </rdfs:subClassOf>
        <rdfs:subClassOf>
            <owl:Restriction>
                <owl:onProperty rdf:resource="#minute"/>
                <owl:allValuesFrom rdf:datatype="http://www.w3.org/2001/XMLSchema#nonNegativeInteger"/>
            </owl:Restriction>
        </rdfs:subClassOf>
        <rdfs:subClassOf>
            <owl:Restriction>
                <owl:onProperty rdf:resource="#second"/>
                <owl:allValuesFrom rdf:datatype="http://www.w3.org/2001/XMLSchema#unsignedLong"/>
            </owl:Restriction>
        </rdfs:subClassOf>
        <rdfs:comment>
            DEFINITION A RepresentationOfGregorianDateAndUtcTime is a
            ClassOfInformationRepresentation whose members are representations of time
            using the UTC system of time identification as specified in ISO 8601:2000
            together with the Gregorian system for representing dates. All times shall
            be represented using UTC representation of time. Dates shall follow the
            Gregorian calendar.
        </rdfs:comment>
        <rdfs:comment>
            NOTE Coordinated Universal Time (UTC) is the basis for legal time worldwide
            and follows TAI (see below) exactly except for an integral number of seconds,
            presently 32. These leap seconds are inserted on the advice of the
            International Earth Rotation Service (IERS) (http://hpiers.obspm.fr) to
            ensure that, on average over the years, the Sun is overhead within 0.9
            seconds of 12:00:00 UTC on the meridian of Greenwich. UTC is thus the modern
            successor of Greenwich Mean Time, GMT, which was used when the unit of time
            was the mean solar day. International Atomic Time (TAI) is calculated by the
            BIPM from the readings of more than 200 atomic clocks located in metrology
            institutes and observatories in more than 30 countries around the world. TAI
            is made available every month in the BIPM Circular T
            (ftp://62.161.69.5/pub/tai/publication). It is estimated that TAI does not
            lose or gain with respect to an imaginary perfect clock by more than about
            one tenth of a microsecond (0.0000001 second) per year.
        </rdfs:comment>
    </owl:Class>

    <owl:Class rdf:ID="RepresentationOfThing">
        <rdf:type rdf:resource="#ClassOfRepresentationOfThing"/>
        <rdfs:subClassOf rdf:resource="#Relationship"/>
        <owl:intersectionOf rdf:parseType="Collection">  
            <owl:Class rdf:about="#Definition"/>  
            <owl:Class rdf:about="#Description"/>  
            <owl:Class rdf:about="#Identification"/>  
        </owl:intersectionOf>
        <owl:disjointWith rdf:resource="#ResponsibilityForRepresentation"/>
        <owl:disjointWith rdf:resource="#TemporalSequence"/>
        <owl:disjointWith rdf:resource="#UsageOfRepresentation"/>
        <rdfs:subClassOf>
            <owl:Restriction>
                <owl:onProperty rdf:resource="#represented"/>
                <owl:allValuesFrom rdf:resource="#Thing"/>
            </owl:Restriction>
        </rdfs:subClassOf>
        <rdfs:subClassOf>
            <owl:Restriction>
                <owl:onProperty rdf:resource="#sign"/>
                <owl:allValuesFrom rdf:resource="#PossibleIndividual"/>
            </owl:Restriction>
        </rdfs:subClassOf>
        <rdfs:comment>
            DEFINITION A RepresentationOfThing is a Relationship that indicates that a
            PossibleIndividual is a sign for a Thing .
        </rdfs:comment>
        <rdfs:comment>
            NOTE In general it will be ClassOfRepresentationOfThing that will be of
            interest, rather than each RepresentationOfThing. However,
            RepresentationOfThing will be of interest when individual copies of documents
            are managed and controlled.
        </rdfs:comment>
        <rdfs:comment>
            EXAMPLE The relationship between a nameplate with its serial number and other
            data, and a particular pressure vessel (MaterializedPhysicalObject) is an
            example of RepresentationOfThing that is an Identification .
        </rdfs:comment>
    </owl:Class>

    <owl:Class rdf:ID="ResponsibilityForRepresentation">
        <rdf:type rdf:resource="#ClassOfResponsibilityForRepresentation"/>
        <rdfs:subClassOf rdf:resource="#Relationship"/>
        <owl:disjointWith rdf:resource="#TemporalSequence"/>
        <owl:disjointWith rdf:resource="#UsageOfRepresentation"/>
        <rdfs:subClassOf>
            <owl:Restriction>
                <owl:onProperty rdf:resource="#controlled"/>
                <owl:allValuesFrom rdf:resource="#RepresentationOfThing"/>
            </owl:Restriction>
        </rdfs:subClassOf>
        <rdfs:subClassOf>
            <owl:Restriction>
                <owl:onProperty rdf:resource="#controller"/>
                <owl:allValuesFrom rdf:resource="#PossibleIndividual"/>
            </owl:Restriction>
        </rdfs:subClassOf>
        <rdfs:comment>
            DEFINITION A ResponsibilityForRepresentation is a Relationship that indicates
            that the controller PossibleIndividual administers the controlled
            RepresentationOfThing .
        </rdfs:comment>
        <rdfs:comment>
            EXAMPLE The responsibility for the administration of this standard lies with
            ISO. This is represented as a PossibleIndividual 'ISO' is linked by an
            instance of ResponsibilityForRepresentation to a RepresentationOfThing; the
            latter links the ClassOfInformationObject 'ISO 15926-7' to a PhysicalObject
            'myNumberedCopy of ISO 15926-7'.
        </rdfs:comment>
    </owl:Class>

    <owl:Class rdf:ID="RightNamespace">
        <rdf:type rdf:resource="#ClassOfRightNamespace"/>
        <rdfs:subClassOf rdf:resource="#Namespace"/>
        <rdfs:comment>
            DEFINITION A RightNamespace is a Namespace that indicates that the
            classOfPart is the right most part of the classOfWhole .
        </rdfs:comment>
        <rdfs:comment>
            EXAMPLE When ZH is the namespace in 5367ZH, this is indicated by a
            Namespace relationship between them.
        </rdfs:comment>
    </owl:Class>

    <owl:Class rdf:ID="Role">
        <rdfs:subClassOf rdf:resource="#RoleAndDomain"/>
        <rdfs:comment>
            DEFINITION A Role is a RoleAndDomain that indicates what some thing has to do
            with an Activity , Relationship , or MultidimensionalObject .
        </rdfs:comment>
        <rdfs:comment>
            EXAMPLE Employee is a Role that indicates what a temporal part of a person
            has to do with an employment relation.
        </rdfs:comment>
        <rdfs:comment>
            EXAMPLE Pumper is a Role that indicates what a temporal part of a pump has to
            do with a pumping Activity.
        </rdfs:comment>
    </owl:Class>

    <owl:Class rdf:ID="RoleAndDomain">
        <rdfs:subClassOf rdf:resource="#Class"/>
        <owl:intersectionOf rdf:parseType="Collection">  
            <owl:Class rdf:about="#ParticipatingRoleAndDomain"/>  
            <owl:Class rdf:about="#Role"/>  
        </owl:intersectionOf>
        <rdfs:comment>
            DEFINITION A RoleAndDomain is a Class that specifies the domain and role for
            an end of a ClassOfRelationship or ClassOfMultidimensionalObject .
        </rdfs:comment>
        <rdfs:comment>
            NOTE A RoleAndDomain is analogous to specifying an EXPRESS attribute or its
            inverse.
        </rdfs:comment>
        <rdfs:comment>
            EXAMPLE "Husband and man" and "wife and woman" are examples of RoleAndDomain.
        </rdfs:comment>
    </owl:Class>

    <owl:Class rdf:ID="Scale">
        <rdf:type rdf:resource="#ClassOfScale"/>
        <rdfs:subClassOf rdf:resource="#ClassOfIsomorphicFunctionalMapping"/>
        <rdfs:subClassOf>
            <owl:Restriction>
                <owl:onProperty rdf:resource="#codomain"/>
                <owl:allValuesFrom rdf:resource="#NumberSpace"/>
            </owl:Restriction>
        </rdfs:subClassOf>
        <rdfs:subClassOf>
            <owl:Restriction>
                <owl:onProperty rdf:resource="#domain"/>
                <owl:allValuesFrom rdf:resource="#PropertySpace"/>
            </owl:Restriction>
        </rdfs:subClassOf>
        <rdfs:comment>
            DEFINITION A Scale is a ClassOfIsomorphicFunctionalMapping whose members are
            members of PropertyQuantification . It indicates the NumberSpace a
            PropertySpace maps to for the Scale in question.
        </rdfs:comment>
        <rdfs:comment>
            EXAMPLE The link that is known as the Celsius scale between the ClassOfNumber
            '[-273, inf]' and the ClassOfProperty 'temperature' can be represented by an
            instance of Scale.
        </rdfs:comment>
    </owl:Class>

    <owl:Class rdf:ID="Shape">
        <rdf:type rdf:resource="#ClassOfShape"/>
        <rdfs:subClassOf rdf:resource="#Property"/>
        <rdfs:comment>
            DEFINITION A Shape is a Property that depends on constant relations of
            position and proportionate distance among all the points composing its
            outline or its external surface.
        </rdfs:comment>
        <rdfs:comment>
            EXAMPLE '20mm diameter circle' and '10-20mm diameter circles' are examples
            of Shape .
        </rdfs:comment>
        <rdfs:comment>
            EXAMPLE 2 Irregular forms such as the outer envelope of a model of pump can
            be represented by instances of Shape .
        </rdfs:comment>
    </owl:Class>

    <owl:Class rdf:ID="ShapeDimension">
        <rdf:type rdf:resource="#ClassOfShapeDimension"/>
        <rdfs:subClassOf rdf:resource="#ClassOfClassOfIndividual"/>
        <rdfs:comment>
            DEFINITION A ShapeDimension is a ClassOfClassOfIndividual that is a set of
            IndividualDimension that defines an aspect of a Shape .
        </rdfs:comment>
        <rdfs:comment>
            EXAMPLE 'Diameter of 5m', 'height of 3mm', and 'width of 10cm' are members
            of ShapeDimension .
        </rdfs:comment>
    </owl:Class>

    <owl:Class rdf:ID="SinglePropertyDimension">
        <rdfs:subClassOf rdf:resource="#PropertySpace"/>
        <rdfs:comment>
            DEFINITION A SinglePropertyDimension is a PropertySpace that is a single and
            complete continuum of properties each of which maps to a single number.
        </rdfs:comment>
        <rdfs:comment>
            EXAMPLE 'Temperature', 'pressure', 'viscosity', and 'length' are examples of
            SinglePropertyDimension .
        </rdfs:comment>
    </owl:Class>

    <owl:Class rdf:ID="SpatialLocation">
        <rdfs:subClassOf rdf:resource="#PhysicalObject"/>
        <rdfs:comment>
            DEFINITION A SpatialLocation is a PhysicalObject that has continuity of
            relative position.
        </rdfs:comment>
        <rdfs:comment>
            EXAMPLE 'Geographic datum', 'license block', 'construction area', 'country',
            'air corridor', 'maritime traffic zone', 'hazard control zone', '4D points',
            'lines', 'planes', 'solids' are instances of SpatialLocation .
        </rdfs:comment>
    </owl:Class>

    <owl:Class rdf:ID="SpecializationOfIndividualDimensionFromProperty">
        <rdfs:subClassOf rdf:resource="#Relationship"/>
        <rdfs:subClassOf>
            <owl:Restriction>
                <owl:onProperty rdf:resource="#dimension"/>
                <owl:allValuesFrom rdf:resource="#IndividualDimension"/>
            </owl:Restriction>
        </rdfs:subClassOf>
        <rdfs:subClassOf>
            <owl:Restriction>
                <owl:onProperty rdf:resource="#property"/>
                <owl:allValuesFrom rdf:resource="#Property"/>
            </owl:Restriction>
        </rdfs:subClassOf>
        <rdfs:comment>
            DEFINITION A SpecializationOfIndividualDimensionFromProperty is a
            Specialization that indicates the members of the IndividualDimension are
            members of the Property .
        </rdfs:comment>
        <rdfs:comment>
            EXAMPLE An IndividualDimension 'diameter of 10m' is a subclass of the
            Property 'length of 10m'.
        </rdfs:comment>
    </owl:Class>

    <owl:Class rdf:ID="Status">
        <rdf:type rdf:resource="#ClassOfStatus"/>
        <rdfs:subClassOf rdf:resource="#ClassOfIndividual"/>
        <rdfs:comment>
            DEFINITION A Status is a ClassOfIndividual that is a characteristic or
            quality that is described by discrete, unordered values.
        </rdfs:comment>
        <rdfs:comment>
            NOTE Degrees of openness or paintedness are represented as instances of
            Property and not instances of Status .
        </rdfs:comment>
        <rdfs:comment>
            EXAMPLE The classes known as 'open', 'painted', 'approved', 'old', 'new',
            'worn', 'hazardous', 'safe', 'dangerous', 'happy', 'sad', and 'rusty' can all
            be represented as instances of Status .
        </rdfs:comment>
    </owl:Class>

    <owl:Class rdf:ID="Stream">
        <rdfs:subClassOf rdf:resource="#PhysicalObject"/>
        <rdfs:comment>
            DEFINITION A Stream is a PhysicalObject that is material or energy moving
            along a path, where the path is the basis of identity and may be constrained.
            The Stream consists of the temporal parts of those things that are in the
            Stream whilst they are in it.
        </rdfs:comment>
        <rdfs:comment>
            EXAMPLE Flux is a 4D-constrained case of Stream where the path crosses a
            surface.
        </rdfs:comment>
        <rdfs:comment>
            EXAMPLE The naphtha flowing in a pipe between a crude distillation unit and a
            platformer is a Stream .
        </rdfs:comment>
    </owl:Class>

    <owl:Class rdf:ID="TemporalBounding">
        <rdfs:subClassOf rdf:resource="#CompositionOfIndividual"/>
        <owl:unionOf rdf:parseType="Collection">  
            <owl:Class rdf:about="#Beginning"/>  
            <owl:Class rdf:about="#Ending"/>  
        </owl:unionOf>
        <owl:disjointWith rdf:resource="#TemporalWholePart"/>
        <rdfs:subClassOf>
            <owl:Restriction>
                <owl:onProperty rdf:resource="#part"/>
                <owl:allValuesFrom rdf:resource="#Event"/>
            </owl:Restriction>
        </rdfs:subClassOf>
        <rdfs:comment>
            DEFINITION A TemporalBounding is a CompositionOfIndividual that indicates
            that the part Event is a temporal boundary of the whole PossibleIndividual .
        </rdfs:comment>
        <rdfs:comment>
            EXAMPLE The Event of the birth of JohnDoe is linked to JohnDoe by an instance
            of TemporalBounding that is a Beginning .
        </rdfs:comment>
    </owl:Class>

    <owl:Class rdf:ID="TemporalSequence">
        <rdf:type rdf:resource="#ClassOfTemporalSequence"/>
        <rdfs:subClassOf rdf:resource="#Relationship"/>
        <owl:disjointWith rdf:resource="#UsageOfRepresentation"/>
        <rdfs:subClassOf>
            <owl:Restriction>
                <owl:onProperty rdf:resource="#predecessor"/>
                <owl:allValuesFrom rdf:resource="#PossibleIndividual"/>
            </owl:Restriction>
        </rdfs:subClassOf>
        <rdfs:subClassOf>
            <owl:Restriction>
                <owl:onProperty rdf:resource="#successor"/>
                <owl:allValuesFrom rdf:resource="#PossibleIndividual"/>
            </owl:Restriction>
        </rdfs:subClassOf>
        <rdfs:comment>
            DEFINITION A TemporalSequence is a Relationship that indicates that one
            PossibleIndividual precedes another in a temporal sense.
        </rdfs:comment>
        <rdfs:comment>
            EXAMPLE The Relationship that indicates that the PossibleIndividual that is
            the construction phase of a plant precedes the PossibleIndividual that is the
            commissioning phase of a plant can be represented by an instance of
            TemporalSequence .
        </rdfs:comment>
        <rdfs:comment>
            EXAMPLE The Relationship that indicates that the PeriodInTime known as the
            industrial revolution preceded the PeriodInTime known as the information
            revolution can be represented by an instance of TemporalSequence .
        </rdfs:comment>
    </owl:Class>

    <owl:Class rdf:ID="TemporalWholePart">
        <rdf:type rdf:resource="#ClassOfTemporalWholePart"/>
        <rdfs:subClassOf rdf:resource="#CompositionOfIndividual"/>
        <rdfs:comment>
            DEFINITION A TemporalWholePart is a CompositionOfIndividual that indicates
            that one PossibleIndividual is a temporal part of another PossibleIndividual.
            The spatial extent of the temporal part is that of the temporal whole for the
            period of the existence of the temporal part. Relationships that apply to the
            whole PossibleIndividual also apply to the temporal parts of the
            PossibleIndividual, except when the relationships relate to the temporal
            nature of the whole. So if a PossibleIndividual is connected so are all its
            temporal parts, but being a WholeLifeIndividual is not inherited by its
            temporal parts.
        </rdfs:comment>
        <rdfs:comment>
            NOTE Since TemporalWholePart is transitive (inherited from its supertype) a
            hierarchy of temporal parts is possible, with a WholeLifeIndividual at the top.
        </rdfs:comment>
        <rdfs:comment>
            EXAMPLE The Relationship that indicates that an operating period of a pump is
            a temporal part of the pump can be represented by an instance of
            TemporalWholePart .
        </rdfs:comment>
        <rdfs:comment>
            EXAMPLE The Relationship that indicates that the time period known as March
            1999 is part of the period known as 1st Quarter 1999 can be represented by an
            instance of TemporalWholePart .
        </rdfs:comment>
    </owl:Class>

    <owl:Class rdf:ID="Thing">
        <owl:unionOf rdf:parseType="Collection">  
            <owl:Class rdf:about="#AbstractObject"/>  
            <owl:Class rdf:about="#PossibleIndividual"/>  
        </owl:unionOf>
        <rdfs:subClassOf>
            <owl:Restriction>
                <owl:onProperty rdf:resource="#recordCopyCreated"/>
                <owl:allValuesFrom rdf:resource="#RepresentationOfGregorianDateAndUtcTime"/>
            </owl:Restriction>
        </rdfs:subClassOf>
        <rdfs:subClassOf>
            <owl:Restriction>
                <owl:onProperty rdf:resource="#recordCreated"/>
                <owl:allValuesFrom rdf:resource="#RepresentationOfGregorianDateAndUtcTime"/>
            </owl:Restriction>
        </rdfs:subClassOf>
        <rdfs:subClassOf>
            <owl:Restriction>
                <owl:onProperty rdf:resource="#recordCreator"/>
                <owl:allValuesFrom rdf:resource="#PossibleIndividual"/>
            </owl:Restriction>
        </rdfs:subClassOf>
        <rdfs:subClassOf>
            <owl:Restriction>
                <owl:onProperty rdf:resource="#recordLogicallyDeleted"/>
                <owl:allValuesFrom rdf:resource="#RepresentationOfGregorianDateAndUtcTime"/>
            </owl:Restriction>
        </rdfs:subClassOf>
        <rdfs:subClassOf>
            <owl:Restriction>
                <owl:onProperty rdf:resource="#whyDeleted"/>
                <owl:allValuesFrom rdf:resource="#ClassOfInformationRepresentation"/>
            </owl:Restriction>
        </rdfs:subClassOf>
        <rdfs:comment>
            DEFINITION A Thing is anything that is or may be thought about or perceived,
            including material and non-material objects, ideas, and actions. Every Thing
            is either a PossibleIndividual , or an AbstractObject .
        </rdfs:comment>
        <rdfs:comment>
            NOTE Every Thing is identifiable within a system by means of rdf:ID..
            System identifiers created by other systems and received as part of a data
            exchange may be stored for future reference as an identification, referring to
            the originating organisation or system.
        </rdfs:comment>
        <rdfs:comment>
            NOTE Every example provided for other entity data types declared in this
            schema is also an example of Thing .
        </rdfs:comment>
    </owl:Class>

    <owl:Class rdf:ID="UnionOfSetOfClass">
        <rdfs:subClassOf rdf:resource="#FunctionalMapping"/>
        <owl:disjointWith rdf:resource="#PropertyQuantification"/>
        <rdfs:subClassOf>
            <owl:Restriction>
                <owl:onProperty rdf:resource="#input"/>
                <owl:allValuesFrom rdf:resource="#EnumeratedSetOfClass"/>
            </owl:Restriction>
        </rdfs:subClassOf>
        <rdfs:subClassOf>
            <owl:Restriction>
                <owl:onProperty rdf:resource="#result"/>
                <owl:allValuesFrom rdf:resource="#Class"/>
            </owl:Restriction>
        </rdfs:subClassOf>
        <rdfs:comment>
            DEFINITION A UnionOfSetOfClass is a FunctionalMapping that indicates that the
            membership of the result Class is the union of the members of the
            EnumeratedSetOfClass classes.
        </rdfs:comment>
        <rdfs:comment>
            EXAMPLE The union of the EnumeratedSetOfClass {{A,B,C},{B,C,D},{C,D,E}} is
            {A,B,C,D,E}.
        </rdfs:comment>
    </owl:Class>

    <owl:Class rdf:ID="UpperBoundOfNumberRange">
        <rdfs:subClassOf rdf:resource="#Relationship"/>
        <rdfs:subClassOf>
            <owl:Restriction>
                <owl:onProperty rdf:resource="#highestNumber"/>
                <owl:allValuesFrom rdf:resource="#ArithmeticNumber"/>
            </owl:Restriction>
        </rdfs:subClassOf>
        <rdfs:subClassOf>
            <owl:Restriction>
                <owl:onProperty rdf:resource="#range"/>
                <owl:allValuesFrom rdf:resource="#NumberRange"/>
            </owl:Restriction>
        </rdfs:subClassOf>
        <rdfs:comment>
            DEFINITION An UpperBoundOfNumberRange is a Relationship that indicates an
            ArithmeticNumber is the largest value in a NumberRange .
        </rdfs:comment>
        <rdfs:comment>
            EXAMPLE The instance of RealNumber that is represented by the instance of
            ExpressReal '5.3' has an UpperBoundOfNumberRange relationship with the
            instance of NumberRange'[3.1 to 5.3]'.
        </rdfs:comment>
    </owl:Class>

    <owl:Class rdf:ID="UpperBoundOfPropertyRange">
        <rdfs:subClassOf rdf:resource="#Relationship"/>
        <rdfs:subClassOf>
            <owl:Restriction>
                <owl:onProperty rdf:resource="#highestProperty"/>
                <owl:allValuesFrom rdf:resource="#Property"/>
            </owl:Restriction>
        </rdfs:subClassOf>
        <rdfs:subClassOf>
            <owl:Restriction>
                <owl:onProperty rdf:resource="#range"/>
                <owl:allValuesFrom rdf:resource="#PropertyRange"/>
            </owl:Restriction>
        </rdfs:subClassOf>
        <rdfs:comment>
            DEFINITION An UpperBoundOfPropertyRange is a Classification that indicates
            that the Property is the upper bound of the PropertyRange .
        </rdfs:comment>
        <rdfs:comment>
            EXAMPLE The instance of Property that is represented by the instance of
            ExpressReal '+20' has an UpperBoundOfPropertyRange relationship with the
            instance of PropertyRange'[-10 to +20 degrees Celsius]'.
        </rdfs:comment>
    </owl:Class>

    <owl:Class rdf:ID="UsageOfRepresentation">
        <rdf:type rdf:resource="#ClassOfUsageOfRepresentation"/>
        <rdfs:subClassOf rdf:resource="#Relationship"/>
        <rdfs:subClassOf>
            <owl:Restriction>
                <owl:onProperty rdf:resource="#used"/>
                <owl:allValuesFrom rdf:resource="#RepresentationOfThing"/>
            </owl:Restriction>
        </rdfs:subClassOf>
        <rdfs:subClassOf>
            <owl:Restriction>
                <owl:onProperty rdf:resource="#user"/>
                <owl:allValuesFrom rdf:resource="#PossibleIndividual"/>
            </owl:Restriction>
        </rdfs:subClassOf>
        <rdfs:comment>
            DEFINITION A UsageOfRepresentation is a Relationship that indicates that the
            RepresentationOfThing is used by the PossibleIndividual . Usage does not
            imply responsibility.
        </rdfs:comment>
        <rdfs:comment>
            EXAMPLE The sign "P101" is used by the XYZ company to represent a particular
            pump in a design.
        </rdfs:comment>
    </owl:Class>

    <owl:Class rdf:ID="WholeLifeIndividual">
        <rdfs:subClassOf rdf:resource="#PossibleIndividual"/>
        <rdfs:comment>
            DEFINITION A WholeLifeIndividual is a PossibleIndividual that is a member of
            a ClassOfIndividual , and is not a temporal part of any other
            PossibleIndividual that is also a member of the same ClassOfIndividual .
            A WholeLifeIndividual includes its past and future.
        </rdfs:comment>
        <rdfs:comment>
            NOTE A possible future temporal part of the WholeLifeIndividual is a
            PossibleIndividual that is related to the WholeLifeIndividual by a
            TemporalWholePart relation.
        </rdfs:comment>
        <rdfs:comment>
            EXAMPLE A plastic cup (bounded by its 'creation' and 'destruction' Event's)
            can be represented by an instance of WholeLifeIndividual . The cup whilst it
            stands on this table is a temporal part of this WholeLifeIndividual .
        </rdfs:comment>
        <rdfs:comment>
            EXAMPLE The universe for all time is a WholeLifeIndividual .
        </rdfs:comment>
    </owl:Class>
</rdf:RDF>

