<?xml version="1.0" encoding="ISO-8859-1"?>
<!DOCTYPE rdf:RDF [
	<!ENTITY java "http://localhost/~dennis/Java.owl#">
	<!ENTITY xsd "http://www.w3.org/2001/XMLSchema#">
	<!ENTITY units "http://localhost/~dennis/Units.owl#">
	<!ENTITY platform "http://localhost/~dennis/Platform.owl#">
	<!ENTITY j2se-1_5 "http://ssel.vub.ac.be/platformkit/j2se-1_5#">
	<!ENTITY j2se-1_6 "http://ssel.vub.ac.be/platformkit/j2se-1_6#">
	<!ENTITY rdf "http://www.w3.org/1999/02/22-rdf-syntax-ns#">
	<!ENTITY rdfs "http://www.w3.org/2000/01/rdf-schema#">
	<!ENTITY owl "http://www.w3.org/2002/07/owl#">
]>
<rdf:RDF
	 xmlns:java="&java;"
	 xmlns:xsd="&xsd;"
	 xmlns:units="&units;"
	 xmlns:platform="&platform;"
	 xmlns:j2se-1_5="&j2se-1_5;"
	 xmlns:j2se-1_6="&j2se-1_6;"
	 xmlns:rdf="&rdf;"
	 xmlns:rdfs="&rdfs;"
	 xmlns:owl="&owl;"
>

	<owl:Ontology rdf:about="http://ssel.vub.ac.be/platformkit/j2se-1_6#">
		<owl:imports rdf:resource="http://localhost/~dennis/Platform.owl"/>
		<owl:imports rdf:resource="http://localhost/~dennis/Java.owl"/>
		<owl:imports rdf:resource="http://ssel.vub.ac.be/platformkit/j2se-1_5#"/>
		<rdfs:comment xml:lang="en">Generated by $Id: UML2ToPackageAPIOntology.atl 7380 2007-11-08 09:49:02Z dwagelaa $ and $Id: UML2ToAPIOntology.atl 7380 2007-11-08 09:49:02Z dwagelaa $ and $Id:UML2Comparison.atl 7084 2007-07-10 13:19:05Z dwagelaa $</rdfs:comment>
		<rdfs:label xml:lang="en">j2se-1_6</rdfs:label>
	</owl:Ontology>
	<owl:Class rdf:about="&j2se-1_6;J2se-1_6ClassLibrary">
		<rdfs:subClassOf rdf:resource="&j2se-1_6;JavaAppletLibrary"/>
		<rdfs:subClassOf rdf:resource="&j2se-1_6;JavaAwtLibrary"/>
		<rdfs:subClassOf rdf:resource="&j2se-1_6;JavaAwtEventLibrary"/>
		<rdfs:subClassOf rdf:resource="&j2se-1_6;JavaAwtColorLibrary"/>
		<rdfs:subClassOf rdf:resource="&j2se-1_6;JavaAwtDatatransferLibrary"/>
		<rdfs:subClassOf rdf:resource="&j2se-1_6;JavaAwtDndLibrary"/>
		<rdfs:subClassOf rdf:resource="&j2se-1_6;JavaAwtDndPeerLibrary"/>
		<rdfs:subClassOf rdf:resource="&j2se-1_6;JavaAwtFontLibrary"/>
		<rdfs:subClassOf rdf:resource="&j2se-1_6;JavaAwtGeomLibrary"/>
		<rdfs:subClassOf rdf:resource="&j2se-1_6;JavaAwtImLibrary"/>
		<rdfs:subClassOf rdf:resource="&j2se-1_6;JavaAwtImSpiLibrary"/>
		<rdfs:subClassOf rdf:resource="&j2se-1_6;JavaAwtImageLibrary"/>
		<rdfs:subClassOf rdf:resource="&j2se-1_6;JavaAwtImageRenderableLibrary"/>
		<rdfs:subClassOf rdf:resource="&j2se-1_6;JavaAwtPeerLibrary"/>
		<rdfs:subClassOf rdf:resource="&j2se-1_6;JavaAwtPrintLibrary"/>
		<rdfs:subClassOf rdf:resource="&j2se-1_6;JavaLangLibrary"/>
		<rdfs:subClassOf rdf:resource="&j2se-1_6;JavaLangAnnotationLibrary"/>
		<rdfs:subClassOf rdf:resource="&j2se-1_6;JavaLangReflectLibrary"/>
		<rdfs:subClassOf rdf:resource="&j2se-1_6;JavaLangInstrumentLibrary"/>
		<rdfs:subClassOf rdf:resource="&j2se-1_6;JavaLangManagementLibrary"/>
		<rdfs:subClassOf rdf:resource="&j2se-1_6;JavaLangRefLibrary"/>
		<rdfs:subClassOf rdf:resource="&j2se-1_6;JavaIoLibrary"/>
		<rdfs:subClassOf rdf:resource="&j2se-1_6;JavaUtilLibrary"/>
		<rdfs:subClassOf rdf:resource="&j2se-1_6;JavaUtilSpiLibrary"/>
		<rdfs:subClassOf rdf:resource="&j2se-1_6;JavaUtilConcurrentLibrary"/>
		<rdfs:subClassOf rdf:resource="&j2se-1_6;JavaUtilConcurrentAtomicLibrary"/>
		<rdfs:subClassOf rdf:resource="&j2se-1_6;JavaUtilConcurrentLocksLibrary"/>
		<rdfs:subClassOf rdf:resource="&j2se-1_6;JavaUtilJarLibrary"/>
		<rdfs:subClassOf rdf:resource="&j2se-1_6;JavaUtilZipLibrary"/>
		<rdfs:subClassOf rdf:resource="&j2se-1_6;JavaUtilLoggingLibrary"/>
		<rdfs:subClassOf rdf:resource="&j2se-1_6;JavaUtilPrefsLibrary"/>
		<rdfs:subClassOf rdf:resource="&j2se-1_6;JavaUtilRegexLibrary"/>
		<rdfs:subClassOf rdf:resource="&j2se-1_6;JavaBeansLibrary"/>
		<rdfs:subClassOf rdf:resource="&j2se-1_6;JavaBeansBeancontextLibrary"/>
		<rdfs:subClassOf rdf:resource="&j2se-1_6;JavaSecurityLibrary"/>
		<rdfs:subClassOf rdf:resource="&j2se-1_6;JavaSecurityAclLibrary"/>
		<rdfs:subClassOf rdf:resource="&j2se-1_6;JavaSecurityCertLibrary"/>
		<rdfs:subClassOf rdf:resource="&j2se-1_6;JavaSecurityInterfacesLibrary"/>
		<rdfs:subClassOf rdf:resource="&j2se-1_6;JavaSecuritySpecLibrary"/>
		<rdfs:subClassOf rdf:resource="&j2se-1_6;JavaMathLibrary"/>
		<rdfs:subClassOf rdf:resource="&j2se-1_6;JavaNetLibrary"/>
		<rdfs:subClassOf rdf:resource="&j2se-1_6;JavaNioLibrary"/>
		<rdfs:subClassOf rdf:resource="&j2se-1_6;JavaNioChannelsLibrary"/>
		<rdfs:subClassOf rdf:resource="&j2se-1_6;JavaNioChannelsSpiLibrary"/>
		<rdfs:subClassOf rdf:resource="&j2se-1_6;JavaNioCharsetLibrary"/>
		<rdfs:subClassOf rdf:resource="&j2se-1_6;JavaNioCharsetSpiLibrary"/>
		<rdfs:subClassOf rdf:resource="&j2se-1_6;JavaRmiLibrary"/>
		<rdfs:subClassOf rdf:resource="&j2se-1_6;JavaRmiActivationLibrary"/>
		<rdfs:subClassOf rdf:resource="&j2se-1_6;JavaRmiServerLibrary"/>
		<rdfs:subClassOf rdf:resource="&j2se-1_6;JavaRmiDgcLibrary"/>
		<rdfs:subClassOf rdf:resource="&j2se-1_6;JavaRmiRegistryLibrary"/>
		<rdfs:subClassOf rdf:resource="&j2se-1_6;JavaSqlLibrary"/>
		<rdfs:subClassOf rdf:resource="&j2se-1_6;JavaTextLibrary"/>
		<rdfs:subClassOf rdf:resource="&j2se-1_6;JavaTextSpiLibrary"/>
		<rdfs:subClassOf rdf:resource="&j2se-1_6;JavaxAccessibilityLibrary"/>
		<rdfs:subClassOf rdf:resource="&j2se-1_6;JavaxSecurityAuthLibrary"/>
		<rdfs:subClassOf rdf:resource="&j2se-1_6;JavaxSecurityAuthLoginLibrary"/>
		<rdfs:subClassOf rdf:resource="&j2se-1_6;JavaxSecurityAuthCallbackLibrary"/>
		<rdfs:subClassOf rdf:resource="&j2se-1_6;JavaxSecurityAuthKerberosLibrary"/>
		<rdfs:subClassOf rdf:resource="&j2se-1_6;JavaxSecurityAuthSpiLibrary"/>
		<rdfs:subClassOf rdf:resource="&j2se-1_6;JavaxSecurityAuthX500Library"/>
		<rdfs:subClassOf rdf:resource="&j2se-1_6;JavaxSecuritySaslLibrary"/>
		<rdfs:subClassOf rdf:resource="&j2se-1_6;JavaxActivationLibrary"/>
		<rdfs:subClassOf rdf:resource="&j2se-1_6;JavaxActivityLibrary"/>
		<rdfs:subClassOf rdf:resource="&j2se-1_6;JavaxAnnotationLibrary"/>
		<rdfs:subClassOf rdf:resource="&j2se-1_6;JavaxAnnotationProcessingLibrary"/>
		<rdfs:subClassOf rdf:resource="&j2se-1_6;JavaxImageioLibrary"/>
		<rdfs:subClassOf rdf:resource="&j2se-1_6;JavaxImageioEventLibrary"/>
		<rdfs:subClassOf rdf:resource="&j2se-1_6;JavaxImageioMetadataLibrary"/>
		<rdfs:subClassOf rdf:resource="&j2se-1_6;JavaxImageioPluginsBmpLibrary"/>
		<rdfs:subClassOf rdf:resource="&j2se-1_6;JavaxImageioPluginsJpegLibrary"/>
		<rdfs:subClassOf rdf:resource="&j2se-1_6;JavaxImageioSpiLibrary"/>
		<rdfs:subClassOf rdf:resource="&j2se-1_6;JavaxImageioStreamLibrary"/>
		<rdfs:subClassOf rdf:resource="&j2se-1_6;JavaxJwsLibrary"/>
		<rdfs:subClassOf rdf:resource="&j2se-1_6;JavaxJwsSoapLibrary"/>
		<rdfs:subClassOf rdf:resource="&j2se-1_6;JavaxLangModelLibrary"/>
		<rdfs:subClassOf rdf:resource="&j2se-1_6;JavaxLangModelElementLibrary"/>
		<rdfs:subClassOf rdf:resource="&j2se-1_6;JavaxLangModelTypeLibrary"/>
		<rdfs:subClassOf rdf:resource="&j2se-1_6;JavaxLangModelUtilLibrary"/>
		<rdfs:subClassOf rdf:resource="&j2se-1_6;JavaxManagementLibrary"/>
		<rdfs:subClassOf rdf:resource="&j2se-1_6;JavaxManagementLoadingLibrary"/>
		<rdfs:subClassOf rdf:resource="&j2se-1_6;JavaxManagementModelmbeanLibrary"/>
		<rdfs:subClassOf rdf:resource="&j2se-1_6;JavaxManagementMonitorLibrary"/>
		<rdfs:subClassOf rdf:resource="&j2se-1_6;JavaxManagementOpenmbeanLibrary"/>
		<rdfs:subClassOf rdf:resource="&j2se-1_6;JavaxManagementRelationLibrary"/>
		<rdfs:subClassOf rdf:resource="&j2se-1_6;JavaxManagementRemoteLibrary"/>
		<rdfs:subClassOf rdf:resource="&j2se-1_6;JavaxManagementRemoteRmiLibrary"/>
		<rdfs:subClassOf rdf:resource="&j2se-1_6;JavaxManagementTimerLibrary"/>
		<rdfs:subClassOf rdf:resource="&j2se-1_6;JavaxRmiLibrary"/>
		<rdfs:subClassOf rdf:resource="&j2se-1_6;JavaxRmiCORBALibrary"/>
		<rdfs:subClassOf rdf:resource="&j2se-1_6;JavaxRmiSslLibrary"/>
		<rdfs:subClassOf rdf:resource="&j2se-1_6;JavaxNamingLibrary"/>
		<rdfs:subClassOf rdf:resource="&j2se-1_6;JavaxNamingDirectoryLibrary"/>
		<rdfs:subClassOf rdf:resource="&j2se-1_6;JavaxNamingEventLibrary"/>
		<rdfs:subClassOf rdf:resource="&j2se-1_6;JavaxNamingLdapLibrary"/>
		<rdfs:subClassOf rdf:resource="&j2se-1_6;JavaxNamingSpiLibrary"/>
		<rdfs:subClassOf rdf:resource="&j2se-1_6;JavaxPrintLibrary"/>
		<rdfs:subClassOf rdf:resource="&j2se-1_6;JavaxPrintAttributeLibrary"/>
		<rdfs:subClassOf rdf:resource="&j2se-1_6;JavaxPrintAttributeStandardLibrary"/>
		<rdfs:subClassOf rdf:resource="&j2se-1_6;JavaxPrintEventLibrary"/>
		<rdfs:subClassOf rdf:resource="&j2se-1_6;JavaxScriptLibrary"/>
		<rdfs:subClassOf rdf:resource="&j2se-1_6;JavaxCryptoLibrary"/>
		<rdfs:subClassOf rdf:resource="&j2se-1_6;JavaxSmartcardioLibrary"/>
		<rdfs:subClassOf rdf:resource="&j2se-1_6;JavaxSoundMidiLibrary"/>
		<rdfs:subClassOf rdf:resource="&j2se-1_6;JavaxSoundMidiSpiLibrary"/>
		<rdfs:subClassOf rdf:resource="&j2se-1_6;JavaxSoundSampledLibrary"/>
		<rdfs:subClassOf rdf:resource="&j2se-1_6;JavaxSoundSampledSpiLibrary"/>
		<rdfs:subClassOf rdf:resource="&j2se-1_6;JavaxSqlLibrary"/>
		<rdfs:subClassOf rdf:resource="&j2se-1_6;JavaxSqlRowsetLibrary"/>
		<rdfs:subClassOf rdf:resource="&j2se-1_6;JavaxSqlRowsetSerialLibrary"/>
		<rdfs:subClassOf rdf:resource="&j2se-1_6;JavaxSqlRowsetSpiLibrary"/>
		<rdfs:subClassOf rdf:resource="&j2se-1_6;JavaxSwingLibrary"/>
		<rdfs:subClassOf rdf:resource="&j2se-1_6;JavaxSwingEventLibrary"/>
		<rdfs:subClassOf rdf:resource="&j2se-1_6;JavaxSwingTextLibrary"/>
		<rdfs:subClassOf rdf:resource="&j2se-1_6;JavaxSwingTextHtmlLibrary"/>
		<rdfs:subClassOf rdf:resource="&j2se-1_6;JavaxSwingTextHtmlParserLibrary"/>
		<rdfs:subClassOf rdf:resource="&j2se-1_6;JavaxSwingTextRtfLibrary"/>
		<rdfs:subClassOf rdf:resource="&j2se-1_6;JavaxSwingTreeLibrary"/>
		<rdfs:subClassOf rdf:resource="&j2se-1_6;JavaxSwingBorderLibrary"/>
		<rdfs:subClassOf rdf:resource="&j2se-1_6;JavaxSwingColorchooserLibrary"/>
		<rdfs:subClassOf rdf:resource="&j2se-1_6;JavaxSwingFilechooserLibrary"/>
		<rdfs:subClassOf rdf:resource="&j2se-1_6;JavaxSwingPlafLibrary"/>
		<rdfs:subClassOf rdf:resource="&j2se-1_6;JavaxSwingPlafBasicLibrary"/>
		<rdfs:subClassOf rdf:resource="&j2se-1_6;JavaxSwingPlafMetalLibrary"/>
		<rdfs:subClassOf rdf:resource="&j2se-1_6;JavaxSwingPlafMultiLibrary"/>
		<rdfs:subClassOf rdf:resource="&j2se-1_6;JavaxSwingPlafSynthLibrary"/>
		<rdfs:subClassOf rdf:resource="&j2se-1_6;JavaxSwingTableLibrary"/>
		<rdfs:subClassOf rdf:resource="&j2se-1_6;JavaxSwingUndoLibrary"/>
		<rdfs:subClassOf rdf:resource="&j2se-1_6;JavaxToolsLibrary"/>
		<rdfs:subClassOf rdf:resource="&j2se-1_6;JavaxTransactionLibrary"/>
		<rdfs:subClassOf rdf:resource="&j2se-1_6;JavaxTransactionXaLibrary"/>
		<rdfs:subClassOf rdf:resource="&j2se-1_6;JavaxXmlLibrary"/>
		<rdfs:subClassOf rdf:resource="&j2se-1_6;JavaxXmlBindLibrary"/>
		<rdfs:subClassOf rdf:resource="&j2se-1_6;JavaxXmlBindAnnotationLibrary"/>
		<rdfs:subClassOf rdf:resource="&j2se-1_6;JavaxXmlBindAnnotationAdaptersLibrary"/>
		<rdfs:subClassOf rdf:resource="&j2se-1_6;JavaxXmlBindAttachmentLibrary"/>
		<rdfs:subClassOf rdf:resource="&j2se-1_6;JavaxXmlBindHelpersLibrary"/>
		<rdfs:subClassOf rdf:resource="&j2se-1_6;JavaxXmlBindUtilLibrary"/>
		<rdfs:subClassOf rdf:resource="&j2se-1_6;JavaxXmlTransformLibrary"/>
		<rdfs:subClassOf rdf:resource="&j2se-1_6;JavaxXmlTransformSaxLibrary"/>
		<rdfs:subClassOf rdf:resource="&j2se-1_6;JavaxXmlTransformDomLibrary"/>
		<rdfs:subClassOf rdf:resource="&j2se-1_6;JavaxXmlTransformStaxLibrary"/>
		<rdfs:subClassOf rdf:resource="&j2se-1_6;JavaxXmlTransformStreamLibrary"/>
		<rdfs:subClassOf rdf:resource="&j2se-1_6;JavaxXmlCryptoLibrary"/>
		<rdfs:subClassOf rdf:resource="&j2se-1_6;JavaxXmlCryptoDomLibrary"/>
		<rdfs:subClassOf rdf:resource="&j2se-1_6;JavaxXmlCryptoDsigLibrary"/>
		<rdfs:subClassOf rdf:resource="&j2se-1_6;JavaxXmlCryptoDsigDomLibrary"/>
		<rdfs:subClassOf rdf:resource="&j2se-1_6;JavaxXmlCryptoDsigKeyinfoLibrary"/>
		<rdfs:subClassOf rdf:resource="&j2se-1_6;JavaxXmlCryptoDsigSpecLibrary"/>
		<rdfs:subClassOf rdf:resource="&j2se-1_6;JavaxXmlDatatypeLibrary"/>
		<rdfs:subClassOf rdf:resource="&j2se-1_6;JavaxXmlNamespaceLibrary"/>
		<rdfs:subClassOf rdf:resource="&j2se-1_6;JavaxXmlParsersLibrary"/>
		<rdfs:subClassOf rdf:resource="&j2se-1_6;JavaxXmlSoapLibrary"/>
		<rdfs:subClassOf rdf:resource="&j2se-1_6;JavaxXmlStreamLibrary"/>
		<rdfs:subClassOf rdf:resource="&j2se-1_6;JavaxXmlStreamUtilLibrary"/>
		<rdfs:subClassOf rdf:resource="&j2se-1_6;JavaxXmlStreamEventsLibrary"/>
		<rdfs:subClassOf rdf:resource="&j2se-1_6;JavaxXmlValidationLibrary"/>
		<rdfs:subClassOf rdf:resource="&j2se-1_6;JavaxXmlWsLibrary"/>
		<rdfs:subClassOf rdf:resource="&j2se-1_6;JavaxXmlWsHandlerLibrary"/>
		<rdfs:subClassOf rdf:resource="&j2se-1_6;JavaxXmlWsHandlerSoapLibrary"/>
		<rdfs:subClassOf rdf:resource="&j2se-1_6;JavaxXmlWsHttpLibrary"/>
		<rdfs:subClassOf rdf:resource="&j2se-1_6;JavaxXmlWsSoapLibrary"/>
		<rdfs:subClassOf rdf:resource="&j2se-1_6;JavaxXmlWsSpiLibrary"/>
		<rdfs:subClassOf rdf:resource="&j2se-1_6;JavaxXmlXpathLibrary"/>
		<rdfs:subClassOf rdf:resource="&j2se-1_6;OrgW3cDomLibrary"/>
		<rdfs:subClassOf rdf:resource="&j2se-1_6;OrgW3cDomBootstrapLibrary"/>
		<rdfs:subClassOf rdf:resource="&j2se-1_6;OrgW3cDomCssLibrary"/>
		<rdfs:subClassOf rdf:resource="&j2se-1_6;OrgW3cDomStylesheetsLibrary"/>
		<rdfs:subClassOf rdf:resource="&j2se-1_6;OrgW3cDomViewsLibrary"/>
		<rdfs:subClassOf rdf:resource="&j2se-1_6;OrgW3cDomEventsLibrary"/>
		<rdfs:subClassOf rdf:resource="&j2se-1_6;OrgW3cDomHtmlLibrary"/>
		<rdfs:subClassOf rdf:resource="&j2se-1_6;OrgW3cDomLsLibrary"/>
		<rdfs:subClassOf rdf:resource="&j2se-1_6;OrgW3cDomTraversalLibrary"/>
		<rdfs:subClassOf rdf:resource="&j2se-1_6;OrgW3cDomRangesLibrary"/>
		<rdfs:subClassOf rdf:resource="&j2se-1_6;OrgW3cDomXpathLibrary"/>
		<rdfs:subClassOf rdf:resource="&j2se-1_6;OrgOmgCORBA_2_3Library"/>
		<rdfs:subClassOf rdf:resource="&j2se-1_6;OrgOmgCORBA_2_3PortableLibrary"/>
		<rdfs:subClassOf rdf:resource="&j2se-1_6;OrgOmgCORBALibrary"/>
		<rdfs:subClassOf rdf:resource="&j2se-1_6;OrgOmgCORBAPortableLibrary"/>
		<rdfs:subClassOf rdf:resource="&j2se-1_6;OrgOmgCORBADynAnyPackageLibrary"/>
		<rdfs:subClassOf rdf:resource="&j2se-1_6;OrgOmgCORBAORBPackageLibrary"/>
		<rdfs:subClassOf rdf:resource="&j2se-1_6;OrgOmgCORBATypeCodePackageLibrary"/>
		<rdfs:subClassOf rdf:resource="&j2se-1_6;OrgOmgCosNamingLibrary"/>
		<rdfs:subClassOf rdf:resource="&j2se-1_6;OrgOmgCosNamingNamingContextExtPackageLibrary"/>
		<rdfs:subClassOf rdf:resource="&j2se-1_6;OrgOmgCosNamingNamingContextPackageLibrary"/>
		<rdfs:subClassOf rdf:resource="&j2se-1_6;OrgOmgPortableServerLibrary"/>
		<rdfs:subClassOf rdf:resource="&j2se-1_6;OrgOmgPortableServerCurrentPackageLibrary"/>
		<rdfs:subClassOf rdf:resource="&j2se-1_6;OrgOmgPortableServerPOAManagerPackageLibrary"/>
		<rdfs:subClassOf rdf:resource="&j2se-1_6;OrgOmgPortableServerPOAPackageLibrary"/>
		<rdfs:subClassOf rdf:resource="&j2se-1_6;OrgOmgPortableServerServantLocatorPackageLibrary"/>
		<rdfs:subClassOf rdf:resource="&j2se-1_6;OrgOmgPortableServerPortableLibrary"/>
		<rdfs:subClassOf rdf:resource="&j2se-1_6;OrgOmgDynamicLibrary"/>
		<rdfs:subClassOf rdf:resource="&j2se-1_6;OrgOmgDynamicAnyLibrary"/>
		<rdfs:subClassOf rdf:resource="&j2se-1_6;OrgOmgDynamicAnyDynAnyFactoryPackageLibrary"/>
		<rdfs:subClassOf rdf:resource="&j2se-1_6;OrgOmgDynamicAnyDynAnyPackageLibrary"/>
		<rdfs:subClassOf rdf:resource="&j2se-1_6;OrgOmgIOPLibrary"/>
		<rdfs:subClassOf rdf:resource="&j2se-1_6;OrgOmgIOPCodecFactoryPackageLibrary"/>
		<rdfs:subClassOf rdf:resource="&j2se-1_6;OrgOmgIOPCodecPackageLibrary"/>
		<rdfs:subClassOf rdf:resource="&j2se-1_6;OrgOmgMessagingLibrary"/>
		<rdfs:subClassOf rdf:resource="&j2se-1_6;OrgOmgPortableInterceptorLibrary"/>
		<rdfs:subClassOf rdf:resource="&j2se-1_6;OrgOmgPortableInterceptorORBInitInfoPackageLibrary"/>
		<rdfs:subClassOf rdf:resource="&j2se-1_6;OrgOmgSendingContextLibrary"/>
		<rdfs:subClassOf rdf:resource="&j2se-1_6;OrgOmgStubJavaRmiLibrary"/>
		<rdfs:subClassOf rdf:resource="&j2se-1_6;OrgOmgStubJavaxManagementRemoteRmiLibrary"/>
		<rdfs:subClassOf rdf:resource="&j2se-1_6;OrgXmlSaxLibrary"/>
		<rdfs:subClassOf rdf:resource="&j2se-1_6;OrgXmlSaxExtLibrary"/>
		<rdfs:subClassOf rdf:resource="&j2se-1_6;OrgXmlSaxHelpersLibrary"/>
		<rdfs:subClassOf rdf:resource="&j2se-1_6;OrgIetfJgssLibrary"/>
		<rdfs:subClassOf rdf:resource="&j2se-1_6;SunAwtLibrary"/>
		<rdfs:comment xml:lang="en">JavaLibrary implementing the entire API for j2se-1_6</rdfs:comment>
	</owl:Class>
	<owl:Class rdf:about="&j2se-1_6;J2se-1_6">
		<rdfs:subClassOf rdf:resource="&java;JRE"/>
		<rdfs:subClassOf>
			<owl:Restriction>
				<owl:onProperty rdf:resource="&java;providesBuiltinJavaLibrary"/>
				<owl:someValuesFrom rdf:resource="&j2se-1_6;J2se-1_6ClassLibrary"/>
			</owl:Restriction>
		</rdfs:subClassOf>
		<rdfs:comment xml:lang="en">j2se-1_6 Java Runtime Environment</rdfs:comment>
	</owl:Class>
	<owl:Class rdf:about="&j2se-1_6;JavaAppletLibrary">
		<rdfs:subClassOf rdf:resource="&j2se-1_5;JavaAppletLibrary"/>
		<rdfs:seeAlso rdf:resource="&j2se-1_6;JavaUtilLibrary"/>
		<rdfs:seeAlso rdf:resource="&j2se-1_6;JavaLangLibrary"/>
		<rdfs:seeAlso rdf:resource="&j2se-1_6;JavaAwtLibrary"/>
		<rdfs:seeAlso rdf:resource="&j2se-1_6;JavaNetLibrary"/>
		<rdfs:seeAlso rdf:resource="&j2se-1_6;JavaIoLibrary"/>
		<rdfs:seeAlso rdf:resource="&j2se-1_6;JavaxAccessibilityLibrary"/>
		<rdfs:comment xml:lang="en">JavaLibrary implementing the java.applet package for j2se-1_6</rdfs:comment>
	</owl:Class>
	<owl:Class rdf:about="&j2se-1_6;JavaAwtLibrary">
		<rdfs:subClassOf rdf:resource="&j2se-1_5;JavaAwtLibrary"/>
		<rdfs:seeAlso rdf:resource="&j2se-1_6;JavaAwtDndLibrary"/>
		<rdfs:seeAlso rdf:resource="&j2se-1_6;JavaxSwingTextLibrary"/>
		<rdfs:seeAlso rdf:resource="&j2se-1_6;JavaAwtImageLibrary"/>
		<rdfs:seeAlso rdf:resource="&j2se-1_6;JavaTextLibrary"/>
		<rdfs:seeAlso rdf:resource="&j2se-1_6;JavaxAccessibilityLibrary"/>
		<rdfs:seeAlso rdf:resource="&j2se-1_6;JavaAwtFontLibrary"/>
		<rdfs:seeAlso rdf:resource="&j2se-1_6;JavaNetLibrary"/>
		<rdfs:seeAlso rdf:resource="&j2se-1_6;JavaIoLibrary"/>
		<rdfs:seeAlso rdf:resource="&j2se-1_6;JavaAwtDatatransferLibrary"/>
		<rdfs:seeAlso rdf:resource="&j2se-1_6;JavaAwtColorLibrary"/>
		<rdfs:seeAlso rdf:resource="&j2se-1_6;JavaSecurityLibrary"/>
		<rdfs:seeAlso rdf:resource="&j2se-1_6;JavaAwtDndPeerLibrary"/>
		<rdfs:seeAlso rdf:resource="&j2se-1_6;JavaUtilLibrary"/>
		<rdfs:seeAlso rdf:resource="&j2se-1_6;JavaAwtImageRenderableLibrary"/>
		<rdfs:seeAlso rdf:resource="&j2se-1_6;JavaAwtGeomLibrary"/>
		<rdfs:seeAlso rdf:resource="&j2se-1_6;JavaAwtPeerLibrary"/>
		<rdfs:seeAlso rdf:resource="&j2se-1_6;JavaBeansLibrary"/>
		<rdfs:seeAlso rdf:resource="&j2se-1_6;JavaAwtEventLibrary"/>
		<rdfs:seeAlso rdf:resource="&j2se-1_6;JavaLangLibrary"/>
		<rdfs:seeAlso rdf:resource="&j2se-1_6;JavaAwtImLibrary"/>
		<rdfs:comment xml:lang="en">JavaLibrary implementing the java.awt package for j2se-1_6</rdfs:comment>
	</owl:Class>
	<owl:Class rdf:about="&j2se-1_6;JavaAwtEventLibrary">
		<rdfs:subClassOf rdf:resource="&j2se-1_5;JavaAwtEventLibrary"/>
		<rdfs:seeAlso rdf:resource="&j2se-1_6;JavaAwtFontLibrary"/>
		<rdfs:seeAlso rdf:resource="&j2se-1_6;JavaUtilLibrary"/>
		<rdfs:seeAlso rdf:resource="&j2se-1_6;JavaLangLibrary"/>
		<rdfs:seeAlso rdf:resource="&j2se-1_6;JavaAwtLibrary"/>
		<rdfs:seeAlso rdf:resource="&j2se-1_6;JavaTextLibrary"/>
		<rdfs:comment xml:lang="en">JavaLibrary implementing the java.awt.event package for j2se-1_6</rdfs:comment>
	</owl:Class>
	<owl:Class rdf:about="&j2se-1_6;JavaAwtColorLibrary">
		<owl:equivalentClass rdf:resource="&j2se-1_5;JavaAwtColorLibrary"/>
		<rdfs:subClassOf rdf:resource="&java;JavaLibrary"/>
		<rdfs:seeAlso rdf:resource="&j2se-1_6;JavaIoLibrary"/>
		<rdfs:seeAlso rdf:resource="&j2se-1_6;JavaLangLibrary"/>
		<rdfs:comment xml:lang="en">JavaLibrary implementing the java.awt.color package for j2se-1_6</rdfs:comment>
	</owl:Class>
	<owl:Class rdf:about="&j2se-1_6;JavaAwtDatatransferLibrary">
		<owl:equivalentClass rdf:resource="&j2se-1_5;JavaAwtDatatransferLibrary"/>
		<rdfs:subClassOf rdf:resource="&java;JavaLibrary"/>
		<rdfs:seeAlso rdf:resource="&j2se-1_6;JavaUtilLibrary"/>
		<rdfs:seeAlso rdf:resource="&j2se-1_6;JavaLangLibrary"/>
		<rdfs:seeAlso rdf:resource="&j2se-1_6;JavaIoLibrary"/>
		<rdfs:comment xml:lang="en">JavaLibrary implementing the java.awt.datatransfer package for j2se-1_6</rdfs:comment>
	</owl:Class>
	<owl:Class rdf:about="&j2se-1_6;JavaAwtDndLibrary">
		<owl:equivalentClass rdf:resource="&j2se-1_5;JavaAwtDndLibrary"/>
		<rdfs:subClassOf rdf:resource="&java;JavaLibrary"/>
		<rdfs:seeAlso rdf:resource="&j2se-1_6;JavaUtilLibrary"/>
		<rdfs:seeAlso rdf:resource="&j2se-1_6;JavaAwtLibrary"/>
		<rdfs:seeAlso rdf:resource="&j2se-1_6;JavaAwtPeerLibrary"/>
		<rdfs:seeAlso rdf:resource="&j2se-1_6;JavaIoLibrary"/>
		<rdfs:seeAlso rdf:resource="&j2se-1_6;JavaAwtEventLibrary"/>
		<rdfs:seeAlso rdf:resource="&j2se-1_6;JavaAwtDatatransferLibrary"/>
		<rdfs:seeAlso rdf:resource="&j2se-1_6;JavaLangLibrary"/>
		<rdfs:seeAlso rdf:resource="&j2se-1_6;JavaAwtDndPeerLibrary"/>
		<rdfs:comment xml:lang="en">JavaLibrary implementing the java.awt.dnd package for j2se-1_6</rdfs:comment>
	</owl:Class>
	<owl:Class rdf:about="&j2se-1_6;JavaAwtDndPeerLibrary">
		<owl:equivalentClass rdf:resource="&j2se-1_5;JavaAwtDndPeerLibrary"/>
		<rdfs:subClassOf rdf:resource="&java;JavaLibrary"/>
		<rdfs:seeAlso rdf:resource="&j2se-1_6;JavaAwtLibrary"/>
		<rdfs:seeAlso rdf:resource="&j2se-1_6;JavaAwtDndLibrary"/>
		<rdfs:seeAlso rdf:resource="&j2se-1_6;JavaAwtDatatransferLibrary"/>
		<rdfs:comment xml:lang="en">JavaLibrary implementing the java.awt.dnd.peer package for j2se-1_6</rdfs:comment>
	</owl:Class>
	<owl:Class rdf:about="&j2se-1_6;JavaAwtFontLibrary">
		<rdfs:subClassOf rdf:resource="&j2se-1_5;JavaAwtFontLibrary"/>
		<rdfs:seeAlso rdf:resource="&j2se-1_6;JavaUtilLibrary"/>
		<rdfs:seeAlso rdf:resource="&j2se-1_6;JavaAwtGeomLibrary"/>
		<rdfs:seeAlso rdf:resource="&j2se-1_6;JavaLangLibrary"/>
		<rdfs:seeAlso rdf:resource="&j2se-1_6;JavaAwtLibrary"/>
		<rdfs:seeAlso rdf:resource="&j2se-1_6;JavaTextLibrary"/>
		<rdfs:seeAlso rdf:resource="&j2se-1_6;JavaIoLibrary"/>
		<rdfs:comment xml:lang="en">JavaLibrary implementing the java.awt.font package for j2se-1_6</rdfs:comment>
	</owl:Class>
	<owl:Class rdf:about="&j2se-1_6;JavaAwtGeomLibrary">
		<rdfs:subClassOf rdf:resource="&java;JavaLibrary"/>
		<rdfs:seeAlso rdf:resource="&j2se-1_6;JavaIoLibrary"/>
		<rdfs:seeAlso rdf:resource="&j2se-1_6;JavaLangLibrary"/>
		<rdfs:seeAlso rdf:resource="&j2se-1_6;JavaAwtLibrary"/>
		<rdfs:comment xml:lang="en">JavaLibrary implementing the java.awt.geom package for j2se-1_6</rdfs:comment>
	</owl:Class>
	<owl:Class rdf:about="&j2se-1_6;JavaAwtImLibrary">
		<owl:equivalentClass rdf:resource="&j2se-1_5;JavaAwtImLibrary"/>
		<rdfs:subClassOf rdf:resource="&java;JavaLibrary"/>
		<rdfs:seeAlso rdf:resource="&j2se-1_6;JavaAwtFontLibrary"/>
		<rdfs:seeAlso rdf:resource="&j2se-1_6;JavaUtilLibrary"/>
		<rdfs:seeAlso rdf:resource="&j2se-1_6;JavaLangLibrary"/>
		<rdfs:seeAlso rdf:resource="&j2se-1_6;JavaAwtLibrary"/>
		<rdfs:seeAlso rdf:resource="&j2se-1_6;JavaTextLibrary"/>
		<rdfs:comment xml:lang="en">JavaLibrary implementing the java.awt.im package for j2se-1_6</rdfs:comment>
	</owl:Class>
	<owl:Class rdf:about="&j2se-1_6;JavaAwtImSpiLibrary">
		<owl:equivalentClass rdf:resource="&j2se-1_5;JavaAwtImSpiLibrary"/>
		<rdfs:subClassOf rdf:resource="&java;JavaLibrary"/>
		<rdfs:seeAlso rdf:resource="&j2se-1_6;JavaAwtFontLibrary"/>
		<rdfs:seeAlso rdf:resource="&j2se-1_6;JavaUtilLibrary"/>
		<rdfs:seeAlso rdf:resource="&j2se-1_6;JavaAwtImLibrary"/>
		<rdfs:seeAlso rdf:resource="&j2se-1_6;JavaLangLibrary"/>
		<rdfs:seeAlso rdf:resource="&j2se-1_6;JavaAwtLibrary"/>
		<rdfs:seeAlso rdf:resource="&j2se-1_6;JavaxSwingLibrary"/>
		<rdfs:seeAlso rdf:resource="&j2se-1_6;JavaTextLibrary"/>
		<rdfs:comment xml:lang="en">JavaLibrary implementing the java.awt.im.spi package for j2se-1_6</rdfs:comment>
	</owl:Class>
	<owl:Class rdf:about="&j2se-1_6;JavaAwtImageLibrary">
		<rdfs:subClassOf rdf:resource="&j2se-1_5;JavaAwtImageLibrary"/>
		<rdfs:seeAlso rdf:resource="&j2se-1_6;JavaUtilLibrary"/>
		<rdfs:seeAlso rdf:resource="&j2se-1_6;JavaAwtGeomLibrary"/>
		<rdfs:seeAlso rdf:resource="&j2se-1_6;JavaLangLibrary"/>
		<rdfs:seeAlso rdf:resource="&j2se-1_6;JavaAwtLibrary"/>
		<rdfs:seeAlso rdf:resource="&j2se-1_6;JavaAwtColorLibrary"/>
		<rdfs:seeAlso rdf:resource="&j2se-1_6;JavaMathLibrary"/>
		<rdfs:comment xml:lang="en">JavaLibrary implementing the java.awt.image package for j2se-1_6</rdfs:comment>
	</owl:Class>
	<owl:Class rdf:about="&j2se-1_6;JavaAwtImageRenderableLibrary">
		<owl:equivalentClass rdf:resource="&j2se-1_5;JavaAwtImageRenderableLibrary"/>
		<rdfs:subClassOf rdf:resource="&java;JavaLibrary"/>
		<rdfs:seeAlso rdf:resource="&j2se-1_6;JavaUtilLibrary"/>
		<rdfs:seeAlso rdf:resource="&j2se-1_6;JavaAwtGeomLibrary"/>
		<rdfs:seeAlso rdf:resource="&j2se-1_6;JavaLangLibrary"/>
		<rdfs:seeAlso rdf:resource="&j2se-1_6;JavaAwtLibrary"/>
		<rdfs:seeAlso rdf:resource="&j2se-1_6;JavaAwtImageLibrary"/>
		<rdfs:seeAlso rdf:resource="&j2se-1_6;JavaIoLibrary"/>
		<rdfs:comment xml:lang="en">JavaLibrary implementing the java.awt.image.renderable package for j2se-1_6</rdfs:comment>
	</owl:Class>
	<owl:Class rdf:about="&j2se-1_6;JavaAwtPeerLibrary">
		<rdfs:subClassOf rdf:resource="&java;JavaLibrary"/>
		<rdfs:seeAlso rdf:resource="&j2se-1_6;JavaAwtLibrary"/>
		<rdfs:seeAlso rdf:resource="&j2se-1_6;JavaNetLibrary"/>
		<rdfs:seeAlso rdf:resource="&j2se-1_6;JavaAwtImageLibrary"/>
		<rdfs:seeAlso rdf:resource="&j2se-1_6;JavaIoLibrary"/>
		<rdfs:seeAlso rdf:resource="&j2se-1_6;JavaAwtEventLibrary"/>
		<rdfs:seeAlso rdf:resource="&j2se-1_6;JavaLangLibrary"/>
		<rdfs:seeAlso rdf:resource="&j2se-1_6;JavaAwtImLibrary"/>
		<rdfs:comment xml:lang="en">JavaLibrary implementing the java.awt.peer package for j2se-1_6</rdfs:comment>
	</owl:Class>
	<owl:Class rdf:about="&j2se-1_6;JavaAwtPrintLibrary">
		<rdfs:subClassOf rdf:resource="&j2se-1_5;JavaAwtPrintLibrary"/>
		<rdfs:seeAlso rdf:resource="&j2se-1_6;JavaIoLibrary"/>
		<rdfs:seeAlso rdf:resource="&j2se-1_6;JavaLangLibrary"/>
		<rdfs:seeAlso rdf:resource="&j2se-1_6;JavaAwtLibrary"/>
		<rdfs:seeAlso rdf:resource="&j2se-1_6;JavaxPrintLibrary"/>
		<rdfs:seeAlso rdf:resource="&j2se-1_6;JavaxPrintAttributeLibrary"/>
		<rdfs:comment xml:lang="en">JavaLibrary implementing the java.awt.print package for j2se-1_6</rdfs:comment>
	</owl:Class>
	<owl:Class rdf:about="&j2se-1_6;JavaLangLibrary">
		<rdfs:subClassOf rdf:resource="&j2se-1_5;JavaLangLibrary"/>
		<rdfs:seeAlso rdf:resource="&j2se-1_6;JavaUtilLibrary"/>
		<rdfs:seeAlso rdf:resource="&j2se-1_6;JavaNioChannelsLibrary"/>
		<rdfs:seeAlso rdf:resource="&j2se-1_6;JavaNetLibrary"/>
		<rdfs:seeAlso rdf:resource="&j2se-1_6;JavaNioLibrary"/>
		<rdfs:seeAlso rdf:resource="&j2se-1_6;JavaIoLibrary"/>
		<rdfs:seeAlso rdf:resource="&j2se-1_6;JavaLangAnnotationLibrary"/>
		<rdfs:seeAlso rdf:resource="&j2se-1_6;JavaNioCharsetLibrary"/>
		<rdfs:seeAlso rdf:resource="&j2se-1_6;JavaSecurityLibrary"/>
		<rdfs:seeAlso rdf:resource="&j2se-1_6;JavaLangReflectLibrary"/>
		<rdfs:comment xml:lang="en">JavaLibrary implementing the java.lang package for j2se-1_6</rdfs:comment>
	</owl:Class>
	<owl:Class rdf:about="&j2se-1_6;JavaLangAnnotationLibrary">
		<rdfs:subClassOf rdf:resource="&j2se-1_5;JavaLangAnnotationLibrary"/>
		<rdfs:seeAlso rdf:resource="&j2se-1_6;JavaLangLibrary"/>
		<rdfs:seeAlso rdf:resource="&j2se-1_6;JavaLangReflectLibrary"/>
		<rdfs:comment xml:lang="en">JavaLibrary implementing the java.lang.annotation package for j2se-1_6</rdfs:comment>
	</owl:Class>
	<owl:Class rdf:about="&j2se-1_6;JavaLangReflectLibrary">
		<owl:equivalentClass rdf:resource="&j2se-1_5;JavaLangReflectLibrary"/>
		<rdfs:subClassOf rdf:resource="&java;JavaLibrary"/>
		<rdfs:seeAlso rdf:resource="&j2se-1_6;JavaIoLibrary"/>
		<rdfs:seeAlso rdf:resource="&j2se-1_6;JavaLangLibrary"/>
		<rdfs:seeAlso rdf:resource="&j2se-1_6;JavaSecurityLibrary"/>
		<rdfs:seeAlso rdf:resource="&j2se-1_6;JavaLangAnnotationLibrary"/>
		<rdfs:comment xml:lang="en">JavaLibrary implementing the java.lang.reflect package for j2se-1_6</rdfs:comment>
	</owl:Class>
	<owl:Class rdf:about="&j2se-1_6;JavaLangInstrumentLibrary">
		<rdfs:subClassOf rdf:resource="&j2se-1_5;JavaLangInstrumentLibrary"/>
		<rdfs:seeAlso rdf:resource="&j2se-1_6;JavaUtilJarLibrary"/>
		<rdfs:seeAlso rdf:resource="&j2se-1_6;JavaLangLibrary"/>
		<rdfs:seeAlso rdf:resource="&j2se-1_6;JavaSecurityLibrary"/>
		<rdfs:comment xml:lang="en">JavaLibrary implementing the java.lang.instrument package for j2se-1_6</rdfs:comment>
	</owl:Class>
	<owl:Class rdf:about="&j2se-1_6;JavaLangManagementLibrary">
		<rdfs:subClassOf rdf:resource="&j2se-1_5;JavaLangManagementLibrary"/>
		<rdfs:seeAlso rdf:resource="&j2se-1_6;JavaUtilLibrary"/>
		<rdfs:seeAlso rdf:resource="&j2se-1_6;JavaLangLibrary"/>
		<rdfs:seeAlso rdf:resource="&j2se-1_6;JavaSecurityLibrary"/>
		<rdfs:seeAlso rdf:resource="&j2se-1_6;JavaxManagementLibrary"/>
		<rdfs:seeAlso rdf:resource="&j2se-1_6;JavaxManagementOpenmbeanLibrary"/>
		<rdfs:comment xml:lang="en">JavaLibrary implementing the java.lang.management package for j2se-1_6</rdfs:comment>
	</owl:Class>
	<owl:Class rdf:about="&j2se-1_6;JavaLangRefLibrary">
		<owl:equivalentClass rdf:resource="&j2se-1_5;JavaLangRefLibrary"/>
		<rdfs:subClassOf rdf:resource="&java;JavaLibrary"/>
		<rdfs:seeAlso rdf:resource="&j2se-1_6;JavaLangLibrary"/>
		<rdfs:comment xml:lang="en">JavaLibrary implementing the java.lang.ref package for j2se-1_6</rdfs:comment>
	</owl:Class>
	<owl:Class rdf:about="&j2se-1_6;JavaIoLibrary">
		<rdfs:subClassOf rdf:resource="&j2se-1_5;JavaIoLibrary"/>
		<rdfs:seeAlso rdf:resource="&j2se-1_6;JavaUtilLibrary"/>
		<rdfs:seeAlso rdf:resource="&j2se-1_6;JavaNioChannelsLibrary"/>
		<rdfs:seeAlso rdf:resource="&j2se-1_6;JavaNioCharsetLibrary"/>
		<rdfs:seeAlso rdf:resource="&j2se-1_6;JavaLangLibrary"/>
		<rdfs:seeAlso rdf:resource="&j2se-1_6;JavaSecurityLibrary"/>
		<rdfs:seeAlso rdf:resource="&j2se-1_6;JavaNetLibrary"/>
		<rdfs:seeAlso rdf:resource="&j2se-1_6;JavaNioLibrary"/>
		<rdfs:comment xml:lang="en">JavaLibrary implementing the java.io package for j2se-1_6</rdfs:comment>
	</owl:Class>
	<owl:Class rdf:about="&j2se-1_6;JavaUtilLibrary">
		<rdfs:subClassOf rdf:resource="&j2se-1_5;JavaUtilLibrary"/>
		<rdfs:seeAlso rdf:resource="&j2se-1_6;JavaNioChannelsLibrary"/>
		<rdfs:seeAlso rdf:resource="&j2se-1_6;JavaIoLibrary"/>
		<rdfs:seeAlso rdf:resource="&j2se-1_6;JavaLangLibrary"/>
		<rdfs:seeAlso rdf:resource="&j2se-1_6;JavaSecurityLibrary"/>
		<rdfs:seeAlso rdf:resource="&j2se-1_6;JavaMathLibrary"/>
		<rdfs:seeAlso rdf:resource="&j2se-1_6;JavaUtilRegexLibrary"/>
		<rdfs:comment xml:lang="en">JavaLibrary implementing the java.util package for j2se-1_6</rdfs:comment>
	</owl:Class>
	<owl:Class rdf:about="&j2se-1_6;JavaUtilSpiLibrary">
		<rdfs:subClassOf rdf:resource="&java;JavaLibrary"/>
		<rdfs:seeAlso rdf:resource="&j2se-1_6;JavaUtilLibrary"/>
		<rdfs:seeAlso rdf:resource="&j2se-1_6;JavaLangLibrary"/>
		<rdfs:comment xml:lang="en">JavaLibrary implementing the java.util.spi package for j2se-1_6</rdfs:comment>
	</owl:Class>
	<owl:Class rdf:about="&j2se-1_6;JavaUtilConcurrentLibrary">
		<rdfs:subClassOf rdf:resource="&java;JavaLibrary"/>
		<rdfs:seeAlso rdf:resource="&j2se-1_6;JavaUtilLibrary"/>
		<rdfs:seeAlso rdf:resource="&j2se-1_6;JavaIoLibrary"/>
		<rdfs:seeAlso rdf:resource="&j2se-1_6;JavaLangLibrary"/>
		<rdfs:seeAlso rdf:resource="&j2se-1_6;JavaSecurityLibrary"/>
		<rdfs:comment xml:lang="en">JavaLibrary implementing the java.util.concurrent package for j2se-1_6</rdfs:comment>
	</owl:Class>
	<owl:Class rdf:about="&j2se-1_6;JavaUtilConcurrentAtomicLibrary">
		<rdfs:subClassOf rdf:resource="&j2se-1_5;JavaUtilConcurrentAtomicLibrary"/>
		<rdfs:seeAlso rdf:resource="&j2se-1_6;JavaIoLibrary"/>
		<rdfs:seeAlso rdf:resource="&j2se-1_6;JavaLangLibrary"/>
		<rdfs:comment xml:lang="en">JavaLibrary implementing the java.util.concurrent.atomic package for j2se-1_6</rdfs:comment>
	</owl:Class>
	<owl:Class rdf:about="&j2se-1_6;JavaUtilConcurrentLocksLibrary">
		<rdfs:subClassOf rdf:resource="&j2se-1_5;JavaUtilConcurrentLocksLibrary"/>
		<rdfs:seeAlso rdf:resource="&j2se-1_6;JavaUtilConcurrentLibrary"/>
		<rdfs:seeAlso rdf:resource="&j2se-1_6;JavaUtilLibrary"/>
		<rdfs:seeAlso rdf:resource="&j2se-1_6;JavaIoLibrary"/>
		<rdfs:seeAlso rdf:resource="&j2se-1_6;JavaLangLibrary"/>
		<rdfs:comment xml:lang="en">JavaLibrary implementing the java.util.concurrent.locks package for j2se-1_6</rdfs:comment>
	</owl:Class>
	<owl:Class rdf:about="&j2se-1_6;JavaUtilJarLibrary">
		<owl:equivalentClass rdf:resource="&j2se-1_5;JavaUtilJarLibrary"/>
		<rdfs:subClassOf rdf:resource="&java;JavaLibrary"/>
		<rdfs:seeAlso rdf:resource="&j2se-1_6;JavaUtilLibrary"/>
		<rdfs:seeAlso rdf:resource="&j2se-1_6;JavaLangLibrary"/>
		<rdfs:seeAlso rdf:resource="&j2se-1_6;JavaBeansLibrary"/>
		<rdfs:seeAlso rdf:resource="&j2se-1_6;JavaUtilZipLibrary"/>
		<rdfs:seeAlso rdf:resource="&j2se-1_6;JavaIoLibrary"/>
		<rdfs:comment xml:lang="en">JavaLibrary implementing the java.util.jar package for j2se-1_6</rdfs:comment>
	</owl:Class>
	<owl:Class rdf:about="&j2se-1_6;JavaUtilZipLibrary">
		<rdfs:subClassOf rdf:resource="&j2se-1_5;JavaUtilZipLibrary"/>
		<rdfs:seeAlso rdf:resource="&j2se-1_6;JavaUtilLibrary"/>
		<rdfs:seeAlso rdf:resource="&j2se-1_6;JavaLangLibrary"/>
		<rdfs:seeAlso rdf:resource="&j2se-1_6;JavaIoLibrary"/>
		<rdfs:comment xml:lang="en">JavaLibrary implementing the java.util.zip package for j2se-1_6</rdfs:comment>
	</owl:Class>
	<owl:Class rdf:about="&j2se-1_6;JavaUtilLoggingLibrary">
		<rdfs:subClassOf rdf:resource="&j2se-1_5;JavaUtilLoggingLibrary"/>
		<rdfs:seeAlso rdf:resource="&j2se-1_6;JavaUtilLibrary"/>
		<rdfs:seeAlso rdf:resource="&j2se-1_6;JavaLangLibrary"/>
		<rdfs:seeAlso rdf:resource="&j2se-1_6;JavaSecurityLibrary"/>
		<rdfs:seeAlso rdf:resource="&j2se-1_6;JavaBeansLibrary"/>
		<rdfs:seeAlso rdf:resource="&j2se-1_6;JavaIoLibrary"/>
		<rdfs:comment xml:lang="en">JavaLibrary implementing the java.util.logging package for j2se-1_6</rdfs:comment>
	</owl:Class>
	<owl:Class rdf:about="&j2se-1_6;JavaUtilPrefsLibrary">
		<owl:equivalentClass rdf:resource="&j2se-1_5;JavaUtilPrefsLibrary"/>
		<rdfs:subClassOf rdf:resource="&java;JavaLibrary"/>
		<rdfs:seeAlso rdf:resource="&j2se-1_6;JavaUtilLibrary"/>
		<rdfs:seeAlso rdf:resource="&j2se-1_6;JavaIoLibrary"/>
		<rdfs:seeAlso rdf:resource="&j2se-1_6;JavaLangLibrary"/>
		<rdfs:comment xml:lang="en">JavaLibrary implementing the java.util.prefs package for j2se-1_6</rdfs:comment>
	</owl:Class>
	<owl:Class rdf:about="&j2se-1_6;JavaUtilRegexLibrary">
		<owl:equivalentClass rdf:resource="&j2se-1_5;JavaUtilRegexLibrary"/>
		<rdfs:subClassOf rdf:resource="&java;JavaLibrary"/>
		<rdfs:seeAlso rdf:resource="&j2se-1_6;JavaIoLibrary"/>
		<rdfs:seeAlso rdf:resource="&j2se-1_6;JavaLangLibrary"/>
		<rdfs:comment xml:lang="en">JavaLibrary implementing the java.util.regex package for j2se-1_6</rdfs:comment>
	</owl:Class>
	<owl:Class rdf:about="&j2se-1_6;JavaBeansLibrary">
		<rdfs:subClassOf rdf:resource="&j2se-1_5;JavaBeansLibrary"/>
		<rdfs:seeAlso rdf:resource="&j2se-1_6;JavaAppletLibrary"/>
		<rdfs:seeAlso rdf:resource="&j2se-1_6;JavaUtilLibrary"/>
		<rdfs:seeAlso rdf:resource="&j2se-1_6;JavaLangLibrary"/>
		<rdfs:seeAlso rdf:resource="&j2se-1_6;JavaAwtLibrary"/>
		<rdfs:seeAlso rdf:resource="&j2se-1_6;JavaIoLibrary"/>
		<rdfs:seeAlso rdf:resource="&j2se-1_6;JavaBeansBeancontextLibrary"/>
		<rdfs:seeAlso rdf:resource="&j2se-1_6;JavaLangAnnotationLibrary"/>
		<rdfs:seeAlso rdf:resource="&j2se-1_6;JavaLangReflectLibrary"/>
		<rdfs:comment xml:lang="en">JavaLibrary implementing the java.beans package for j2se-1_6</rdfs:comment>
	</owl:Class>
	<owl:Class rdf:about="&j2se-1_6;JavaBeansBeancontextLibrary">
		<owl:equivalentClass rdf:resource="&j2se-1_5;JavaBeansBeancontextLibrary"/>
		<rdfs:subClassOf rdf:resource="&java;JavaLibrary"/>
		<rdfs:seeAlso rdf:resource="&j2se-1_6;JavaUtilLibrary"/>
		<rdfs:seeAlso rdf:resource="&j2se-1_6;JavaAwtLibrary"/>
		<rdfs:seeAlso rdf:resource="&j2se-1_6;JavaNetLibrary"/>
		<rdfs:seeAlso rdf:resource="&j2se-1_6;JavaBeansLibrary"/>
		<rdfs:seeAlso rdf:resource="&j2se-1_6;JavaIoLibrary"/>
		<rdfs:seeAlso rdf:resource="&j2se-1_6;JavaLangLibrary"/>
		<rdfs:comment xml:lang="en">JavaLibrary implementing the java.beans.beancontext package for j2se-1_6</rdfs:comment>
	</owl:Class>
	<owl:Class rdf:about="&j2se-1_6;JavaSecurityLibrary">
		<rdfs:subClassOf rdf:resource="&j2se-1_5;JavaSecurityLibrary"/>
		<rdfs:seeAlso rdf:resource="&j2se-1_6;JavaUtilLibrary"/>
		<rdfs:seeAlso rdf:resource="&j2se-1_6;JavaxSecurityAuthCallbackLibrary"/>
		<rdfs:seeAlso rdf:resource="&j2se-1_6;JavaxSecurityAuthLoginLibrary"/>
		<rdfs:seeAlso rdf:resource="&j2se-1_6;JavaNetLibrary"/>
		<rdfs:seeAlso rdf:resource="&j2se-1_6;JavaxCryptoLibrary"/>
		<rdfs:seeAlso rdf:resource="&j2se-1_6;JavaxSecurityAuthLibrary"/>
		<rdfs:seeAlso rdf:resource="&j2se-1_6;JavaNioLibrary"/>
		<rdfs:seeAlso rdf:resource="&j2se-1_6;JavaIoLibrary"/>
		<rdfs:seeAlso rdf:resource="&j2se-1_6;JavaLangLibrary"/>
		<rdfs:seeAlso rdf:resource="&j2se-1_6;JavaSecuritySpecLibrary"/>
		<rdfs:seeAlso rdf:resource="&j2se-1_6;JavaSecurityCertLibrary"/>
		<rdfs:comment xml:lang="en">JavaLibrary implementing the java.security package for j2se-1_6</rdfs:comment>
	</owl:Class>
	<owl:Class rdf:about="&j2se-1_6;JavaSecurityAclLibrary">
		<owl:equivalentClass rdf:resource="&j2se-1_5;JavaSecurityAclLibrary"/>
		<rdfs:subClassOf rdf:resource="&java;JavaLibrary"/>
		<rdfs:seeAlso rdf:resource="&j2se-1_6;JavaUtilLibrary"/>
		<rdfs:seeAlso rdf:resource="&j2se-1_6;JavaLangLibrary"/>
		<rdfs:seeAlso rdf:resource="&j2se-1_6;JavaSecurityLibrary"/>
		<rdfs:comment xml:lang="en">JavaLibrary implementing the java.security.acl package for j2se-1_6</rdfs:comment>
	</owl:Class>
	<owl:Class rdf:about="&j2se-1_6;JavaSecurityCertLibrary">
		<owl:equivalentClass rdf:resource="&j2se-1_5;JavaSecurityCertLibrary"/>
		<rdfs:subClassOf rdf:resource="&java;JavaLibrary"/>
		<rdfs:seeAlso rdf:resource="&j2se-1_6;JavaUtilLibrary"/>
		<rdfs:seeAlso rdf:resource="&j2se-1_6;JavaLangLibrary"/>
		<rdfs:seeAlso rdf:resource="&j2se-1_6;JavaSecurityLibrary"/>
		<rdfs:seeAlso rdf:resource="&j2se-1_6;JavaxSecurityAuthX500Library"/>
		<rdfs:seeAlso rdf:resource="&j2se-1_6;JavaMathLibrary"/>
		<rdfs:seeAlso rdf:resource="&j2se-1_6;JavaIoLibrary"/>
		<rdfs:comment xml:lang="en">JavaLibrary implementing the java.security.cert package for j2se-1_6</rdfs:comment>
	</owl:Class>
	<owl:Class rdf:about="&j2se-1_6;JavaSecurityInterfacesLibrary">
		<owl:equivalentClass rdf:resource="&j2se-1_5;JavaSecurityInterfacesLibrary"/>
		<rdfs:subClassOf rdf:resource="&java;JavaLibrary"/>
		<rdfs:seeAlso rdf:resource="&j2se-1_6;JavaMathLibrary"/>
		<rdfs:seeAlso rdf:resource="&j2se-1_6;JavaSecuritySpecLibrary"/>
		<rdfs:seeAlso rdf:resource="&j2se-1_6;JavaSecurityLibrary"/>
		<rdfs:comment xml:lang="en">JavaLibrary implementing the java.security.interfaces package for j2se-1_6</rdfs:comment>
	</owl:Class>
	<owl:Class rdf:about="&j2se-1_6;JavaSecuritySpecLibrary">
		<owl:equivalentClass rdf:resource="&j2se-1_5;JavaSecuritySpecLibrary"/>
		<rdfs:subClassOf rdf:resource="&java;JavaLibrary"/>
		<rdfs:seeAlso rdf:resource="&j2se-1_6;JavaMathLibrary"/>
		<rdfs:seeAlso rdf:resource="&j2se-1_6;JavaSecurityInterfacesLibrary"/>
		<rdfs:seeAlso rdf:resource="&j2se-1_6;JavaLangLibrary"/>
		<rdfs:seeAlso rdf:resource="&j2se-1_6;JavaSecurityLibrary"/>
		<rdfs:comment xml:lang="en">JavaLibrary implementing the java.security.spec package for j2se-1_6</rdfs:comment>
	</owl:Class>
	<owl:Class rdf:about="&j2se-1_6;JavaMathLibrary">
		<rdfs:subClassOf rdf:resource="&j2se-1_5;JavaMathLibrary"/>
		<rdfs:seeAlso rdf:resource="&j2se-1_6;JavaUtilLibrary"/>
		<rdfs:seeAlso rdf:resource="&j2se-1_6;JavaIoLibrary"/>
		<rdfs:seeAlso rdf:resource="&j2se-1_6;JavaLangLibrary"/>
		<rdfs:comment xml:lang="en">JavaLibrary implementing the java.math package for j2se-1_6</rdfs:comment>
	</owl:Class>
	<owl:Class rdf:about="&j2se-1_6;JavaNetLibrary">
		<rdfs:subClassOf rdf:resource="&j2se-1_5;JavaNetLibrary"/>
		<rdfs:seeAlso rdf:resource="&j2se-1_6;JavaUtilLibrary"/>
		<rdfs:seeAlso rdf:resource="&j2se-1_6;JavaNioChannelsLibrary"/>
		<rdfs:seeAlso rdf:resource="&j2se-1_6;JavaIoLibrary"/>
		<rdfs:seeAlso rdf:resource="&j2se-1_6;JavaUtilJarLibrary"/>
		<rdfs:seeAlso rdf:resource="&j2se-1_6;JavaLangLibrary"/>
		<rdfs:seeAlso rdf:resource="&j2se-1_6;JavaSecurityLibrary"/>
		<rdfs:comment xml:lang="en">JavaLibrary implementing the java.net package for j2se-1_6</rdfs:comment>
	</owl:Class>
	<owl:Class rdf:about="&j2se-1_6;JavaNioLibrary">
		<rdfs:subClassOf rdf:resource="&j2se-1_5;JavaNioLibrary"/>
		<rdfs:seeAlso rdf:resource="&j2se-1_6;JavaLangLibrary"/>
		<rdfs:comment xml:lang="en">JavaLibrary implementing the java.nio package for j2se-1_6</rdfs:comment>
	</owl:Class>
	<owl:Class rdf:about="&j2se-1_6;JavaNioChannelsLibrary">
		<owl:equivalentClass rdf:resource="&j2se-1_5;JavaNioChannelsLibrary"/>
		<rdfs:subClassOf rdf:resource="&java;JavaLibrary"/>
		<rdfs:seeAlso rdf:resource="&j2se-1_6;JavaUtilLibrary"/>
		<rdfs:seeAlso rdf:resource="&j2se-1_6;JavaNioChannelsSpiLibrary"/>
		<rdfs:seeAlso rdf:resource="&j2se-1_6;JavaNioCharsetLibrary"/>
		<rdfs:seeAlso rdf:resource="&j2se-1_6;JavaLangLibrary"/>
		<rdfs:seeAlso rdf:resource="&j2se-1_6;JavaNetLibrary"/>
		<rdfs:seeAlso rdf:resource="&j2se-1_6;JavaNioLibrary"/>
		<rdfs:seeAlso rdf:resource="&j2se-1_6;JavaIoLibrary"/>
		<rdfs:comment xml:lang="en">JavaLibrary implementing the java.nio.channels package for j2se-1_6</rdfs:comment>
	</owl:Class>
	<owl:Class rdf:about="&j2se-1_6;JavaNioChannelsSpiLibrary">
		<owl:equivalentClass rdf:resource="&j2se-1_5;JavaNioChannelsSpiLibrary"/>
		<rdfs:subClassOf rdf:resource="&java;JavaLibrary"/>
		<rdfs:seeAlso rdf:resource="&j2se-1_6;JavaUtilLibrary"/>
		<rdfs:seeAlso rdf:resource="&j2se-1_6;JavaNioChannelsLibrary"/>
		<rdfs:seeAlso rdf:resource="&j2se-1_6;JavaLangLibrary"/>
		<rdfs:comment xml:lang="en">JavaLibrary implementing the java.nio.channels.spi package for j2se-1_6</rdfs:comment>
	</owl:Class>
	<owl:Class rdf:about="&j2se-1_6;JavaNioCharsetLibrary">
		<owl:equivalentClass rdf:resource="&j2se-1_5;JavaNioCharsetLibrary"/>
		<rdfs:subClassOf rdf:resource="&java;JavaLibrary"/>
		<rdfs:seeAlso rdf:resource="&j2se-1_6;JavaUtilLibrary"/>
		<rdfs:seeAlso rdf:resource="&j2se-1_6;JavaLangLibrary"/>
		<rdfs:seeAlso rdf:resource="&j2se-1_6;JavaNioLibrary"/>
		<rdfs:seeAlso rdf:resource="&j2se-1_6;JavaIoLibrary"/>
		<rdfs:comment xml:lang="en">JavaLibrary implementing the java.nio.charset package for j2se-1_6</rdfs:comment>
	</owl:Class>
	<owl:Class rdf:about="&j2se-1_6;JavaNioCharsetSpiLibrary">
		<owl:equivalentClass rdf:resource="&j2se-1_5;JavaNioCharsetSpiLibrary"/>
		<rdfs:subClassOf rdf:resource="&java;JavaLibrary"/>
		<rdfs:seeAlso rdf:resource="&j2se-1_6;JavaUtilLibrary"/>
		<rdfs:seeAlso rdf:resource="&j2se-1_6;JavaNioCharsetLibrary"/>
		<rdfs:seeAlso rdf:resource="&j2se-1_6;JavaLangLibrary"/>
		<rdfs:comment xml:lang="en">JavaLibrary implementing the java.nio.charset.spi package for j2se-1_6</rdfs:comment>
	</owl:Class>
	<owl:Class rdf:about="&j2se-1_6;JavaRmiLibrary">
		<owl:equivalentClass rdf:resource="&j2se-1_5;JavaRmiLibrary"/>
		<rdfs:subClassOf rdf:resource="&java;JavaLibrary"/>
		<rdfs:seeAlso rdf:resource="&j2se-1_6;JavaIoLibrary"/>
		<rdfs:seeAlso rdf:resource="&j2se-1_6;JavaLangLibrary"/>
		<rdfs:comment xml:lang="en">JavaLibrary implementing the java.rmi package for j2se-1_6</rdfs:comment>
	</owl:Class>
	<owl:Class rdf:about="&j2se-1_6;JavaRmiActivationLibrary">
		<owl:equivalentClass rdf:resource="&j2se-1_5;JavaRmiActivationLibrary"/>
		<rdfs:subClassOf rdf:resource="&java;JavaLibrary"/>
		<rdfs:seeAlso rdf:resource="&j2se-1_6;JavaUtilLibrary"/>
		<rdfs:seeAlso rdf:resource="&j2se-1_6;JavaRmiLibrary"/>
		<rdfs:seeAlso rdf:resource="&j2se-1_6;JavaLangLibrary"/>
		<rdfs:seeAlso rdf:resource="&j2se-1_6;JavaRmiServerLibrary"/>
		<rdfs:seeAlso rdf:resource="&j2se-1_6;JavaIoLibrary"/>
		<rdfs:comment xml:lang="en">JavaLibrary implementing the java.rmi.activation package for j2se-1_6</rdfs:comment>
	</owl:Class>
	<owl:Class rdf:about="&j2se-1_6;JavaRmiServerLibrary">
		<rdfs:subClassOf rdf:resource="&j2se-1_5;JavaRmiServerLibrary"/>
		<rdfs:seeAlso rdf:resource="&j2se-1_6;JavaRmiLibrary"/>
		<rdfs:seeAlso rdf:resource="&j2se-1_6;JavaLangLibrary"/>
		<rdfs:seeAlso rdf:resource="&j2se-1_6;JavaNetLibrary"/>
		<rdfs:seeAlso rdf:resource="&j2se-1_6;JavaIoLibrary"/>
		<rdfs:seeAlso rdf:resource="&j2se-1_6;JavaLangReflectLibrary"/>
		<rdfs:comment xml:lang="en">JavaLibrary implementing the java.rmi.server package for j2se-1_6</rdfs:comment>
	</owl:Class>
	<owl:Class rdf:about="&j2se-1_6;JavaRmiDgcLibrary">
		<owl:equivalentClass rdf:resource="&j2se-1_5;JavaRmiDgcLibrary"/>
		<rdfs:subClassOf rdf:resource="&java;JavaLibrary"/>
		<rdfs:seeAlso rdf:resource="&j2se-1_6;JavaRmiLibrary"/>
		<rdfs:seeAlso rdf:resource="&j2se-1_6;JavaIoLibrary"/>
		<rdfs:seeAlso rdf:resource="&j2se-1_6;JavaLangLibrary"/>
		<rdfs:comment xml:lang="en">JavaLibrary implementing the java.rmi.dgc package for j2se-1_6</rdfs:comment>
	</owl:Class>
	<owl:Class rdf:about="&j2se-1_6;JavaRmiRegistryLibrary">
		<owl:equivalentClass rdf:resource="&j2se-1_5;JavaRmiRegistryLibrary"/>
		<rdfs:subClassOf rdf:resource="&java;JavaLibrary"/>
		<rdfs:seeAlso rdf:resource="&j2se-1_6;JavaRmiLibrary"/>
		<rdfs:seeAlso rdf:resource="&j2se-1_6;JavaLangLibrary"/>
		<rdfs:seeAlso rdf:resource="&j2se-1_6;JavaRmiServerLibrary"/>
		<rdfs:comment xml:lang="en">JavaLibrary implementing the java.rmi.registry package for j2se-1_6</rdfs:comment>
	</owl:Class>
	<owl:Class rdf:about="&j2se-1_6;JavaSqlLibrary">
		<rdfs:subClassOf rdf:resource="&j2se-1_5;JavaSqlLibrary"/>
		<rdfs:seeAlso rdf:resource="&j2se-1_6;JavaUtilLibrary"/>
		<rdfs:seeAlso rdf:resource="&j2se-1_6;JavaxXmlTransformLibrary"/>
		<rdfs:seeAlso rdf:resource="&j2se-1_6;JavaNetLibrary"/>
		<rdfs:seeAlso rdf:resource="&j2se-1_6;JavaIoLibrary"/>
		<rdfs:seeAlso rdf:resource="&j2se-1_6;JavaLangLibrary"/>
		<rdfs:seeAlso rdf:resource="&j2se-1_6;JavaSecurityLibrary"/>
		<rdfs:seeAlso rdf:resource="&j2se-1_6;JavaMathLibrary"/>
		<rdfs:comment xml:lang="en">JavaLibrary implementing the java.sql package for j2se-1_6</rdfs:comment>
	</owl:Class>
	<owl:Class rdf:about="&j2se-1_6;JavaTextLibrary">
		<rdfs:subClassOf rdf:resource="&java;JavaLibrary"/>
		<rdfs:seeAlso rdf:resource="&j2se-1_6;JavaUtilLibrary"/>
		<rdfs:seeAlso rdf:resource="&j2se-1_6;JavaLangLibrary"/>
		<rdfs:seeAlso rdf:resource="&j2se-1_6;JavaMathLibrary"/>
		<rdfs:seeAlso rdf:resource="&j2se-1_6;JavaIoLibrary"/>
		<rdfs:comment xml:lang="en">JavaLibrary implementing the java.text package for j2se-1_6</rdfs:comment>
	</owl:Class>
	<owl:Class rdf:about="&j2se-1_6;JavaTextSpiLibrary">
		<rdfs:subClassOf rdf:resource="&java;JavaLibrary"/>
		<rdfs:seeAlso rdf:resource="&j2se-1_6;JavaUtilLibrary"/>
		<rdfs:seeAlso rdf:resource="&j2se-1_6;JavaUtilSpiLibrary"/>
		<rdfs:seeAlso rdf:resource="&j2se-1_6;JavaTextLibrary"/>
		<rdfs:comment xml:lang="en">JavaLibrary implementing the java.text.spi package for j2se-1_6</rdfs:comment>
	</owl:Class>
	<owl:Class rdf:about="&j2se-1_6;JavaxAccessibilityLibrary">
		<rdfs:subClassOf rdf:resource="&j2se-1_5;JavaxAccessibilityLibrary"/>
		<rdfs:seeAlso rdf:resource="&j2se-1_6;JavaUtilLibrary"/>
		<rdfs:seeAlso rdf:resource="&j2se-1_6;JavaLangLibrary"/>
		<rdfs:seeAlso rdf:resource="&j2se-1_6;JavaAwtLibrary"/>
		<rdfs:seeAlso rdf:resource="&j2se-1_6;JavaxSwingTextLibrary"/>
		<rdfs:seeAlso rdf:resource="&j2se-1_6;JavaBeansLibrary"/>
		<rdfs:seeAlso rdf:resource="&j2se-1_6;JavaIoLibrary"/>
		<rdfs:seeAlso rdf:resource="&j2se-1_6;JavaAwtEventLibrary"/>
		<rdfs:seeAlso rdf:resource="&j2se-1_6;JavaAwtDatatransferLibrary"/>
		<rdfs:comment xml:lang="en">JavaLibrary implementing the javax.accessibility package for j2se-1_6</rdfs:comment>
	</owl:Class>
	<owl:Class rdf:about="&j2se-1_6;JavaxSecurityAuthLibrary">
		<owl:equivalentClass rdf:resource="&j2se-1_5;JavaxSecurityAuthLibrary"/>
		<rdfs:subClassOf rdf:resource="&java;JavaLibrary"/>
		<rdfs:seeAlso rdf:resource="&j2se-1_6;JavaUtilLibrary"/>
		<rdfs:seeAlso rdf:resource="&j2se-1_6;JavaLangLibrary"/>
		<rdfs:seeAlso rdf:resource="&j2se-1_6;JavaSecurityLibrary"/>
		<rdfs:seeAlso rdf:resource="&j2se-1_6;JavaIoLibrary"/>
		<rdfs:comment xml:lang="en">JavaLibrary implementing the javax.security.auth package for j2se-1_6</rdfs:comment>
	</owl:Class>
	<owl:Class rdf:about="&j2se-1_6;JavaxSecurityAuthLoginLibrary">
		<rdfs:subClassOf rdf:resource="&j2se-1_5;JavaxSecurityAuthLoginLibrary"/>
		<rdfs:seeAlso rdf:resource="&j2se-1_6;JavaUtilLibrary"/>
		<rdfs:seeAlso rdf:resource="&j2se-1_6;JavaxSecurityAuthLibrary"/>
		<rdfs:seeAlso rdf:resource="&j2se-1_6;JavaxSecurityAuthCallbackLibrary"/>
		<rdfs:seeAlso rdf:resource="&j2se-1_6;JavaLangLibrary"/>
		<rdfs:seeAlso rdf:resource="&j2se-1_6;JavaSecurityLibrary"/>
		<rdfs:comment xml:lang="en">JavaLibrary implementing the javax.security.auth.login package for j2se-1_6</rdfs:comment>
	</owl:Class>
	<owl:Class rdf:about="&j2se-1_6;JavaxSecurityAuthCallbackLibrary">
		<owl:equivalentClass rdf:resource="&j2se-1_5;JavaxSecurityAuthCallbackLibrary"/>
		<rdfs:subClassOf rdf:resource="&java;JavaLibrary"/>
		<rdfs:seeAlso rdf:resource="&j2se-1_6;JavaUtilLibrary"/>
		<rdfs:seeAlso rdf:resource="&j2se-1_6;JavaIoLibrary"/>
		<rdfs:seeAlso rdf:resource="&j2se-1_6;JavaLangLibrary"/>
		<rdfs:comment xml:lang="en">JavaLibrary implementing the javax.security.auth.callback package for j2se-1_6</rdfs:comment>
	</owl:Class>
	<owl:Class rdf:about="&j2se-1_6;JavaxSecurityAuthKerberosLibrary">
		<owl:equivalentClass rdf:resource="&j2se-1_5;JavaxSecurityAuthKerberosLibrary"/>
		<rdfs:subClassOf rdf:resource="&java;JavaLibrary"/>
		<rdfs:seeAlso rdf:resource="&j2se-1_6;JavaxCryptoLibrary"/>
		<rdfs:seeAlso rdf:resource="&j2se-1_6;JavaUtilLibrary"/>
		<rdfs:seeAlso rdf:resource="&j2se-1_6;JavaxSecurityAuthLibrary"/>
		<rdfs:seeAlso rdf:resource="&j2se-1_6;JavaIoLibrary"/>
		<rdfs:seeAlso rdf:resource="&j2se-1_6;JavaLangLibrary"/>
		<rdfs:seeAlso rdf:resource="&j2se-1_6;JavaSecurityLibrary"/>
		<rdfs:comment xml:lang="en">JavaLibrary implementing the javax.security.auth.kerberos package for j2se-1_6</rdfs:comment>
	</owl:Class>
	<owl:Class rdf:about="&j2se-1_6;JavaxSecurityAuthSpiLibrary">
		<owl:equivalentClass rdf:resource="&j2se-1_5;JavaxSecurityAuthSpiLibrary"/>
		<rdfs:subClassOf rdf:resource="&java;JavaLibrary"/>
		<rdfs:seeAlso rdf:resource="&j2se-1_6;JavaxSecurityAuthLibrary"/>
		<rdfs:seeAlso rdf:resource="&j2se-1_6;JavaUtilLibrary"/>
		<rdfs:seeAlso rdf:resource="&j2se-1_6;JavaxSecurityAuthCallbackLibrary"/>
		<rdfs:comment xml:lang="en">JavaLibrary implementing the javax.security.auth.spi package for j2se-1_6</rdfs:comment>
	</owl:Class>
	<owl:Class rdf:about="&j2se-1_6;JavaxSecurityAuthX500Library">
		<rdfs:subClassOf rdf:resource="&j2se-1_5;JavaxSecurityAuthX500Library"/>
		<rdfs:seeAlso rdf:resource="&j2se-1_6;JavaUtilLibrary"/>
		<rdfs:seeAlso rdf:resource="&j2se-1_6;JavaxSecurityAuthLibrary"/>
		<rdfs:seeAlso rdf:resource="&j2se-1_6;JavaIoLibrary"/>
		<rdfs:seeAlso rdf:resource="&j2se-1_6;JavaLangLibrary"/>
		<rdfs:seeAlso rdf:resource="&j2se-1_6;JavaSecurityLibrary"/>
		<rdfs:seeAlso rdf:resource="&j2se-1_6;JavaSecurityCertLibrary"/>
		<rdfs:comment xml:lang="en">JavaLibrary implementing the javax.security.auth.x500 package for j2se-1_6</rdfs:comment>
	</owl:Class>
	<owl:Class rdf:about="&j2se-1_6;JavaxSecuritySaslLibrary">
		<rdfs:subClassOf rdf:resource="&j2se-1_5;JavaxSecuritySaslLibrary"/>
		<rdfs:seeAlso rdf:resource="&j2se-1_6;JavaUtilLibrary"/>
		<rdfs:seeAlso rdf:resource="&j2se-1_6;JavaxSecurityAuthCallbackLibrary"/>
		<rdfs:seeAlso rdf:resource="&j2se-1_6;JavaIoLibrary"/>
		<rdfs:seeAlso rdf:resource="&j2se-1_6;JavaLangLibrary"/>
		<rdfs:comment xml:lang="en">JavaLibrary implementing the javax.security.sasl package for j2se-1_6</rdfs:comment>
	</owl:Class>
	<owl:Class rdf:about="&j2se-1_6;JavaxActivationLibrary">
		<rdfs:subClassOf rdf:resource="&java;JavaLibrary"/>
		<rdfs:seeAlso rdf:resource="&j2se-1_6;JavaUtilLibrary"/>
		<rdfs:seeAlso rdf:resource="&j2se-1_6;JavaLangLibrary"/>
		<rdfs:seeAlso rdf:resource="&j2se-1_6;JavaNetLibrary"/>
		<rdfs:seeAlso rdf:resource="&j2se-1_6;JavaIoLibrary"/>
		<rdfs:seeAlso rdf:resource="&j2se-1_6;JavaAwtDatatransferLibrary"/>
		<rdfs:comment xml:lang="en">JavaLibrary implementing the javax.activation package for j2se-1_6</rdfs:comment>
	</owl:Class>
	<owl:Class rdf:about="&j2se-1_6;JavaxActivityLibrary">
		<owl:equivalentClass rdf:resource="&j2se-1_5;JavaxActivityLibrary"/>
		<rdfs:subClassOf rdf:resource="&java;JavaLibrary"/>
		<rdfs:seeAlso rdf:resource="&j2se-1_6;JavaRmiLibrary"/>
		<rdfs:seeAlso rdf:resource="&j2se-1_6;JavaLangLibrary"/>
		<rdfs:comment xml:lang="en">JavaLibrary implementing the javax.activity package for j2se-1_6</rdfs:comment>
	</owl:Class>
	<owl:Class rdf:about="&j2se-1_6;JavaxAnnotationLibrary">
		<rdfs:subClassOf rdf:resource="&java;JavaLibrary"/>
		<rdfs:seeAlso rdf:resource="&j2se-1_6;JavaLangLibrary"/>
		<rdfs:seeAlso rdf:resource="&j2se-1_6;JavaLangAnnotationLibrary"/>
		<rdfs:comment xml:lang="en">JavaLibrary implementing the javax.annotation package for j2se-1_6</rdfs:comment>
	</owl:Class>
	<owl:Class rdf:about="&j2se-1_6;JavaxAnnotationProcessingLibrary">
		<rdfs:subClassOf rdf:resource="&java;JavaLibrary"/>
		<rdfs:seeAlso rdf:resource="&j2se-1_6;JavaUtilLibrary"/>
		<rdfs:seeAlso rdf:resource="&j2se-1_6;JavaxLangModelUtilLibrary"/>
		<rdfs:seeAlso rdf:resource="&j2se-1_6;JavaLangLibrary"/>
		<rdfs:seeAlso rdf:resource="&j2se-1_6;JavaxToolsLibrary"/>
		<rdfs:seeAlso rdf:resource="&j2se-1_6;JavaxLangModelLibrary"/>
		<rdfs:seeAlso rdf:resource="&j2se-1_6;JavaxLangModelElementLibrary"/>
		<rdfs:seeAlso rdf:resource="&j2se-1_6;JavaIoLibrary"/>
		<rdfs:seeAlso rdf:resource="&j2se-1_6;JavaLangAnnotationLibrary"/>
		<rdfs:comment xml:lang="en">JavaLibrary implementing the javax.annotation.processing package for j2se-1_6</rdfs:comment>
	</owl:Class>
	<owl:Class rdf:about="&j2se-1_6;JavaxImageioLibrary">
		<rdfs:subClassOf rdf:resource="&j2se-1_5;JavaxImageioLibrary"/>
		<rdfs:seeAlso rdf:resource="&j2se-1_6;JavaUtilLibrary"/>
		<rdfs:seeAlso rdf:resource="&j2se-1_6;JavaAwtLibrary"/>
		<rdfs:seeAlso rdf:resource="&j2se-1_6;JavaxImageioMetadataLibrary"/>
		<rdfs:seeAlso rdf:resource="&j2se-1_6;JavaNetLibrary"/>
		<rdfs:seeAlso rdf:resource="&j2se-1_6;JavaAwtImageLibrary"/>
		<rdfs:seeAlso rdf:resource="&j2se-1_6;JavaIoLibrary"/>
		<rdfs:seeAlso rdf:resource="&j2se-1_6;JavaxImageioEventLibrary"/>
		<rdfs:seeAlso rdf:resource="&j2se-1_6;JavaLangLibrary"/>
		<rdfs:seeAlso rdf:resource="&j2se-1_6;JavaxImageioStreamLibrary"/>
		<rdfs:seeAlso rdf:resource="&j2se-1_6;JavaAwtColorLibrary"/>
		<rdfs:seeAlso rdf:resource="&j2se-1_6;JavaxImageioSpiLibrary"/>
		<rdfs:comment xml:lang="en">JavaLibrary implementing the javax.imageio package for j2se-1_6</rdfs:comment>
	</owl:Class>
	<owl:Class rdf:about="&j2se-1_6;JavaxImageioEventLibrary">
		<owl:equivalentClass rdf:resource="&j2se-1_5;JavaxImageioEventLibrary"/>
		<rdfs:subClassOf rdf:resource="&java;JavaLibrary"/>
		<rdfs:seeAlso rdf:resource="&j2se-1_6;JavaUtilLibrary"/>
		<rdfs:seeAlso rdf:resource="&j2se-1_6;JavaAwtImageLibrary"/>
		<rdfs:seeAlso rdf:resource="&j2se-1_6;JavaLangLibrary"/>
		<rdfs:seeAlso rdf:resource="&j2se-1_6;JavaxImageioLibrary"/>
		<rdfs:comment xml:lang="en">JavaLibrary implementing the javax.imageio.event package for j2se-1_6</rdfs:comment>
	</owl:Class>
	<owl:Class rdf:about="&j2se-1_6;JavaxImageioMetadataLibrary">
		<owl:equivalentClass rdf:resource="&j2se-1_5;JavaxImageioMetadataLibrary"/>
		<rdfs:subClassOf rdf:resource="&java;JavaLibrary"/>
		<rdfs:seeAlso rdf:resource="&j2se-1_6;JavaUtilLibrary"/>
		<rdfs:seeAlso rdf:resource="&j2se-1_6;JavaLangLibrary"/>
		<rdfs:seeAlso rdf:resource="&j2se-1_6;OrgW3cDomLibrary"/>
		<rdfs:seeAlso rdf:resource="&j2se-1_6;JavaxImageioLibrary"/>
		<rdfs:comment xml:lang="en">JavaLibrary implementing the javax.imageio.metadata package for j2se-1_6</rdfs:comment>
	</owl:Class>
	<owl:Class rdf:about="&j2se-1_6;JavaxImageioPluginsBmpLibrary">
		<owl:equivalentClass rdf:resource="&j2se-1_5;JavaxImageioPluginsBmpLibrary"/>
		<rdfs:subClassOf rdf:resource="&java;JavaLibrary"/>
		<rdfs:seeAlso rdf:resource="&j2se-1_6;JavaUtilLibrary"/>
		<rdfs:seeAlso rdf:resource="&j2se-1_6;JavaxImageioLibrary"/>
		<rdfs:comment xml:lang="en">JavaLibrary implementing the javax.imageio.plugins.bmp package for j2se-1_6</rdfs:comment>
	</owl:Class>
	<owl:Class rdf:about="&j2se-1_6;JavaxImageioPluginsJpegLibrary">
		<owl:equivalentClass rdf:resource="&j2se-1_5;JavaxImageioPluginsJpegLibrary"/>
		<rdfs:subClassOf rdf:resource="&java;JavaLibrary"/>
		<rdfs:seeAlso rdf:resource="&j2se-1_6;JavaUtilLibrary"/>
		<rdfs:seeAlso rdf:resource="&j2se-1_6;JavaLangLibrary"/>
		<rdfs:seeAlso rdf:resource="&j2se-1_6;JavaxImageioLibrary"/>
		<rdfs:comment xml:lang="en">JavaLibrary implementing the javax.imageio.plugins.jpeg package for j2se-1_6</rdfs:comment>
	</owl:Class>
	<owl:Class rdf:about="&j2se-1_6;JavaxImageioSpiLibrary">
		<owl:equivalentClass rdf:resource="&j2se-1_5;JavaxImageioSpiLibrary"/>
		<rdfs:subClassOf rdf:resource="&java;JavaLibrary"/>
		<rdfs:seeAlso rdf:resource="&j2se-1_6;JavaUtilLibrary"/>
		<rdfs:seeAlso rdf:resource="&j2se-1_6;JavaLangLibrary"/>
		<rdfs:seeAlso rdf:resource="&j2se-1_6;JavaxImageioLibrary"/>
		<rdfs:seeAlso rdf:resource="&j2se-1_6;JavaxImageioMetadataLibrary"/>
		<rdfs:seeAlso rdf:resource="&j2se-1_6;JavaxImageioStreamLibrary"/>
		<rdfs:seeAlso rdf:resource="&j2se-1_6;JavaAwtImageLibrary"/>
		<rdfs:seeAlso rdf:resource="&j2se-1_6;JavaIoLibrary"/>
		<rdfs:comment xml:lang="en">JavaLibrary implementing the javax.imageio.spi package for j2se-1_6</rdfs:comment>
	</owl:Class>
	<owl:Class rdf:about="&j2se-1_6;JavaxImageioStreamLibrary">
		<owl:equivalentClass rdf:resource="&j2se-1_5;JavaxImageioStreamLibrary"/>
		<rdfs:subClassOf rdf:resource="&java;JavaLibrary"/>
		<rdfs:seeAlso rdf:resource="&j2se-1_6;JavaNioLibrary"/>
		<rdfs:seeAlso rdf:resource="&j2se-1_6;JavaIoLibrary"/>
		<rdfs:seeAlso rdf:resource="&j2se-1_6;JavaLangLibrary"/>
		<rdfs:comment xml:lang="en">JavaLibrary implementing the javax.imageio.stream package for j2se-1_6</rdfs:comment>
	</owl:Class>
	<owl:Class rdf:about="&j2se-1_6;JavaxJwsLibrary">
		<rdfs:subClassOf rdf:resource="&java;JavaLibrary"/>
		<rdfs:seeAlso rdf:resource="&j2se-1_6;JavaLangLibrary"/>
		<rdfs:seeAlso rdf:resource="&j2se-1_6;JavaLangAnnotationLibrary"/>
		<rdfs:comment xml:lang="en">JavaLibrary implementing the javax.jws package for j2se-1_6</rdfs:comment>
	</owl:Class>
	<owl:Class rdf:about="&j2se-1_6;JavaxJwsSoapLibrary">
		<rdfs:subClassOf rdf:resource="&java;JavaLibrary"/>
		<rdfs:seeAlso rdf:resource="&j2se-1_6;JavaLangLibrary"/>
		<rdfs:seeAlso rdf:resource="&j2se-1_6;JavaLangAnnotationLibrary"/>
		<rdfs:comment xml:lang="en">JavaLibrary implementing the javax.jws.soap package for j2se-1_6</rdfs:comment>
	</owl:Class>
	<owl:Class rdf:about="&j2se-1_6;JavaxLangModelLibrary">
		<rdfs:subClassOf rdf:resource="&java;JavaLibrary"/>
		<rdfs:seeAlso rdf:resource="&j2se-1_6;JavaLangLibrary"/>
		<rdfs:comment xml:lang="en">JavaLibrary implementing the javax.lang.model package for j2se-1_6</rdfs:comment>
	</owl:Class>
	<owl:Class rdf:about="&j2se-1_6;JavaxLangModelElementLibrary">
		<rdfs:subClassOf rdf:resource="&java;JavaLibrary"/>
		<rdfs:seeAlso rdf:resource="&j2se-1_6;JavaUtilLibrary"/>
		<rdfs:seeAlso rdf:resource="&j2se-1_6;JavaLangLibrary"/>
		<rdfs:seeAlso rdf:resource="&j2se-1_6;JavaxLangModelTypeLibrary"/>
		<rdfs:seeAlso rdf:resource="&j2se-1_6;JavaLangAnnotationLibrary"/>
		<rdfs:comment xml:lang="en">JavaLibrary implementing the javax.lang.model.element package for j2se-1_6</rdfs:comment>
	</owl:Class>
	<owl:Class rdf:about="&j2se-1_6;JavaxLangModelTypeLibrary">
		<rdfs:subClassOf rdf:resource="&java;JavaLibrary"/>
		<rdfs:seeAlso rdf:resource="&j2se-1_6;JavaUtilLibrary"/>
		<rdfs:seeAlso rdf:resource="&j2se-1_6;JavaLangLibrary"/>
		<rdfs:seeAlso rdf:resource="&j2se-1_6;JavaxLangModelElementLibrary"/>
		<rdfs:comment xml:lang="en">JavaLibrary implementing the javax.lang.model.type package for j2se-1_6</rdfs:comment>
	</owl:Class>
	<owl:Class rdf:about="&j2se-1_6;JavaxLangModelUtilLibrary">
		<rdfs:subClassOf rdf:resource="&java;JavaLibrary"/>
		<rdfs:seeAlso rdf:resource="&j2se-1_6;JavaUtilLibrary"/>
		<rdfs:seeAlso rdf:resource="&j2se-1_6;JavaxLangModelTypeLibrary"/>
		<rdfs:seeAlso rdf:resource="&j2se-1_6;JavaxLangModelElementLibrary"/>
		<rdfs:seeAlso rdf:resource="&j2se-1_6;JavaIoLibrary"/>
		<rdfs:seeAlso rdf:resource="&j2se-1_6;JavaLangLibrary"/>
		<rdfs:comment xml:lang="en">JavaLibrary implementing the javax.lang.model.util package for j2se-1_6</rdfs:comment>
	</owl:Class>
	<owl:Class rdf:about="&j2se-1_6;JavaxManagementLibrary">
		<rdfs:subClassOf rdf:resource="&j2se-1_5;JavaxManagementLibrary"/>
		<rdfs:seeAlso rdf:resource="&j2se-1_6;JavaUtilLibrary"/>
		<rdfs:seeAlso rdf:resource="&j2se-1_6;JavaxManagementLoadingLibrary"/>
		<rdfs:seeAlso rdf:resource="&j2se-1_6;JavaIoLibrary"/>
		<rdfs:seeAlso rdf:resource="&j2se-1_6;JavaLangAnnotationLibrary"/>
		<rdfs:seeAlso rdf:resource="&j2se-1_6;JavaLangLibrary"/>
		<rdfs:seeAlso rdf:resource="&j2se-1_6;JavaSecurityLibrary"/>
		<rdfs:seeAlso rdf:resource="&j2se-1_6;JavaUtilConcurrentLibrary"/>
		<rdfs:seeAlso rdf:resource="&j2se-1_6;JavaLangReflectLibrary"/>
		<rdfs:comment xml:lang="en">JavaLibrary implementing the javax.management package for j2se-1_6</rdfs:comment>
	</owl:Class>
	<owl:Class rdf:about="&j2se-1_6;JavaxManagementLoadingLibrary">
		<rdfs:subClassOf rdf:resource="&j2se-1_5;JavaxManagementLoadingLibrary"/>
		<rdfs:seeAlso rdf:resource="&j2se-1_6;JavaUtilLibrary"/>
		<rdfs:seeAlso rdf:resource="&j2se-1_6;JavaLangLibrary"/>
		<rdfs:seeAlso rdf:resource="&j2se-1_6;JavaNetLibrary"/>
		<rdfs:seeAlso rdf:resource="&j2se-1_6;JavaIoLibrary"/>
		<rdfs:seeAlso rdf:resource="&j2se-1_6;JavaxManagementLibrary"/>
		<rdfs:comment xml:lang="en">JavaLibrary implementing the javax.management.loading package for j2se-1_6</rdfs:comment>
	</owl:Class>
	<owl:Class rdf:about="&j2se-1_6;JavaxManagementModelmbeanLibrary">
		<rdfs:subClassOf rdf:resource="&j2se-1_5;JavaxManagementModelmbeanLibrary"/>
		<rdfs:seeAlso rdf:resource="&j2se-1_6;JavaxManagementLoadingLibrary"/>
		<rdfs:seeAlso rdf:resource="&j2se-1_6;JavaxManagementLibrary"/>
		<rdfs:seeAlso rdf:resource="&j2se-1_6;JavaLangLibrary"/>
		<rdfs:seeAlso rdf:resource="&j2se-1_6;JavaLangReflectLibrary"/>
		<rdfs:comment xml:lang="en">JavaLibrary implementing the javax.management.modelmbean package for j2se-1_6</rdfs:comment>
	</owl:Class>
	<owl:Class rdf:about="&j2se-1_6;JavaxManagementMonitorLibrary">
		<rdfs:subClassOf rdf:resource="&j2se-1_5;JavaxManagementMonitorLibrary"/>
		<rdfs:seeAlso rdf:resource="&j2se-1_6;JavaLangLibrary"/>
		<rdfs:seeAlso rdf:resource="&j2se-1_6;JavaxManagementLibrary"/>
		<rdfs:comment xml:lang="en">JavaLibrary implementing the javax.management.monitor package for j2se-1_6</rdfs:comment>
	</owl:Class>
	<owl:Class rdf:about="&j2se-1_6;JavaxManagementOpenmbeanLibrary">
		<rdfs:subClassOf rdf:resource="&j2se-1_5;JavaxManagementOpenmbeanLibrary"/>
		<rdfs:seeAlso rdf:resource="&j2se-1_6;JavaUtilLibrary"/>
		<rdfs:seeAlso rdf:resource="&j2se-1_6;JavaLangLibrary"/>
		<rdfs:seeAlso rdf:resource="&j2se-1_6;JavaIoLibrary"/>
		<rdfs:seeAlso rdf:resource="&j2se-1_6;JavaxManagementLibrary"/>
		<rdfs:seeAlso rdf:resource="&j2se-1_6;JavaLangReflectLibrary"/>
		<rdfs:comment xml:lang="en">JavaLibrary implementing the javax.management.openmbean package for j2se-1_6</rdfs:comment>
	</owl:Class>
	<owl:Class rdf:about="&j2se-1_6;JavaxManagementRelationLibrary">
		<rdfs:subClassOf rdf:resource="&j2se-1_5;JavaxManagementRelationLibrary"/>
		<rdfs:seeAlso rdf:resource="&j2se-1_6;JavaUtilLibrary"/>
		<rdfs:seeAlso rdf:resource="&j2se-1_6;JavaLangLibrary"/>
		<rdfs:seeAlso rdf:resource="&j2se-1_6;JavaIoLibrary"/>
		<rdfs:seeAlso rdf:resource="&j2se-1_6;JavaxManagementLibrary"/>
		<rdfs:comment xml:lang="en">JavaLibrary implementing the javax.management.relation package for j2se-1_6</rdfs:comment>
	</owl:Class>
	<owl:Class rdf:about="&j2se-1_6;JavaxManagementRemoteLibrary">
		<rdfs:subClassOf rdf:resource="&j2se-1_5;JavaxManagementRemoteLibrary"/>
		<rdfs:seeAlso rdf:resource="&j2se-1_6;JavaUtilLibrary"/>
		<rdfs:seeAlso rdf:resource="&j2se-1_6;JavaLangLibrary"/>
		<rdfs:seeAlso rdf:resource="&j2se-1_6;JavaSecurityLibrary"/>
		<rdfs:seeAlso rdf:resource="&j2se-1_6;JavaxSecurityAuthLibrary"/>
		<rdfs:seeAlso rdf:resource="&j2se-1_6;JavaIoLibrary"/>
		<rdfs:seeAlso rdf:resource="&j2se-1_6;JavaxManagementLibrary"/>
		<rdfs:comment xml:lang="en">JavaLibrary implementing the javax.management.remote package for j2se-1_6</rdfs:comment>
	</owl:Class>
	<owl:Class rdf:about="&j2se-1_6;JavaxManagementRemoteRmiLibrary">
		<rdfs:subClassOf rdf:resource="&j2se-1_5;JavaxManagementRemoteRmiLibrary"/>
		<rdfs:seeAlso rdf:resource="&j2se-1_6;JavaUtilLibrary"/>
		<rdfs:seeAlso rdf:resource="&j2se-1_6;OrgOmgCORBALibrary"/>
		<rdfs:seeAlso rdf:resource="&j2se-1_6;JavaRmiServerLibrary"/>
		<rdfs:seeAlso rdf:resource="&j2se-1_6;JavaxSecurityAuthLibrary"/>
		<rdfs:seeAlso rdf:resource="&j2se-1_6;JavaIoLibrary"/>
		<rdfs:seeAlso rdf:resource="&j2se-1_6;JavaxManagementLibrary"/>
		<rdfs:seeAlso rdf:resource="&j2se-1_6;JavaxRmiCORBALibrary"/>
		<rdfs:seeAlso rdf:resource="&j2se-1_6;JavaRmiLibrary"/>
		<rdfs:seeAlso rdf:resource="&j2se-1_6;JavaLangLibrary"/>
		<rdfs:seeAlso rdf:resource="&j2se-1_6;OrgOmgCORBAPortableLibrary"/>
		<rdfs:seeAlso rdf:resource="&j2se-1_6;JavaxManagementRemoteLibrary"/>
		<rdfs:seeAlso rdf:resource="&j2se-1_6;OrgOmgCORBA_2_3PortableLibrary"/>
		<rdfs:comment xml:lang="en">JavaLibrary implementing the javax.management.remote.rmi package for j2se-1_6</rdfs:comment>
	</owl:Class>
	<owl:Class rdf:about="&j2se-1_6;JavaxManagementTimerLibrary">
		<rdfs:subClassOf rdf:resource="&java;JavaLibrary"/>
		<rdfs:seeAlso rdf:resource="&j2se-1_6;JavaUtilLibrary"/>
		<rdfs:seeAlso rdf:resource="&j2se-1_6;JavaLangLibrary"/>
		<rdfs:seeAlso rdf:resource="&j2se-1_6;JavaxManagementLibrary"/>
		<rdfs:comment xml:lang="en">JavaLibrary implementing the javax.management.timer package for j2se-1_6</rdfs:comment>
	</owl:Class>
	<owl:Class rdf:about="&j2se-1_6;JavaxRmiLibrary">
		<owl:equivalentClass rdf:resource="&j2se-1_5;JavaxRmiLibrary"/>
		<rdfs:subClassOf rdf:resource="&java;JavaLibrary"/>
		<rdfs:seeAlso rdf:resource="&j2se-1_6;JavaRmiLibrary"/>
		<rdfs:seeAlso rdf:resource="&j2se-1_6;JavaLangLibrary"/>
		<rdfs:comment xml:lang="en">JavaLibrary implementing the javax.rmi package for j2se-1_6</rdfs:comment>
	</owl:Class>
	<owl:Class rdf:about="&j2se-1_6;JavaxRmiCORBALibrary">
		<owl:equivalentClass rdf:resource="&j2se-1_5;JavaxRmiCORBALibrary"/>
		<rdfs:subClassOf rdf:resource="&java;JavaLibrary"/>
		<rdfs:seeAlso rdf:resource="&j2se-1_6;OrgOmgCORBALibrary"/>
		<rdfs:seeAlso rdf:resource="&j2se-1_6;JavaRmiLibrary"/>
		<rdfs:seeAlso rdf:resource="&j2se-1_6;OrgOmgSendingContextLibrary"/>
		<rdfs:seeAlso rdf:resource="&j2se-1_6;JavaLangLibrary"/>
		<rdfs:seeAlso rdf:resource="&j2se-1_6;OrgOmgCORBAPortableLibrary"/>
		<rdfs:seeAlso rdf:resource="&j2se-1_6;JavaIoLibrary"/>
		<rdfs:seeAlso rdf:resource="&j2se-1_6;OrgOmgCORBA_2_3PortableLibrary"/>
		<rdfs:comment xml:lang="en">JavaLibrary implementing the javax.rmi.CORBA package for j2se-1_6</rdfs:comment>
	</owl:Class>
	<owl:Class rdf:about="&j2se-1_6;JavaxRmiSslLibrary">
		<owl:equivalentClass rdf:resource="&j2se-1_5;JavaxRmiSslLibrary"/>
		<rdfs:subClassOf rdf:resource="&java;JavaLibrary"/>
		<rdfs:seeAlso rdf:resource="&j2se-1_6;JavaIoLibrary"/>
		<rdfs:seeAlso rdf:resource="&j2se-1_6;JavaLangLibrary"/>
		<rdfs:seeAlso rdf:resource="&j2se-1_6;JavaRmiServerLibrary"/>
		<rdfs:seeAlso rdf:resource="&j2se-1_6;JavaNetLibrary"/>
		<rdfs:comment xml:lang="en">JavaLibrary implementing the javax.rmi.ssl package for j2se-1_6</rdfs:comment>
	</owl:Class>
	<owl:Class rdf:about="&j2se-1_6;JavaxNamingLibrary">
		<rdfs:subClassOf rdf:resource="&j2se-1_5;JavaxNamingLibrary"/>
		<rdfs:seeAlso rdf:resource="&j2se-1_6;JavaUtilLibrary"/>
		<rdfs:seeAlso rdf:resource="&j2se-1_6;JavaIoLibrary"/>
		<rdfs:seeAlso rdf:resource="&j2se-1_6;JavaLangLibrary"/>
		<rdfs:comment xml:lang="en">JavaLibrary implementing the javax.naming package for j2se-1_6</rdfs:comment>
	</owl:Class>
	<owl:Class rdf:about="&j2se-1_6;JavaxNamingDirectoryLibrary">
		<rdfs:subClassOf rdf:resource="&j2se-1_5;JavaxNamingDirectoryLibrary"/>
		<rdfs:seeAlso rdf:resource="&j2se-1_6;JavaUtilLibrary"/>
		<rdfs:seeAlso rdf:resource="&j2se-1_6;JavaLangLibrary"/>
		<rdfs:seeAlso rdf:resource="&j2se-1_6;JavaIoLibrary"/>
		<rdfs:seeAlso rdf:resource="&j2se-1_6;JavaxNamingLibrary"/>
		<rdfs:comment xml:lang="en">JavaLibrary implementing the javax.naming.directory package for j2se-1_6</rdfs:comment>
	</owl:Class>
	<owl:Class rdf:about="&j2se-1_6;JavaxNamingEventLibrary">
		<owl:equivalentClass rdf:resource="&j2se-1_5;JavaxNamingEventLibrary"/>
		<rdfs:subClassOf rdf:resource="&java;JavaLibrary"/>
		<rdfs:seeAlso rdf:resource="&j2se-1_6;JavaUtilLibrary"/>
		<rdfs:seeAlso rdf:resource="&j2se-1_6;JavaxNamingDirectoryLibrary"/>
		<rdfs:seeAlso rdf:resource="&j2se-1_6;JavaLangLibrary"/>
		<rdfs:seeAlso rdf:resource="&j2se-1_6;JavaxNamingLibrary"/>
		<rdfs:comment xml:lang="en">JavaLibrary implementing the javax.naming.event package for j2se-1_6</rdfs:comment>
	</owl:Class>
	<owl:Class rdf:about="&j2se-1_6;JavaxNamingLdapLibrary">
		<rdfs:subClassOf rdf:resource="&j2se-1_5;JavaxNamingLdapLibrary"/>
		<rdfs:seeAlso rdf:resource="&j2se-1_6;JavaUtilLibrary"/>
		<rdfs:seeAlso rdf:resource="&j2se-1_6;JavaxNamingDirectoryLibrary"/>
		<rdfs:seeAlso rdf:resource="&j2se-1_6;JavaxNamingEventLibrary"/>
		<rdfs:seeAlso rdf:resource="&j2se-1_6;JavaLangLibrary"/>
		<rdfs:seeAlso rdf:resource="&j2se-1_6;JavaIoLibrary"/>
		<rdfs:seeAlso rdf:resource="&j2se-1_6;JavaxNamingLibrary"/>
		<rdfs:comment xml:lang="en">JavaLibrary implementing the javax.naming.ldap package for j2se-1_6</rdfs:comment>
	</owl:Class>
	<owl:Class rdf:about="&j2se-1_6;JavaxNamingSpiLibrary">
		<owl:equivalentClass rdf:resource="&j2se-1_5;JavaxNamingSpiLibrary"/>
		<rdfs:subClassOf rdf:resource="&java;JavaLibrary"/>
		<rdfs:seeAlso rdf:resource="&j2se-1_6;JavaUtilLibrary"/>
		<rdfs:seeAlso rdf:resource="&j2se-1_6;JavaxNamingDirectoryLibrary"/>
		<rdfs:seeAlso rdf:resource="&j2se-1_6;JavaIoLibrary"/>
		<rdfs:seeAlso rdf:resource="&j2se-1_6;JavaLangLibrary"/>
		<rdfs:seeAlso rdf:resource="&j2se-1_6;JavaxNamingLibrary"/>
		<rdfs:comment xml:lang="en">JavaLibrary implementing the javax.naming.spi package for j2se-1_6</rdfs:comment>
	</owl:Class>
	<owl:Class rdf:about="&j2se-1_6;JavaxPrintLibrary">
		<owl:equivalentClass rdf:resource="&j2se-1_5;JavaxPrintLibrary"/>
		<rdfs:subClassOf rdf:resource="&java;JavaLibrary"/>
		<rdfs:seeAlso rdf:resource="&j2se-1_6;JavaLangLibrary"/>
		<rdfs:seeAlso rdf:resource="&j2se-1_6;JavaAwtLibrary"/>
		<rdfs:seeAlso rdf:resource="&j2se-1_6;JavaxPrintAttributeLibrary"/>
		<rdfs:seeAlso rdf:resource="&j2se-1_6;JavaNetLibrary"/>
		<rdfs:seeAlso rdf:resource="&j2se-1_6;JavaxPrintEventLibrary"/>
		<rdfs:seeAlso rdf:resource="&j2se-1_6;JavaIoLibrary"/>
		<rdfs:comment xml:lang="en">JavaLibrary implementing the javax.print package for j2se-1_6</rdfs:comment>
	</owl:Class>
	<owl:Class rdf:about="&j2se-1_6;JavaxPrintAttributeLibrary">
		<owl:equivalentClass rdf:resource="&j2se-1_5;JavaxPrintAttributeLibrary"/>
		<rdfs:subClassOf rdf:resource="&java;JavaLibrary"/>
		<rdfs:seeAlso rdf:resource="&j2se-1_6;JavaUtilLibrary"/>
		<rdfs:seeAlso rdf:resource="&j2se-1_6;JavaIoLibrary"/>
		<rdfs:seeAlso rdf:resource="&j2se-1_6;JavaLangLibrary"/>
		<rdfs:seeAlso rdf:resource="&j2se-1_6;JavaNetLibrary"/>
		<rdfs:comment xml:lang="en">JavaLibrary implementing the javax.print.attribute package for j2se-1_6</rdfs:comment>
	</owl:Class>
	<owl:Class rdf:about="&j2se-1_6;JavaxPrintAttributeStandardLibrary">
		<owl:equivalentClass rdf:resource="&j2se-1_5;JavaxPrintAttributeStandardLibrary"/>
		<rdfs:subClassOf rdf:resource="&java;JavaLibrary"/>
		<rdfs:seeAlso rdf:resource="&j2se-1_6;JavaUtilLibrary"/>
		<rdfs:seeAlso rdf:resource="&j2se-1_6;JavaNetLibrary"/>
		<rdfs:seeAlso rdf:resource="&j2se-1_6;JavaLangLibrary"/>
		<rdfs:seeAlso rdf:resource="&j2se-1_6;JavaxPrintAttributeLibrary"/>
		<rdfs:comment xml:lang="en">JavaLibrary implementing the javax.print.attribute.standard package for j2se-1_6</rdfs:comment>
	</owl:Class>
	<owl:Class rdf:about="&j2se-1_6;JavaxPrintEventLibrary">
		<owl:equivalentClass rdf:resource="&j2se-1_5;JavaxPrintEventLibrary"/>
		<rdfs:subClassOf rdf:resource="&java;JavaLibrary"/>
		<rdfs:seeAlso rdf:resource="&j2se-1_6;JavaUtilLibrary"/>
		<rdfs:seeAlso rdf:resource="&j2se-1_6;JavaLangLibrary"/>
		<rdfs:seeAlso rdf:resource="&j2se-1_6;JavaxPrintLibrary"/>
		<rdfs:seeAlso rdf:resource="&j2se-1_6;JavaxPrintAttributeLibrary"/>
		<rdfs:comment xml:lang="en">JavaLibrary implementing the javax.print.event package for j2se-1_6</rdfs:comment>
	</owl:Class>
	<owl:Class rdf:about="&j2se-1_6;JavaxScriptLibrary">
		<rdfs:subClassOf rdf:resource="&java;JavaLibrary"/>
		<rdfs:seeAlso rdf:resource="&j2se-1_6;JavaUtilLibrary"/>
		<rdfs:seeAlso rdf:resource="&j2se-1_6;JavaIoLibrary"/>
		<rdfs:seeAlso rdf:resource="&j2se-1_6;JavaLangLibrary"/>
		<rdfs:comment xml:lang="en">JavaLibrary implementing the javax.script package for j2se-1_6</rdfs:comment>
	</owl:Class>
	<owl:Class rdf:about="&j2se-1_6;JavaxCryptoLibrary">
		<owl:equivalentClass rdf:resource="&j2se-1_5;JavaxCryptoLibrary"/>
		<rdfs:subClassOf rdf:resource="&java;JavaLibrary"/>
		<rdfs:comment xml:lang="en">JavaLibrary implementing the javax.crypto package for j2se-1_6</rdfs:comment>
	</owl:Class>
	<owl:Class rdf:about="&j2se-1_6;JavaxSmartcardioLibrary">
		<rdfs:subClassOf rdf:resource="&java;JavaLibrary"/>
		<rdfs:seeAlso rdf:resource="&j2se-1_6;JavaUtilLibrary"/>
		<rdfs:seeAlso rdf:resource="&j2se-1_6;JavaNioLibrary"/>
		<rdfs:seeAlso rdf:resource="&j2se-1_6;JavaIoLibrary"/>
		<rdfs:seeAlso rdf:resource="&j2se-1_6;JavaLangLibrary"/>
		<rdfs:seeAlso rdf:resource="&j2se-1_6;JavaSecurityLibrary"/>
		<rdfs:comment xml:lang="en">JavaLibrary implementing the javax.smartcardio package for j2se-1_6</rdfs:comment>
	</owl:Class>
	<owl:Class rdf:about="&j2se-1_6;JavaxSoundMidiLibrary">
		<owl:equivalentClass rdf:resource="&j2se-1_5;JavaxSoundMidiLibrary"/>
		<rdfs:subClassOf rdf:resource="&java;JavaLibrary"/>
		<rdfs:seeAlso rdf:resource="&j2se-1_6;JavaUtilLibrary"/>
		<rdfs:seeAlso rdf:resource="&j2se-1_6;JavaLangLibrary"/>
		<rdfs:seeAlso rdf:resource="&j2se-1_6;JavaNetLibrary"/>
		<rdfs:seeAlso rdf:resource="&j2se-1_6;JavaIoLibrary"/>
		<rdfs:comment xml:lang="en">JavaLibrary implementing the javax.sound.midi package for j2se-1_6</rdfs:comment>
	</owl:Class>
	<owl:Class rdf:about="&j2se-1_6;JavaxSoundMidiSpiLibrary">
		<owl:equivalentClass rdf:resource="&j2se-1_5;JavaxSoundMidiSpiLibrary"/>
		<rdfs:subClassOf rdf:resource="&java;JavaLibrary"/>
		<rdfs:seeAlso rdf:resource="&j2se-1_6;JavaxSoundMidiLibrary"/>
		<rdfs:seeAlso rdf:resource="&j2se-1_6;JavaIoLibrary"/>
		<rdfs:seeAlso rdf:resource="&j2se-1_6;JavaLangLibrary"/>
		<rdfs:seeAlso rdf:resource="&j2se-1_6;JavaNetLibrary"/>
		<rdfs:comment xml:lang="en">JavaLibrary implementing the javax.sound.midi.spi package for j2se-1_6</rdfs:comment>
	</owl:Class>
	<owl:Class rdf:about="&j2se-1_6;JavaxSoundSampledLibrary">
		<owl:equivalentClass rdf:resource="&j2se-1_5;JavaxSoundSampledLibrary"/>
		<rdfs:subClassOf rdf:resource="&java;JavaLibrary"/>
		<rdfs:seeAlso rdf:resource="&j2se-1_6;JavaUtilLibrary"/>
		<rdfs:seeAlso rdf:resource="&j2se-1_6;JavaLangLibrary"/>
		<rdfs:seeAlso rdf:resource="&j2se-1_6;JavaSecurityLibrary"/>
		<rdfs:seeAlso rdf:resource="&j2se-1_6;JavaNetLibrary"/>
		<rdfs:seeAlso rdf:resource="&j2se-1_6;JavaIoLibrary"/>
		<rdfs:comment xml:lang="en">JavaLibrary implementing the javax.sound.sampled package for j2se-1_6</rdfs:comment>
	</owl:Class>
	<owl:Class rdf:about="&j2se-1_6;JavaxSoundSampledSpiLibrary">
		<owl:equivalentClass rdf:resource="&j2se-1_5;JavaxSoundSampledSpiLibrary"/>
		<rdfs:subClassOf rdf:resource="&java;JavaLibrary"/>
		<rdfs:seeAlso rdf:resource="&j2se-1_6;JavaLangLibrary"/>
		<rdfs:seeAlso rdf:resource="&j2se-1_6;JavaNetLibrary"/>
		<rdfs:seeAlso rdf:resource="&j2se-1_6;JavaxSoundSampledLibrary"/>
		<rdfs:seeAlso rdf:resource="&j2se-1_6;JavaIoLibrary"/>
		<rdfs:comment xml:lang="en">JavaLibrary implementing the javax.sound.sampled.spi package for j2se-1_6</rdfs:comment>
	</owl:Class>
	<owl:Class rdf:about="&j2se-1_6;JavaxSqlLibrary">
		<rdfs:subClassOf rdf:resource="&j2se-1_5;JavaxSqlLibrary"/>
		<rdfs:seeAlso rdf:resource="&j2se-1_6;JavaUtilLibrary"/>
		<rdfs:seeAlso rdf:resource="&j2se-1_6;JavaxTransactionXaLibrary"/>
		<rdfs:seeAlso rdf:resource="&j2se-1_6;JavaNetLibrary"/>
		<rdfs:seeAlso rdf:resource="&j2se-1_6;JavaIoLibrary"/>
		<rdfs:seeAlso rdf:resource="&j2se-1_6;JavaSqlLibrary"/>
		<rdfs:seeAlso rdf:resource="&j2se-1_6;JavaLangLibrary"/>
		<rdfs:seeAlso rdf:resource="&j2se-1_6;JavaMathLibrary"/>
		<rdfs:comment xml:lang="en">JavaLibrary implementing the javax.sql package for j2se-1_6</rdfs:comment>
	</owl:Class>
	<owl:Class rdf:about="&j2se-1_6;JavaxSqlRowsetLibrary">
		<rdfs:subClassOf rdf:resource="&j2se-1_5;JavaxSqlRowsetLibrary"/>
		<rdfs:seeAlso rdf:resource="&j2se-1_6;JavaUtilLibrary"/>
		<rdfs:seeAlso rdf:resource="&j2se-1_6;JavaNetLibrary"/>
		<rdfs:seeAlso rdf:resource="&j2se-1_6;JavaIoLibrary"/>
		<rdfs:seeAlso rdf:resource="&j2se-1_6;JavaxSqlRowsetSpiLibrary"/>
		<rdfs:seeAlso rdf:resource="&j2se-1_6;JavaSqlLibrary"/>
		<rdfs:seeAlso rdf:resource="&j2se-1_6;JavaLangLibrary"/>
		<rdfs:seeAlso rdf:resource="&j2se-1_6;JavaMathLibrary"/>
		<rdfs:seeAlso rdf:resource="&j2se-1_6;JavaxSqlLibrary"/>
		<rdfs:comment xml:lang="en">JavaLibrary implementing the javax.sql.rowset package for j2se-1_6</rdfs:comment>
	</owl:Class>
	<owl:Class rdf:about="&j2se-1_6;JavaxSqlRowsetSerialLibrary">
		<rdfs:subClassOf rdf:resource="&j2se-1_5;JavaxSqlRowsetSerialLibrary"/>
		<rdfs:seeAlso rdf:resource="&j2se-1_6;JavaUtilLibrary"/>
		<rdfs:seeAlso rdf:resource="&j2se-1_6;JavaNetLibrary"/>
		<rdfs:seeAlso rdf:resource="&j2se-1_6;JavaIoLibrary"/>
		<rdfs:seeAlso rdf:resource="&j2se-1_6;JavaSqlLibrary"/>
		<rdfs:seeAlso rdf:resource="&j2se-1_6;JavaLangLibrary"/>
		<rdfs:seeAlso rdf:resource="&j2se-1_6;JavaMathLibrary"/>
		<rdfs:comment xml:lang="en">JavaLibrary implementing the javax.sql.rowset.serial package for j2se-1_6</rdfs:comment>
	</owl:Class>
	<owl:Class rdf:about="&j2se-1_6;JavaxSqlRowsetSpiLibrary">
		<rdfs:subClassOf rdf:resource="&j2se-1_5;JavaxSqlRowsetSpiLibrary"/>
		<rdfs:seeAlso rdf:resource="&j2se-1_6;JavaUtilLoggingLibrary"/>
		<rdfs:seeAlso rdf:resource="&j2se-1_6;JavaUtilLibrary"/>
		<rdfs:seeAlso rdf:resource="&j2se-1_6;JavaxSqlRowsetLibrary"/>
		<rdfs:seeAlso rdf:resource="&j2se-1_6;JavaLangLibrary"/>
		<rdfs:seeAlso rdf:resource="&j2se-1_6;JavaIoLibrary"/>
		<rdfs:seeAlso rdf:resource="&j2se-1_6;JavaxSqlLibrary"/>
		<rdfs:seeAlso rdf:resource="&j2se-1_6;JavaxNamingLibrary"/>
		<rdfs:seeAlso rdf:resource="&j2se-1_6;JavaSqlLibrary"/>
		<rdfs:comment xml:lang="en">JavaLibrary implementing the javax.sql.rowset.spi package for j2se-1_6</rdfs:comment>
	</owl:Class>
	<owl:Class rdf:about="&j2se-1_6;JavaxSwingLibrary">
		<rdfs:subClassOf rdf:resource="&j2se-1_5;JavaxSwingLibrary"/>
		<rdfs:seeAlso rdf:resource="&j2se-1_6;JavaxSwingPlafLibrary"/>
		<rdfs:seeAlso rdf:resource="&j2se-1_6;JavaAwtLibrary"/>
		<rdfs:seeAlso rdf:resource="&j2se-1_6;JavaxSwingColorchooserLibrary"/>
		<rdfs:seeAlso rdf:resource="&j2se-1_6;JavaxPrintLibrary"/>
		<rdfs:seeAlso rdf:resource="&j2se-1_6;JavaxSwingFilechooserLibrary"/>
		<rdfs:seeAlso rdf:resource="&j2se-1_6;JavaUtilLibrary"/>
		<rdfs:seeAlso rdf:resource="&j2se-1_6;JavaBeansLibrary"/>
		<rdfs:seeAlso rdf:resource="&j2se-1_6;JavaLangLibrary"/>
		<rdfs:seeAlso rdf:resource="&j2se-1_6;JavaUtilConcurrentLibrary"/>
		<rdfs:seeAlso rdf:resource="&j2se-1_6;JavaxSwingTableLibrary"/>
		<rdfs:seeAlso rdf:resource="&j2se-1_6;JavaxSwingTextLibrary"/>
		<rdfs:seeAlso rdf:resource="&j2se-1_6;JavaxSwingEventLibrary"/>
		<rdfs:seeAlso rdf:resource="&j2se-1_6;JavaAwtImageLibrary"/>
		<rdfs:seeAlso rdf:resource="&j2se-1_6;JavaxSwingTreeLibrary"/>
		<rdfs:seeAlso rdf:resource="&j2se-1_6;JavaAwtPrintLibrary"/>
		<rdfs:seeAlso rdf:resource="&j2se-1_6;JavaTextLibrary"/>
		<rdfs:seeAlso rdf:resource="&j2se-1_6;JavaxAccessibilityLibrary"/>
		<rdfs:seeAlso rdf:resource="&j2se-1_6;JavaNetLibrary"/>
		<rdfs:seeAlso rdf:resource="&j2se-1_6;JavaIoLibrary"/>
		<rdfs:seeAlso rdf:resource="&j2se-1_6;JavaAwtDatatransferLibrary"/>
		<rdfs:seeAlso rdf:resource="&j2se-1_6;JavaxPrintAttributeLibrary"/>
		<rdfs:seeAlso rdf:resource="&j2se-1_6;JavaAppletLibrary"/>
		<rdfs:seeAlso rdf:resource="&j2se-1_6;JavaAwtEventLibrary"/>
		<rdfs:seeAlso rdf:resource="&j2se-1_6;JavaxSwingBorderLibrary"/>
		<rdfs:comment xml:lang="en">JavaLibrary implementing the javax.swing package for j2se-1_6</rdfs:comment>
	</owl:Class>
	<owl:Class rdf:about="&j2se-1_6;JavaxSwingEventLibrary">
		<rdfs:subClassOf rdf:resource="&j2se-1_5;JavaxSwingEventLibrary"/>
		<rdfs:seeAlso rdf:resource="&j2se-1_6;JavaUtilLibrary"/>
		<rdfs:seeAlso rdf:resource="&j2se-1_6;JavaAwtLibrary"/>
		<rdfs:seeAlso rdf:resource="&j2se-1_6;JavaxSwingLibrary"/>
		<rdfs:seeAlso rdf:resource="&j2se-1_6;JavaxSwingTextLibrary"/>
		<rdfs:seeAlso rdf:resource="&j2se-1_6;JavaNetLibrary"/>
		<rdfs:seeAlso rdf:resource="&j2se-1_6;JavaxSwingTreeLibrary"/>
		<rdfs:seeAlso rdf:resource="&j2se-1_6;JavaBeansLibrary"/>
		<rdfs:seeAlso rdf:resource="&j2se-1_6;JavaIoLibrary"/>
		<rdfs:seeAlso rdf:resource="&j2se-1_6;JavaAwtEventLibrary"/>
		<rdfs:seeAlso rdf:resource="&j2se-1_6;JavaLangLibrary"/>
		<rdfs:seeAlso rdf:resource="&j2se-1_6;JavaxSwingUndoLibrary"/>
		<rdfs:seeAlso rdf:resource="&j2se-1_6;JavaxSwingTableLibrary"/>
		<rdfs:comment xml:lang="en">JavaLibrary implementing the javax.swing.event package for j2se-1_6</rdfs:comment>
	</owl:Class>
	<owl:Class rdf:about="&j2se-1_6;JavaxSwingTextLibrary">
		<rdfs:subClassOf rdf:resource="&j2se-1_5;JavaxSwingTextLibrary"/>
		<rdfs:seeAlso rdf:resource="&j2se-1_6;JavaxSwingPlafBasicLibrary"/>
		<rdfs:seeAlso rdf:resource="&j2se-1_6;JavaAwtLibrary"/>
		<rdfs:seeAlso rdf:resource="&j2se-1_6;JavaxSwingEventLibrary"/>
		<rdfs:seeAlso rdf:resource="&j2se-1_6;JavaxSwingTreeLibrary"/>
		<rdfs:seeAlso rdf:resource="&j2se-1_6;JavaAwtPrintLibrary"/>
		<rdfs:seeAlso rdf:resource="&j2se-1_6;JavaxSwingUndoLibrary"/>
		<rdfs:seeAlso rdf:resource="&j2se-1_6;JavaTextLibrary"/>
		<rdfs:seeAlso rdf:resource="&j2se-1_6;JavaxPrintLibrary"/>
		<rdfs:seeAlso rdf:resource="&j2se-1_6;JavaxSwingPlafLibrary"/>
		<rdfs:seeAlso rdf:resource="&j2se-1_6;JavaxAccessibilityLibrary"/>
		<rdfs:seeAlso rdf:resource="&j2se-1_6;JavaUtilLibrary"/>
		<rdfs:seeAlso rdf:resource="&j2se-1_6;JavaxSwingLibrary"/>
		<rdfs:seeAlso rdf:resource="&j2se-1_6;JavaIoLibrary"/>
		<rdfs:seeAlso rdf:resource="&j2se-1_6;JavaAwtEventLibrary"/>
		<rdfs:seeAlso rdf:resource="&j2se-1_6;JavaLangLibrary"/>
		<rdfs:seeAlso rdf:resource="&j2se-1_6;JavaxPrintAttributeLibrary"/>
		<rdfs:seeAlso rdf:resource="&j2se-1_6;JavaAwtImLibrary"/>
		<rdfs:comment xml:lang="en">JavaLibrary implementing the javax.swing.text package for j2se-1_6</rdfs:comment>
	</owl:Class>
	<owl:Class rdf:about="&j2se-1_6;JavaxSwingTextHtmlLibrary">
		<rdfs:subClassOf rdf:resource="&j2se-1_5;JavaxSwingTextHtmlLibrary"/>
		<rdfs:seeAlso rdf:resource="&j2se-1_6;JavaAwtLibrary"/>
		<rdfs:seeAlso rdf:resource="&j2se-1_6;JavaxSwingTextLibrary"/>
		<rdfs:seeAlso rdf:resource="&j2se-1_6;JavaxSwingEventLibrary"/>
		<rdfs:seeAlso rdf:resource="&j2se-1_6;JavaxAccessibilityLibrary"/>
		<rdfs:seeAlso rdf:resource="&j2se-1_6;JavaUtilLibrary"/>
		<rdfs:seeAlso rdf:resource="&j2se-1_6;JavaxSwingLibrary"/>
		<rdfs:seeAlso rdf:resource="&j2se-1_6;JavaNetLibrary"/>
		<rdfs:seeAlso rdf:resource="&j2se-1_6;JavaIoLibrary"/>
		<rdfs:seeAlso rdf:resource="&j2se-1_6;JavaAwtEventLibrary"/>
		<rdfs:seeAlso rdf:resource="&j2se-1_6;JavaLangLibrary"/>
		<rdfs:comment xml:lang="en">JavaLibrary implementing the javax.swing.text.html package for j2se-1_6</rdfs:comment>
	</owl:Class>
	<owl:Class rdf:about="&j2se-1_6;JavaxSwingTextHtmlParserLibrary">
		<owl:equivalentClass rdf:resource="&j2se-1_5;JavaxSwingTextHtmlParserLibrary"/>
		<rdfs:subClassOf rdf:resource="&java;JavaLibrary"/>
		<rdfs:seeAlso rdf:resource="&j2se-1_6;JavaUtilLibrary"/>
		<rdfs:seeAlso rdf:resource="&j2se-1_6;JavaxSwingTextHtmlLibrary"/>
		<rdfs:seeAlso rdf:resource="&j2se-1_6;JavaLangLibrary"/>
		<rdfs:seeAlso rdf:resource="&j2se-1_6;JavaxSwingTextLibrary"/>
		<rdfs:seeAlso rdf:resource="&j2se-1_6;JavaIoLibrary"/>
		<rdfs:comment xml:lang="en">JavaLibrary implementing the javax.swing.text.html.parser package for j2se-1_6</rdfs:comment>
	</owl:Class>
	<owl:Class rdf:about="&j2se-1_6;JavaxSwingTextRtfLibrary">
		<rdfs:subClassOf rdf:resource="&j2se-1_5;JavaxSwingTextRtfLibrary"/>
		<rdfs:seeAlso rdf:resource="&j2se-1_6;JavaIoLibrary"/>
		<rdfs:seeAlso rdf:resource="&j2se-1_6;JavaLangLibrary"/>
		<rdfs:seeAlso rdf:resource="&j2se-1_6;JavaxSwingTextLibrary"/>
		<rdfs:comment xml:lang="en">JavaLibrary implementing the javax.swing.text.rtf package for j2se-1_6</rdfs:comment>
	</owl:Class>
	<owl:Class rdf:about="&j2se-1_6;JavaxSwingTreeLibrary">
		<rdfs:subClassOf rdf:resource="&j2se-1_5;JavaxSwingTreeLibrary"/>
		<rdfs:seeAlso rdf:resource="&j2se-1_6;JavaUtilLibrary"/>
		<rdfs:seeAlso rdf:resource="&j2se-1_6;JavaAwtLibrary"/>
		<rdfs:seeAlso rdf:resource="&j2se-1_6;JavaxSwingLibrary"/>
		<rdfs:seeAlso rdf:resource="&j2se-1_6;JavaxSwingEventLibrary"/>
		<rdfs:seeAlso rdf:resource="&j2se-1_6;JavaBeansLibrary"/>
		<rdfs:seeAlso rdf:resource="&j2se-1_6;JavaIoLibrary"/>
		<rdfs:seeAlso rdf:resource="&j2se-1_6;JavaAwtEventLibrary"/>
		<rdfs:seeAlso rdf:resource="&j2se-1_6;JavaLangLibrary"/>
		<rdfs:seeAlso rdf:resource="&j2se-1_6;JavaxSwingBorderLibrary"/>
		<rdfs:comment xml:lang="en">JavaLibrary implementing the javax.swing.tree package for j2se-1_6</rdfs:comment>
	</owl:Class>
	<owl:Class rdf:about="&j2se-1_6;JavaxSwingBorderLibrary">
		<rdfs:subClassOf rdf:resource="&j2se-1_5;JavaxSwingBorderLibrary"/>
		<rdfs:seeAlso rdf:resource="&j2se-1_6;JavaLangLibrary"/>
		<rdfs:seeAlso rdf:resource="&j2se-1_6;JavaAwtLibrary"/>
		<rdfs:seeAlso rdf:resource="&j2se-1_6;JavaxSwingLibrary"/>
		<rdfs:seeAlso rdf:resource="&j2se-1_6;JavaIoLibrary"/>
		<rdfs:comment xml:lang="en">JavaLibrary implementing the javax.swing.border package for j2se-1_6</rdfs:comment>
	</owl:Class>
	<owl:Class rdf:about="&j2se-1_6;JavaxSwingColorchooserLibrary">
		<rdfs:subClassOf rdf:resource="&j2se-1_5;JavaxSwingColorchooserLibrary"/>
		<rdfs:seeAlso rdf:resource="&j2se-1_6;JavaLangLibrary"/>
		<rdfs:seeAlso rdf:resource="&j2se-1_6;JavaAwtLibrary"/>
		<rdfs:seeAlso rdf:resource="&j2se-1_6;JavaxSwingLibrary"/>
		<rdfs:seeAlso rdf:resource="&j2se-1_6;JavaxSwingEventLibrary"/>
		<rdfs:seeAlso rdf:resource="&j2se-1_6;JavaIoLibrary"/>
		<rdfs:comment xml:lang="en">JavaLibrary implementing the javax.swing.colorchooser package for j2se-1_6</rdfs:comment>
	</owl:Class>
	<owl:Class rdf:about="&j2se-1_6;JavaxSwingFilechooserLibrary">
		<rdfs:subClassOf rdf:resource="&j2se-1_5;JavaxSwingFilechooserLibrary"/>
		<rdfs:seeAlso rdf:resource="&j2se-1_6;JavaIoLibrary"/>
		<rdfs:seeAlso rdf:resource="&j2se-1_6;JavaLangLibrary"/>
		<rdfs:seeAlso rdf:resource="&j2se-1_6;JavaxSwingLibrary"/>
		<rdfs:comment xml:lang="en">JavaLibrary implementing the javax.swing.filechooser package for j2se-1_6</rdfs:comment>
	</owl:Class>
	<owl:Class rdf:about="&j2se-1_6;JavaxSwingPlafLibrary">
		<rdfs:subClassOf rdf:resource="&j2se-1_5;JavaxSwingPlafLibrary"/>
		<rdfs:seeAlso rdf:resource="&j2se-1_6;JavaAwtLibrary"/>
		<rdfs:seeAlso rdf:resource="&j2se-1_6;JavaxSwingLibrary"/>
		<rdfs:seeAlso rdf:resource="&j2se-1_6;JavaxSwingTextLibrary"/>
		<rdfs:seeAlso rdf:resource="&j2se-1_6;JavaxSwingTreeLibrary"/>
		<rdfs:seeAlso rdf:resource="&j2se-1_6;JavaIoLibrary"/>
		<rdfs:seeAlso rdf:resource="&j2se-1_6;JavaAwtEventLibrary"/>
		<rdfs:seeAlso rdf:resource="&j2se-1_6;JavaLangLibrary"/>
		<rdfs:seeAlso rdf:resource="&j2se-1_6;JavaxAccessibilityLibrary"/>
		<rdfs:seeAlso rdf:resource="&j2se-1_6;JavaxSwingFilechooserLibrary"/>
		<rdfs:seeAlso rdf:resource="&j2se-1_6;JavaxSwingBorderLibrary"/>
		<rdfs:comment xml:lang="en">JavaLibrary implementing the javax.swing.plaf package for j2se-1_6</rdfs:comment>
	</owl:Class>
	<owl:Class rdf:about="&j2se-1_6;JavaxSwingPlafBasicLibrary">
		<rdfs:subClassOf rdf:resource="&j2se-1_5;JavaxSwingPlafBasicLibrary"/>
		<rdfs:seeAlso rdf:resource="&j2se-1_6;JavaxSwingTextLibrary"/>
		<rdfs:seeAlso rdf:resource="&j2se-1_6;JavaxSwingEventLibrary"/>
		<rdfs:seeAlso rdf:resource="&j2se-1_6;JavaxSwingTreeLibrary"/>
		<rdfs:seeAlso rdf:resource="&j2se-1_6;JavaxSwingPlafLibrary"/>
		<rdfs:seeAlso rdf:resource="&j2se-1_6;JavaxAccessibilityLibrary"/>
		<rdfs:seeAlso rdf:resource="&j2se-1_6;JavaxSwingLibrary"/>
		<rdfs:seeAlso rdf:resource="&j2se-1_6;JavaIoLibrary"/>
		<rdfs:seeAlso rdf:resource="&j2se-1_6;JavaAwtLibrary"/>
		<rdfs:seeAlso rdf:resource="&j2se-1_6;JavaxSwingFilechooserLibrary"/>
		<rdfs:seeAlso rdf:resource="&j2se-1_6;JavaUtilLibrary"/>
		<rdfs:seeAlso rdf:resource="&j2se-1_6;JavaBeansLibrary"/>
		<rdfs:seeAlso rdf:resource="&j2se-1_6;JavaAwtEventLibrary"/>
		<rdfs:seeAlso rdf:resource="&j2se-1_6;JavaLangLibrary"/>
		<rdfs:seeAlso rdf:resource="&j2se-1_6;JavaxSwingTableLibrary"/>
		<rdfs:seeAlso rdf:resource="&j2se-1_6;JavaxSwingBorderLibrary"/>
		<rdfs:comment xml:lang="en">JavaLibrary implementing the javax.swing.plaf.basic package for j2se-1_6</rdfs:comment>
	</owl:Class>
	<owl:Class rdf:about="&j2se-1_6;JavaxSwingPlafMetalLibrary">
		<rdfs:subClassOf rdf:resource="&j2se-1_5;JavaxSwingPlafMetalLibrary"/>
		<rdfs:seeAlso rdf:resource="&j2se-1_6;JavaxSwingPlafBasicLibrary"/>
		<rdfs:seeAlso rdf:resource="&j2se-1_6;JavaAwtLibrary"/>
		<rdfs:seeAlso rdf:resource="&j2se-1_6;JavaxSwingEventLibrary"/>
		<rdfs:seeAlso rdf:resource="&j2se-1_6;JavaxSwingTreeLibrary"/>
		<rdfs:seeAlso rdf:resource="&j2se-1_6;JavaxSwingPlafLibrary"/>
		<rdfs:seeAlso rdf:resource="&j2se-1_6;JavaxSwingLibrary"/>
		<rdfs:seeAlso rdf:resource="&j2se-1_6;JavaBeansLibrary"/>
		<rdfs:seeAlso rdf:resource="&j2se-1_6;JavaIoLibrary"/>
		<rdfs:seeAlso rdf:resource="&j2se-1_6;JavaAwtEventLibrary"/>
		<rdfs:seeAlso rdf:resource="&j2se-1_6;JavaLangLibrary"/>
		<rdfs:seeAlso rdf:resource="&j2se-1_6;JavaxSwingBorderLibrary"/>
		<rdfs:comment xml:lang="en">JavaLibrary implementing the javax.swing.plaf.metal package for j2se-1_6</rdfs:comment>
	</owl:Class>
	<owl:Class rdf:about="&j2se-1_6;JavaxSwingPlafMultiLibrary">
		<rdfs:subClassOf rdf:resource="&j2se-1_5;JavaxSwingPlafMultiLibrary"/>
		<rdfs:seeAlso rdf:resource="&j2se-1_6;JavaAwtLibrary"/>
		<rdfs:seeAlso rdf:resource="&j2se-1_6;JavaxSwingTextLibrary"/>
		<rdfs:seeAlso rdf:resource="&j2se-1_6;JavaxSwingTreeLibrary"/>
		<rdfs:seeAlso rdf:resource="&j2se-1_6;JavaxSwingPlafLibrary"/>
		<rdfs:seeAlso rdf:resource="&j2se-1_6;JavaxAccessibilityLibrary"/>
		<rdfs:seeAlso rdf:resource="&j2se-1_6;JavaxSwingFilechooserLibrary"/>
		<rdfs:seeAlso rdf:resource="&j2se-1_6;JavaUtilLibrary"/>
		<rdfs:seeAlso rdf:resource="&j2se-1_6;JavaxSwingLibrary"/>
		<rdfs:seeAlso rdf:resource="&j2se-1_6;JavaIoLibrary"/>
		<rdfs:seeAlso rdf:resource="&j2se-1_6;JavaAwtEventLibrary"/>
		<rdfs:seeAlso rdf:resource="&j2se-1_6;JavaLangLibrary"/>
		<rdfs:comment xml:lang="en">JavaLibrary implementing the javax.swing.plaf.multi package for j2se-1_6</rdfs:comment>
	</owl:Class>
	<owl:Class rdf:about="&j2se-1_6;JavaxSwingPlafSynthLibrary">
		<rdfs:subClassOf rdf:resource="&j2se-1_5;JavaxSwingPlafSynthLibrary"/>
		<rdfs:seeAlso rdf:resource="&j2se-1_6;JavaxSwingPlafBasicLibrary"/>
		<rdfs:seeAlso rdf:resource="&j2se-1_6;JavaLangLibrary"/>
		<rdfs:seeAlso rdf:resource="&j2se-1_6;JavaAwtLibrary"/>
		<rdfs:seeAlso rdf:resource="&j2se-1_6;JavaxSwingLibrary"/>
		<rdfs:seeAlso rdf:resource="&j2se-1_6;JavaNetLibrary"/>
		<rdfs:seeAlso rdf:resource="&j2se-1_6;JavaIoLibrary"/>
		<rdfs:seeAlso rdf:resource="&j2se-1_6;JavaAwtEventLibrary"/>
		<rdfs:seeAlso rdf:resource="&j2se-1_6;JavaxSwingPlafLibrary"/>
		<rdfs:comment xml:lang="en">JavaLibrary implementing the javax.swing.plaf.synth package for j2se-1_6</rdfs:comment>
	</owl:Class>
	<owl:Class rdf:about="&j2se-1_6;JavaxSwingTableLibrary">
		<rdfs:subClassOf rdf:resource="&j2se-1_5;JavaxSwingTableLibrary"/>
		<rdfs:seeAlso rdf:resource="&j2se-1_6;JavaUtilLibrary"/>
		<rdfs:seeAlso rdf:resource="&j2se-1_6;JavaAwtLibrary"/>
		<rdfs:seeAlso rdf:resource="&j2se-1_6;JavaxSwingLibrary"/>
		<rdfs:seeAlso rdf:resource="&j2se-1_6;JavaxSwingEventLibrary"/>
		<rdfs:seeAlso rdf:resource="&j2se-1_6;JavaBeansLibrary"/>
		<rdfs:seeAlso rdf:resource="&j2se-1_6;JavaIoLibrary"/>
		<rdfs:seeAlso rdf:resource="&j2se-1_6;JavaAwtEventLibrary"/>
		<rdfs:seeAlso rdf:resource="&j2se-1_6;JavaLangLibrary"/>
		<rdfs:seeAlso rdf:resource="&j2se-1_6;JavaxSwingPlafLibrary"/>
		<rdfs:seeAlso rdf:resource="&j2se-1_6;JavaxAccessibilityLibrary"/>
		<rdfs:seeAlso rdf:resource="&j2se-1_6;JavaxSwingBorderLibrary"/>
		<rdfs:comment xml:lang="en">JavaLibrary implementing the javax.swing.table package for j2se-1_6</rdfs:comment>
	</owl:Class>
	<owl:Class rdf:about="&j2se-1_6;JavaxSwingUndoLibrary">
		<owl:equivalentClass rdf:resource="&j2se-1_5;JavaxSwingUndoLibrary"/>
		<rdfs:subClassOf rdf:resource="&java;JavaLibrary"/>
		<rdfs:seeAlso rdf:resource="&j2se-1_6;JavaUtilLibrary"/>
		<rdfs:seeAlso rdf:resource="&j2se-1_6;JavaIoLibrary"/>
		<rdfs:seeAlso rdf:resource="&j2se-1_6;JavaLangLibrary"/>
		<rdfs:seeAlso rdf:resource="&j2se-1_6;JavaxSwingEventLibrary"/>
		<rdfs:comment xml:lang="en">JavaLibrary implementing the javax.swing.undo package for j2se-1_6</rdfs:comment>
	</owl:Class>
	<owl:Class rdf:about="&j2se-1_6;JavaxToolsLibrary">
		<rdfs:subClassOf rdf:resource="&java;JavaLibrary"/>
		<rdfs:seeAlso rdf:resource="&j2se-1_6;JavaUtilLibrary"/>
		<rdfs:seeAlso rdf:resource="&j2se-1_6;JavaNioCharsetLibrary"/>
		<rdfs:seeAlso rdf:resource="&j2se-1_6;JavaLangLibrary"/>
		<rdfs:seeAlso rdf:resource="&j2se-1_6;JavaNetLibrary"/>
		<rdfs:seeAlso rdf:resource="&j2se-1_6;JavaxLangModelElementLibrary"/>
		<rdfs:seeAlso rdf:resource="&j2se-1_6;JavaUtilConcurrentLibrary"/>
		<rdfs:seeAlso rdf:resource="&j2se-1_6;JavaIoLibrary"/>
		<rdfs:comment xml:lang="en">JavaLibrary implementing the javax.tools package for j2se-1_6</rdfs:comment>
	</owl:Class>
	<owl:Class rdf:about="&j2se-1_6;JavaxTransactionLibrary">
		<owl:equivalentClass rdf:resource="&j2se-1_5;JavaxTransactionLibrary"/>
		<rdfs:subClassOf rdf:resource="&java;JavaLibrary"/>
		<rdfs:seeAlso rdf:resource="&j2se-1_6;JavaRmiLibrary"/>
		<rdfs:seeAlso rdf:resource="&j2se-1_6;JavaLangLibrary"/>
		<rdfs:comment xml:lang="en">JavaLibrary implementing the javax.transaction package for j2se-1_6</rdfs:comment>
	</owl:Class>
	<owl:Class rdf:about="&j2se-1_6;JavaxTransactionXaLibrary">
		<owl:equivalentClass rdf:resource="&j2se-1_5;JavaxTransactionXaLibrary"/>
		<rdfs:subClassOf rdf:resource="&java;JavaLibrary"/>
		<rdfs:seeAlso rdf:resource="&j2se-1_6;JavaLangLibrary"/>
		<rdfs:comment xml:lang="en">JavaLibrary implementing the javax.transaction.xa package for j2se-1_6</rdfs:comment>
	</owl:Class>
	<owl:Class rdf:about="&j2se-1_6;JavaxXmlLibrary">
		<owl:equivalentClass rdf:resource="&j2se-1_5;JavaxXmlLibrary"/>
		<rdfs:subClassOf rdf:resource="&java;JavaLibrary"/>
		<rdfs:seeAlso rdf:resource="&j2se-1_6;JavaLangLibrary"/>
		<rdfs:comment xml:lang="en">JavaLibrary implementing the javax.xml package for j2se-1_6</rdfs:comment>
	</owl:Class>
	<owl:Class rdf:about="&j2se-1_6;JavaxXmlBindLibrary">
		<rdfs:subClassOf rdf:resource="&java;JavaLibrary"/>
		<rdfs:seeAlso rdf:resource="&j2se-1_6;JavaUtilLibrary"/>
		<rdfs:seeAlso rdf:resource="&j2se-1_6;JavaxXmlNamespaceLibrary"/>
		<rdfs:seeAlso rdf:resource="&j2se-1_6;JavaxXmlTransformLibrary"/>
		<rdfs:seeAlso rdf:resource="&j2se-1_6;JavaxXmlBindAnnotationAdaptersLibrary"/>
		<rdfs:seeAlso rdf:resource="&j2se-1_6;OrgW3cDomLibrary"/>
		<rdfs:seeAlso rdf:resource="&j2se-1_6;JavaNetLibrary"/>
		<rdfs:seeAlso rdf:resource="&j2se-1_6;JavaxXmlValidationLibrary"/>
		<rdfs:seeAlso rdf:resource="&j2se-1_6;JavaIoLibrary"/>
		<rdfs:seeAlso rdf:resource="&j2se-1_6;JavaxXmlBindAttachmentLibrary"/>
		<rdfs:seeAlso rdf:resource="&j2se-1_6;JavaLangLibrary"/>
		<rdfs:seeAlso rdf:resource="&j2se-1_6;OrgXmlSaxLibrary"/>
		<rdfs:seeAlso rdf:resource="&j2se-1_6;JavaxXmlStreamLibrary"/>
		<rdfs:seeAlso rdf:resource="&j2se-1_6;JavaMathLibrary"/>
		<rdfs:comment xml:lang="en">JavaLibrary implementing the javax.xml.bind package for j2se-1_6</rdfs:comment>
	</owl:Class>
	<owl:Class rdf:about="&j2se-1_6;JavaxXmlBindAnnotationLibrary">
		<rdfs:subClassOf rdf:resource="&java;JavaLibrary"/>
		<rdfs:seeAlso rdf:resource="&j2se-1_6;JavaxXmlBindLibrary"/>
		<rdfs:seeAlso rdf:resource="&j2se-1_6;JavaxXmlParsersLibrary"/>
		<rdfs:seeAlso rdf:resource="&j2se-1_6;JavaxXmlTransformLibrary"/>
		<rdfs:seeAlso rdf:resource="&j2se-1_6;JavaLangLibrary"/>
		<rdfs:seeAlso rdf:resource="&j2se-1_6;OrgW3cDomLibrary"/>
		<rdfs:seeAlso rdf:resource="&j2se-1_6;JavaLangAnnotationLibrary"/>
		<rdfs:seeAlso rdf:resource="&j2se-1_6;JavaxXmlTransformDomLibrary"/>
		<rdfs:comment xml:lang="en">JavaLibrary implementing the javax.xml.bind.annotation package for j2se-1_6</rdfs:comment>
	</owl:Class>
	<owl:Class rdf:about="&j2se-1_6;JavaxXmlBindAnnotationAdaptersLibrary">
		<rdfs:subClassOf rdf:resource="&java;JavaLibrary"/>
		<rdfs:seeAlso rdf:resource="&j2se-1_6;JavaLangLibrary"/>
		<rdfs:seeAlso rdf:resource="&j2se-1_6;JavaLangAnnotationLibrary"/>
		<rdfs:comment xml:lang="en">JavaLibrary implementing the javax.xml.bind.annotation.adapters package for j2se-1_6</rdfs:comment>
	</owl:Class>
	<owl:Class rdf:about="&j2se-1_6;JavaxXmlBindAttachmentLibrary">
		<rdfs:subClassOf rdf:resource="&java;JavaLibrary"/>
		<rdfs:seeAlso rdf:resource="&j2se-1_6;JavaLangLibrary"/>
		<rdfs:seeAlso rdf:resource="&j2se-1_6;JavaxActivationLibrary"/>
		<rdfs:comment xml:lang="en">JavaLibrary implementing the javax.xml.bind.attachment package for j2se-1_6</rdfs:comment>
	</owl:Class>
	<owl:Class rdf:about="&j2se-1_6;JavaxXmlBindHelpersLibrary">
		<rdfs:subClassOf rdf:resource="&java;JavaLibrary"/>
		<rdfs:seeAlso rdf:resource="&j2se-1_6;JavaxXmlTransformLibrary"/>
		<rdfs:seeAlso rdf:resource="&j2se-1_6;JavaxXmlBindAnnotationAdaptersLibrary"/>
		<rdfs:seeAlso rdf:resource="&j2se-1_6;OrgW3cDomLibrary"/>
		<rdfs:seeAlso rdf:resource="&j2se-1_6;JavaNetLibrary"/>
		<rdfs:seeAlso rdf:resource="&j2se-1_6;JavaxXmlValidationLibrary"/>
		<rdfs:seeAlso rdf:resource="&j2se-1_6;JavaIoLibrary"/>
		<rdfs:seeAlso rdf:resource="&j2se-1_6;JavaxXmlBindAttachmentLibrary"/>
		<rdfs:seeAlso rdf:resource="&j2se-1_6;JavaxXmlBindLibrary"/>
		<rdfs:seeAlso rdf:resource="&j2se-1_6;JavaLangLibrary"/>
		<rdfs:seeAlso rdf:resource="&j2se-1_6;OrgXmlSaxLibrary"/>
		<rdfs:seeAlso rdf:resource="&j2se-1_6;JavaxXmlStreamLibrary"/>
		<rdfs:comment xml:lang="en">JavaLibrary implementing the javax.xml.bind.helpers package for j2se-1_6</rdfs:comment>
	</owl:Class>
	<owl:Class rdf:about="&j2se-1_6;JavaxXmlBindUtilLibrary">
		<rdfs:subClassOf rdf:resource="&java;JavaLibrary"/>
		<rdfs:seeAlso rdf:resource="&j2se-1_6;JavaxXmlBindLibrary"/>
		<rdfs:seeAlso rdf:resource="&j2se-1_6;JavaxXmlTransformSaxLibrary"/>
		<rdfs:seeAlso rdf:resource="&j2se-1_6;JavaLangLibrary"/>
		<rdfs:comment xml:lang="en">JavaLibrary implementing the javax.xml.bind.util package for j2se-1_6</rdfs:comment>
	</owl:Class>
	<owl:Class rdf:about="&j2se-1_6;JavaxXmlTransformLibrary">
		<rdfs:subClassOf rdf:resource="&j2se-1_5;JavaxXmlTransformLibrary"/>
		<rdfs:seeAlso rdf:resource="&j2se-1_6;JavaUtilLibrary"/>
		<rdfs:seeAlso rdf:resource="&j2se-1_6;JavaIoLibrary"/>
		<rdfs:seeAlso rdf:resource="&j2se-1_6;JavaLangLibrary"/>
		<rdfs:comment xml:lang="en">JavaLibrary implementing the javax.xml.transform package for j2se-1_6</rdfs:comment>
	</owl:Class>
	<owl:Class rdf:about="&j2se-1_6;JavaxXmlTransformSaxLibrary">
		<rdfs:subClassOf rdf:resource="&j2se-1_5;JavaxXmlTransformSaxLibrary"/>
		<rdfs:seeAlso rdf:resource="&j2se-1_6;JavaxXmlTransformLibrary"/>
		<rdfs:seeAlso rdf:resource="&j2se-1_6;JavaLangLibrary"/>
		<rdfs:seeAlso rdf:resource="&j2se-1_6;OrgXmlSaxExtLibrary"/>
		<rdfs:seeAlso rdf:resource="&j2se-1_6;OrgXmlSaxLibrary"/>
		<rdfs:comment xml:lang="en">JavaLibrary implementing the javax.xml.transform.sax package for j2se-1_6</rdfs:comment>
	</owl:Class>
	<owl:Class rdf:about="&j2se-1_6;JavaxXmlTransformDomLibrary">
		<owl:equivalentClass rdf:resource="&j2se-1_5;JavaxXmlTransformDomLibrary"/>
		<rdfs:subClassOf rdf:resource="&java;JavaLibrary"/>
		<rdfs:seeAlso rdf:resource="&j2se-1_6;JavaxXmlTransformLibrary"/>
		<rdfs:seeAlso rdf:resource="&j2se-1_6;JavaLangLibrary"/>
		<rdfs:seeAlso rdf:resource="&j2se-1_6;OrgW3cDomLibrary"/>
		<rdfs:comment xml:lang="en">JavaLibrary implementing the javax.xml.transform.dom package for j2se-1_6</rdfs:comment>
	</owl:Class>
	<owl:Class rdf:about="&j2se-1_6;JavaxXmlTransformStaxLibrary">
		<rdfs:subClassOf rdf:resource="&java;JavaLibrary"/>
		<rdfs:seeAlso rdf:resource="&j2se-1_6;JavaxXmlTransformLibrary"/>
		<rdfs:seeAlso rdf:resource="&j2se-1_6;JavaLangLibrary"/>
		<rdfs:seeAlso rdf:resource="&j2se-1_6;JavaxXmlStreamLibrary"/>
		<rdfs:comment xml:lang="en">JavaLibrary implementing the javax.xml.transform.stax package for j2se-1_6</rdfs:comment>
	</owl:Class>
	<owl:Class rdf:about="&j2se-1_6;JavaxXmlTransformStreamLibrary">
		<owl:equivalentClass rdf:resource="&j2se-1_5;JavaxXmlTransformStreamLibrary"/>
		<rdfs:subClassOf rdf:resource="&java;JavaLibrary"/>
		<rdfs:seeAlso rdf:resource="&j2se-1_6;JavaxXmlTransformLibrary"/>
		<rdfs:seeAlso rdf:resource="&j2se-1_6;JavaIoLibrary"/>
		<rdfs:seeAlso rdf:resource="&j2se-1_6;JavaLangLibrary"/>
		<rdfs:comment xml:lang="en">JavaLibrary implementing the javax.xml.transform.stream package for j2se-1_6</rdfs:comment>
	</owl:Class>
	<owl:Class rdf:about="&j2se-1_6;JavaxXmlCryptoLibrary">
		<rdfs:subClassOf rdf:resource="&java;JavaLibrary"/>
		<rdfs:seeAlso rdf:resource="&j2se-1_6;JavaUtilLibrary"/>
		<rdfs:seeAlso rdf:resource="&j2se-1_6;JavaLangLibrary"/>
		<rdfs:seeAlso rdf:resource="&j2se-1_6;JavaSecurityLibrary"/>
		<rdfs:seeAlso rdf:resource="&j2se-1_6;JavaxXmlCryptoDsigKeyinfoLibrary"/>
		<rdfs:seeAlso rdf:resource="&j2se-1_6;JavaIoLibrary"/>
		<rdfs:seeAlso rdf:resource="&j2se-1_6;JavaSecuritySpecLibrary"/>
		<rdfs:comment xml:lang="en">JavaLibrary implementing the javax.xml.crypto package for j2se-1_6</rdfs:comment>
	</owl:Class>
	<owl:Class rdf:about="&j2se-1_6;JavaxXmlCryptoDomLibrary">
		<rdfs:subClassOf rdf:resource="&java;JavaLibrary"/>
		<rdfs:seeAlso rdf:resource="&j2se-1_6;JavaUtilLibrary"/>
		<rdfs:seeAlso rdf:resource="&j2se-1_6;JavaLangLibrary"/>
		<rdfs:seeAlso rdf:resource="&j2se-1_6;JavaxXmlCryptoLibrary"/>
		<rdfs:seeAlso rdf:resource="&j2se-1_6;OrgW3cDomLibrary"/>
		<rdfs:comment xml:lang="en">JavaLibrary implementing the javax.xml.crypto.dom package for j2se-1_6</rdfs:comment>
	</owl:Class>
	<owl:Class rdf:about="&j2se-1_6;JavaxXmlCryptoDsigLibrary">
		<rdfs:subClassOf rdf:resource="&java;JavaLibrary"/>
		<rdfs:seeAlso rdf:resource="&j2se-1_6;JavaUtilLibrary"/>
		<rdfs:seeAlso rdf:resource="&j2se-1_6;JavaxXmlCryptoDsigSpecLibrary"/>
		<rdfs:seeAlso rdf:resource="&j2se-1_6;JavaxXmlCryptoDsigKeyinfoLibrary"/>
		<rdfs:seeAlso rdf:resource="&j2se-1_6;JavaIoLibrary"/>
		<rdfs:seeAlso rdf:resource="&j2se-1_6;JavaxXmlCryptoLibrary"/>
		<rdfs:seeAlso rdf:resource="&j2se-1_6;JavaLangLibrary"/>
		<rdfs:seeAlso rdf:resource="&j2se-1_6;JavaSecurityLibrary"/>
		<rdfs:seeAlso rdf:resource="&j2se-1_6;JavaSecuritySpecLibrary"/>
		<rdfs:comment xml:lang="en">JavaLibrary implementing the javax.xml.crypto.dsig package for j2se-1_6</rdfs:comment>
	</owl:Class>
	<owl:Class rdf:about="&j2se-1_6;JavaxXmlCryptoDsigDomLibrary">
		<rdfs:subClassOf rdf:resource="&java;JavaLibrary"/>
		<rdfs:seeAlso rdf:resource="&j2se-1_6;JavaxXmlCryptoDsigLibrary"/>
		<rdfs:seeAlso rdf:resource="&j2se-1_6;JavaxXmlCryptoLibrary"/>
		<rdfs:seeAlso rdf:resource="&j2se-1_6;JavaSecurityLibrary"/>
		<rdfs:seeAlso rdf:resource="&j2se-1_6;OrgW3cDomLibrary"/>
		<rdfs:seeAlso rdf:resource="&j2se-1_6;JavaxXmlCryptoDomLibrary"/>
		<rdfs:comment xml:lang="en">JavaLibrary implementing the javax.xml.crypto.dsig.dom package for j2se-1_6</rdfs:comment>
	</owl:Class>
	<owl:Class rdf:about="&j2se-1_6;JavaxXmlCryptoDsigKeyinfoLibrary">
		<rdfs:subClassOf rdf:resource="&java;JavaLibrary"/>
		<rdfs:seeAlso rdf:resource="&j2se-1_6;JavaUtilLibrary"/>
		<rdfs:seeAlso rdf:resource="&j2se-1_6;JavaMathLibrary"/>
		<rdfs:seeAlso rdf:resource="&j2se-1_6;JavaLangLibrary"/>
		<rdfs:seeAlso rdf:resource="&j2se-1_6;JavaxXmlCryptoLibrary"/>
		<rdfs:seeAlso rdf:resource="&j2se-1_6;JavaSecurityLibrary"/>
		<rdfs:comment xml:lang="en">JavaLibrary implementing the javax.xml.crypto.dsig.keyinfo package for j2se-1_6</rdfs:comment>
	</owl:Class>
	<owl:Class rdf:about="&j2se-1_6;JavaxXmlCryptoDsigSpecLibrary">
		<rdfs:subClassOf rdf:resource="&java;JavaLibrary"/>
		<rdfs:seeAlso rdf:resource="&j2se-1_6;JavaUtilLibrary"/>
		<rdfs:seeAlso rdf:resource="&j2se-1_6;JavaSecuritySpecLibrary"/>
		<rdfs:seeAlso rdf:resource="&j2se-1_6;JavaLangLibrary"/>
		<rdfs:seeAlso rdf:resource="&j2se-1_6;JavaxXmlCryptoLibrary"/>
		<rdfs:comment xml:lang="en">JavaLibrary implementing the javax.xml.crypto.dsig.spec package for j2se-1_6</rdfs:comment>
	</owl:Class>
	<owl:Class rdf:about="&j2se-1_6;JavaxXmlDatatypeLibrary">
		<rdfs:subClassOf rdf:resource="&j2se-1_5;JavaxXmlDatatypeLibrary"/>
		<rdfs:seeAlso rdf:resource="&j2se-1_6;JavaUtilLibrary"/>
		<rdfs:seeAlso rdf:resource="&j2se-1_6;JavaxXmlNamespaceLibrary"/>
		<rdfs:seeAlso rdf:resource="&j2se-1_6;JavaLangLibrary"/>
		<rdfs:seeAlso rdf:resource="&j2se-1_6;JavaMathLibrary"/>
		<rdfs:comment xml:lang="en">JavaLibrary implementing the javax.xml.datatype package for j2se-1_6</rdfs:comment>
	</owl:Class>
	<owl:Class rdf:about="&j2se-1_6;JavaxXmlNamespaceLibrary">
		<owl:equivalentClass rdf:resource="&j2se-1_5;JavaxXmlNamespaceLibrary"/>
		<rdfs:subClassOf rdf:resource="&java;JavaLibrary"/>
		<rdfs:seeAlso rdf:resource="&j2se-1_6;JavaUtilLibrary"/>
		<rdfs:seeAlso rdf:resource="&j2se-1_6;JavaIoLibrary"/>
		<rdfs:seeAlso rdf:resource="&j2se-1_6;JavaLangLibrary"/>
		<rdfs:comment xml:lang="en">JavaLibrary implementing the javax.xml.namespace package for j2se-1_6</rdfs:comment>
	</owl:Class>
	<owl:Class rdf:about="&j2se-1_6;JavaxXmlParsersLibrary">
		<rdfs:subClassOf rdf:resource="&j2se-1_5;JavaxXmlParsersLibrary"/>
		<rdfs:seeAlso rdf:resource="&j2se-1_6;JavaLangLibrary"/>
		<rdfs:seeAlso rdf:resource="&j2se-1_6;OrgW3cDomLibrary"/>
		<rdfs:seeAlso rdf:resource="&j2se-1_6;OrgXmlSaxLibrary"/>
		<rdfs:seeAlso rdf:resource="&j2se-1_6;JavaxXmlValidationLibrary"/>
		<rdfs:seeAlso rdf:resource="&j2se-1_6;OrgXmlSaxHelpersLibrary"/>
		<rdfs:seeAlso rdf:resource="&j2se-1_6;JavaIoLibrary"/>
		<rdfs:comment xml:lang="en">JavaLibrary implementing the javax.xml.parsers package for j2se-1_6</rdfs:comment>
	</owl:Class>
	<owl:Class rdf:about="&j2se-1_6;JavaxXmlSoapLibrary">
		<rdfs:subClassOf rdf:resource="&java;JavaLibrary"/>
		<rdfs:seeAlso rdf:resource="&j2se-1_6;JavaUtilLibrary"/>
		<rdfs:seeAlso rdf:resource="&j2se-1_6;JavaxXmlNamespaceLibrary"/>
		<rdfs:seeAlso rdf:resource="&j2se-1_6;JavaxXmlTransformLibrary"/>
		<rdfs:seeAlso rdf:resource="&j2se-1_6;JavaLangLibrary"/>
		<rdfs:seeAlso rdf:resource="&j2se-1_6;OrgW3cDomLibrary"/>
		<rdfs:seeAlso rdf:resource="&j2se-1_6;JavaxActivationLibrary"/>
		<rdfs:seeAlso rdf:resource="&j2se-1_6;JavaIoLibrary"/>
		<rdfs:seeAlso rdf:resource="&j2se-1_6;JavaxXmlTransformDomLibrary"/>
		<rdfs:comment xml:lang="en">JavaLibrary implementing the javax.xml.soap package for j2se-1_6</rdfs:comment>
	</owl:Class>
	<owl:Class rdf:about="&j2se-1_6;JavaxXmlStreamLibrary">
		<rdfs:subClassOf rdf:resource="&java;JavaLibrary"/>
		<rdfs:seeAlso rdf:resource="&j2se-1_6;JavaUtilLibrary"/>
		<rdfs:seeAlso rdf:resource="&j2se-1_6;JavaxXmlNamespaceLibrary"/>
		<rdfs:seeAlso rdf:resource="&j2se-1_6;JavaxXmlTransformLibrary"/>
		<rdfs:seeAlso rdf:resource="&j2se-1_6;JavaIoLibrary"/>
		<rdfs:seeAlso rdf:resource="&j2se-1_6;JavaLangLibrary"/>
		<rdfs:seeAlso rdf:resource="&j2se-1_6;JavaxXmlStreamUtilLibrary"/>
		<rdfs:seeAlso rdf:resource="&j2se-1_6;JavaxXmlStreamEventsLibrary"/>
		<rdfs:comment xml:lang="en">JavaLibrary implementing the javax.xml.stream package for j2se-1_6</rdfs:comment>
	</owl:Class>
	<owl:Class rdf:about="&j2se-1_6;JavaxXmlStreamUtilLibrary">
		<rdfs:subClassOf rdf:resource="&java;JavaLibrary"/>
		<rdfs:seeAlso rdf:resource="&j2se-1_6;JavaxXmlNamespaceLibrary"/>
		<rdfs:seeAlso rdf:resource="&j2se-1_6;JavaLangLibrary"/>
		<rdfs:seeAlso rdf:resource="&j2se-1_6;JavaxXmlStreamEventsLibrary"/>
		<rdfs:seeAlso rdf:resource="&j2se-1_6;JavaxXmlStreamLibrary"/>
		<rdfs:comment xml:lang="en">JavaLibrary implementing the javax.xml.stream.util package for j2se-1_6</rdfs:comment>
	</owl:Class>
	<owl:Class rdf:about="&j2se-1_6;JavaxXmlStreamEventsLibrary">
		<rdfs:subClassOf rdf:resource="&java;JavaLibrary"/>
		<rdfs:seeAlso rdf:resource="&j2se-1_6;JavaUtilLibrary"/>
		<rdfs:seeAlso rdf:resource="&j2se-1_6;JavaxXmlNamespaceLibrary"/>
		<rdfs:seeAlso rdf:resource="&j2se-1_6;JavaIoLibrary"/>
		<rdfs:seeAlso rdf:resource="&j2se-1_6;JavaLangLibrary"/>
		<rdfs:seeAlso rdf:resource="&j2se-1_6;JavaxXmlStreamLibrary"/>
		<rdfs:comment xml:lang="en">JavaLibrary implementing the javax.xml.stream.events package for j2se-1_6</rdfs:comment>
	</owl:Class>
	<owl:Class rdf:about="&j2se-1_6;JavaxXmlValidationLibrary">
		<rdfs:subClassOf rdf:resource="&j2se-1_5;JavaxXmlValidationLibrary"/>
		<rdfs:seeAlso rdf:resource="&j2se-1_6;JavaxXmlTransformLibrary"/>
		<rdfs:seeAlso rdf:resource="&j2se-1_6;JavaIoLibrary"/>
		<rdfs:seeAlso rdf:resource="&j2se-1_6;JavaLangLibrary"/>
		<rdfs:seeAlso rdf:resource="&j2se-1_6;OrgW3cDomLibrary"/>
		<rdfs:seeAlso rdf:resource="&j2se-1_6;OrgXmlSaxLibrary"/>
		<rdfs:seeAlso rdf:resource="&j2se-1_6;OrgW3cDomLsLibrary"/>
		<rdfs:seeAlso rdf:resource="&j2se-1_6;JavaNetLibrary"/>
		<rdfs:comment xml:lang="en">JavaLibrary implementing the javax.xml.validation package for j2se-1_6</rdfs:comment>
	</owl:Class>
	<owl:Class rdf:about="&j2se-1_6;JavaxXmlWsLibrary">
		<rdfs:subClassOf rdf:resource="&java;JavaLibrary"/>
		<rdfs:seeAlso rdf:resource="&j2se-1_6;JavaUtilLibrary"/>
		<rdfs:seeAlso rdf:resource="&j2se-1_6;JavaxXmlBindLibrary"/>
		<rdfs:seeAlso rdf:resource="&j2se-1_6;JavaxXmlNamespaceLibrary"/>
		<rdfs:seeAlso rdf:resource="&j2se-1_6;JavaxXmlTransformLibrary"/>
		<rdfs:seeAlso rdf:resource="&j2se-1_6;JavaLangLibrary"/>
		<rdfs:seeAlso rdf:resource="&j2se-1_6;JavaSecurityLibrary"/>
		<rdfs:seeAlso rdf:resource="&j2se-1_6;JavaNetLibrary"/>
		<rdfs:seeAlso rdf:resource="&j2se-1_6;JavaUtilConcurrentLibrary"/>
		<rdfs:seeAlso rdf:resource="&j2se-1_6;JavaxXmlWsHandlerLibrary"/>
		<rdfs:seeAlso rdf:resource="&j2se-1_6;JavaLangAnnotationLibrary"/>
		<rdfs:comment xml:lang="en">JavaLibrary implementing the javax.xml.ws package for j2se-1_6</rdfs:comment>
	</owl:Class>
	<owl:Class rdf:about="&j2se-1_6;JavaxXmlWsHandlerLibrary">
		<rdfs:subClassOf rdf:resource="&java;JavaLibrary"/>
		<rdfs:seeAlso rdf:resource="&j2se-1_6;JavaUtilLibrary"/>
		<rdfs:seeAlso rdf:resource="&j2se-1_6;JavaxXmlNamespaceLibrary"/>
		<rdfs:seeAlso rdf:resource="&j2se-1_6;JavaLangLibrary"/>
		<rdfs:seeAlso rdf:resource="&j2se-1_6;JavaxXmlWsLibrary"/>
		<rdfs:comment xml:lang="en">JavaLibrary implementing the javax.xml.ws.handler package for j2se-1_6</rdfs:comment>
	</owl:Class>
	<owl:Class rdf:about="&j2se-1_6;JavaxXmlWsHandlerSoapLibrary">
		<rdfs:subClassOf rdf:resource="&java;JavaLibrary"/>
		<rdfs:seeAlso rdf:resource="&j2se-1_6;JavaUtilLibrary"/>
		<rdfs:seeAlso rdf:resource="&j2se-1_6;JavaxXmlBindLibrary"/>
		<rdfs:seeAlso rdf:resource="&j2se-1_6;JavaxXmlWsHandlerLibrary"/>
		<rdfs:seeAlso rdf:resource="&j2se-1_6;JavaxXmlNamespaceLibrary"/>
		<rdfs:seeAlso rdf:resource="&j2se-1_6;JavaxXmlSoapLibrary"/>
		<rdfs:comment xml:lang="en">JavaLibrary implementing the javax.xml.ws.handler.soap package for j2se-1_6</rdfs:comment>
	</owl:Class>
	<owl:Class rdf:about="&j2se-1_6;JavaxXmlWsHttpLibrary">
		<rdfs:subClassOf rdf:resource="&java;JavaLibrary"/>
		<rdfs:seeAlso rdf:resource="&j2se-1_6;JavaLangLibrary"/>
		<rdfs:seeAlso rdf:resource="&j2se-1_6;JavaxXmlWsLibrary"/>
		<rdfs:comment xml:lang="en">JavaLibrary implementing the javax.xml.ws.http package for j2se-1_6</rdfs:comment>
	</owl:Class>
	<owl:Class rdf:about="&j2se-1_6;JavaxXmlWsSoapLibrary">
		<rdfs:subClassOf rdf:resource="&java;JavaLibrary"/>
		<rdfs:seeAlso rdf:resource="&j2se-1_6;JavaUtilLibrary"/>
		<rdfs:seeAlso rdf:resource="&j2se-1_6;JavaLangLibrary"/>
		<rdfs:seeAlso rdf:resource="&j2se-1_6;JavaxXmlWsLibrary"/>
		<rdfs:seeAlso rdf:resource="&j2se-1_6;JavaxXmlSoapLibrary"/>
		<rdfs:comment xml:lang="en">JavaLibrary implementing the javax.xml.ws.soap package for j2se-1_6</rdfs:comment>
	</owl:Class>
	<owl:Class rdf:about="&j2se-1_6;JavaxXmlWsSpiLibrary">
		<rdfs:subClassOf rdf:resource="&java;JavaLibrary"/>
		<rdfs:seeAlso rdf:resource="&j2se-1_6;JavaUtilLibrary"/>
		<rdfs:seeAlso rdf:resource="&j2se-1_6;JavaxXmlBindLibrary"/>
		<rdfs:seeAlso rdf:resource="&j2se-1_6;JavaxXmlNamespaceLibrary"/>
		<rdfs:seeAlso rdf:resource="&j2se-1_6;JavaLangLibrary"/>
		<rdfs:seeAlso rdf:resource="&j2se-1_6;JavaxXmlWsLibrary"/>
		<rdfs:seeAlso rdf:resource="&j2se-1_6;JavaNetLibrary"/>
		<rdfs:seeAlso rdf:resource="&j2se-1_6;JavaUtilConcurrentLibrary"/>
		<rdfs:seeAlso rdf:resource="&j2se-1_6;JavaxXmlWsHandlerLibrary"/>
		<rdfs:comment xml:lang="en">JavaLibrary implementing the javax.xml.ws.spi package for j2se-1_6</rdfs:comment>
	</owl:Class>
	<owl:Class rdf:about="&j2se-1_6;JavaxXmlXpathLibrary">
		<rdfs:subClassOf rdf:resource="&j2se-1_5;JavaxXmlXpathLibrary"/>
		<rdfs:seeAlso rdf:resource="&j2se-1_6;JavaUtilLibrary"/>
		<rdfs:seeAlso rdf:resource="&j2se-1_6;JavaxXmlNamespaceLibrary"/>
		<rdfs:seeAlso rdf:resource="&j2se-1_6;JavaIoLibrary"/>
		<rdfs:seeAlso rdf:resource="&j2se-1_6;JavaLangLibrary"/>
		<rdfs:seeAlso rdf:resource="&j2se-1_6;OrgXmlSaxLibrary"/>
		<rdfs:comment xml:lang="en">JavaLibrary implementing the javax.xml.xpath package for j2se-1_6</rdfs:comment>
	</owl:Class>
	<owl:Class rdf:about="&j2se-1_6;OrgW3cDomLibrary">
		<owl:equivalentClass rdf:resource="&j2se-1_5;OrgW3cDomLibrary"/>
		<rdfs:subClassOf rdf:resource="&java;JavaLibrary"/>
		<rdfs:seeAlso rdf:resource="&j2se-1_6;JavaLangLibrary"/>
		<rdfs:comment xml:lang="en">JavaLibrary implementing the org.w3c.dom package for j2se-1_6</rdfs:comment>
	</owl:Class>
	<owl:Class rdf:about="&j2se-1_6;OrgW3cDomBootstrapLibrary">
		<owl:equivalentClass rdf:resource="&j2se-1_5;OrgW3cDomBootstrapLibrary"/>
		<rdfs:subClassOf rdf:resource="&java;JavaLibrary"/>
		<rdfs:seeAlso rdf:resource="&j2se-1_6;JavaLangLibrary"/>
		<rdfs:seeAlso rdf:resource="&j2se-1_6;OrgW3cDomLibrary"/>
		<rdfs:comment xml:lang="en">JavaLibrary implementing the org.w3c.dom.bootstrap package for j2se-1_6</rdfs:comment>
	</owl:Class>
	<owl:Class rdf:about="&j2se-1_6;OrgW3cDomCssLibrary">
		<owl:equivalentClass rdf:resource="&j2se-1_5;OrgW3cDomCssLibrary"/>
		<rdfs:subClassOf rdf:resource="&java;JavaLibrary"/>
		<rdfs:seeAlso rdf:resource="&j2se-1_6;OrgW3cDomViewsLibrary"/>
		<rdfs:seeAlso rdf:resource="&j2se-1_6;JavaLangLibrary"/>
		<rdfs:seeAlso rdf:resource="&j2se-1_6;OrgW3cDomLibrary"/>
		<rdfs:seeAlso rdf:resource="&j2se-1_6;OrgW3cDomStylesheetsLibrary"/>
		<rdfs:comment xml:lang="en">JavaLibrary implementing the org.w3c.dom.css package for j2se-1_6</rdfs:comment>
	</owl:Class>
	<owl:Class rdf:about="&j2se-1_6;OrgW3cDomStylesheetsLibrary">
		<owl:equivalentClass rdf:resource="&j2se-1_5;OrgW3cDomStylesheetsLibrary"/>
		<rdfs:subClassOf rdf:resource="&java;JavaLibrary"/>
		<rdfs:seeAlso rdf:resource="&j2se-1_6;JavaLangLibrary"/>
		<rdfs:seeAlso rdf:resource="&j2se-1_6;OrgW3cDomLibrary"/>
		<rdfs:comment xml:lang="en">JavaLibrary implementing the org.w3c.dom.stylesheets package for j2se-1_6</rdfs:comment>
	</owl:Class>
	<owl:Class rdf:about="&j2se-1_6;OrgW3cDomViewsLibrary">
		<owl:equivalentClass rdf:resource="&j2se-1_5;OrgW3cDomViewsLibrary"/>
		<rdfs:subClassOf rdf:resource="&java;JavaLibrary"/>
		<rdfs:comment xml:lang="en">JavaLibrary implementing the org.w3c.dom.views package for j2se-1_6</rdfs:comment>
	</owl:Class>
	<owl:Class rdf:about="&j2se-1_6;OrgW3cDomEventsLibrary">
		<owl:equivalentClass rdf:resource="&j2se-1_5;OrgW3cDomEventsLibrary"/>
		<rdfs:subClassOf rdf:resource="&java;JavaLibrary"/>
		<rdfs:seeAlso rdf:resource="&j2se-1_6;OrgW3cDomViewsLibrary"/>
		<rdfs:seeAlso rdf:resource="&j2se-1_6;JavaLangLibrary"/>
		<rdfs:seeAlso rdf:resource="&j2se-1_6;OrgW3cDomLibrary"/>
		<rdfs:comment xml:lang="en">JavaLibrary implementing the org.w3c.dom.events package for j2se-1_6</rdfs:comment>
	</owl:Class>
	<owl:Class rdf:about="&j2se-1_6;OrgW3cDomHtmlLibrary">
		<owl:equivalentClass rdf:resource="&j2se-1_5;OrgW3cDomHtmlLibrary"/>
		<rdfs:subClassOf rdf:resource="&java;JavaLibrary"/>
		<rdfs:seeAlso rdf:resource="&j2se-1_6;JavaLangLibrary"/>
		<rdfs:seeAlso rdf:resource="&j2se-1_6;OrgW3cDomLibrary"/>
		<rdfs:comment xml:lang="en">JavaLibrary implementing the org.w3c.dom.html package for j2se-1_6</rdfs:comment>
	</owl:Class>
	<owl:Class rdf:about="&j2se-1_6;OrgW3cDomLsLibrary">
		<owl:equivalentClass rdf:resource="&j2se-1_5;OrgW3cDomLsLibrary"/>
		<rdfs:subClassOf rdf:resource="&java;JavaLibrary"/>
		<rdfs:seeAlso rdf:resource="&j2se-1_6;OrgW3cDomEventsLibrary"/>
		<rdfs:seeAlso rdf:resource="&j2se-1_6;JavaLangLibrary"/>
		<rdfs:seeAlso rdf:resource="&j2se-1_6;OrgW3cDomLibrary"/>
		<rdfs:seeAlso rdf:resource="&j2se-1_6;OrgW3cDomTraversalLibrary"/>
		<rdfs:seeAlso rdf:resource="&j2se-1_6;JavaIoLibrary"/>
		<rdfs:comment xml:lang="en">JavaLibrary implementing the org.w3c.dom.ls package for j2se-1_6</rdfs:comment>
	</owl:Class>
	<owl:Class rdf:about="&j2se-1_6;OrgW3cDomTraversalLibrary">
		<owl:equivalentClass rdf:resource="&j2se-1_5;OrgW3cDomTraversalLibrary"/>
		<rdfs:subClassOf rdf:resource="&java;JavaLibrary"/>
		<rdfs:seeAlso rdf:resource="&j2se-1_6;OrgW3cDomLibrary"/>
		<rdfs:comment xml:lang="en">JavaLibrary implementing the org.w3c.dom.traversal package for j2se-1_6</rdfs:comment>
	</owl:Class>
	<owl:Class rdf:about="&j2se-1_6;OrgW3cDomRangesLibrary">
		<owl:equivalentClass rdf:resource="&j2se-1_5;OrgW3cDomRangesLibrary"/>
		<rdfs:subClassOf rdf:resource="&java;JavaLibrary"/>
		<rdfs:seeAlso rdf:resource="&j2se-1_6;JavaLangLibrary"/>
		<rdfs:seeAlso rdf:resource="&j2se-1_6;OrgW3cDomLibrary"/>
		<rdfs:comment xml:lang="en">JavaLibrary implementing the org.w3c.dom.ranges package for j2se-1_6</rdfs:comment>
	</owl:Class>
	<owl:Class rdf:about="&j2se-1_6;OrgW3cDomXpathLibrary">
		<rdfs:subClassOf rdf:resource="&java;JavaLibrary"/>
		<rdfs:seeAlso rdf:resource="&j2se-1_6;JavaLangLibrary"/>
		<rdfs:seeAlso rdf:resource="&j2se-1_6;OrgW3cDomLibrary"/>
		<rdfs:comment xml:lang="en">JavaLibrary implementing the org.w3c.dom.xpath package for j2se-1_6</rdfs:comment>
	</owl:Class>
	<owl:Class rdf:about="&j2se-1_6;OrgOmgCORBA_2_3Library">
		<owl:equivalentClass rdf:resource="&j2se-1_5;OrgOmgCORBA_2_3Library"/>
		<rdfs:subClassOf rdf:resource="&java;JavaLibrary"/>
		<rdfs:seeAlso rdf:resource="&j2se-1_6;OrgOmgCORBALibrary"/>
		<rdfs:seeAlso rdf:resource="&j2se-1_6;JavaLangLibrary"/>
		<rdfs:seeAlso rdf:resource="&j2se-1_6;OrgOmgCORBAPortableLibrary"/>
		<rdfs:comment xml:lang="en">JavaLibrary implementing the org.omg.CORBA_2_3 package for j2se-1_6</rdfs:comment>
	</owl:Class>
	<owl:Class rdf:about="&j2se-1_6;OrgOmgCORBA_2_3PortableLibrary">
		<owl:equivalentClass rdf:resource="&j2se-1_5;OrgOmgCORBA_2_3PortableLibrary"/>
		<rdfs:subClassOf rdf:resource="&java;JavaLibrary"/>
		<rdfs:seeAlso rdf:resource="&j2se-1_6;OrgOmgCORBALibrary"/>
		<rdfs:seeAlso rdf:resource="&j2se-1_6;JavaIoLibrary"/>
		<rdfs:seeAlso rdf:resource="&j2se-1_6;JavaLangLibrary"/>
		<rdfs:seeAlso rdf:resource="&j2se-1_6;OrgOmgCORBAPortableLibrary"/>
		<rdfs:comment xml:lang="en">JavaLibrary implementing the org.omg.CORBA_2_3.portable package for j2se-1_6</rdfs:comment>
	</owl:Class>
	<owl:Class rdf:about="&j2se-1_6;OrgOmgCORBALibrary">
		<owl:equivalentClass rdf:resource="&j2se-1_5;OrgOmgCORBALibrary"/>
		<rdfs:subClassOf rdf:resource="&java;JavaLibrary"/>
		<rdfs:seeAlso rdf:resource="&j2se-1_6;JavaAppletLibrary"/>
		<rdfs:seeAlso rdf:resource="&j2se-1_6;JavaUtilLibrary"/>
		<rdfs:seeAlso rdf:resource="&j2se-1_6;JavaLangLibrary"/>
		<rdfs:seeAlso rdf:resource="&j2se-1_6;OrgOmgCORBAPortableLibrary"/>
		<rdfs:seeAlso rdf:resource="&j2se-1_6;JavaMathLibrary"/>
		<rdfs:seeAlso rdf:resource="&j2se-1_6;JavaIoLibrary"/>
		<rdfs:comment xml:lang="en">JavaLibrary implementing the org.omg.CORBA package for j2se-1_6</rdfs:comment>
	</owl:Class>
	<owl:Class rdf:about="&j2se-1_6;OrgOmgCORBAPortableLibrary">
		<owl:equivalentClass rdf:resource="&j2se-1_5;OrgOmgCORBAPortableLibrary"/>
		<rdfs:subClassOf rdf:resource="&java;JavaLibrary"/>
		<rdfs:seeAlso rdf:resource="&j2se-1_6;OrgOmgCORBALibrary"/>
		<rdfs:seeAlso rdf:resource="&j2se-1_6;JavaIoLibrary"/>
		<rdfs:seeAlso rdf:resource="&j2se-1_6;JavaLangLibrary"/>
		<rdfs:seeAlso rdf:resource="&j2se-1_6;JavaMathLibrary"/>
		<rdfs:seeAlso rdf:resource="&j2se-1_6;OrgOmgCORBA_2_3PortableLibrary"/>
		<rdfs:comment xml:lang="en">JavaLibrary implementing the org.omg.CORBA.portable package for j2se-1_6</rdfs:comment>
	</owl:Class>
	<owl:Class rdf:about="&j2se-1_6;OrgOmgCORBADynAnyPackageLibrary">
		<owl:equivalentClass rdf:resource="&j2se-1_5;OrgOmgCORBADynAnyPackageLibrary"/>
		<rdfs:subClassOf rdf:resource="&java;JavaLibrary"/>
		<rdfs:seeAlso rdf:resource="&j2se-1_6;OrgOmgCORBALibrary"/>
		<rdfs:seeAlso rdf:resource="&j2se-1_6;JavaLangLibrary"/>
		<rdfs:comment xml:lang="en">JavaLibrary implementing the org.omg.CORBA.DynAnyPackage package for j2se-1_6</rdfs:comment>
	</owl:Class>
	<owl:Class rdf:about="&j2se-1_6;OrgOmgCORBAORBPackageLibrary">
		<owl:equivalentClass rdf:resource="&j2se-1_5;OrgOmgCORBAORBPackageLibrary"/>
		<rdfs:subClassOf rdf:resource="&java;JavaLibrary"/>
		<rdfs:seeAlso rdf:resource="&j2se-1_6;OrgOmgCORBALibrary"/>
		<rdfs:seeAlso rdf:resource="&j2se-1_6;JavaLangLibrary"/>
		<rdfs:comment xml:lang="en">JavaLibrary implementing the org.omg.CORBA.ORBPackage package for j2se-1_6</rdfs:comment>
	</owl:Class>
	<owl:Class rdf:about="&j2se-1_6;OrgOmgCORBATypeCodePackageLibrary">
		<owl:equivalentClass rdf:resource="&j2se-1_5;OrgOmgCORBATypeCodePackageLibrary"/>
		<rdfs:subClassOf rdf:resource="&java;JavaLibrary"/>
		<rdfs:seeAlso rdf:resource="&j2se-1_6;OrgOmgCORBALibrary"/>
		<rdfs:seeAlso rdf:resource="&j2se-1_6;JavaLangLibrary"/>
		<rdfs:comment xml:lang="en">JavaLibrary implementing the org.omg.CORBA.TypeCodePackage package for j2se-1_6</rdfs:comment>
	</owl:Class>
	<owl:Class rdf:about="&j2se-1_6;OrgOmgCosNamingLibrary">
		<owl:equivalentClass rdf:resource="&j2se-1_5;OrgOmgCosNamingLibrary"/>
		<rdfs:subClassOf rdf:resource="&java;JavaLibrary"/>
		<rdfs:seeAlso rdf:resource="&j2se-1_6;OrgOmgCORBALibrary"/>
		<rdfs:seeAlso rdf:resource="&j2se-1_6;OrgOmgPortableServerLibrary"/>
		<rdfs:seeAlso rdf:resource="&j2se-1_6;JavaLangLibrary"/>
		<rdfs:seeAlso rdf:resource="&j2se-1_6;OrgOmgCORBAPortableLibrary"/>
		<rdfs:comment xml:lang="en">JavaLibrary implementing the org.omg.CosNaming package for j2se-1_6</rdfs:comment>
	</owl:Class>
	<owl:Class rdf:about="&j2se-1_6;OrgOmgCosNamingNamingContextExtPackageLibrary">
		<owl:equivalentClass rdf:resource="&j2se-1_5;OrgOmgCosNamingNamingContextExtPackageLibrary"/>
		<rdfs:subClassOf rdf:resource="&java;JavaLibrary"/>
		<rdfs:seeAlso rdf:resource="&j2se-1_6;OrgOmgCORBALibrary"/>
		<rdfs:seeAlso rdf:resource="&j2se-1_6;JavaLangLibrary"/>
		<rdfs:seeAlso rdf:resource="&j2se-1_6;OrgOmgCORBAPortableLibrary"/>
		<rdfs:comment xml:lang="en">JavaLibrary implementing the org.omg.CosNaming.NamingContextExtPackage package for j2se-1_6</rdfs:comment>
	</owl:Class>
	<owl:Class rdf:about="&j2se-1_6;OrgOmgCosNamingNamingContextPackageLibrary">
		<owl:equivalentClass rdf:resource="&j2se-1_5;OrgOmgCosNamingNamingContextPackageLibrary"/>
		<rdfs:subClassOf rdf:resource="&java;JavaLibrary"/>
		<rdfs:seeAlso rdf:resource="&j2se-1_6;OrgOmgCosNamingLibrary"/>
		<rdfs:seeAlso rdf:resource="&j2se-1_6;OrgOmgCORBALibrary"/>
		<rdfs:seeAlso rdf:resource="&j2se-1_6;JavaLangLibrary"/>
		<rdfs:seeAlso rdf:resource="&j2se-1_6;OrgOmgCORBAPortableLibrary"/>
		<rdfs:comment xml:lang="en">JavaLibrary implementing the org.omg.CosNaming.NamingContextPackage package for j2se-1_6</rdfs:comment>
	</owl:Class>
	<owl:Class rdf:about="&j2se-1_6;OrgOmgPortableServerLibrary">
		<owl:equivalentClass rdf:resource="&j2se-1_5;OrgOmgPortableServerLibrary"/>
		<rdfs:subClassOf rdf:resource="&java;JavaLibrary"/>
		<rdfs:seeAlso rdf:resource="&j2se-1_6;OrgOmgCORBALibrary"/>
		<rdfs:seeAlso rdf:resource="&j2se-1_6;JavaLangLibrary"/>
		<rdfs:seeAlso rdf:resource="&j2se-1_6;OrgOmgCORBAPortableLibrary"/>
		<rdfs:seeAlso rdf:resource="&j2se-1_6;OrgOmgPortableServerPortableLibrary"/>
		<rdfs:seeAlso rdf:resource="&j2se-1_6;OrgOmgPortableServerPOAManagerPackageLibrary"/>
		<rdfs:seeAlso rdf:resource="&j2se-1_6;OrgOmgPortableServerServantLocatorPackageLibrary"/>
		<rdfs:comment xml:lang="en">JavaLibrary implementing the org.omg.PortableServer package for j2se-1_6</rdfs:comment>
	</owl:Class>
	<owl:Class rdf:about="&j2se-1_6;OrgOmgPortableServerCurrentPackageLibrary">
		<owl:equivalentClass rdf:resource="&j2se-1_5;OrgOmgPortableServerCurrentPackageLibrary"/>
		<rdfs:subClassOf rdf:resource="&java;JavaLibrary"/>
		<rdfs:seeAlso rdf:resource="&j2se-1_6;OrgOmgCORBALibrary"/>
		<rdfs:seeAlso rdf:resource="&j2se-1_6;JavaLangLibrary"/>
		<rdfs:seeAlso rdf:resource="&j2se-1_6;OrgOmgCORBAPortableLibrary"/>
		<rdfs:comment xml:lang="en">JavaLibrary implementing the org.omg.PortableServer.CurrentPackage package for j2se-1_6</rdfs:comment>
	</owl:Class>
	<owl:Class rdf:about="&j2se-1_6;OrgOmgPortableServerPOAManagerPackageLibrary">
		<owl:equivalentClass rdf:resource="&j2se-1_5;OrgOmgPortableServerPOAManagerPackageLibrary"/>
		<rdfs:subClassOf rdf:resource="&java;JavaLibrary"/>
		<rdfs:seeAlso rdf:resource="&j2se-1_6;OrgOmgCORBALibrary"/>
		<rdfs:seeAlso rdf:resource="&j2se-1_6;JavaLangLibrary"/>
		<rdfs:seeAlso rdf:resource="&j2se-1_6;OrgOmgCORBAPortableLibrary"/>
		<rdfs:comment xml:lang="en">JavaLibrary implementing the org.omg.PortableServer.POAManagerPackage package for j2se-1_6</rdfs:comment>
	</owl:Class>
	<owl:Class rdf:about="&j2se-1_6;OrgOmgPortableServerPOAPackageLibrary">
		<owl:equivalentClass rdf:resource="&j2se-1_5;OrgOmgPortableServerPOAPackageLibrary"/>
		<rdfs:subClassOf rdf:resource="&java;JavaLibrary"/>
		<rdfs:seeAlso rdf:resource="&j2se-1_6;OrgOmgCORBALibrary"/>
		<rdfs:seeAlso rdf:resource="&j2se-1_6;JavaLangLibrary"/>
		<rdfs:seeAlso rdf:resource="&j2se-1_6;OrgOmgCORBAPortableLibrary"/>
		<rdfs:comment xml:lang="en">JavaLibrary implementing the org.omg.PortableServer.POAPackage package for j2se-1_6</rdfs:comment>
	</owl:Class>
	<owl:Class rdf:about="&j2se-1_6;OrgOmgPortableServerServantLocatorPackageLibrary">
		<owl:equivalentClass rdf:resource="&j2se-1_5;OrgOmgPortableServerServantLocatorPackageLibrary"/>
		<rdfs:subClassOf rdf:resource="&java;JavaLibrary"/>
		<rdfs:seeAlso rdf:resource="&j2se-1_6;OrgOmgCORBALibrary"/>
		<rdfs:seeAlso rdf:resource="&j2se-1_6;JavaLangLibrary"/>
		<rdfs:seeAlso rdf:resource="&j2se-1_6;OrgOmgCORBAPortableLibrary"/>
		<rdfs:comment xml:lang="en">JavaLibrary implementing the org.omg.PortableServer.ServantLocatorPackage package for j2se-1_6</rdfs:comment>
	</owl:Class>
	<owl:Class rdf:about="&j2se-1_6;OrgOmgPortableServerPortableLibrary">
		<owl:equivalentClass rdf:resource="&j2se-1_5;OrgOmgPortableServerPortableLibrary"/>
		<rdfs:subClassOf rdf:resource="&java;JavaLibrary"/>
		<rdfs:seeAlso rdf:resource="&j2se-1_6;OrgOmgCORBALibrary"/>
		<rdfs:seeAlso rdf:resource="&j2se-1_6;OrgOmgPortableServerLibrary"/>
		<rdfs:seeAlso rdf:resource="&j2se-1_6;JavaLangLibrary"/>
		<rdfs:comment xml:lang="en">JavaLibrary implementing the org.omg.PortableServer.portable package for j2se-1_6</rdfs:comment>
	</owl:Class>
	<owl:Class rdf:about="&j2se-1_6;OrgOmgDynamicLibrary">
		<owl:equivalentClass rdf:resource="&j2se-1_5;OrgOmgDynamicLibrary"/>
		<rdfs:subClassOf rdf:resource="&java;JavaLibrary"/>
		<rdfs:seeAlso rdf:resource="&j2se-1_6;OrgOmgCORBALibrary"/>
		<rdfs:seeAlso rdf:resource="&j2se-1_6;JavaLangLibrary"/>
		<rdfs:seeAlso rdf:resource="&j2se-1_6;OrgOmgCORBAPortableLibrary"/>
		<rdfs:comment xml:lang="en">JavaLibrary implementing the org.omg.Dynamic package for j2se-1_6</rdfs:comment>
	</owl:Class>
	<owl:Class rdf:about="&j2se-1_6;OrgOmgDynamicAnyLibrary">
		<owl:equivalentClass rdf:resource="&j2se-1_5;OrgOmgDynamicAnyLibrary"/>
		<rdfs:subClassOf rdf:resource="&java;JavaLibrary"/>
		<rdfs:seeAlso rdf:resource="&j2se-1_6;OrgOmgCORBALibrary"/>
		<rdfs:seeAlso rdf:resource="&j2se-1_6;JavaLangLibrary"/>
		<rdfs:seeAlso rdf:resource="&j2se-1_6;OrgOmgCORBAPortableLibrary"/>
		<rdfs:seeAlso rdf:resource="&j2se-1_6;JavaIoLibrary"/>
		<rdfs:comment xml:lang="en">JavaLibrary implementing the org.omg.DynamicAny package for j2se-1_6</rdfs:comment>
	</owl:Class>
	<owl:Class rdf:about="&j2se-1_6;OrgOmgDynamicAnyDynAnyFactoryPackageLibrary">
		<owl:equivalentClass rdf:resource="&j2se-1_5;OrgOmgDynamicAnyDynAnyFactoryPackageLibrary"/>
		<rdfs:subClassOf rdf:resource="&java;JavaLibrary"/>
		<rdfs:seeAlso rdf:resource="&j2se-1_6;OrgOmgCORBALibrary"/>
		<rdfs:seeAlso rdf:resource="&j2se-1_6;JavaLangLibrary"/>
		<rdfs:seeAlso rdf:resource="&j2se-1_6;OrgOmgCORBAPortableLibrary"/>
		<rdfs:comment xml:lang="en">JavaLibrary implementing the org.omg.DynamicAny.DynAnyFactoryPackage package for j2se-1_6</rdfs:comment>
	</owl:Class>
	<owl:Class rdf:about="&j2se-1_6;OrgOmgDynamicAnyDynAnyPackageLibrary">
		<owl:equivalentClass rdf:resource="&j2se-1_5;OrgOmgDynamicAnyDynAnyPackageLibrary"/>
		<rdfs:subClassOf rdf:resource="&java;JavaLibrary"/>
		<rdfs:seeAlso rdf:resource="&j2se-1_6;OrgOmgCORBALibrary"/>
		<rdfs:seeAlso rdf:resource="&j2se-1_6;JavaLangLibrary"/>
		<rdfs:seeAlso rdf:resource="&j2se-1_6;OrgOmgCORBAPortableLibrary"/>
		<rdfs:comment xml:lang="en">JavaLibrary implementing the org.omg.DynamicAny.DynAnyPackage package for j2se-1_6</rdfs:comment>
	</owl:Class>
	<owl:Class rdf:about="&j2se-1_6;OrgOmgIOPLibrary">
		<owl:equivalentClass rdf:resource="&j2se-1_5;OrgOmgIOPLibrary"/>
		<rdfs:subClassOf rdf:resource="&java;JavaLibrary"/>
		<rdfs:seeAlso rdf:resource="&j2se-1_6;OrgOmgCORBALibrary"/>
		<rdfs:seeAlso rdf:resource="&j2se-1_6;JavaLangLibrary"/>
		<rdfs:seeAlso rdf:resource="&j2se-1_6;OrgOmgCORBAPortableLibrary"/>
		<rdfs:comment xml:lang="en">JavaLibrary implementing the org.omg.IOP package for j2se-1_6</rdfs:comment>
	</owl:Class>
	<owl:Class rdf:about="&j2se-1_6;OrgOmgIOPCodecFactoryPackageLibrary">
		<owl:equivalentClass rdf:resource="&j2se-1_5;OrgOmgIOPCodecFactoryPackageLibrary"/>
		<rdfs:subClassOf rdf:resource="&java;JavaLibrary"/>
		<rdfs:seeAlso rdf:resource="&j2se-1_6;OrgOmgCORBALibrary"/>
		<rdfs:seeAlso rdf:resource="&j2se-1_6;JavaLangLibrary"/>
		<rdfs:seeAlso rdf:resource="&j2se-1_6;OrgOmgCORBAPortableLibrary"/>
		<rdfs:comment xml:lang="en">JavaLibrary implementing the org.omg.IOP.CodecFactoryPackage package for j2se-1_6</rdfs:comment>
	</owl:Class>
	<owl:Class rdf:about="&j2se-1_6;OrgOmgIOPCodecPackageLibrary">
		<owl:equivalentClass rdf:resource="&j2se-1_5;OrgOmgIOPCodecPackageLibrary"/>
		<rdfs:subClassOf rdf:resource="&java;JavaLibrary"/>
		<rdfs:seeAlso rdf:resource="&j2se-1_6;OrgOmgCORBALibrary"/>
		<rdfs:seeAlso rdf:resource="&j2se-1_6;JavaLangLibrary"/>
		<rdfs:seeAlso rdf:resource="&j2se-1_6;OrgOmgCORBAPortableLibrary"/>
		<rdfs:comment xml:lang="en">JavaLibrary implementing the org.omg.IOP.CodecPackage package for j2se-1_6</rdfs:comment>
	</owl:Class>
	<owl:Class rdf:about="&j2se-1_6;OrgOmgMessagingLibrary">
		<owl:equivalentClass rdf:resource="&j2se-1_5;OrgOmgMessagingLibrary"/>
		<rdfs:subClassOf rdf:resource="&java;JavaLibrary"/>
		<rdfs:seeAlso rdf:resource="&j2se-1_6;OrgOmgCORBALibrary"/>
		<rdfs:seeAlso rdf:resource="&j2se-1_6;JavaLangLibrary"/>
		<rdfs:seeAlso rdf:resource="&j2se-1_6;OrgOmgCORBAPortableLibrary"/>
		<rdfs:comment xml:lang="en">JavaLibrary implementing the org.omg.Messaging package for j2se-1_6</rdfs:comment>
	</owl:Class>
	<owl:Class rdf:about="&j2se-1_6;OrgOmgPortableInterceptorLibrary">
		<owl:equivalentClass rdf:resource="&j2se-1_5;OrgOmgPortableInterceptorLibrary"/>
		<rdfs:subClassOf rdf:resource="&java;JavaLibrary"/>
		<rdfs:seeAlso rdf:resource="&j2se-1_6;OrgOmgCORBALibrary"/>
		<rdfs:seeAlso rdf:resource="&j2se-1_6;JavaLangLibrary"/>
		<rdfs:seeAlso rdf:resource="&j2se-1_6;OrgOmgCORBAPortableLibrary"/>
		<rdfs:seeAlso rdf:resource="&j2se-1_6;OrgOmgIOPLibrary"/>
		<rdfs:comment xml:lang="en">JavaLibrary implementing the org.omg.PortableInterceptor package for j2se-1_6</rdfs:comment>
	</owl:Class>
	<owl:Class rdf:about="&j2se-1_6;OrgOmgPortableInterceptorORBInitInfoPackageLibrary">
		<owl:equivalentClass rdf:resource="&j2se-1_5;OrgOmgPortableInterceptorORBInitInfoPackageLibrary"/>
		<rdfs:subClassOf rdf:resource="&java;JavaLibrary"/>
		<rdfs:seeAlso rdf:resource="&j2se-1_6;OrgOmgCORBALibrary"/>
		<rdfs:seeAlso rdf:resource="&j2se-1_6;JavaLangLibrary"/>
		<rdfs:seeAlso rdf:resource="&j2se-1_6;OrgOmgCORBAPortableLibrary"/>
		<rdfs:comment xml:lang="en">JavaLibrary implementing the org.omg.PortableInterceptor.ORBInitInfoPackage package for j2se-1_6</rdfs:comment>
	</owl:Class>
	<owl:Class rdf:about="&j2se-1_6;OrgOmgSendingContextLibrary">
		<owl:equivalentClass rdf:resource="&j2se-1_5;OrgOmgSendingContextLibrary"/>
		<rdfs:subClassOf rdf:resource="&java;JavaLibrary"/>
		<rdfs:seeAlso rdf:resource="&j2se-1_6;OrgOmgCORBALibrary"/>
		<rdfs:seeAlso rdf:resource="&j2se-1_6;OrgOmgCORBAPortableLibrary"/>
		<rdfs:comment xml:lang="en">JavaLibrary implementing the org.omg.SendingContext package for j2se-1_6</rdfs:comment>
	</owl:Class>
	<owl:Class rdf:about="&j2se-1_6;OrgOmgStubJavaRmiLibrary">
		<owl:equivalentClass rdf:resource="&j2se-1_5;OrgOmgStubJavaRmiLibrary"/>
		<rdfs:subClassOf rdf:resource="&java;JavaLibrary"/>
		<rdfs:seeAlso rdf:resource="&j2se-1_6;JavaRmiLibrary"/>
		<rdfs:seeAlso rdf:resource="&j2se-1_6;JavaxRmiCORBALibrary"/>
		<rdfs:comment xml:lang="en">JavaLibrary implementing the org.omg.stub.java.rmi package for j2se-1_6</rdfs:comment>
	</owl:Class>
	<owl:Class rdf:about="&j2se-1_6;OrgOmgStubJavaxManagementRemoteRmiLibrary">
		<owl:equivalentClass rdf:resource="&j2se-1_5;OrgOmgStubJavaxManagementRemoteRmiLibrary"/>
		<rdfs:subClassOf rdf:resource="&java;JavaLibrary"/>
		<rdfs:seeAlso rdf:resource="&j2se-1_6;JavaUtilLibrary"/>
		<rdfs:seeAlso rdf:resource="&j2se-1_6;OrgOmgCORBALibrary"/>
		<rdfs:seeAlso rdf:resource="&j2se-1_6;JavaRmiLibrary"/>
		<rdfs:seeAlso rdf:resource="&j2se-1_6;JavaLangLibrary"/>
		<rdfs:seeAlso rdf:resource="&j2se-1_6;OrgOmgCORBAPortableLibrary"/>
		<rdfs:seeAlso rdf:resource="&j2se-1_6;JavaxSecurityAuthLibrary"/>
		<rdfs:seeAlso rdf:resource="&j2se-1_6;JavaxManagementRemoteLibrary"/>
		<rdfs:seeAlso rdf:resource="&j2se-1_6;JavaxManagementLibrary"/>
		<rdfs:seeAlso rdf:resource="&j2se-1_6;JavaxManagementRemoteRmiLibrary"/>
		<rdfs:seeAlso rdf:resource="&j2se-1_6;OrgOmgCORBA_2_3PortableLibrary"/>
		<rdfs:seeAlso rdf:resource="&j2se-1_6;JavaxRmiCORBALibrary"/>
		<rdfs:comment xml:lang="en">JavaLibrary implementing the org.omg.stub.javax.management.remote.rmi package for j2se-1_6</rdfs:comment>
	</owl:Class>
	<owl:Class rdf:about="&j2se-1_6;OrgXmlSaxLibrary">
		<owl:equivalentClass rdf:resource="&j2se-1_5;OrgXmlSaxLibrary"/>
		<rdfs:subClassOf rdf:resource="&java;JavaLibrary"/>
		<rdfs:seeAlso rdf:resource="&j2se-1_6;JavaUtilLibrary"/>
		<rdfs:seeAlso rdf:resource="&j2se-1_6;JavaIoLibrary"/>
		<rdfs:seeAlso rdf:resource="&j2se-1_6;JavaLangLibrary"/>
		<rdfs:comment xml:lang="en">JavaLibrary implementing the org.xml.sax package for j2se-1_6</rdfs:comment>
	</owl:Class>
	<owl:Class rdf:about="&j2se-1_6;OrgXmlSaxExtLibrary">
		<owl:equivalentClass rdf:resource="&j2se-1_5;OrgXmlSaxExtLibrary"/>
		<rdfs:subClassOf rdf:resource="&java;JavaLibrary"/>
		<rdfs:seeAlso rdf:resource="&j2se-1_6;OrgXmlSaxHelpersLibrary"/>
		<rdfs:seeAlso rdf:resource="&j2se-1_6;JavaLangLibrary"/>
		<rdfs:seeAlso rdf:resource="&j2se-1_6;OrgXmlSaxLibrary"/>
		<rdfs:comment xml:lang="en">JavaLibrary implementing the org.xml.sax.ext package for j2se-1_6</rdfs:comment>
	</owl:Class>
	<owl:Class rdf:about="&j2se-1_6;OrgXmlSaxHelpersLibrary">
		<owl:equivalentClass rdf:resource="&j2se-1_5;OrgXmlSaxHelpersLibrary"/>
		<rdfs:subClassOf rdf:resource="&java;JavaLibrary"/>
		<rdfs:seeAlso rdf:resource="&j2se-1_6;JavaUtilLibrary"/>
		<rdfs:seeAlso rdf:resource="&j2se-1_6;JavaLangLibrary"/>
		<rdfs:seeAlso rdf:resource="&j2se-1_6;OrgXmlSaxLibrary"/>
		<rdfs:comment xml:lang="en">JavaLibrary implementing the org.xml.sax.helpers package for j2se-1_6</rdfs:comment>
	</owl:Class>
	<owl:Class rdf:about="&j2se-1_6;OrgIetfJgssLibrary">
		<owl:equivalentClass rdf:resource="&j2se-1_5;OrgIetfJgssLibrary"/>
		<rdfs:subClassOf rdf:resource="&java;JavaLibrary"/>
		<rdfs:seeAlso rdf:resource="&j2se-1_6;JavaIoLibrary"/>
		<rdfs:seeAlso rdf:resource="&j2se-1_6;JavaLangLibrary"/>
		<rdfs:seeAlso rdf:resource="&j2se-1_6;JavaSecurityLibrary"/>
		<rdfs:seeAlso rdf:resource="&j2se-1_6;JavaNetLibrary"/>
		<rdfs:comment xml:lang="en">JavaLibrary implementing the org.ietf.jgss package for j2se-1_6</rdfs:comment>
	</owl:Class>
	<owl:Class rdf:about="&j2se-1_6;SunAwtLibrary">
		<rdfs:subClassOf rdf:resource="&java;JavaLibrary"/>
		<rdfs:comment xml:lang="en">JavaLibrary implementing the sun.awt package for j2se-1_6</rdfs:comment>
	</owl:Class>
</rdf:RDF>
